# DDWikiVersion: 1.5
#
# Copyright 2016 RESO.
# By using this document you agree to the RESO End User License Agreement (EULA) posted at:
# https://reso.memberclicks.net/assets/docs/reso%20eula.pdf 

# Generated by reso-parse-wiki
@prefix reso: <https://yodata.io/reso/dd#> .
@prefix enum: <https://yodata.io/reso/enum#> .
@prefix rdf: <http://www.w3.org/1999/02/22-rdf-syntax-ns#> .
@prefix rdfs: <http://www.w3.org/2000/01/rdf-schema#> .
@prefix xsd: <http://www.w3.org/2001/XMLSchema#> .
@prefix owl: <http://www.w3.org/2002/07/owl#> .
@prefix dc: <http://purl.org/dc/elements/1.1/> .
@prefix schema: <http://schema.org/> .
@prefix vs: <http://www.w3.org/2003/06/sw-vocab-status/ns#> .


<> a owl:Ontology ;
  dc:creator       _:DaveDuran ;
  dc:description   "Mapping of the RESO Data Dictionary to RDF." ;
  dc:publisher     <http://www.reso.org> ;
  dc:title         "Real Estate Standards Vocabulary (RESO)" ;
  rdfs:label       "RESO Data Diction - RDF Vocabulary"
.
_:DaveDuran a schema:Person ;
  schema:email     "dave@yodata.io" ;
  schema:name      "Dave Duran"
.


# classes

reso:Property a rdfs:Class ;
  rdfs:comment     "Property Resource" ;
  rdfs:label       "Property" ;
  schema:sameAs    <http://ddwiki.reso.org/display/DDW/Property+Resource>
.
reso:Member a rdfs:Class ;
  rdfs:comment     "Member Resource" ;
  rdfs:label       "Member" ;
  schema:sameAs    <http://ddwiki.reso.org/display/DDW/Member+Resource>
.
reso:Office a rdfs:Class ;
  rdfs:comment     "Office Resource" ;
  rdfs:label       "Office" ;
  schema:sameAs    <http://ddwiki.reso.org/display/DDW/Office+Resource>
.
reso:Contacts a rdfs:Class ;
  rdfs:comment     "Contacts Resource" ;
  rdfs:label       "Contacts" ;
  schema:sameAs    <http://ddwiki.reso.org/display/DDW/Contacts+Resource>
.
reso:Media a rdfs:Class ;
  rdfs:comment     "Media Resource" ;
  rdfs:label       "Media" ;
  schema:sameAs    <http://ddwiki.reso.org/display/DDW/Media+Resource>
.
reso:HistoryTransactional a rdfs:Class ;
  rdfs:comment     "HistoryTransactional Resource" ;
  rdfs:label       "HistoryTransactional" ;
  schema:sameAs    <http://ddwiki.reso.org/display/DDW/HistoryTransactional+Resource>
.
reso:SavedSearch a rdfs:Class ;
  rdfs:comment     "SavedSearch Resource" ;
  rdfs:label       "SavedSearch" ;
  schema:sameAs    <http://ddwiki.reso.org/display/DDW/SavedSearch+Resource>
.
reso:OpenHouse a rdfs:Class ;
  rdfs:comment     "OpenHouse Resource" ;
  rdfs:label       "OpenHouse" ;
  schema:sameAs    <http://ddwiki.reso.org/display/DDW/OpenHouse+Resource>
.
reso:Teams a rdfs:Class ;
  rdfs:comment     "Teams Resource" ;
  rdfs:label       "Teams" ;
  schema:sameAs    <http://ddwiki.reso.org/display/DDW/Teams+Resource>
.
reso:TeamMembers a rdfs:Class ;
  rdfs:comment     "TeamMembers Resource" ;
  rdfs:label       "TeamMembers" ;
  schema:sameAs    <http://ddwiki.reso.org/display/DDW/TeamMembers+Resource>
.
reso:OUID a rdfs:Class ;
  rdfs:comment     "OUID Resource" ;
  rdfs:label       "OUID" ;
  schema:sameAs    <http://ddwiki.reso.org/display/DDW/OUID+Resource>
.

# properties 

reso:AboveGradeFinishedArea a rdf:Property ;
  rdfs:comment     "Finished area within the structure that is at or above the surface of the ground." ;
  rdfs:domain      reso:Property ;
  rdfs:label       "AboveGradeFinishedArea" ;
  rdfs:range       xsd:decimal ;
  reso:CertificationLevel "Silver" ;
  reso:PropertyTypes "RESI","RLSE","RINC","MOBI","FARM" ;
  schema:sameAs    <http://ddwiki.reso.org/display/DDW/AboveGradeFinishedArea+Field> ;
  vs:term_status   "stable"
.
reso:AboveGradeFinishedAreaSource a rdf:Property ;
  rdfs:comment     "The source of the measurements. This is a pick list of options showing the source of the measurement. i.e. Agent, Assessor, Estimate, etc." ;
  rdfs:domain      reso:Property ;
  rdfs:label       "AboveGradeFinishedAreaSource" ;
  rdfs:range       enum:AreaSource ;
  reso:CertificationLevel "Silver" ;
  reso:PropertyTypes "RESI","RLSE","RINC","MOBI","FARM" ;
  schema:sameAs    <http://ddwiki.reso.org/display/DDW/AboveGradeFinishedAreaSource+Field> ;
  vs:term_status   "stable"
.
reso:AboveGradeFinishedAreaUnits a rdf:Property ;
  rdfs:comment     "A pick list of the unit of measurement for the area.  i.e. Square Feet, Square Meters, Acres, etc." ;
  rdfs:domain      reso:Property ;
  rdfs:label       "AboveGradeFinishedAreaUnits" ;
  rdfs:range       enum:AreaUnits ;
  reso:CertificationLevel "Silver" ;
  reso:PropertyTypes "RESI","RLSE","RINC","MOBI","FARM" ;
  schema:sameAs    <http://ddwiki.reso.org/display/DDW/AboveGradeFinishedAreaUnits+Field> ;
  vs:term_status   "stable"
.
reso:AccessCode a rdf:Property ;
  rdfs:comment     "If the property is located behind an unmanned security gate such as in a Gated Community, what is the code to gain access through the secured gate." ;
  rdfs:domain      reso:Property ;
  rdfs:label       "AccessCode" ;
  rdfs:range       xsd:string ;
  reso:CertificationLevel "Bronze" ;
  reso:PropertyTypes "RESI","RLSE","RINC","LAND","MOBI","FARM" ;
  schema:sameAs    <http://ddwiki.reso.org/display/DDW/AccessCode+Field> ;
  vs:term_status   "stable"
.
reso:AccessibilityFeatures a rdf:Property ;
  rdfs:comment     "A list or description of the accessibility features included in the sale/lease." ;
  rdfs:domain      reso:Property ;
  rdfs:label       "AccessibilityFeatures" ;
  rdfs:range       xsd:string ;
  reso:CertificationLevel "Silver" ;
  reso:PropertyTypes "RESI","RLSE","RINC","MOBI","FARM","COMS","COML" ;
  schema:sameAs    <http://ddwiki.reso.org/display/DDW/AccessibilityFeatures+Field> ;
  vs:term_status   "stable"
.
reso:AdditionalParcelsDescription a rdf:Property ;
  rdfs:comment     "If additional parcels are included in the sale, a list of those parcel's IDs separated by commas.  Do not include the first or primary parcel number, that should be located in the Parcel Number field." ;
  rdfs:domain      reso:Property ;
  rdfs:label       "AdditionalParcelsDescription" ;
  rdfs:range       xsd:string ;
  reso:CertificationLevel "Bronze" ;
  reso:PropertyTypes "RESI","RLSE","RINC","LAND","MOBI","FARM","COMS","COML" ;
  schema:sameAs    <http://ddwiki.reso.org/display/DDW/AdditionalParcelsDescription+Field> ;
  vs:term_status   "stable"
.
reso:AdditionalParcelsYN a rdf:Property ;
  rdfs:comment     "Are there more than one parcel or lot included in the sale?" ;
  rdfs:domain      reso:Property ;
  rdfs:label       "AdditionalParcelsYN" ;
  rdfs:range       xsd:boolean ;
  reso:CertificationLevel "Bronze" ;
  reso:PropertyTypes "RESI","RLSE","RINC","LAND","MOBI","FARM","COMS","COML" ;
  schema:sameAs    <http://ddwiki.reso.org/display/DDW/AdditionalParcelsYN+Field> ;
  vs:term_status   "stable"
.
reso:AnchorsCoTenants a rdf:Property ;
  rdfs:comment     "The main or most notable tenants as well as other tenants of the shopping center or mall in which the commercial property is located." ;
  rdfs:domain      reso:Property ;
  rdfs:label       "AnchorsCoTenants" ;
  rdfs:range       xsd:string ;
  reso:CertificationLevel "Platinum" ;
  reso:PropertyTypes "COMS","COML" ;
  schema:sameAs    <http://ddwiki.reso.org/display/DDW/AnchorsCoTenants+Field> ;
  vs:term_status   "stable"
.
reso:Appliances a rdf:Property ;
  rdfs:comment     "A list of the appliances that will be included in the sale/lease of the property." ;
  rdfs:domain      reso:Property ;
  rdfs:label       "Appliances" ;
  rdfs:range       xsd:string ;
  reso:CertificationLevel "Platinum" ;
  reso:PropertyTypes "RESI","RLSE","RINC","MOBI","FARM","COMS","COML" ;
  schema:sameAs    <http://ddwiki.reso.org/display/DDW/Appliances+Field> ;
  vs:term_status   "stable"
.
reso:ApprovalStatus a rdf:Property ;
  rdfs:comment     "When an MLS has the ability to set a listing to Draft and/or has facility to allow an agent to input, but their manager to approve the listings before publishing, this field is used for such control." ;
  rdfs:domain      reso:Property ;
  rdfs:label       "ApprovalStatus" ;
  rdfs:range       xsd:string ;
  reso:CertificationLevel "Silver" ;
  reso:PropertyTypes "RESI","RLSE","RINC","LAND","MOBI","FARM","COMS","COML","BUSO" ;
  schema:sameAs    <http://ddwiki.reso.org/display/DDW/ApprovalStatus+Field> ;
  vs:term_status   "stable"
.
reso:ArchitecturalStyle a rdf:Property ;
  rdfs:comment     "A list describing the style of the structure.  For example, Victorian, Ranch, Craftsman, etc." ;
  rdfs:domain      reso:Property ;
  rdfs:label       "ArchitecturalStyle" ;
  rdfs:range       xsd:string ;
  reso:CertificationLevel "Silver" ;
  reso:PropertyTypes "RESI","RLSE","RINC","MOBI","FARM" ;
  schema:sameAs    <http://ddwiki.reso.org/display/DDW/ArchitecturalStyle+Field> ;
  vs:term_status   "stable"
.
reso:AssociationAmenities a rdf:Property ;
  rdfs:comment     "Amenities provided by the Home Owners Association, Mobile Park or Complex. For example Pool, Clubhouse, etc." ;
  rdfs:domain      reso:Property ;
  rdfs:label       "AssociationAmenities" ;
  rdfs:range       xsd:string ;
  reso:CertificationLevel "Platinum" ;
  reso:PropertyTypes "RESI","RLSE","RINC","LAND","MOBI" ;
  schema:sameAs    <http://ddwiki.reso.org/display/DDW/AssociationAmenities+Field> ;
  vs:term_status   "stable"
.
reso:AssociationFee a rdf:Property ;
  rdfs:comment     "A fee paid by the homeowner to the Home Owners Association which is used for the upkeep of the common area, neighborhood or other association related benefits." ;
  rdfs:domain      reso:Property ;
  rdfs:label       "AssociationFee" ;
  rdfs:range       xsd:decimal ;
  reso:CertificationLevel "Bronze" ;
  reso:PropertyTypes "RESI","RLSE","RINC","LAND","MOBI" ;
  schema:sameAs    <http://ddwiki.reso.org/display/DDW/AssociationFee+Field> ;
  vs:term_status   "stable"
.
reso:AssociationFee2 a rdf:Property ;
  rdfs:comment     "A fee paid by the homeowner to the second of two Home Owners Associations, which is used for the upkeep of the common area, neighborhood or other association related benefits." ;
  rdfs:domain      reso:Property ;
  rdfs:label       "AssociationFee2" ;
  rdfs:range       xsd:decimal ;
  reso:CertificationLevel "Bronze" ;
  reso:PropertyTypes "RESI","RLSE","RINC","LAND","MOBI" ;
  schema:sameAs    <http://ddwiki.reso.org/display/DDW/AssociationFee2+Field> ;
  vs:term_status   "stable"
.
reso:AssociationFee2Frequency a rdf:Property ;
  rdfs:comment     "The frequency the association fee is paid.  For example, Weekly, Monthly, Annually, Bi-Monthly, One Time, etc." ;
  rdfs:domain      reso:Property ;
  rdfs:label       "AssociationFee2Frequency" ;
  rdfs:range       enum:FeeFrequency ;
  reso:CertificationLevel "Bronze" ;
  reso:PropertyTypes "RESI","RLSE","RINC","LAND","MOBI" ;
  schema:sameAs    <http://ddwiki.reso.org/display/DDW/AssociationFee2Frequency+Field> ;
  vs:term_status   "stable"
.
reso:AssociationFeeFrequency a rdf:Property ;
  rdfs:comment     "The frequency the association fee is paid.  For example, Weekly, Monthly, Annually, Bi-Monthly, One Time, etc." ;
  rdfs:domain      reso:Property ;
  rdfs:label       "AssociationFeeFrequency" ;
  rdfs:range       enum:FeeFrequency ;
  reso:CertificationLevel "Bronze" ;
  reso:PropertyTypes "RESI","RLSE","RINC","LAND","MOBI" ;
  schema:sameAs    <http://ddwiki.reso.org/display/DDW/AssociationFeeFrequency+Field> ;
  vs:term_status   "stable"
.
reso:AssociationFeeIncludes a rdf:Property ;
  rdfs:comment     "Services included with the association fee.  For example Landscaping, Trash, Water, etc." ;
  rdfs:domain      reso:Property ;
  rdfs:label       "AssociationFeeIncludes" ;
  rdfs:range       enum:AssociationFeeIncludes ;
  reso:CertificationLevel "Bronze" ;
  reso:PropertyTypes "RESI","RLSE","RINC","LAND","MOBI" ;
  schema:sameAs    <http://ddwiki.reso.org/display/DDW/AssociationFeeIncludes+Field> ;
  vs:term_status   "stable"
.
reso:AssociationName a rdf:Property ;
  rdfs:comment     "The name of the Home Owners Association." ;
  rdfs:domain      reso:Property ;
  rdfs:label       "AssociationName" ;
  rdfs:range       xsd:string ;
  reso:CertificationLevel "Bronze" ;
  reso:PropertyTypes "RESI","RLSE","RINC","LAND","MOBI" ;
  schema:sameAs    <http://ddwiki.reso.org/display/DDW/AssociationName+Field> ;
  vs:term_status   "stable"
.
reso:AssociationName2 a rdf:Property ;
  rdfs:comment     "The name of the second of two Home Owners Association." ;
  rdfs:domain      reso:Property ;
  rdfs:label       "AssociationName2" ;
  rdfs:range       xsd:string ;
  reso:CertificationLevel "Bronze" ;
  reso:PropertyTypes "RESI","RLSE","RINC","LAND","MOBI" ;
  schema:sameAs    <http://ddwiki.reso.org/display/DDW/AssociationName2+Field> ;
  vs:term_status   "stable"
.
reso:AssociationPhone a rdf:Property ;
  rdfs:comment     "The phone number of the Home Owners Association. North American 10 digit phone numbers should be in the format of ###-###-#### (separated by hyphens).  Other conventions should use the common local standard.  International numbers should be preceded by a plus symbol." ;
  rdfs:domain      reso:Property ;
  rdfs:label       "AssociationPhone" ;
  rdfs:range       xsd:string ;
  reso:CertificationLevel "Bronze" ;
  reso:PropertyTypes "RESI","RLSE","RINC","LAND","MOBI" ;
  schema:sameAs    <http://ddwiki.reso.org/display/DDW/AssociationPhone+Field> ;
  vs:term_status   "stable"
.
reso:AssociationPhone2 a rdf:Property ;
  rdfs:comment     "The phone number of the second of two Home Owners Association. North American 10 digit phone numbers should be in the format of ###-###-#### (separated by hyphens).  Other conventions should use the common local standard.  International numbers should be preceded by a plus symbol." ;
  rdfs:domain      reso:Property ;
  rdfs:label       "AssociationPhone2" ;
  rdfs:range       xsd:string ;
  reso:CertificationLevel "Bronze" ;
  reso:PropertyTypes "RESI","RLSE","RINC","LAND","MOBI" ;
  schema:sameAs    <http://ddwiki.reso.org/display/DDW/AssociationPhone2+Field> ;
  vs:term_status   "stable"
.
reso:AssociationYN a rdf:Property ;
  rdfs:comment     "Is there a Home Owners Association.  A separate Y/N field is needed because not all associations have dues." ;
  rdfs:domain      reso:Property ;
  rdfs:label       "AssociationYN" ;
  rdfs:range       xsd:boolean ;
  reso:CertificationLevel "Bronze" ;
  reso:PropertyTypes "RESI","RLSE","RINC","LAND","MOBI" ;
  schema:sameAs    <http://ddwiki.reso.org/display/DDW/AssociationYN+Field> ;
  vs:term_status   "stable"
.
reso:AttachedGarageYN a rdf:Property ;
  rdfs:comment     "A flag indicating that the garage attached to the dwelling." ;
  rdfs:domain      reso:Property ;
  rdfs:label       "AttachedGarageYN" ;
  rdfs:range       xsd:boolean ;
  reso:CertificationLevel "Silver" ;
  reso:PropertyTypes "RESI","RLSE","RINC","MOBI","FARM" ;
  schema:sameAs    <http://ddwiki.reso.org/display/DDW/AttachedGarageYN+Field> ;
  vs:term_status   "stable"
.
reso:AvailabilityDate a rdf:Property ;
  rdfs:comment     "The date the property will be available for possession/occupation." ;
  rdfs:domain      reso:Property ;
  rdfs:label       "AvailabilityDate" ;
  rdfs:range       xsd:date ;
  reso:CertificationLevel "Silver" ;
  reso:PropertyTypes "RLSE","COMS","COML" ;
  schema:sameAs    <http://ddwiki.reso.org/display/DDW/AvailabilityDate+Field> ;
  vs:term_status   "stable"
.
reso:Basement a rdf:Property ;
  rdfs:comment     "A list of information and features about the basement.  i.e. None/Slab, Finished, Partially Finished, Crawl Space, Dirt, Outside Entrance, Radon Mitigation" ;
  rdfs:domain      reso:Property ;
  rdfs:label       "Basement" ;
  rdfs:range       xsd:string ;
  reso:CertificationLevel "Platinum" ;
  reso:PropertyTypes "RESI","RLSE","RINC","MOBI","FARM" ;
  schema:sameAs    <http://ddwiki.reso.org/display/DDW/Basement+Field> ;
  vs:term_status   "stable"
.
reso:BathroomsFull a rdf:Property ;
  rdfs:comment     "A room containing all 4 of the 4 elements constituting a bath, which are; Toilet, Sink, Bathtub or Shower Head.  A Full Bath will typically contain four elements; Sink, Toilet, Tub and Shower Head (in tub or stall).  However, some may considered a Sink, Toilet and Tub (without a shower) a Full Bath, others consider this to be a Three Quarter Bath.  In the event that BathroomsThreeQuarter is not in use, this field may represent the sum of all Full and Three Quarter bathrooms." ;
  rdfs:domain      reso:Property ;
  rdfs:label       "BathroomsFull" ;
  rdfs:range       xsd:decimal ;
  reso:CertificationLevel "Core" ;
  reso:PropertyTypes "RESI","RLSE","RINC","MOBI","FARM" ;
  schema:sameAs    <http://ddwiki.reso.org/display/DDW/BathroomsFull+Field> ;
  vs:term_status   "stable"
.
reso:BathroomsHalf a rdf:Property ;
  rdfs:comment     "A room containing 2 of the 4 elements constituting a bath, which are; Toilet, Sink, Bathtub or Shower Head.  A Half Bath will typically contain a Sink and Toilet." ;
  rdfs:domain      reso:Property ;
  rdfs:label       "BathroomsHalf" ;
  rdfs:range       xsd:decimal ;
  reso:CertificationLevel "Core" ;
  reso:PropertyTypes "RESI","RLSE","RINC","MOBI","FARM" ;
  schema:sameAs    <http://ddwiki.reso.org/display/DDW/BathroomsHalf+Field> ;
  vs:term_status   "stable"
.
reso:BathroomsOneQuarter a rdf:Property ;
  rdfs:comment     "A room containing 1 of the 4 elements constituting a bath which are; Toilet, Sink, Bathtub or Shower Head.  Examples are a vanity with a sink or a WC (Water Closet, which is a room with only a toilet)." ;
  rdfs:domain      reso:Property ;
  rdfs:label       "BathroomsOneQuarter" ;
  rdfs:range       xsd:decimal ;
  reso:CertificationLevel "Core" ;
  reso:PropertyTypes "RESI","RLSE","RINC","MOBI","FARM" ;
  schema:sameAs    <http://ddwiki.reso.org/display/DDW/BathroomsOneQuarter+Field> ;
  vs:term_status   "stable"
.
reso:BathroomsPartial a rdf:Property ;
  rdfs:comment     "The number of partial bathrooms in the property being sold/leased.  When used in combination with the BathroomsFull field, this replaces (or is the sum of) all Half and One Quarter bathrooms; and in the event BathroomsThreeQuarter is not used, BathroomsFull replaces (or is the sum of) all Full and Three Quarter baths.  This field should not be used in combination with the BathroomsOneQuarter or the BathroomsHalf." ;
  rdfs:domain      reso:Property ;
  rdfs:label       "BathroomsPartial" ;
  rdfs:range       xsd:decimal ;
  reso:CertificationLevel "Silver" ;
  reso:PropertyTypes "RESI","RLSE","RINC","MOBI","FARM" ;
  schema:sameAs    <http://ddwiki.reso.org/display/DDW/BathroomsPartial+Field> ;
  vs:term_status   "stable"
.
reso:BathroomsThreeQuarter a rdf:Property ;
  rdfs:comment     "A room containing 3 of the 4 elements constituting a bath, which are; Toilet, Sink, Bathtub or Shower Head. A typical Three Quarter Bath will contain Sink, Toilet and Shower.  Some may considered a Sink, Toilet and Tub (without a shower) a Three Quarter Bath, others consider this to be a Full Bath." ;
  rdfs:domain      reso:Property ;
  rdfs:label       "BathroomsThreeQuarter" ;
  rdfs:range       xsd:decimal ;
  reso:CertificationLevel "Core" ;
  reso:PropertyTypes "RESI","RLSE","RINC","MOBI","FARM" ;
  schema:sameAs    <http://ddwiki.reso.org/display/DDW/BathroomsThreeQuarter+Field> ;
  vs:term_status   "stable"
.
reso:BathroomsTotalInteger a rdf:Property ;
  rdfs:comment     "The simple sum of the number of bathrooms.  For example for a property with two Full Bathrooms and one Half Bathroom, the Bathrooms Total Integer will be 3.  To express this example as 2.5, use the BathroomsTotalDecimal field.  To express this example as 2.1, use the BathroomsTotalNotational." ;
  rdfs:domain      reso:Property ;
  rdfs:label       "BathroomsTotalInteger" ;
  rdfs:range       xsd:decimal ;
  reso:CertificationLevel "Core" ;
  reso:PropertyTypes "RESI","RLSE","RINC","MOBI","FARM" ;
  schema:sameAs    <http://ddwiki.reso.org/display/DDW/BathroomsTotalInteger+Field> ;
  vs:term_status   "stable"
.
reso:BedroomsPossible a rdf:Property ;
  rdfs:comment     "The sum of BedroomsTotal plus other rooms that may be used as a bedroom but are not defined as bedroom per local policy." ;
  rdfs:domain      reso:Property ;
  rdfs:label       "BedroomsPossible" ;
  rdfs:range       xsd:decimal ;
  reso:CertificationLevel "Silver" ;
  reso:PropertyTypes "RESI","RLSE","RINC","MOBI","FARM" ;
  schema:sameAs    <http://ddwiki.reso.org/display/DDW/BedroomsPossible+Field> ;
  vs:term_status   "stable"
.
reso:BedroomsTotal a rdf:Property ;
  rdfs:comment     "The total number of bedrooms in the dwelling." ;
  rdfs:domain      reso:Property ;
  rdfs:label       "BedroomsTotal" ;
  rdfs:range       xsd:decimal ;
  reso:CertificationLevel "Core" ;
  reso:PropertyTypes "RESI","RLSE","RINC","MOBI","FARM" ;
  schema:sameAs    <http://ddwiki.reso.org/display/DDW/BedroomsTotal+Field> ;
  vs:term_status   "stable"
.
reso:BelowGradeFinishedArea a rdf:Property ;
  rdfs:comment     "Finished area within the structure that is below ground." ;
  rdfs:domain      reso:Property ;
  rdfs:label       "BelowGradeFinishedArea" ;
  rdfs:range       xsd:decimal ;
  reso:CertificationLevel "Silver" ;
  reso:PropertyTypes "RESI","RLSE","RINC","MOBI","FARM" ;
  schema:sameAs    <http://ddwiki.reso.org/display/DDW/BelowGradeFinishedArea+Field> ;
  vs:term_status   "stable"
.
reso:BelowGradeFinishedAreaSource a rdf:Property ;
  rdfs:comment     "The source of the measurements. This is a pick list of options showing the source of the measurement. i.e. Agent, Assessor, Estimate, etc." ;
  rdfs:domain      reso:Property ;
  rdfs:label       "BelowGradeFinishedAreaSource" ;
  rdfs:range       enum:AreaSource ;
  reso:CertificationLevel "Silver" ;
  reso:PropertyTypes "RESI","RLSE","RINC","MOBI","FARM" ;
  schema:sameAs    <http://ddwiki.reso.org/display/DDW/BelowGradeFinishedAreaSource+Field> ;
  vs:term_status   "stable"
.
reso:BelowGradeFinishedAreaUnits a rdf:Property ;
  rdfs:comment     "A pick list of the unit of measurement for the area.  i.e. Square Feet, Square Meters, Acres, etc." ;
  rdfs:domain      reso:Property ;
  rdfs:label       "BelowGradeFinishedAreaUnits" ;
  rdfs:range       enum:AreaUnits ;
  reso:CertificationLevel "Silver" ;
  reso:PropertyTypes "RESI","RLSE","RINC","MOBI","FARM" ;
  schema:sameAs    <http://ddwiki.reso.org/display/DDW/BelowGradeFinishedAreaUnits+Field> ;
  vs:term_status   "stable"
.
reso:BodyType a rdf:Property ;
  rdfs:comment     "Type of mobile home." ;
  rdfs:domain      reso:Property ;
  rdfs:label       "BodyType" ;
  rdfs:range       enum:BodyType ;
  reso:CertificationLevel "Silver" ;
  reso:PropertyTypes "MOBI" ;
  schema:sameAs    <http://ddwiki.reso.org/display/DDW/BodyType+Field> ;
  vs:term_status   "stable"
.
reso:BuilderModel a rdf:Property ;
  rdfs:comment     "The builders model name or number for the property." ;
  rdfs:domain      reso:Property ;
  rdfs:label       "BuilderModel" ;
  rdfs:range       xsd:string ;
  reso:CertificationLevel "Gold" ;
  reso:PropertyTypes "RESI","RLSE","RINC","FARM" ;
  schema:sameAs    <http://ddwiki.reso.org/display/DDW/BuilderModel+Field> ;
  vs:term_status   "stable"
.
reso:BuilderName a rdf:Property ;
  rdfs:comment     "Name of the builder of the property or builder's tract." ;
  rdfs:domain      reso:Property ;
  rdfs:label       "BuilderName" ;
  rdfs:range       xsd:string ;
  reso:CertificationLevel "Gold" ;
  reso:PropertyTypes "RESI","RLSE","RINC","MOBI","FARM","COMS","COML" ;
  schema:sameAs    <http://ddwiki.reso.org/display/DDW/BuilderName+Field> ;
  vs:term_status   "stable"
.
reso:BuildingAreaSource a rdf:Property ;
  rdfs:comment     "The source of the measurements. This is a pick list of options showing the source of the measurement. i.e. Agent, Assessor, Estimate, etc." ;
  rdfs:domain      reso:Property ;
  rdfs:label       "BuildingAreaSource" ;
  rdfs:range       enum:AreaSource ;
  reso:CertificationLevel "Silver" ;
  reso:PropertyTypes "RESI","RLSE","RINC","MOBI","FARM","COMS","COML" ;
  schema:sameAs    <http://ddwiki.reso.org/display/DDW/BuildingAreaSource+Field> ;
  vs:term_status   "stable"
.
reso:BuildingAreaTotal a rdf:Property ;
  rdfs:comment     "Total area of the structure. Includes both finished and unfinished areas." ;
  rdfs:domain      reso:Property ;
  rdfs:label       "BuildingAreaTotal" ;
  rdfs:range       xsd:decimal ;
  reso:CertificationLevel "Silver" ;
  reso:PropertyTypes "RESI","RLSE","RINC","MOBI","FARM","COMS","COML" ;
  schema:sameAs    <http://ddwiki.reso.org/display/DDW/BuildingAreaTotal+Field> ;
  vs:term_status   "stable"
.
reso:BuildingAreaUnits a rdf:Property ;
  rdfs:comment     "A pick list of the unit of measurement for the area.  i.e. Square Feet, Square Meters, Acres, etc." ;
  rdfs:domain      reso:Property ;
  rdfs:label       "BuildingAreaUnits" ;
  rdfs:range       enum:AreaUnits ;
  reso:CertificationLevel "Silver" ;
  reso:PropertyTypes "RESI","RLSE","RINC","MOBI","FARM","COMS","COML" ;
  schema:sameAs    <http://ddwiki.reso.org/display/DDW/BuildingAreaUnits+Field> ;
  vs:term_status   "stable"
.
reso:BuildingFeatures a rdf:Property ;
  rdfs:comment     "Features or amenities of the building or business park." ;
  rdfs:domain      reso:Property ;
  rdfs:label       "BuildingFeatures" ;
  rdfs:range       xsd:string ;
  reso:CertificationLevel "Platinum" ;
  reso:PropertyTypes "COMS","COML" ;
  schema:sameAs    <http://ddwiki.reso.org/display/DDW/BuildingFeatures+Field> ;
  vs:term_status   "stable"
.
reso:BuildingName a rdf:Property ;
  rdfs:comment     "Name of the building or business park." ;
  rdfs:domain      reso:Property ;
  rdfs:label       "BuildingName" ;
  rdfs:range       xsd:string ;
  reso:CertificationLevel "Gold" ;
  reso:PropertyTypes "COMS","COML" ;
  schema:sameAs    <http://ddwiki.reso.org/display/DDW/BuildingName+Field> ;
  vs:term_status   "stable"
.
reso:BusinessName a rdf:Property ;
  rdfs:comment     "Name of the business being sold." ;
  rdfs:domain      reso:Property ;
  rdfs:label       "BusinessName" ;
  rdfs:range       xsd:string ;
  reso:CertificationLevel "Bronze" ;
  reso:PropertyTypes "BUSO" ;
  schema:sameAs    <http://ddwiki.reso.org/display/DDW/BusinessName+Field> ;
  vs:term_status   "stable"
.
reso:BusinessType a rdf:Property ;
  rdfs:comment     "The type of business being sold.  Retail, Wholesale, Grocery, Food & Bev, etc.&#x2026;" ;
  rdfs:domain      reso:Property ;
  rdfs:label       "BusinessType" ;
  rdfs:range       enum:BusinessType ;
  reso:CertificationLevel "Core" ;
  reso:PropertyTypes "COMS","COML","BUSO" ;
  schema:sameAs    <http://ddwiki.reso.org/display/DDW/BusinessType+Field> ;
  vs:term_status   "stable"
.
reso:BuyerAgencyCompensation a rdf:Property ;
  rdfs:comment     "The total commission to be paid for this sale, expressed as either a percentage or a constant currency amount." ;
  rdfs:domain      reso:Property ;
  rdfs:label       "BuyerAgencyCompensation" ;
  rdfs:range       xsd:string ;
  reso:CertificationLevel "Core" ;
  reso:PropertyTypes "RESI","RLSE","RINC","LAND","MOBI","FARM","COMS","COML","BUSO" ;
  schema:sameAs    <http://ddwiki.reso.org/display/DDW/BuyerAgencyCompensation+Field> ;
  vs:term_status   "stable"
.
reso:BuyerAgencyCompensationType a rdf:Property ;
  rdfs:comment     "A list of types to clarify the value entered in the BuyerAgencyCompensation field.  For example $, % or some other clarification of the BuyerAgencyCompensation." ;
  rdfs:domain      reso:Property ;
  rdfs:label       "BuyerAgencyCompensationType" ;
  rdfs:range       enum:CompensationType ;
  reso:CertificationLevel "Core" ;
  reso:PropertyTypes "RESI","RLSE","RINC","LAND","MOBI","FARM","COMS","COML","BUSO" ;
  schema:sameAs    <http://ddwiki.reso.org/display/DDW/BuyerAgencyCompensationType+Field> ;
  vs:term_status   "stable"
.
reso:BuyerAgentAOR a rdf:Property ;
  rdfs:comment     "The Buyer's Agent's Board or Association of REALTORS." ;
  rdfs:domain      reso:Property ;
  rdfs:label       "BuyerAgentAOR" ;
  rdfs:range       xsd:string ;
  reso:CertificationLevel "Bronze" ;
  reso:PropertyTypes "RESI","RLSE","RINC","LAND","MOBI","FARM","COMS","COML","BUSO" ;
  schema:sameAs    <http://ddwiki.reso.org/display/DDW/BuyerAgentAOR+Field> ;
  vs:term_status   "stable"
.
reso:BuyerAgentCellPhone a rdf:Property ;
  rdfs:comment     "North American 10 digit phone numbers should be in the format of ###-###-#### (separated by hyphens).  Other conventions should use the common local standard.  International numbers should be preceded by a plus symbol." ;
  rdfs:domain      reso:Property ;
  rdfs:label       "BuyerAgentCellPhone" ;
  rdfs:range       xsd:string ;
  reso:CertificationLevel "Core" ;
  reso:PropertyTypes "RESI","RLSE","RINC","LAND","MOBI","FARM","COMS","COML","BUSO" ;
  schema:sameAs    <http://ddwiki.reso.org/display/DDW/BuyerAgentCellPhone+Field> ;
  vs:term_status   "stable"
.
reso:BuyerAgentDesignation a rdf:Property ;
  rdfs:comment     "Designations and certifications acknowledging experience and expertise in various real estate sectors are awarded by NAR and each affiliated group upon completion of required courses." ;
  rdfs:domain      reso:Property ;
  rdfs:label       "BuyerAgentDesignation" ;
  rdfs:range       xsd:string ;
  reso:CertificationLevel "Bronze" ;
  reso:PropertyTypes "RESI","RLSE","RINC","LAND","MOBI","FARM","COMS","COML","BUSO" ;
  schema:sameAs    <http://ddwiki.reso.org/display/DDW/BuyerAgentDesignation+Field> ;
  vs:term_status   "stable"
.
reso:BuyerAgentDirectPhone a rdf:Property ;
  rdfs:comment     "North American 10 digit phone numbers should be in the format of ###-###-#### (separated by hyphens).  Other conventions should use the common local standard.  International numbers should be preceded by a plus symbol." ;
  rdfs:domain      reso:Property ;
  rdfs:label       "BuyerAgentDirectPhone" ;
  rdfs:range       xsd:string ;
  reso:CertificationLevel "Bronze" ;
  reso:PropertyTypes "RESI","RLSE","RINC","LAND","MOBI","FARM","COMS","COML","BUSO" ;
  schema:sameAs    <http://ddwiki.reso.org/display/DDW/BuyerAgentDirectPhone+Field> ;
  vs:term_status   "stable"
.
reso:BuyerAgentEmail a rdf:Property ;
  rdfs:comment     "The email address of the Buyer's Agent." ;
  rdfs:domain      reso:Property ;
  rdfs:label       "BuyerAgentEmail" ;
  rdfs:range       xsd:string ;
  reso:CertificationLevel "Core" ;
  reso:PropertyTypes "RESI","RLSE","RINC","LAND","MOBI","FARM","COMS","COML","BUSO" ;
  schema:sameAs    <http://ddwiki.reso.org/display/DDW/BuyerAgentEmail+Field> ;
  vs:term_status   "stable"
.
reso:BuyerAgentFax a rdf:Property ;
  rdfs:comment     "North American 10 digit phone numbers should be in the format of ###-###-#### (separated by hyphens).  Other conventions should use the common local standard.  International numbers should be preceded by a plus symbol." ;
  rdfs:domain      reso:Property ;
  rdfs:label       "BuyerAgentFax" ;
  rdfs:range       xsd:string ;
  reso:CertificationLevel "Bronze" ;
  reso:PropertyTypes "RESI","RLSE","RINC","LAND","MOBI","FARM","COMS","COML","BUSO" ;
  schema:sameAs    <http://ddwiki.reso.org/display/DDW/BuyerAgentFax+Field> ;
  vs:term_status   "stable"
.
reso:BuyerAgentFirstName a rdf:Property ;
  rdfs:comment     "The first name of the buyer's agent." ;
  rdfs:domain      reso:Property ;
  rdfs:label       "BuyerAgentFirstName" ;
  rdfs:range       xsd:string ;
  reso:CertificationLevel "Core" ;
  reso:PropertyTypes "RESI","RLSE","RINC","LAND","MOBI","FARM","COMS","COML","BUSO" ;
  schema:sameAs    <http://ddwiki.reso.org/display/DDW/BuyerAgentFirstName+Field> ;
  vs:term_status   "stable"
.
reso:BuyerAgentFullName a rdf:Property ;
  rdfs:comment     "The full name of the buyer's agent. (First Middle Last)" ;
  rdfs:domain      reso:Property ;
  rdfs:label       "BuyerAgentFullName" ;
  rdfs:range       xsd:string ;
  reso:CertificationLevel "Bronze" ;
  reso:PropertyTypes "RESI","RLSE","RINC","LAND","MOBI","FARM","COMS","COML","BUSO" ;
  schema:sameAs    <http://ddwiki.reso.org/display/DDW/BuyerAgentFullName+Field> ;
  vs:term_status   "stable"
.
reso:BuyerAgentHomePhone a rdf:Property ;
  rdfs:comment     "North American 10 digit phone numbers should be in the format of ###-###-#### (separated by hyphens).  Other conventions should use the common local standard.  International numbers should be preceded by a plus symbol." ;
  rdfs:domain      reso:Property ;
  rdfs:label       "BuyerAgentHomePhone" ;
  rdfs:range       xsd:string ;
  reso:CertificationLevel "Bronze" ;
  reso:PropertyTypes "RESI","RLSE","RINC","LAND","MOBI","FARM","COMS","COML","BUSO" ;
  schema:sameAs    <http://ddwiki.reso.org/display/DDW/BuyerAgentHomePhone+Field> ;
  vs:term_status   "stable"
.
reso:BuyerAgentKey a rdf:Property ;
  rdfs:comment     "A system unique identifier. Specifically, in aggregation systems, the Key is the system unique identifier from the system that the record was just retrieved. This may be identical to the related xxxId identifier, but the key is guaranteed unique for this record set.  This is a foreign key relating to the Member resource's MemberKey." ;
  rdfs:domain      reso:Property ;
  rdfs:label       "BuyerAgentKey" ;
  rdfs:range       xsd:string ;
  reso:CertificationLevel "Core" ;
  reso:PropertyTypes "RESI","RLSE","RINC","LAND","MOBI","FARM","COMS","COML","BUSO" ;
  schema:sameAs    <http://ddwiki.reso.org/display/DDW/BuyerAgentKey+Field> ;
  vs:term_status   "stable"
.
reso:BuyerAgentKeyNumeric a rdf:Property ;
  rdfs:comment     "A system unique identifier. Specifically, in aggregation systems, the Key is the system unique identifier from the system that the record was just retrieved. This may be identical to the related xxxId identifier, but the key is guaranteed unique for this record set.  This is a foreign key relating to the Member resource's MemberKey.  This is the numeric only key and used as an alternative to the BuyerAgentKey field." ;
  rdfs:domain      reso:Property ;
  rdfs:label       "BuyerAgentKeyNumeric" ;
  rdfs:range       xsd:decimal ;
  reso:CertificationLevel "Platinum" ;
  reso:PropertyTypes "RESI","RLSE","RINC","LAND","MOBI","FARM","COMS","COML","BUSO" ;
  schema:sameAs    <http://ddwiki.reso.org/display/DDW/BuyerAgentKeyNumeric+Field> ;
  vs:term_status   "stable"
.
reso:BuyerAgentLastName a rdf:Property ;
  rdfs:comment     "The last name of the buyer's agent." ;
  rdfs:domain      reso:Property ;
  rdfs:label       "BuyerAgentLastName" ;
  rdfs:range       xsd:string ;
  reso:CertificationLevel "Core" ;
  reso:PropertyTypes "RESI","RLSE","RINC","LAND","MOBI","FARM","COMS","COML","BUSO" ;
  schema:sameAs    <http://ddwiki.reso.org/display/DDW/BuyerAgentLastName+Field> ;
  vs:term_status   "stable"
.
reso:BuyerAgentMiddleName a rdf:Property ;
  rdfs:comment     "The middle name of the buyer's agent." ;
  rdfs:domain      reso:Property ;
  rdfs:label       "BuyerAgentMiddleName" ;
  rdfs:range       xsd:string ;
  reso:CertificationLevel "Core" ;
  reso:PropertyTypes "RESI","RLSE","RINC","LAND","MOBI","FARM","COMS","COML","BUSO" ;
  schema:sameAs    <http://ddwiki.reso.org/display/DDW/BuyerAgentMiddleName+Field> ;
  vs:term_status   "stable"
.
reso:BuyerAgentMlsId a rdf:Property ;
  rdfs:comment     "The local, well-known identifier. This value may not be unique, specifically in the case of aggregation systems, this value should be the identifier from the original system." ;
  rdfs:domain      reso:Property ;
  rdfs:label       "BuyerAgentMlsId" ;
  rdfs:range       xsd:string ;
  reso:CertificationLevel "Core" ;
  reso:PropertyTypes "RESI","RLSE","RINC","LAND","MOBI","FARM","COMS","COML","BUSO" ;
  schema:sameAs    <http://ddwiki.reso.org/display/DDW/BuyerAgentMlsId+Field> ;
  vs:term_status   "stable"
.
reso:BuyerAgentNamePrefix a rdf:Property ;
  rdfs:comment     "Prefix to the name (e.g. Dr. Mr. Ms. etc.)" ;
  rdfs:domain      reso:Property ;
  rdfs:label       "BuyerAgentNamePrefix" ;
  rdfs:range       xsd:string ;
  reso:CertificationLevel "Bronze" ;
  reso:PropertyTypes "RESI","RLSE","RINC","LAND","MOBI","FARM","COMS","COML","BUSO" ;
  schema:sameAs    <http://ddwiki.reso.org/display/DDW/BuyerAgentNamePrefix+Field> ;
  vs:term_status   "stable"
.
reso:BuyerAgentNameSuffix a rdf:Property ;
  rdfs:comment     "Suffix to the BuyerAgentLastName (e.g. Esq.,  Jr.,  III etc.)" ;
  rdfs:domain      reso:Property ;
  rdfs:label       "BuyerAgentNameSuffix" ;
  rdfs:range       xsd:string ;
  reso:CertificationLevel "Bronze" ;
  reso:PropertyTypes "RESI","RLSE","RINC","LAND","MOBI","FARM","COMS","COML","BUSO" ;
  schema:sameAs    <http://ddwiki.reso.org/display/DDW/BuyerAgentNameSuffix+Field> ;
  vs:term_status   "stable"
.
reso:BuyerAgentOfficePhone a rdf:Property ;
  rdfs:comment     "North American 10 digit phone numbers should be in the format of ###-###-#### (separated by hyphens).  Other conventions should use the common local standard.  International numbers should be preceded by a plus symbol." ;
  rdfs:domain      reso:Property ;
  rdfs:label       "BuyerAgentOfficePhone" ;
  rdfs:range       xsd:string ;
  reso:CertificationLevel "Core" ;
  reso:PropertyTypes "RESI","RLSE","RINC","LAND","MOBI","FARM","COMS","COML","BUSO" ;
  schema:sameAs    <http://ddwiki.reso.org/display/DDW/BuyerAgentOfficePhone+Field> ;
  vs:term_status   "stable"
.
reso:BuyerAgentOfficePhoneExt a rdf:Property ;
  rdfs:comment     "The extension of the given phone number (if applicable)." ;
  rdfs:domain      reso:Property ;
  rdfs:label       "BuyerAgentOfficePhoneExt" ;
  rdfs:range       xsd:string ;
  reso:CertificationLevel "Core" ;
  reso:PropertyTypes "RESI","RLSE","RINC","LAND","MOBI","FARM","COMS","COML","BUSO" ;
  schema:sameAs    <http://ddwiki.reso.org/display/DDW/BuyerAgentOfficePhoneExt+Field> ;
  vs:term_status   "stable"
.
reso:BuyerAgentPager a rdf:Property ;
  rdfs:comment     "North American 10 digit phone numbers should be in the format of ###-###-#### (separated by hyphens).  Other conventions should use the common local standard.  International numbers should be preceded by a plus symbol." ;
  rdfs:domain      reso:Property ;
  rdfs:label       "BuyerAgentPager" ;
  rdfs:range       xsd:string ;
  reso:CertificationLevel "Bronze" ;
  reso:PropertyTypes "RESI","RLSE","RINC","LAND","MOBI","FARM","COMS","COML","BUSO" ;
  schema:sameAs    <http://ddwiki.reso.org/display/DDW/BuyerAgentPager+Field> ;
  vs:term_status   "stable"
.
reso:BuyerAgentPreferredPhone a rdf:Property ;
  rdfs:comment     "North American 10 digit phone numbers should be in the format of ###-###-#### (separated by hyphens).  Other conventions should use the common local standard.  International numbers should be preceded by a plus symbol." ;
  rdfs:domain      reso:Property ;
  rdfs:label       "BuyerAgentPreferredPhone" ;
  rdfs:range       xsd:string ;
  reso:CertificationLevel "Core" ;
  reso:PropertyTypes "RESI","RLSE","RINC","LAND","MOBI","FARM","COMS","COML","BUSO" ;
  schema:sameAs    <http://ddwiki.reso.org/display/DDW/BuyerAgentPreferredPhone+Field> ;
  vs:term_status   "stable"
.
reso:BuyerAgentPreferredPhoneExt a rdf:Property ;
  rdfs:comment     "The extension of the given phone number (if applicable)." ;
  rdfs:domain      reso:Property ;
  rdfs:label       "BuyerAgentPreferredPhoneExt" ;
  rdfs:range       xsd:string ;
  reso:CertificationLevel "Core" ;
  reso:PropertyTypes "RESI","RLSE","RINC","LAND","MOBI","FARM","COMS","COML","BUSO" ;
  schema:sameAs    <http://ddwiki.reso.org/display/DDW/BuyerAgentPreferredPhoneExt+Field> ;
  vs:term_status   "stable"
.
reso:BuyerAgentStateLicense a rdf:Property ;
  rdfs:comment     "The license of the buyers agent. Separate multiple licenses with a comma and space." ;
  rdfs:domain      reso:Property ;
  rdfs:label       "BuyerAgentStateLicense" ;
  rdfs:range       xsd:string ;
  reso:CertificationLevel "Core" ;
  reso:PropertyTypes "RESI","RLSE","RINC","LAND","MOBI","FARM","COMS","COML","BUSO" ;
  schema:sameAs    <http://ddwiki.reso.org/display/DDW/BuyerAgentStateLicense+Field> ;
  vs:term_status   "stable"
.
reso:BuyerAgentTollFreePhone a rdf:Property ;
  rdfs:comment     "North American 10 digit phone numbers should be in the format of ###-###-#### (separated by hyphens).  Other conventions should use the common local standard.  International numbers should be preceded by a plus symbol." ;
  rdfs:domain      reso:Property ;
  rdfs:label       "BuyerAgentTollFreePhone" ;
  rdfs:range       xsd:string ;
  reso:CertificationLevel "Bronze" ;
  reso:PropertyTypes "RESI","RLSE","RINC","LAND","MOBI","FARM","COMS","COML","BUSO" ;
  schema:sameAs    <http://ddwiki.reso.org/display/DDW/BuyerAgentTollFreePhone+Field> ;
  vs:term_status   "stable"
.
reso:BuyerAgentURL a rdf:Property ;
  rdfs:comment     "The website URI of the buyers agent." ;
  rdfs:domain      reso:Property ;
  rdfs:label       "BuyerAgentURL" ;
  rdfs:range       xsd:string ;
  reso:CertificationLevel "Bronze" ;
  reso:PropertyTypes "RESI","RLSE","RINC","LAND","MOBI","FARM","COMS","COML","BUSO" ;
  schema:sameAs    <http://ddwiki.reso.org/display/DDW/BuyerAgentURL+Field> ;
  vs:term_status   "stable"
.
reso:BuyerAgentVoiceMail a rdf:Property ;
  rdfs:comment     "North American 10 digit phone numbers should be in the format of ###-###-#### (separated by hyphens).  Other conventions should use the common local standard.  International numbers should be preceded by a plus symbol." ;
  rdfs:domain      reso:Property ;
  rdfs:label       "BuyerAgentVoiceMail" ;
  rdfs:range       xsd:string ;
  reso:CertificationLevel "Bronze" ;
  reso:PropertyTypes "RESI","RLSE","RINC","LAND","MOBI","FARM","COMS","COML","BUSO" ;
  schema:sameAs    <http://ddwiki.reso.org/display/DDW/BuyerAgentVoiceMail+Field> ;
  vs:term_status   "stable"
.
reso:BuyerAgentVoiceMailExt a rdf:Property ;
  rdfs:comment     "The extension of the given phone number (if applicable)." ;
  rdfs:domain      reso:Property ;
  rdfs:label       "BuyerAgentVoiceMailExt" ;
  rdfs:range       xsd:string ;
  reso:CertificationLevel "Bronze" ;
  reso:PropertyTypes "RESI","RLSE","RINC","LAND","MOBI","FARM","COMS","COML","BUSO" ;
  schema:sameAs    <http://ddwiki.reso.org/display/DDW/BuyerAgentVoiceMailExt+Field> ;
  vs:term_status   "stable"
.
reso:BuyerFinancing a rdf:Property ;
  rdfs:comment     "A list of options that describe the type of financing used.  This field is used when setting a listing to Closed.  i.e. cash, FHA loan, etc." ;
  rdfs:domain      reso:Property ;
  rdfs:label       "BuyerFinancing" ;
  rdfs:range       enum:BuyerFinancing ;
  reso:CertificationLevel "Bronze" ;
  reso:PropertyTypes "RESI","RLSE","RINC","LAND","MOBI","FARM","COMS","COML","BUSO" ;
  schema:sameAs    <http://ddwiki.reso.org/display/DDW/BuyerFinancing+Field> ;
  vs:term_status   "stable"
.
reso:BuyerOfficeAOR a rdf:Property ;
  rdfs:comment     "The Buyer's Office's Board or Association of REALTORS." ;
  rdfs:domain      reso:Property ;
  rdfs:label       "BuyerOfficeAOR" ;
  rdfs:range       xsd:string ;
  reso:CertificationLevel "Bronze" ;
  reso:PropertyTypes "RESI","RLSE","RINC","LAND","MOBI","FARM","COMS","COML","BUSO" ;
  schema:sameAs    <http://ddwiki.reso.org/display/DDW/BuyerOfficeAOR+Field> ;
  vs:term_status   "stable"
.
reso:BuyerOfficeEmail a rdf:Property ;
  rdfs:comment     "The email address of the Buyer's Office." ;
  rdfs:domain      reso:Property ;
  rdfs:label       "BuyerOfficeEmail" ;
  rdfs:range       xsd:string ;
  reso:CertificationLevel "Bronze" ;
  reso:PropertyTypes "RESI","RLSE","RINC","LAND","MOBI","FARM","COMS","COML","BUSO" ;
  schema:sameAs    <http://ddwiki.reso.org/display/DDW/BuyerOfficeEmail+Field> ;
  vs:term_status   "stable"
.
reso:BuyerOfficeFax a rdf:Property ;
  rdfs:comment     "North American 10 digit phone numbers should be in the format of ###-###-#### (separated by hyphens).  Other conventions should use the common local standard.  International numbers should be preceded by a plus symbol." ;
  rdfs:domain      reso:Property ;
  rdfs:label       "BuyerOfficeFax" ;
  rdfs:range       xsd:string ;
  reso:CertificationLevel "Bronze" ;
  reso:PropertyTypes "RESI","RLSE","RINC","LAND","MOBI","FARM","COMS","COML","BUSO" ;
  schema:sameAs    <http://ddwiki.reso.org/display/DDW/BuyerOfficeFax+Field> ;
  vs:term_status   "stable"
.
reso:BuyerOfficeKey a rdf:Property ;
  rdfs:comment     "A system unique identifier. Specifically, in aggregation systems, the Key is the system unique identifier from the system that the record was just retrieved. This may be identical to the related xxxId identifier, but the key is guaranteed unique for this record set.  This is a foreign key relating to the Office resource's OfficeKey." ;
  rdfs:domain      reso:Property ;
  rdfs:label       "BuyerOfficeKey" ;
  rdfs:range       xsd:string ;
  reso:CertificationLevel "Core" ;
  reso:PropertyTypes "RESI","RLSE","RINC","LAND","MOBI","FARM","COMS","COML","BUSO" ;
  schema:sameAs    <http://ddwiki.reso.org/display/DDW/BuyerOfficeKey+Field> ;
  vs:term_status   "stable"
.
reso:BuyerOfficeKeyNumeric a rdf:Property ;
  rdfs:comment     "A system unique identifier. Specifically, in aggregation systems, the Key is the system unique identifier from the system that the record was just retrieved. This may be identical to the related xxxId identifier, but the key is guaranteed unique for this record set.  This is a foreign key relating to the Office resource's OfficeKey.  This is the numeric only key and used as an alternative to the BuyerOfficeKey field." ;
  rdfs:domain      reso:Property ;
  rdfs:label       "BuyerOfficeKeyNumeric" ;
  rdfs:range       xsd:decimal ;
  reso:CertificationLevel "Platinum" ;
  reso:PropertyTypes "RESI","RLSE","RINC","LAND","MOBI","FARM","COMS","COML","BUSO" ;
  schema:sameAs    <http://ddwiki.reso.org/display/DDW/BuyerOfficeKeyNumeric+Field> ;
  vs:term_status   "stable"
.
reso:BuyerOfficeMlsId a rdf:Property ;
  rdfs:comment     "The local, well-known identifier. This value may not be unique, specifically in the case of aggregation systems, this value should be the identifier from the original system." ;
  rdfs:domain      reso:Property ;
  rdfs:label       "BuyerOfficeMlsId" ;
  rdfs:range       xsd:string ;
  reso:CertificationLevel "Core" ;
  reso:PropertyTypes "RESI","RLSE","RINC","LAND","MOBI","FARM","COMS","COML","BUSO" ;
  schema:sameAs    <http://ddwiki.reso.org/display/DDW/BuyerOfficeMlsId+Field> ;
  vs:term_status   "stable"
.
reso:BuyerOfficeName a rdf:Property ;
  rdfs:comment     "The legal name of the brokerage representing the buyer." ;
  rdfs:domain      reso:Property ;
  rdfs:label       "BuyerOfficeName" ;
  rdfs:range       xsd:string ;
  reso:CertificationLevel "Core" ;
  reso:PropertyTypes "RESI","RLSE","RINC","LAND","MOBI","FARM","COMS","COML","BUSO" ;
  schema:sameAs    <http://ddwiki.reso.org/display/DDW/BuyerOfficeName+Field> ;
  vs:term_status   "stable"
.
reso:BuyerOfficePhone a rdf:Property ;
  rdfs:comment     "North American 10 digit phone numbers should be in the format of ###-###-#### (separated by hyphens).  Other conventions should use the common local standard.  International numbers should be preceded by a plus symbol." ;
  rdfs:domain      reso:Property ;
  rdfs:label       "BuyerOfficePhone" ;
  rdfs:range       xsd:string ;
  reso:CertificationLevel "Core" ;
  reso:PropertyTypes "RESI","RLSE","RINC","LAND","MOBI","FARM","COMS","COML","BUSO" ;
  schema:sameAs    <http://ddwiki.reso.org/display/DDW/BuyerOfficePhone+Field> ;
  vs:term_status   "stable"
.
reso:BuyerOfficePhoneExt a rdf:Property ;
  rdfs:comment     "The extension of the given phone number (if applicable)." ;
  rdfs:domain      reso:Property ;
  rdfs:label       "BuyerOfficePhoneExt" ;
  rdfs:range       xsd:string ;
  reso:CertificationLevel "Core" ;
  reso:PropertyTypes "RESI","RLSE","RINC","LAND","MOBI","FARM","COMS","COML","BUSO" ;
  schema:sameAs    <http://ddwiki.reso.org/display/DDW/BuyerOfficePhoneExt+Field> ;
  vs:term_status   "stable"
.
reso:BuyerOfficeURL a rdf:Property ;
  rdfs:comment     "The website URI for the buyers office." ;
  rdfs:domain      reso:Property ;
  rdfs:label       "BuyerOfficeURL" ;
  rdfs:range       xsd:string ;
  reso:CertificationLevel "Bronze" ;
  reso:PropertyTypes "RESI","RLSE","RINC","LAND","MOBI","FARM","COMS","COML","BUSO" ;
  schema:sameAs    <http://ddwiki.reso.org/display/DDW/BuyerOfficeURL+Field> ;
  vs:term_status   "stable"
.
reso:BuyerTeamKey a rdf:Property ;
  rdfs:comment     "A system unique identifier. Specifically, in aggregation systems, the Key is the system unique identifier from the system that the record was just retrieved. This may be identical to the related xxxId identifier, but the key is guaranteed unique for this record set.  This is a foreign key relating to the Teams resource's TeamKey." ;
  rdfs:domain      reso:Property ;
  rdfs:label       "BuyerTeamKey" ;
  rdfs:range       xsd:string ;
  reso:CertificationLevel "Silver" ;
  reso:PropertyTypes "RESI","RLSE","RINC","LAND","MOBI","FARM","COMS","COML","BUSO" ;
  schema:sameAs    <http://ddwiki.reso.org/display/DDW/BuyerTeamKey+Field> ;
  vs:term_status   "stable"
.
reso:BuyerTeamKeyNumeric a rdf:Property ;
  rdfs:comment     "A system unique identifier. Specifically, in aggregation systems, the Key is the system unique identifier from the system that the record was just retrieved. This may be identical to the related xxxId identifier, but the key is guaranteed unique for this record set.  This is a foreign key relating to the Teams resource's TeamKey.  This is the numeric only key and used as an alternative to the BuyerTeamKey field." ;
  rdfs:domain      reso:Property ;
  rdfs:label       "BuyerTeamKeyNumeric" ;
  rdfs:range       xsd:decimal ;
  reso:CertificationLevel "Platinum" ;
  reso:PropertyTypes "RESI","RLSE","RINC","LAND","MOBI","FARM","COMS","COML","BUSO" ;
  schema:sameAs    <http://ddwiki.reso.org/display/DDW/BuyerTeamKeyNumeric+Field> ;
  vs:term_status   "stable"
.
reso:BuyerTeamName a rdf:Property ;
  rdfs:comment     "The name of the team representing the buyer." ;
  rdfs:domain      reso:Property ;
  rdfs:label       "BuyerTeamName" ;
  rdfs:range       xsd:string ;
  reso:CertificationLevel "Silver" ;
  reso:PropertyTypes "RESI","RLSE","RINC","LAND","MOBI","FARM","COMS","COML","BUSO" ;
  schema:sameAs    <http://ddwiki.reso.org/display/DDW/BuyerTeamName+Field> ;
  vs:term_status   "stable"
.
reso:CableTvExpense a rdf:Property ;
  rdfs:comment     "The annual expense that is not paid directly by the tenant and is included in the Operating Expense calculations." ;
  rdfs:domain      reso:Property ;
  rdfs:label       "CableTvExpense" ;
  rdfs:range       xsd:decimal ;
  reso:CertificationLevel "Silver" ;
  reso:PropertyTypes "RINC" ;
  schema:sameAs    <http://ddwiki.reso.org/display/DDW/CableTvExpense+Field> ;
  vs:term_status   "stable"
.
reso:CancelationDate a rdf:Property ;
  rdfs:comment     "Date the listing contract between the seller and listing agent was cancelled.  This is the date entered by the agent reflecting when the change occurred contractually, not a timestamp of when the change was made in the MLS." ;
  rdfs:domain      reso:Property ;
  rdfs:label       "CancelationDate" ;
  rdfs:range       xsd:date ;
  reso:CertificationLevel "Core" ;
  reso:PropertyTypes "RESI","RLSE","RINC","LAND","MOBI","FARM","COMS","COML","BUSO" ;
  schema:sameAs    <http://ddwiki.reso.org/display/DDW/CancelationDate+Field> ;
  vs:term_status   "stable"
.
reso:CapRate a rdf:Property ;
  rdfs:comment     "Cap Rate is equivalent to the return on investment you would receive if you pay cash for a property. The ratio between the net operating income produced by an asset and its capital cost (the original price paid to buy the asset) or alternatively its current market value." ;
  rdfs:domain      reso:Property ;
  rdfs:label       "CapRate" ;
  rdfs:range       xsd:decimal ;
  reso:CertificationLevel "Core" ;
  reso:PropertyTypes "RINC","COMS","COML" ;
  schema:sameAs    <http://ddwiki.reso.org/display/DDW/CapRate+Field> ;
  vs:term_status   "stable"
.
reso:CarportSpaces a rdf:Property ;
  rdfs:comment     "The number of carport spaces included in the sale." ;
  rdfs:domain      reso:Property ;
  rdfs:label       "CarportSpaces" ;
  rdfs:range       xsd:decimal ;
  reso:CertificationLevel "Silver" ;
  reso:PropertyTypes "RESI","RLSE","RINC","MOBI","FARM" ;
  schema:sameAs    <http://ddwiki.reso.org/display/DDW/CarportSpaces+Field> ;
  vs:term_status   "stable"
.
reso:CarportYN a rdf:Property ;
  rdfs:comment     "A flag indicating that the listing has a car port. This flag may be T/F, Y/N or other true, false or unknown indicator. As with all flags, the field may be null." ;
  rdfs:domain      reso:Property ;
  rdfs:label       "CarportYN" ;
  rdfs:range       xsd:boolean ;
  reso:CertificationLevel "Silver" ;
  reso:PropertyTypes "RESI","RLSE","RINC","MOBI","FARM" ;
  schema:sameAs    <http://ddwiki.reso.org/display/DDW/CarportYN+Field> ;
  vs:term_status   "stable"
.
reso:CarrierRoute a rdf:Property ;
  rdfs:domain      reso:Property ;
  rdfs:label       "CarrierRoute" ;
  rdfs:range       xsd:string ;
  reso:CertificationLevel "Bronze" ;
  reso:PropertyTypes "RESI","RLSE","RINC","LAND","MOBI","FARM","COMS","COML","BUSO" ;
  schema:sameAs    <http://ddwiki.reso.org/display/DDW/CarrierRoute+Field> ;
  vs:term_status   "stable"
.
reso:City a rdf:Property ;
  rdfs:comment     "The city in listing address." ;
  rdfs:domain      reso:Property ;
  rdfs:label       "City" ;
  rdfs:range       xsd:string ;
  reso:CertificationLevel "Core" ;
  reso:PropertyTypes "RESI","RLSE","RINC","LAND","MOBI","FARM","COMS","COML","BUSO" ;
  schema:sameAs    <http://ddwiki.reso.org/display/DDW/City+Field> ;
  vs:term_status   "stable"
.
reso:CityRegion a rdf:Property ;
  rdfs:comment     "A sub-section or area of a defined city.  Examples would be SOHO in New York, NY, Ironbound in Newark, NJ or Inside the Beltway." ;
  rdfs:domain      reso:Property ;
  rdfs:label       "CityRegion" ;
  rdfs:range       xsd:string ;
  reso:CertificationLevel "Platinum" ;
  reso:PropertyTypes "RESI","RLSE","RINC","LAND","MOBI","FARM","COMS","COML","BUSO" ;
  schema:sameAs    <http://ddwiki.reso.org/display/DDW/CityRegion+Field> ;
  vs:term_status   "stable"
.
reso:CloseDate a rdf:Property ;
  rdfs:comment     "With for-sale listings, the date the purchase agreement was fulfilled. With lease listings, the date the requirements were fulfilled, such as contract and/or deposit.  This is the date entered by the agent reflecting when the change occurred contractually, not a timestamp of when the change was made in the MLS." ;
  rdfs:domain      reso:Property ;
  rdfs:label       "CloseDate" ;
  rdfs:range       xsd:date ;
  reso:CertificationLevel "Core" ;
  reso:PropertyTypes "RESI","RLSE","RINC","LAND","MOBI","FARM","COMS","COML","BUSO" ;
  schema:sameAs    <http://ddwiki.reso.org/display/DDW/CloseDate+Field> ;
  vs:term_status   "stable"
.
reso:ClosePrice a rdf:Property ;
  rdfs:comment     "The amount of money paid by the purchaser to the seller for the property under the agreement." ;
  rdfs:domain      reso:Property ;
  rdfs:label       "ClosePrice" ;
  rdfs:range       xsd:decimal ;
  reso:CertificationLevel "Core" ;
  reso:PropertyTypes "RESI","RLSE","RINC","LAND","MOBI","FARM","COMS","COML","BUSO" ;
  schema:sameAs    <http://ddwiki.reso.org/display/DDW/ClosePrice+Field> ;
  vs:term_status   "stable"
.
reso:CoBuyerAgentAOR a rdf:Property ;
  rdfs:comment     "The Co Buyer's Agent's Board or Association of REALTORS." ;
  rdfs:domain      reso:Property ;
  rdfs:label       "CoBuyerAgentAOR" ;
  rdfs:range       xsd:string ;
  reso:CertificationLevel "Bronze" ;
  reso:PropertyTypes "RESI","RLSE","RINC","LAND","MOBI","FARM","COMS","COML","BUSO" ;
  schema:sameAs    <http://ddwiki.reso.org/display/DDW/CoBuyerAgentAOR+Field> ;
  vs:term_status   "stable"
.
reso:CoBuyerAgentCellPhone a rdf:Property ;
  rdfs:comment     "North American 10 digit phone numbers should be in the format of ###-###-#### (separated by hyphens).  Other conventions should use the common local standard.  International numbers should be preceded by a plus symbol." ;
  rdfs:domain      reso:Property ;
  rdfs:label       "CoBuyerAgentCellPhone" ;
  rdfs:range       xsd:string ;
  reso:CertificationLevel "Core" ;
  reso:PropertyTypes "RESI","RLSE","RINC","LAND","MOBI","FARM","COMS","COML","BUSO" ;
  schema:sameAs    <http://ddwiki.reso.org/display/DDW/CoBuyerAgentCellPhone+Field> ;
  vs:term_status   "stable"
.
reso:CoBuyerAgentDesignation a rdf:Property ;
  rdfs:comment     "Designations and certifications acknowledging experience and expertise in various real estate sectors are awarded by NAR and each affiliated group upon completion of required courses." ;
  rdfs:domain      reso:Property ;
  rdfs:label       "CoBuyerAgentDesignation" ;
  rdfs:range       xsd:string ;
  reso:CertificationLevel "Bronze" ;
  reso:PropertyTypes "RESI","RLSE","RINC","LAND","MOBI","FARM","COMS","COML","BUSO" ;
  schema:sameAs    <http://ddwiki.reso.org/display/DDW/CoBuyerAgentDesignation+Field> ;
  vs:term_status   "stable"
.
reso:CoBuyerAgentDirectPhone a rdf:Property ;
  rdfs:comment     "North American 10 digit phone numbers should be in the format of ###-###-#### (separated by hyphens).  Other conventions should use the common local standard.  International numbers should be preceded by a plus symbol." ;
  rdfs:domain      reso:Property ;
  rdfs:label       "CoBuyerAgentDirectPhone" ;
  rdfs:range       xsd:string ;
  reso:CertificationLevel "Bronze" ;
  reso:PropertyTypes "RESI","RLSE","RINC","LAND","MOBI","FARM","COMS","COML","BUSO" ;
  schema:sameAs    <http://ddwiki.reso.org/display/DDW/CoBuyerAgentDirectPhone+Field> ;
  vs:term_status   "stable"
.
reso:CoBuyerAgentEmail a rdf:Property ;
  rdfs:comment     "The email address of the Buyer's Co Agent." ;
  rdfs:domain      reso:Property ;
  rdfs:label       "CoBuyerAgentEmail" ;
  rdfs:range       xsd:string ;
  reso:CertificationLevel "Core" ;
  reso:PropertyTypes "RESI","RLSE","RINC","LAND","MOBI","FARM","COMS","COML","BUSO" ;
  schema:sameAs    <http://ddwiki.reso.org/display/DDW/CoBuyerAgentEmail+Field> ;
  vs:term_status   "stable"
.
reso:CoBuyerAgentFax a rdf:Property ;
  rdfs:comment     "North American 10 digit phone numbers should be in the format of ###-###-#### (separated by hyphens).  Other conventions should use the common local standard.  International numbers should be preceded by a plus symbol." ;
  rdfs:domain      reso:Property ;
  rdfs:label       "CoBuyerAgentFax" ;
  rdfs:range       xsd:string ;
  reso:CertificationLevel "Bronze" ;
  reso:PropertyTypes "RESI","RLSE","RINC","LAND","MOBI","FARM","COMS","COML","BUSO" ;
  schema:sameAs    <http://ddwiki.reso.org/display/DDW/CoBuyerAgentFax+Field> ;
  vs:term_status   "stable"
.
reso:CoBuyerAgentFirstName a rdf:Property ;
  rdfs:comment     "The first name of the buyer's co-agent." ;
  rdfs:domain      reso:Property ;
  rdfs:label       "CoBuyerAgentFirstName" ;
  rdfs:range       xsd:string ;
  reso:CertificationLevel "Core" ;
  reso:PropertyTypes "RESI","RLSE","RINC","LAND","MOBI","FARM","COMS","COML","BUSO" ;
  schema:sameAs    <http://ddwiki.reso.org/display/DDW/CoBuyerAgentFirstName+Field> ;
  vs:term_status   "stable"
.
reso:CoBuyerAgentFullName a rdf:Property ;
  rdfs:comment     "The full name of the buyer's co-agent. (First Middle Last)" ;
  rdfs:domain      reso:Property ;
  rdfs:label       "CoBuyerAgentFullName" ;
  rdfs:range       xsd:string ;
  reso:CertificationLevel "Bronze" ;
  reso:PropertyTypes "RESI","RLSE","RINC","LAND","MOBI","FARM","COMS","COML","BUSO" ;
  schema:sameAs    <http://ddwiki.reso.org/display/DDW/CoBuyerAgentFullName+Field> ;
  vs:term_status   "stable"
.
reso:CoBuyerAgentHomePhone a rdf:Property ;
  rdfs:comment     "North American 10 digit phone numbers should be in the format of ###-###-#### (separated by hyphens).  Other conventions should use the common local standard.  International numbers should be preceded by a plus symbol." ;
  rdfs:domain      reso:Property ;
  rdfs:label       "CoBuyerAgentHomePhone" ;
  rdfs:range       xsd:string ;
  reso:CertificationLevel "Bronze" ;
  reso:PropertyTypes "RESI","RLSE","RINC","LAND","MOBI","FARM","COMS","COML","BUSO" ;
  schema:sameAs    <http://ddwiki.reso.org/display/DDW/CoBuyerAgentHomePhone+Field> ;
  vs:term_status   "stable"
.
reso:CoBuyerAgentKey a rdf:Property ;
  rdfs:comment     "A system unique identifier. Specifically, in aggregation systems, the Key is the system unique identifier from the system that the record was just retrieved. This may be identical to the related xxxId identifier, but the key is guaranteed unique for this record set.  This is a foreign key relating to the Member resource's MemberKey." ;
  rdfs:domain      reso:Property ;
  rdfs:label       "CoBuyerAgentKey" ;
  rdfs:range       xsd:string ;
  reso:CertificationLevel "Core" ;
  reso:PropertyTypes "RESI","RLSE","RINC","LAND","MOBI","FARM","COMS","COML","BUSO" ;
  schema:sameAs    <http://ddwiki.reso.org/display/DDW/CoBuyerAgentKey+Field> ;
  vs:term_status   "stable"
.
reso:CoBuyerAgentKeyNumeric a rdf:Property ;
  rdfs:comment     "A system unique identifier. Specifically, in aggregation systems, the Key is the system unique identifier from the system that the record was just retrieved. This may be identical to the related xxxId identifier, but the key is guaranteed unique for this record set.  This is a foreign key relating to the Member resource's MemberKey.  This is the numeric only key and used as an alternative to the CoBuyerAgentKey field." ;
  rdfs:domain      reso:Property ;
  rdfs:label       "CoBuyerAgentKeyNumeric" ;
  rdfs:range       xsd:decimal ;
  reso:CertificationLevel "Platinum" ;
  reso:PropertyTypes "RESI","RLSE","RINC","LAND","MOBI","FARM","COMS","COML","BUSO" ;
  schema:sameAs    <http://ddwiki.reso.org/display/DDW/CoBuyerAgentKeyNumeric+Field> ;
  vs:term_status   "stable"
.
reso:CoBuyerAgentLastName a rdf:Property ;
  rdfs:comment     "The last name of the buyer's co-agent." ;
  rdfs:domain      reso:Property ;
  rdfs:label       "CoBuyerAgentLastName" ;
  rdfs:range       xsd:string ;
  reso:CertificationLevel "Core" ;
  reso:PropertyTypes "RESI","RLSE","RINC","LAND","MOBI","FARM","COMS","COML","BUSO" ;
  schema:sameAs    <http://ddwiki.reso.org/display/DDW/CoBuyerAgentLastName+Field> ;
  vs:term_status   "stable"
.
reso:CoBuyerAgentMiddleName a rdf:Property ;
  rdfs:comment     "The middle name of the buyer's co-agent." ;
  rdfs:domain      reso:Property ;
  rdfs:label       "CoBuyerAgentMiddleName" ;
  rdfs:range       xsd:string ;
  reso:CertificationLevel "Core" ;
  reso:PropertyTypes "RESI","RLSE","RINC","LAND","MOBI","FARM","COMS","COML","BUSO" ;
  schema:sameAs    <http://ddwiki.reso.org/display/DDW/CoBuyerAgentMiddleName+Field> ;
  vs:term_status   "stable"
.
reso:CoBuyerAgentMlsId a rdf:Property ;
  rdfs:comment     "The local, well-known identifier. This value may not be unique, specifically in the case of aggregation systems, this value should be the identifier from the original system." ;
  rdfs:domain      reso:Property ;
  rdfs:label       "CoBuyerAgentMlsId" ;
  rdfs:range       xsd:string ;
  reso:CertificationLevel "Core" ;
  reso:PropertyTypes "RESI","RLSE","RINC","LAND","MOBI","FARM","COMS","COML","BUSO" ;
  schema:sameAs    <http://ddwiki.reso.org/display/DDW/CoBuyerAgentMlsId+Field> ;
  vs:term_status   "stable"
.
reso:CoBuyerAgentNamePrefix a rdf:Property ;
  rdfs:comment     "Prefix to the name (e.g. Dr. Mr. Ms. etc.)" ;
  rdfs:domain      reso:Property ;
  rdfs:label       "CoBuyerAgentNamePrefix" ;
  rdfs:range       xsd:string ;
  reso:CertificationLevel "Bronze" ;
  reso:PropertyTypes "RESI","RLSE","RINC","LAND","MOBI","FARM","COMS","COML","BUSO" ;
  schema:sameAs    <http://ddwiki.reso.org/display/DDW/CoBuyerAgentNamePrefix+Field> ;
  vs:term_status   "stable"
.
reso:CoBuyerAgentNameSuffix a rdf:Property ;
  rdfs:comment     "Suffix to the CoBuyerAgentLastName (e.g. Esq.,  Jr.,  III etc.)" ;
  rdfs:domain      reso:Property ;
  rdfs:label       "CoBuyerAgentNameSuffix" ;
  rdfs:range       xsd:string ;
  reso:CertificationLevel "Bronze" ;
  reso:PropertyTypes "RESI","RLSE","RINC","LAND","MOBI","FARM","COMS","COML","BUSO" ;
  schema:sameAs    <http://ddwiki.reso.org/display/DDW/CoBuyerAgentNameSuffix+Field> ;
  vs:term_status   "stable"
.
reso:CoBuyerAgentOfficePhone a rdf:Property ;
  rdfs:comment     "North American 10 digit phone numbers should be in the format of ###-###-#### (separated by hyphens).  Other conventions should use the common local standard.  International numbers should be preceded by a plus symbol." ;
  rdfs:domain      reso:Property ;
  rdfs:label       "CoBuyerAgentOfficePhone" ;
  rdfs:range       xsd:string ;
  reso:CertificationLevel "Core" ;
  reso:PropertyTypes "RESI","RLSE","RINC","LAND","MOBI","FARM","COMS","COML","BUSO" ;
  schema:sameAs    <http://ddwiki.reso.org/display/DDW/CoBuyerAgentOfficePhone+Field> ;
  vs:term_status   "stable"
.
reso:CoBuyerAgentOfficePhoneExt a rdf:Property ;
  rdfs:comment     "The extension of the given phone number (if applicable)." ;
  rdfs:domain      reso:Property ;
  rdfs:label       "CoBuyerAgentOfficePhoneExt" ;
  rdfs:range       xsd:string ;
  reso:CertificationLevel "Core" ;
  reso:PropertyTypes "RESI","RLSE","RINC","LAND","MOBI","FARM","COMS","COML","BUSO" ;
  schema:sameAs    <http://ddwiki.reso.org/display/DDW/CoBuyerAgentOfficePhoneExt+Field> ;
  vs:term_status   "stable"
.
reso:CoBuyerAgentPager a rdf:Property ;
  rdfs:comment     "North American 10 digit phone numbers should be in the format of ###-###-#### (separated by hyphens).  Other conventions should use the common local standard.  International numbers should be preceded by a plus symbol." ;
  rdfs:domain      reso:Property ;
  rdfs:label       "CoBuyerAgentPager" ;
  rdfs:range       xsd:string ;
  reso:CertificationLevel "Bronze" ;
  reso:PropertyTypes "RESI","RLSE","RINC","LAND","MOBI","FARM","COMS","COML","BUSO" ;
  schema:sameAs    <http://ddwiki.reso.org/display/DDW/CoBuyerAgentPager+Field> ;
  vs:term_status   "stable"
.
reso:CoBuyerAgentPreferredPhone a rdf:Property ;
  rdfs:comment     "North American 10 digit phone numbers should be in the format of ###-###-#### (separated by hyphens).  Other conventions should use the common local standard.  International numbers should be preceded by a plus symbol." ;
  rdfs:domain      reso:Property ;
  rdfs:label       "CoBuyerAgentPreferredPhone" ;
  rdfs:range       xsd:string ;
  reso:CertificationLevel "Core" ;
  reso:PropertyTypes "RESI","RLSE","RINC","LAND","MOBI","FARM","COMS","COML","BUSO" ;
  schema:sameAs    <http://ddwiki.reso.org/display/DDW/CoBuyerAgentPreferredPhone+Field> ;
  vs:term_status   "stable"
.
reso:CoBuyerAgentPreferredPhoneExt a rdf:Property ;
  rdfs:comment     "The extension of the given phone number (if applicable)." ;
  rdfs:domain      reso:Property ;
  rdfs:label       "CoBuyerAgentPreferredPhoneExt" ;
  rdfs:range       xsd:string ;
  reso:CertificationLevel "Core" ;
  reso:PropertyTypes "RESI","RLSE","RINC","LAND","MOBI","FARM","COMS","COML","BUSO" ;
  schema:sameAs    <http://ddwiki.reso.org/display/DDW/CoBuyerAgentPreferredPhoneExt+Field> ;
  vs:term_status   "stable"
.
reso:CoBuyerAgentStateLicense a rdf:Property ;
  rdfs:comment     "The license of the co-buyers agent. Separate multiple licenses with a comma and space." ;
  rdfs:domain      reso:Property ;
  rdfs:label       "CoBuyerAgentStateLicense" ;
  rdfs:range       xsd:string ;
  reso:CertificationLevel "Bronze" ;
  reso:PropertyTypes "RESI","RLSE","RINC","LAND","MOBI","FARM","COMS","COML","BUSO" ;
  schema:sameAs    <http://ddwiki.reso.org/display/DDW/CoBuyerAgentStateLicense+Field> ;
  vs:term_status   "stable"
.
reso:CoBuyerAgentTollFreePhone a rdf:Property ;
  rdfs:comment     "North American 10 digit phone numbers should be in the format of ###-###-#### (separated by hyphens).  Other conventions should use the common local standard.  International numbers should be preceded by a plus symbol." ;
  rdfs:domain      reso:Property ;
  rdfs:label       "CoBuyerAgentTollFreePhone" ;
  rdfs:range       xsd:string ;
  reso:CertificationLevel "Bronze" ;
  reso:PropertyTypes "RESI","RLSE","RINC","LAND","MOBI","FARM","COMS","COML","BUSO" ;
  schema:sameAs    <http://ddwiki.reso.org/display/DDW/CoBuyerAgentTollFreePhone+Field> ;
  vs:term_status   "stable"
.
reso:CoBuyerAgentURL a rdf:Property ;
  rdfs:comment     "The website URI of the co-buyers agent." ;
  rdfs:domain      reso:Property ;
  rdfs:label       "CoBuyerAgentURL" ;
  rdfs:range       xsd:string ;
  reso:CertificationLevel "Bronze" ;
  reso:PropertyTypes "RESI","RLSE","RINC","LAND","MOBI","FARM","COMS","COML","BUSO" ;
  schema:sameAs    <http://ddwiki.reso.org/display/DDW/CoBuyerAgentURL+Field> ;
  vs:term_status   "stable"
.
reso:CoBuyerAgentVoiceMail a rdf:Property ;
  rdfs:comment     "North American 10 digit phone numbers should be in the format of ###-###-#### (separated by hyphens).  Other conventions should use the common local standard.  International numbers should be preceded by a plus symbol." ;
  rdfs:domain      reso:Property ;
  rdfs:label       "CoBuyerAgentVoiceMail" ;
  rdfs:range       xsd:string ;
  reso:CertificationLevel "Bronze" ;
  reso:PropertyTypes "RESI","RLSE","RINC","LAND","MOBI","FARM","COMS","COML","BUSO" ;
  schema:sameAs    <http://ddwiki.reso.org/display/DDW/CoBuyerAgentVoiceMail+Field> ;
  vs:term_status   "stable"
.
reso:CoBuyerAgentVoiceMailExt a rdf:Property ;
  rdfs:comment     "The extension of the given phone number (if applicable)." ;
  rdfs:domain      reso:Property ;
  rdfs:label       "CoBuyerAgentVoiceMailExt" ;
  rdfs:range       xsd:string ;
  reso:CertificationLevel "Bronze" ;
  reso:PropertyTypes "RESI","RLSE","RINC","LAND","MOBI","FARM","COMS","COML","BUSO" ;
  schema:sameAs    <http://ddwiki.reso.org/display/DDW/CoBuyerAgentVoiceMailExt+Field> ;
  vs:term_status   "stable"
.
reso:CoBuyerOfficeAOR a rdf:Property ;
  rdfs:comment     "The Co Buyer's Office's Board or Association of REALTORS." ;
  rdfs:domain      reso:Property ;
  rdfs:label       "CoBuyerOfficeAOR" ;
  rdfs:range       xsd:string ;
  reso:CertificationLevel "Bronze" ;
  reso:PropertyTypes "RESI","RLSE","RINC","LAND","MOBI","FARM","COMS","COML","BUSO" ;
  schema:sameAs    <http://ddwiki.reso.org/display/DDW/CoBuyerOfficeAOR+Field> ;
  vs:term_status   "stable"
.
reso:CoBuyerOfficeEmail a rdf:Property ;
  rdfs:comment     "The email address of the Buyer's Co Office." ;
  rdfs:domain      reso:Property ;
  rdfs:label       "CoBuyerOfficeEmail" ;
  rdfs:range       xsd:string ;
  reso:CertificationLevel "Bronze" ;
  reso:PropertyTypes "RESI","RLSE","RINC","LAND","MOBI","FARM","COMS","COML","BUSO" ;
  schema:sameAs    <http://ddwiki.reso.org/display/DDW/CoBuyerOfficeEmail+Field> ;
  vs:term_status   "stable"
.
reso:CoBuyerOfficeFax a rdf:Property ;
  rdfs:comment     "North American 10 digit phone numbers should be in the format of ###-###-#### (separated by hyphens).  Other conventions should use the common local standard.  International numbers should be preceded by a plus symbol." ;
  rdfs:domain      reso:Property ;
  rdfs:label       "CoBuyerOfficeFax" ;
  rdfs:range       xsd:string ;
  reso:CertificationLevel "Bronze" ;
  reso:PropertyTypes "RESI","RLSE","RINC","LAND","MOBI","FARM","COMS","COML","BUSO" ;
  schema:sameAs    <http://ddwiki.reso.org/display/DDW/CoBuyerOfficeFax+Field> ;
  vs:term_status   "stable"
.
reso:CoBuyerOfficeKey a rdf:Property ;
  rdfs:comment     "A system unique identifier. Specifically, in aggregation systems, the Key is the system unique identifier from the system that the record was just retrieved. This may be identical to the related xxxId identifier, but the key is guaranteed unique for this record set.  This is a foreign key relating to the Office resource's OfficeKey." ;
  rdfs:domain      reso:Property ;
  rdfs:label       "CoBuyerOfficeKey" ;
  rdfs:range       xsd:string ;
  reso:CertificationLevel "Core" ;
  reso:PropertyTypes "RESI","RLSE","RINC","LAND","MOBI","FARM","COMS","COML","BUSO" ;
  schema:sameAs    <http://ddwiki.reso.org/display/DDW/CoBuyerOfficeKey+Field> ;
  vs:term_status   "stable"
.
reso:CoBuyerOfficeKeyNumeric a rdf:Property ;
  rdfs:comment     "A system unique identifier. Specifically, in aggregation systems, the Key is the system unique identifier from the system that the record was just retrieved. This may be identical to the related xxxId identifier, but the key is guaranteed unique for this record set.  This is a foreign key relating to the Office resource's OfficeKey.  This is the numeric only key and used as an alternative to the CoBuyerOfficeKey field." ;
  rdfs:domain      reso:Property ;
  rdfs:label       "CoBuyerOfficeKeyNumeric" ;
  rdfs:range       xsd:decimal ;
  reso:CertificationLevel "Platinum" ;
  reso:PropertyTypes "RESI","RLSE","RINC","LAND","MOBI","FARM","COMS","COML","BUSO" ;
  schema:sameAs    <http://ddwiki.reso.org/display/DDW/CoBuyerOfficeKeyNumeric+Field> ;
  vs:term_status   "stable"
.
reso:CoBuyerOfficeMlsId a rdf:Property ;
  rdfs:comment     "The local, well-known identifier. This value may not be unique, specifically in the case of aggregation systems, this value should be the identifier from the original system." ;
  rdfs:domain      reso:Property ;
  rdfs:label       "CoBuyerOfficeMlsId" ;
  rdfs:range       xsd:string ;
  reso:CertificationLevel "Core" ;
  reso:PropertyTypes "RESI","RLSE","RINC","LAND","MOBI","FARM","COMS","COML","BUSO" ;
  schema:sameAs    <http://ddwiki.reso.org/display/DDW/CoBuyerOfficeMlsId+Field> ;
  vs:term_status   "stable"
.
reso:CoBuyerOfficeName a rdf:Property ;
  rdfs:comment     "The legal name of the brokerage co-representing the buyer." ;
  rdfs:domain      reso:Property ;
  rdfs:label       "CoBuyerOfficeName" ;
  rdfs:range       xsd:string ;
  reso:CertificationLevel "Core" ;
  reso:PropertyTypes "RESI","RLSE","RINC","LAND","MOBI","FARM","COMS","COML","BUSO" ;
  schema:sameAs    <http://ddwiki.reso.org/display/DDW/CoBuyerOfficeName+Field> ;
  vs:term_status   "stable"
.
reso:CoBuyerOfficePhone a rdf:Property ;
  rdfs:comment     "North American 10 digit phone numbers should be in the format of ###-###-#### (separated by hyphens).  Other conventions should use the common local standard.  International numbers should be preceded by a plus symbol." ;
  rdfs:domain      reso:Property ;
  rdfs:label       "CoBuyerOfficePhone" ;
  rdfs:range       xsd:string ;
  reso:CertificationLevel "Core" ;
  reso:PropertyTypes "RESI","RLSE","RINC","LAND","MOBI","FARM","COMS","COML","BUSO" ;
  schema:sameAs    <http://ddwiki.reso.org/display/DDW/CoBuyerOfficePhone+Field> ;
  vs:term_status   "stable"
.
reso:CoBuyerOfficePhoneExt a rdf:Property ;
  rdfs:comment     "The extension of the given phone number (if applicable)." ;
  rdfs:domain      reso:Property ;
  rdfs:label       "CoBuyerOfficePhoneExt" ;
  rdfs:range       xsd:string ;
  reso:CertificationLevel "Core" ;
  reso:PropertyTypes "RESI","RLSE","RINC","LAND","MOBI","FARM","COMS","COML","BUSO" ;
  schema:sameAs    <http://ddwiki.reso.org/display/DDW/CoBuyerOfficePhoneExt+Field> ;
  vs:term_status   "stable"
.
reso:CoBuyerOfficeURL a rdf:Property ;
  rdfs:comment     "The website URI for the co-buyers office." ;
  rdfs:domain      reso:Property ;
  rdfs:label       "CoBuyerOfficeURL" ;
  rdfs:range       xsd:string ;
  reso:CertificationLevel "Bronze" ;
  reso:PropertyTypes "RESI","RLSE","RINC","LAND","MOBI","FARM","COMS","COML","BUSO" ;
  schema:sameAs    <http://ddwiki.reso.org/display/DDW/CoBuyerOfficeURL+Field> ;
  vs:term_status   "stable"
.
reso:CoListAgentAOR a rdf:Property ;
  rdfs:comment     "The Co Listing Agent's Board or Association of REALTORS." ;
  rdfs:domain      reso:Property ;
  rdfs:label       "CoListAgentAOR" ;
  rdfs:range       xsd:string ;
  reso:CertificationLevel "Bronze" ;
  reso:PropertyTypes "RESI","RLSE","RINC","LAND","MOBI","FARM","COMS","COML","BUSO" ;
  schema:sameAs    <http://ddwiki.reso.org/display/DDW/CoListAgentAOR+Field> ;
  vs:term_status   "stable"
.
reso:CoListAgentCellPhone a rdf:Property ;
  rdfs:comment     "North American 10 digit phone numbers should be in the format of ###-###-#### (separated by hyphens).  Other conventions should use the common local standard.  International numbers should be preceded by a plus symbol." ;
  rdfs:domain      reso:Property ;
  rdfs:label       "CoListAgentCellPhone" ;
  rdfs:range       xsd:string ;
  reso:CertificationLevel "Core" ;
  reso:PropertyTypes "RESI","RLSE","RINC","LAND","MOBI","FARM","COMS","COML","BUSO" ;
  schema:sameAs    <http://ddwiki.reso.org/display/DDW/CoListAgentCellPhone+Field> ;
  vs:term_status   "stable"
.
reso:CoListAgentDesignation a rdf:Property ;
  rdfs:comment     "Designations and certifications acknowledging experience and expertise in various real estate sectors are awarded by NAR and each affiliated group upon completion of required courses." ;
  rdfs:domain      reso:Property ;
  rdfs:label       "CoListAgentDesignation" ;
  rdfs:range       xsd:string ;
  reso:CertificationLevel "Bronze" ;
  reso:PropertyTypes "RESI","RLSE","RINC","LAND","MOBI","FARM","COMS","COML","BUSO" ;
  schema:sameAs    <http://ddwiki.reso.org/display/DDW/CoListAgentDesignation+Field> ;
  vs:term_status   "stable"
.
reso:CoListAgentDirectPhone a rdf:Property ;
  rdfs:comment     "North American 10 digit phone numbers should be in the format of ###-###-#### (separated by hyphens).  Other conventions should use the common local standard.  International numbers should be preceded by a plus symbol." ;
  rdfs:domain      reso:Property ;
  rdfs:label       "CoListAgentDirectPhone" ;
  rdfs:range       xsd:string ;
  reso:CertificationLevel "Bronze" ;
  reso:PropertyTypes "RESI","RLSE","RINC","LAND","MOBI","FARM","COMS","COML","BUSO" ;
  schema:sameAs    <http://ddwiki.reso.org/display/DDW/CoListAgentDirectPhone+Field> ;
  vs:term_status   "stable"
.
reso:CoListAgentEmail a rdf:Property ;
  rdfs:comment     "The email address of the Co Listing Agent." ;
  rdfs:domain      reso:Property ;
  rdfs:label       "CoListAgentEmail" ;
  rdfs:range       xsd:string ;
  reso:CertificationLevel "Core" ;
  reso:PropertyTypes "RESI","RLSE","RINC","LAND","MOBI","FARM","COMS","COML","BUSO" ;
  schema:sameAs    <http://ddwiki.reso.org/display/DDW/CoListAgentEmail+Field> ;
  vs:term_status   "stable"
.
reso:CoListAgentFax a rdf:Property ;
  rdfs:comment     "North American 10 digit phone numbers should be in the format of ###-###-#### (separated by hyphens).  Other conventions should use the common local standard.  International numbers should be preceded by a plus symbol." ;
  rdfs:domain      reso:Property ;
  rdfs:label       "CoListAgentFax" ;
  rdfs:range       xsd:string ;
  reso:CertificationLevel "Bronze" ;
  reso:PropertyTypes "RESI","RLSE","RINC","LAND","MOBI","FARM","COMS","COML","BUSO" ;
  schema:sameAs    <http://ddwiki.reso.org/display/DDW/CoListAgentFax+Field> ;
  vs:term_status   "stable"
.
reso:CoListAgentFirstName a rdf:Property ;
  rdfs:comment     "The first name of the co-listing agent." ;
  rdfs:domain      reso:Property ;
  rdfs:label       "CoListAgentFirstName" ;
  rdfs:range       xsd:string ;
  reso:CertificationLevel "Core" ;
  reso:PropertyTypes "RESI","RLSE","RINC","LAND","MOBI","FARM","COMS","COML","BUSO" ;
  schema:sameAs    <http://ddwiki.reso.org/display/DDW/CoListAgentFirstName+Field> ;
  vs:term_status   "stable"
.
reso:CoListAgentFullName a rdf:Property ;
  rdfs:comment     "The full name of the co-listing agent. (First Middle Last)" ;
  rdfs:domain      reso:Property ;
  rdfs:label       "CoListAgentFullName" ;
  rdfs:range       xsd:string ;
  reso:CertificationLevel "Bronze" ;
  reso:PropertyTypes "RESI","RLSE","RINC","LAND","MOBI","FARM","COMS","COML","BUSO" ;
  schema:sameAs    <http://ddwiki.reso.org/display/DDW/CoListAgentFullName+Field> ;
  vs:term_status   "stable"
.
reso:CoListAgentHomePhone a rdf:Property ;
  rdfs:comment     "North American 10 digit phone numbers should be in the format of ###-###-#### (separated by hyphens).  Other conventions should use the common local standard.  International numbers should be preceded by a plus symbol." ;
  rdfs:domain      reso:Property ;
  rdfs:label       "CoListAgentHomePhone" ;
  rdfs:range       xsd:string ;
  reso:CertificationLevel "Bronze" ;
  reso:PropertyTypes "RESI","RLSE","RINC","LAND","MOBI","FARM","COMS","COML","BUSO" ;
  schema:sameAs    <http://ddwiki.reso.org/display/DDW/CoListAgentHomePhone+Field> ;
  vs:term_status   "stable"
.
reso:CoListAgentKey a rdf:Property ;
  rdfs:comment     "A system unique identifier. Specifically, in aggregation systems, the Key is the system unique identifier from the system that the record was just retrieved. This may be identical to the related xxxId identifier, but the key is guaranteed unique for this record set.  This is a foreign key relating to the Member resource's MemberKey." ;
  rdfs:domain      reso:Property ;
  rdfs:label       "CoListAgentKey" ;
  rdfs:range       xsd:string ;
  reso:CertificationLevel "Core" ;
  reso:PropertyTypes "RESI","RLSE","RINC","LAND","MOBI","FARM","COMS","COML","BUSO" ;
  schema:sameAs    <http://ddwiki.reso.org/display/DDW/CoListAgentKey+Field> ;
  vs:term_status   "stable"
.
reso:CoListAgentKeyNumeric a rdf:Property ;
  rdfs:comment     "A system unique identifier. Specifically, in aggregation systems, the Key is the system unique identifier from the system that the record was just retrieved. This may be identical to the related xxxId identifier, but the key is guaranteed unique for this record set.  This is a foreign key relating to the Member resource's MemberKey.  This is the numeric only key and used as an alternative to the CoListAgentKey field." ;
  rdfs:domain      reso:Property ;
  rdfs:label       "CoListAgentKeyNumeric" ;
  rdfs:range       xsd:decimal ;
  reso:CertificationLevel "Platinum" ;
  reso:PropertyTypes "RESI","RLSE","RINC","LAND","MOBI","FARM","COMS","COML","BUSO" ;
  schema:sameAs    <http://ddwiki.reso.org/display/DDW/CoListAgentKeyNumeric+Field> ;
  vs:term_status   "stable"
.
reso:CoListAgentLastName a rdf:Property ;
  rdfs:comment     "The last name of the co-listing agent." ;
  rdfs:domain      reso:Property ;
  rdfs:label       "CoListAgentLastName" ;
  rdfs:range       xsd:string ;
  reso:CertificationLevel "Core" ;
  reso:PropertyTypes "RESI","RLSE","RINC","LAND","MOBI","FARM","COMS","COML","BUSO" ;
  schema:sameAs    <http://ddwiki.reso.org/display/DDW/CoListAgentLastName+Field> ;
  vs:term_status   "stable"
.
reso:CoListAgentMiddleName a rdf:Property ;
  rdfs:comment     "The middle name of the co-listing agent." ;
  rdfs:domain      reso:Property ;
  rdfs:label       "CoListAgentMiddleName" ;
  rdfs:range       xsd:string ;
  reso:CertificationLevel "Core" ;
  reso:PropertyTypes "RESI","RLSE","RINC","LAND","MOBI","FARM","COMS","COML","BUSO" ;
  schema:sameAs    <http://ddwiki.reso.org/display/DDW/CoListAgentMiddleName+Field> ;
  vs:term_status   "stable"
.
reso:CoListAgentMlsId a rdf:Property ;
  rdfs:comment     "The local, well-known identifier. This value may not be unique, specifically in the case of aggregation systems, this value should be the identifier from the original system." ;
  rdfs:domain      reso:Property ;
  rdfs:label       "CoListAgentMlsId" ;
  rdfs:range       xsd:string ;
  reso:CertificationLevel "Core" ;
  reso:PropertyTypes "RESI","RLSE","RINC","LAND","MOBI","FARM","COMS","COML","BUSO" ;
  schema:sameAs    <http://ddwiki.reso.org/display/DDW/CoListAgentMlsId+Field> ;
  vs:term_status   "stable"
.
reso:CoListAgentNamePrefix a rdf:Property ;
  rdfs:comment     "Prefix to the name (e.g. Dr. Mr. Ms. etc.)" ;
  rdfs:domain      reso:Property ;
  rdfs:label       "CoListAgentNamePrefix" ;
  rdfs:range       xsd:string ;
  reso:CertificationLevel "Bronze" ;
  reso:PropertyTypes "RESI","RLSE","RINC","LAND","MOBI","FARM","COMS","COML","BUSO" ;
  schema:sameAs    <http://ddwiki.reso.org/display/DDW/CoListAgentNamePrefix+Field> ;
  vs:term_status   "stable"
.
reso:CoListAgentNameSuffix a rdf:Property ;
  rdfs:comment     "Suffix to the CoListAgentLastName (e.g. Esq.,  Jr.,  III etc.)" ;
  rdfs:domain      reso:Property ;
  rdfs:label       "CoListAgentNameSuffix" ;
  rdfs:range       xsd:string ;
  reso:CertificationLevel "Bronze" ;
  reso:PropertyTypes "RESI","RLSE","RINC","LAND","MOBI","FARM","COMS","COML","BUSO" ;
  schema:sameAs    <http://ddwiki.reso.org/display/DDW/CoListAgentNameSuffix+Field> ;
  vs:term_status   "stable"
.
reso:CoListAgentOfficePhone a rdf:Property ;
  rdfs:comment     "North American 10 digit phone numbers should be in the format of ###-###-#### (separated by hyphens).  Other conventions should use the common local standard.  International numbers should be preceded by a plus symbol." ;
  rdfs:domain      reso:Property ;
  rdfs:label       "CoListAgentOfficePhone" ;
  rdfs:range       xsd:string ;
  reso:CertificationLevel "Core" ;
  reso:PropertyTypes "RESI","RLSE","RINC","LAND","MOBI","FARM","COMS","COML","BUSO" ;
  schema:sameAs    <http://ddwiki.reso.org/display/DDW/CoListAgentOfficePhone+Field> ;
  vs:term_status   "stable"
.
reso:CoListAgentOfficePhoneExt a rdf:Property ;
  rdfs:comment     "The extension of the given phone number (if applicable)." ;
  rdfs:domain      reso:Property ;
  rdfs:label       "CoListAgentOfficePhoneExt" ;
  rdfs:range       xsd:string ;
  reso:CertificationLevel "Core" ;
  reso:PropertyTypes "RESI","RLSE","RINC","LAND","MOBI","FARM","COMS","COML","BUSO" ;
  schema:sameAs    <http://ddwiki.reso.org/display/DDW/CoListAgentOfficePhoneExt+Field> ;
  vs:term_status   "stable"
.
reso:CoListAgentPager a rdf:Property ;
  rdfs:comment     "North American 10 digit phone numbers should be in the format of ###-###-#### (separated by hyphens).  Other conventions should use the common local standard.  International numbers should be preceded by a plus symbol." ;
  rdfs:domain      reso:Property ;
  rdfs:label       "CoListAgentPager" ;
  rdfs:range       xsd:string ;
  reso:CertificationLevel "Bronze" ;
  reso:PropertyTypes "RESI","RLSE","RINC","LAND","MOBI","FARM","COMS","COML","BUSO" ;
  schema:sameAs    <http://ddwiki.reso.org/display/DDW/CoListAgentPager+Field> ;
  vs:term_status   "stable"
.
reso:CoListAgentPreferredPhone a rdf:Property ;
  rdfs:comment     "North American 10 digit phone numbers should be in the format of ###-###-#### (separated by hyphens).  Other conventions should use the common local standard.  International numbers should be preceded by a plus symbol." ;
  rdfs:domain      reso:Property ;
  rdfs:label       "CoListAgentPreferredPhone" ;
  rdfs:range       xsd:string ;
  reso:CertificationLevel "Core" ;
  reso:PropertyTypes "RESI","RLSE","RINC","LAND","MOBI","FARM","COMS","COML","BUSO" ;
  schema:sameAs    <http://ddwiki.reso.org/display/DDW/CoListAgentPreferredPhone+Field> ;
  vs:term_status   "stable"
.
reso:CoListAgentPreferredPhoneExt a rdf:Property ;
  rdfs:comment     "The extension of the given phone number (if applicable)." ;
  rdfs:domain      reso:Property ;
  rdfs:label       "CoListAgentPreferredPhoneExt" ;
  rdfs:range       xsd:string ;
  reso:CertificationLevel "Core" ;
  reso:PropertyTypes "RESI","RLSE","RINC","LAND","MOBI","FARM","COMS","COML","BUSO" ;
  schema:sameAs    <http://ddwiki.reso.org/display/DDW/CoListAgentPreferredPhoneExt+Field> ;
  vs:term_status   "stable"
.
reso:CoListAgentStateLicense a rdf:Property ;
  rdfs:comment     "The license of the co-listing agent. Separate multiple licenses with a comma and space." ;
  rdfs:domain      reso:Property ;
  rdfs:label       "CoListAgentStateLicense" ;
  rdfs:range       xsd:string ;
  reso:CertificationLevel "Core" ;
  reso:PropertyTypes "RESI","RLSE","RINC","LAND","MOBI","FARM","COMS","COML","BUSO" ;
  schema:sameAs    <http://ddwiki.reso.org/display/DDW/CoListAgentStateLicense+Field> ;
  vs:term_status   "stable"
.
reso:CoListAgentTollFreePhone a rdf:Property ;
  rdfs:comment     "North American 10 digit phone numbers should be in the format of ###-###-#### (separated by hyphens).  Other conventions should use the common local standard.  International numbers should be preceded by a plus symbol." ;
  rdfs:domain      reso:Property ;
  rdfs:label       "CoListAgentTollFreePhone" ;
  rdfs:range       xsd:string ;
  reso:CertificationLevel "Bronze" ;
  reso:PropertyTypes "RESI","RLSE","RINC","LAND","MOBI","FARM","COMS","COML","BUSO" ;
  schema:sameAs    <http://ddwiki.reso.org/display/DDW/CoListAgentTollFreePhone+Field> ;
  vs:term_status   "stable"
.
reso:CoListAgentURL a rdf:Property ;
  rdfs:comment     "The website URI of the co-listing agent." ;
  rdfs:domain      reso:Property ;
  rdfs:label       "CoListAgentURL" ;
  rdfs:range       xsd:string ;
  reso:CertificationLevel "Bronze" ;
  reso:PropertyTypes "RESI","RLSE","RINC","LAND","MOBI","FARM","COMS","COML","BUSO" ;
  schema:sameAs    <http://ddwiki.reso.org/display/DDW/CoListAgentURL+Field> ;
  vs:term_status   "stable"
.
reso:CoListAgentVoiceMail a rdf:Property ;
  rdfs:comment     "North American 10 digit phone numbers should be in the format of ###-###-#### (separated by hyphens).  Other conventions should use the common local standard.  International numbers should be preceded by a plus symbol." ;
  rdfs:domain      reso:Property ;
  rdfs:label       "CoListAgentVoiceMail" ;
  rdfs:range       xsd:string ;
  reso:CertificationLevel "Bronze" ;
  reso:PropertyTypes "RESI","RLSE","RINC","LAND","MOBI","FARM","COMS","COML","BUSO" ;
  schema:sameAs    <http://ddwiki.reso.org/display/DDW/CoListAgentVoiceMail+Field> ;
  vs:term_status   "stable"
.
reso:CoListAgentVoiceMailExt a rdf:Property ;
  rdfs:comment     "The extension of the given phone number (if applicable)." ;
  rdfs:domain      reso:Property ;
  rdfs:label       "CoListAgentVoiceMailExt" ;
  rdfs:range       xsd:string ;
  reso:CertificationLevel "Bronze" ;
  reso:PropertyTypes "RESI","RLSE","RINC","LAND","MOBI","FARM","COMS","COML","BUSO" ;
  schema:sameAs    <http://ddwiki.reso.org/display/DDW/CoListAgentVoiceMailExt+Field> ;
  vs:term_status   "stable"
.
reso:CoListOfficeAOR a rdf:Property ;
  rdfs:comment     "The Co Listing Office's Board or Association of REALTORS." ;
  rdfs:domain      reso:Property ;
  rdfs:label       "CoListOfficeAOR" ;
  rdfs:range       xsd:string ;
  reso:CertificationLevel "Bronze" ;
  reso:PropertyTypes "RESI","RLSE","RINC","LAND","MOBI","FARM","COMS","COML","BUSO" ;
  schema:sameAs    <http://ddwiki.reso.org/display/DDW/CoListOfficeAOR+Field> ;
  vs:term_status   "stable"
.
reso:CoListOfficeEmail a rdf:Property ;
  rdfs:comment     "The email address of the Co Listing Office." ;
  rdfs:domain      reso:Property ;
  rdfs:label       "CoListOfficeEmail" ;
  rdfs:range       xsd:string ;
  reso:CertificationLevel "Bronze" ;
  reso:PropertyTypes "RESI","RLSE","RINC","LAND","MOBI","FARM","COMS","COML","BUSO" ;
  schema:sameAs    <http://ddwiki.reso.org/display/DDW/CoListOfficeEmail+Field> ;
  vs:term_status   "stable"
.
reso:CoListOfficeFax a rdf:Property ;
  rdfs:comment     "North American 10 digit phone numbers should be in the format of ###-###-#### (separated by hyphens).  Other conventions should use the common local standard.  International numbers should be preceded by a plus symbol." ;
  rdfs:domain      reso:Property ;
  rdfs:label       "CoListOfficeFax" ;
  rdfs:range       xsd:string ;
  reso:CertificationLevel "Bronze" ;
  reso:PropertyTypes "RESI","RLSE","RINC","LAND","MOBI","FARM","COMS","COML","BUSO" ;
  schema:sameAs    <http://ddwiki.reso.org/display/DDW/CoListOfficeFax+Field> ;
  vs:term_status   "stable"
.
reso:CoListOfficeKey a rdf:Property ;
  rdfs:comment     "A system unique identifier. Specifically, in aggregation systems, the Key is the system unique identifier from the system that the record was just retrieved. This may be identical to the related xxxId identifier, but the key is guaranteed unique for this record set.  This is a foreign key relating to the Office resource's OfficeKey." ;
  rdfs:domain      reso:Property ;
  rdfs:label       "CoListOfficeKey" ;
  rdfs:range       xsd:string ;
  reso:CertificationLevel "Core" ;
  reso:PropertyTypes "RESI","RLSE","RINC","LAND","MOBI","FARM","COMS","COML","BUSO" ;
  schema:sameAs    <http://ddwiki.reso.org/display/DDW/CoListOfficeKey+Field> ;
  vs:term_status   "stable"
.
reso:CoListOfficeKeyNumeric a rdf:Property ;
  rdfs:comment     "A system unique identifier. Specifically, in aggregation systems, the Key is the system unique identifier from the system that the record was just retrieved. This may be identical to the related xxxId identifier, but the key is guaranteed unique for this record set.  This is a foreign key relating to the Office resource's OfficeKey.  This is the numeric only key and used as an alternative to the CoListOfficeKey field." ;
  rdfs:domain      reso:Property ;
  rdfs:label       "CoListOfficeKeyNumeric" ;
  rdfs:range       xsd:decimal ;
  reso:CertificationLevel "Platinum" ;
  reso:PropertyTypes "RESI","RLSE","RINC","LAND","MOBI","FARM","COMS","COML","BUSO" ;
  schema:sameAs    <http://ddwiki.reso.org/display/DDW/CoListOfficeKeyNumeric+Field> ;
  vs:term_status   "stable"
.
reso:CoListOfficeMlsId a rdf:Property ;
  rdfs:comment     "The local, well-known identifier. This value may not be unique, specifically in the case of aggregation systems, this value should be the identifier from the original system." ;
  rdfs:domain      reso:Property ;
  rdfs:label       "CoListOfficeMlsId" ;
  rdfs:range       xsd:string ;
  reso:CertificationLevel "Core" ;
  reso:PropertyTypes "RESI","RLSE","RINC","LAND","MOBI","FARM","COMS","COML","BUSO" ;
  schema:sameAs    <http://ddwiki.reso.org/display/DDW/CoListOfficeMlsId+Field> ;
  vs:term_status   "stable"
.
reso:CoListOfficeName a rdf:Property ;
  rdfs:comment     "The legal name of the brokerage co-representing the seller." ;
  rdfs:domain      reso:Property ;
  rdfs:label       "CoListOfficeName" ;
  rdfs:range       xsd:string ;
  reso:CertificationLevel "Core" ;
  reso:PropertyTypes "RESI","RLSE","RINC","LAND","MOBI","FARM","COMS","COML","BUSO" ;
  schema:sameAs    <http://ddwiki.reso.org/display/DDW/CoListOfficeName+Field> ;
  vs:term_status   "stable"
.
reso:CoListOfficePhone a rdf:Property ;
  rdfs:comment     "North American 10 digit phone numbers should be in the format of ###-###-#### (separated by hyphens).  Other conventions should use the common local standard.  International numbers should be preceded by a plus symbol." ;
  rdfs:domain      reso:Property ;
  rdfs:label       "CoListOfficePhone" ;
  rdfs:range       xsd:string ;
  reso:CertificationLevel "Core" ;
  reso:PropertyTypes "RESI","RLSE","RINC","LAND","MOBI","FARM","COMS","COML","BUSO" ;
  schema:sameAs    <http://ddwiki.reso.org/display/DDW/CoListOfficePhone+Field> ;
  vs:term_status   "stable"
.
reso:CoListOfficePhoneExt a rdf:Property ;
  rdfs:comment     "The extension of the given phone number (if applicable)." ;
  rdfs:domain      reso:Property ;
  rdfs:label       "CoListOfficePhoneExt" ;
  rdfs:range       xsd:string ;
  reso:CertificationLevel "Core" ;
  reso:PropertyTypes "RESI","RLSE","RINC","LAND","MOBI","FARM","COMS","COML","BUSO" ;
  schema:sameAs    <http://ddwiki.reso.org/display/DDW/CoListOfficePhoneExt+Field> ;
  vs:term_status   "stable"
.
reso:CoListOfficeURL a rdf:Property ;
  rdfs:comment     "The website URI for the co-listing office." ;
  rdfs:domain      reso:Property ;
  rdfs:label       "CoListOfficeURL" ;
  rdfs:range       xsd:string ;
  reso:CertificationLevel "Bronze" ;
  reso:PropertyTypes "RESI","RLSE","RINC","LAND","MOBI","FARM","COMS","COML","BUSO" ;
  schema:sameAs    <http://ddwiki.reso.org/display/DDW/CoListOfficeURL+Field> ;
  vs:term_status   "stable"
.
reso:CommonWalls a rdf:Property ;
  rdfs:comment     "A multi select list with options like 1 Common Wall, 2 Common Walls, No Common Walls, No One Above, No One Below.  Implementation should include rules preventing illogical selection combinations and to ensure consistency with the Property Attached Y/N field." ;
  rdfs:domain      reso:Property ;
  rdfs:label       "CommonWalls" ;
  rdfs:range       enum:CommonWalls ;
  reso:CertificationLevel "Bronze" ;
  reso:PropertyTypes "RESI","RLSE","RINC","MOBI","FARM" ;
  schema:sameAs    <http://ddwiki.reso.org/display/DDW/CommonWalls+Field> ;
  vs:term_status   "stable"
.
reso:CommunityFeatures a rdf:Property ;
  rdfs:comment     "A list of features related to, or available within, the community." ;
  rdfs:domain      reso:Property ;
  rdfs:label       "CommunityFeatures" ;
  rdfs:range       xsd:string ;
  reso:CertificationLevel "Platinum" ;
  reso:PropertyTypes "RESI","RLSE","RINC","LAND","MOBI","FARM" ;
  schema:sameAs    <http://ddwiki.reso.org/display/DDW/CommunityFeatures+Field> ;
  vs:term_status   "stable"
.
reso:Concessions a rdf:Property ;
  rdfs:comment     "Are there concessions included in the sales agreement? Yes, No or Call Listing Agent" ;
  rdfs:domain      reso:Property ;
  rdfs:label       "Concessions" ;
  rdfs:range       enum:Concessions ;
  reso:CertificationLevel "Silver" ;
  reso:PropertyTypes "RESI","RLSE","RINC","LAND","MOBI","FARM","COMS","COML","BUSO" ;
  schema:sameAs    <http://ddwiki.reso.org/display/DDW/Concessions+Field> ;
  vs:term_status   "stable"
.
reso:ConcessionsAmount a rdf:Property ;
  rdfs:comment     "The dollar amount of the concessions.  If the concessions are made by the seller, some may subtract this value from the sales price as a means of calculating their own true price.  If concessions are made by the buyer, some may add this amount to the sale price to create their own true price.  Concessions made by both buyer and seller should be subtracted from each other providing a net value.  Details of this calculation should be added to the Concessions Comments field." ;
  rdfs:domain      reso:Property ;
  rdfs:label       "ConcessionsAmount" ;
  rdfs:range       xsd:decimal ;
  reso:CertificationLevel "Silver" ;
  reso:PropertyTypes "RESI","RLSE","RINC","LAND","MOBI","FARM","COMS","COML","BUSO" ;
  schema:sameAs    <http://ddwiki.reso.org/display/DDW/ConcessionsAmount+Field> ;
  vs:term_status   "stable"
.
reso:ConcessionsComments a rdf:Property ;
  rdfs:comment     "Comments describing the concessions made by the buyer or the seller." ;
  rdfs:domain      reso:Property ;
  rdfs:label       "ConcessionsComments" ;
  rdfs:range       xsd:string ;
  reso:CertificationLevel "Silver" ;
  reso:PropertyTypes "RESI","RLSE","RINC","LAND","MOBI","FARM","COMS","COML","BUSO" ;
  schema:sameAs    <http://ddwiki.reso.org/display/DDW/ConcessionsComments+Field> ;
  vs:term_status   "stable"
.
reso:ConstructionMaterials a rdf:Property ;
  rdfs:comment     "A list of the materials that were used in the construction of the property." ;
  rdfs:domain      reso:Property ;
  rdfs:label       "ConstructionMaterials" ;
  rdfs:range       enum:ConstructionMaterials ;
  reso:CertificationLevel "Silver" ;
  reso:PropertyTypes "RESI","RLSE","RINC","MOBI","FARM","COMS","COML" ;
  schema:sameAs    <http://ddwiki.reso.org/display/DDW/ConstructionMaterials+Field> ;
  vs:term_status   "stable"
.
reso:ContinentRegion a rdf:Property ;
  rdfs:comment     "A sub-section or area of a continent.  Examples would be Southern Europe or Scandinavia." ;
  rdfs:domain      reso:Property ;
  rdfs:label       "ContinentRegion" ;
  rdfs:range       xsd:string ;
  reso:CertificationLevel "Platinum" ;
  reso:PropertyTypes "RESI","RLSE","RINC","LAND","MOBI","FARM","COMS","COML","BUSO" ;
  schema:sameAs    <http://ddwiki.reso.org/display/DDW/ContinentRegion+Field> ;
  vs:term_status   "stable"
.
reso:Contingency a rdf:Property ;
  rdfs:comment     "A list of contingencies that must be satisfied in order to complete the transaction." ;
  rdfs:domain      reso:Property ;
  rdfs:label       "Contingency" ;
  rdfs:range       xsd:string ;
  reso:CertificationLevel "Bronze" ;
  reso:PropertyTypes "RESI","RLSE","RINC","LAND","MOBI","FARM","COMS","COML","BUSO" ;
  schema:sameAs    <http://ddwiki.reso.org/display/DDW/Contingency+Field> ;
  vs:term_status   "stable"
.
reso:ContingentDate a rdf:Property ;
  rdfs:comment     "The date an offer was made with a contingency. The Listing remains On Market.  This is the date entered by the agent reflecting when the change occurred contractually, not a timestamp of when the change was made in the MLS." ;
  rdfs:domain      reso:Property ;
  rdfs:label       "ContingentDate" ;
  rdfs:range       xsd:date ;
  reso:CertificationLevel "Core" ;
  reso:PropertyTypes "RESI","RLSE","RINC","LAND","MOBI","FARM" ;
  schema:sameAs    <http://ddwiki.reso.org/display/DDW/ContingentDate+Field> ;
  vs:term_status   "stable"
.
reso:ContractStatusChangeDate a rdf:Property ;
  rdfs:comment     "The date of the listings contractual status change. This is not necessarily the time the agent made the change in the MLS system, but rather the date of the contractual change." ;
  rdfs:domain      reso:Property ;
  rdfs:label       "ContractStatusChangeDate" ;
  rdfs:range       xsd:date ;
  reso:CertificationLevel "Core" ;
  reso:PropertyTypes "RESI","RLSE","RINC","LAND","MOBI","FARM","COMS","COML","BUSO" ;
  schema:sameAs    <http://ddwiki.reso.org/display/DDW/ContractStatusChangeDate+Field> ;
  vs:term_status   "stable"
.
reso:Cooling a rdf:Property ;
  rdfs:comment     "A list describing the cooling or air conditioning features of the property." ;
  rdfs:domain      reso:Property ;
  rdfs:label       "Cooling" ;
  rdfs:range       xsd:string ;
  reso:CertificationLevel "Platinum" ;
  reso:PropertyTypes "RESI","RLSE","RINC","MOBI","FARM","COMS","COML" ;
  schema:sameAs    <http://ddwiki.reso.org/display/DDW/Cooling+Field> ;
  vs:term_status   "stable"
.
reso:CoolingYN a rdf:Property ;
  rdfs:comment     "The property has cooling or Air Conditioning." ;
  rdfs:domain      reso:Property ;
  rdfs:label       "CoolingYN" ;
  rdfs:range       xsd:boolean ;
  reso:CertificationLevel "Platinum" ;
  reso:PropertyTypes "RESI","RLSE","RINC","LAND","MOBI","FARM","COMS","COML" ;
  schema:sameAs    <http://ddwiki.reso.org/display/DDW/CoolingYN+Field> ;
  vs:term_status   "stable"
.
reso:CopyrightNotice a rdf:Property ;
  rdfs:comment     "Notice of the legal rights of the owner of the information or data." ;
  rdfs:domain      reso:Property ;
  rdfs:label       "CopyrightNotice" ;
  rdfs:range       xsd:string ;
  reso:CertificationLevel "Bronze" ;
  reso:PropertyTypes "RESI","RLSE","RINC","LAND","MOBI","FARM","COMS","COML","BUSO" ;
  schema:sameAs    <http://ddwiki.reso.org/display/DDW/CopyrightNotice+Field> ;
  vs:term_status   "stable"
.
reso:Country a rdf:Property ;
  rdfs:comment     "The country abbreviation in a postal address." ;
  rdfs:domain      reso:Property ;
  rdfs:label       "Country" ;
  rdfs:range       enum:Country ;
  reso:CertificationLevel "Core" ;
  reso:PropertyTypes "RESI","RLSE","RINC","LAND","MOBI","FARM","COMS","COML","BUSO" ;
  schema:sameAs    <http://ddwiki.reso.org/display/DDW/Country+Field> ;
  vs:term_status   "stable"
.
reso:CountryRegion a rdf:Property ;
  rdfs:comment     "A sub-section or area of a defined country.  Examples would be Napa Valley in the US, or the Amalfi Coast in Italy." ;
  rdfs:domain      reso:Property ;
  rdfs:label       "CountryRegion" ;
  rdfs:range       xsd:string ;
  reso:CertificationLevel "Platinum" ;
  reso:PropertyTypes "RESI","RLSE","RINC","LAND","MOBI","FARM","COMS","COML","BUSO" ;
  schema:sameAs    <http://ddwiki.reso.org/display/DDW/CountryRegion+Field> ;
  vs:term_status   "stable"
.
reso:CountyOrParish a rdf:Property ;
  rdfs:comment     "The County, Parish or other regional authority" ;
  rdfs:domain      reso:Property ;
  rdfs:label       "CountyOrParish" ;
  rdfs:range       xsd:string ;
  reso:CertificationLevel "Core" ;
  reso:PropertyTypes "RESI","RLSE","RINC","LAND","MOBI","FARM","COMS","COML","BUSO" ;
  schema:sameAs    <http://ddwiki.reso.org/display/DDW/CountyOrParish+Field> ;
  vs:term_status   "stable"
.
reso:CoveredSpaces a rdf:Property ;
  rdfs:comment     "The total number of garage and carport spaces." ;
  rdfs:domain      reso:Property ;
  rdfs:label       "CoveredSpaces" ;
  rdfs:range       xsd:decimal ;
  reso:CertificationLevel "Bronze" ;
  reso:PropertyTypes "RESI","RLSE","RINC","MOBI","FARM","COMS","COML" ;
  schema:sameAs    <http://ddwiki.reso.org/display/DDW/CoveredSpaces+Field> ;
  vs:term_status   "stable"
.
reso:CropsIncludedYN a rdf:Property ;
  rdfs:comment     "Are crops included in the sale of the property." ;
  rdfs:domain      reso:Property ;
  rdfs:label       "CropsIncludedYN" ;
  rdfs:range       xsd:boolean ;
  reso:CertificationLevel "Gold" ;
  reso:PropertyTypes "FARM" ;
  schema:sameAs    <http://ddwiki.reso.org/display/DDW/CropsIncludedYN+Field> ;
  vs:term_status   "stable"
.
reso:CrossStreet a rdf:Property ;
  rdfs:comment     "Nearest cross streets to the property.  This field is in addition to, and independent of, the driving directions field." ;
  rdfs:domain      reso:Property ;
  rdfs:label       "CrossStreet" ;
  rdfs:range       xsd:string ;
  reso:CertificationLevel "Silver" ;
  reso:PropertyTypes "RESI","RLSE","RINC","LAND","MOBI","FARM","COMS","COML","BUSO" ;
  schema:sameAs    <http://ddwiki.reso.org/display/DDW/CrossStreet+Field> ;
  vs:term_status   "stable"
.
reso:CultivatedArea a rdf:Property ;
  rdfs:comment     "Measurement or percentage of the property that has been cultivated." ;
  rdfs:domain      reso:Property ;
  rdfs:label       "CultivatedArea" ;
  rdfs:range       xsd:decimal ;
  reso:CertificationLevel "Gold" ;
  reso:PropertyTypes "FARM" ;
  schema:sameAs    <http://ddwiki.reso.org/display/DDW/CultivatedArea+Field> ;
  vs:term_status   "stable"
.
reso:CumulativeDaysOnMarket a rdf:Property ;
  rdfs:comment     "The number of days the property is on market, as defined by the MLS business rules." ;
  rdfs:domain      reso:Property ;
  rdfs:label       "CumulativeDaysOnMarket" ;
  rdfs:range       xsd:decimal ;
  reso:CertificationLevel "Bronze" ;
  reso:PropertyTypes "RESI","RLSE","RINC","LAND","MOBI","FARM","COMS","COML","BUSO" ;
  schema:sameAs    <http://ddwiki.reso.org/display/DDW/CumulativeDaysOnMarket+Field> ;
  vs:term_status   "stable"
.
reso:CurrentFinancing a rdf:Property ;
  rdfs:comment     "A list of options that describe the type of financing that the seller currently has in place for the property being sold.  i.e. cash, assumable, FHA loan, etc." ;
  rdfs:domain      reso:Property ;
  rdfs:label       "CurrentFinancing" ;
  rdfs:range       enum:CurrentFinancing ;
  reso:CertificationLevel "Bronze" ;
  reso:PropertyTypes "RESI","RLSE","RINC","LAND","MOBI","FARM","COMS","COML","BUSO" ;
  schema:sameAs    <http://ddwiki.reso.org/display/DDW/CurrentFinancing+Field> ;
  vs:term_status   "stable"
.
reso:CurrentUse a rdf:Property ;
  rdfs:comment     "A list of the type(s) of current use of the property. The current use of the property is an important factor in understanding the overall condition of the land and determining it&#x2019;s appropriateness for intended use." ;
  rdfs:domain      reso:Property ;
  rdfs:label       "CurrentUse" ;
  rdfs:range       xsd:string ;
  reso:CertificationLevel "Gold" ;
  reso:PropertyTypes "LAND" ;
  schema:sameAs    <http://ddwiki.reso.org/display/DDW/CurrentUse+Field> ;
  vs:term_status   "stable"
.
reso:DOH1 a rdf:Property ;
  rdfs:comment     "Department of Housing decal number for the mobile or manufactured home.  For the first or only unit/section use DOH 1 over DOH 2 or 3." ;
  rdfs:domain      reso:Property ;
  rdfs:label       "DOH1" ;
  rdfs:range       xsd:string ;
  reso:CertificationLevel "Silver" ;
  reso:PropertyTypes "RESI","RLSE","MOBI" ;
  schema:sameAs    <http://ddwiki.reso.org/display/DDW/DOH1+Field> ;
  vs:term_status   "stable"
.
reso:DOH2 a rdf:Property ;
  rdfs:comment     "Department of Housing decal number for the mobile or manufactured home.  For two units/sections use DOH 1 and 2 over DOH 3." ;
  rdfs:domain      reso:Property ;
  rdfs:label       "DOH2" ;
  rdfs:range       xsd:string ;
  reso:CertificationLevel "Silver" ;
  reso:PropertyTypes "RESI","RLSE","MOBI" ;
  schema:sameAs    <http://ddwiki.reso.org/display/DDW/DOH2+Field> ;
  vs:term_status   "stable"
.
reso:DOH3 a rdf:Property ;
  rdfs:comment     "Department of Housing decal number for the mobile or manufactured home.  For two units/sections use DOH 1 and 2 over DOH 3." ;
  rdfs:domain      reso:Property ;
  rdfs:label       "DOH3" ;
  rdfs:range       xsd:string ;
  reso:CertificationLevel "Silver" ;
  reso:PropertyTypes "RESI","RLSE","MOBI" ;
  schema:sameAs    <http://ddwiki.reso.org/display/DDW/DOH3+Field> ;
  vs:term_status   "stable"
.
reso:DaysOnMarket a rdf:Property ;
  rdfs:comment     "The number of days the listing is on market, as defined by the MLS business rules." ;
  rdfs:domain      reso:Property ;
  rdfs:label       "DaysOnMarket" ;
  rdfs:range       xsd:decimal ;
  reso:CertificationLevel "Bronze" ;
  reso:PropertyTypes "RESI","RLSE","RINC","LAND","MOBI","FARM","COMS","COML","BUSO" ;
  schema:sameAs    <http://ddwiki.reso.org/display/DDW/DaysOnMarket+Field> ;
  vs:term_status   "stable"
.
reso:DevelopmentStatus a rdf:Property ;
  rdfs:comment     "A list of the Development Status of the property.  The developmental status of land is an important factor in selling, purchasing and developing of land properties." ;
  rdfs:domain      reso:Property ;
  rdfs:label       "DevelopmentStatus" ;
  rdfs:range       xsd:string ;
  reso:CertificationLevel "Gold" ;
  reso:PropertyTypes "LAND" ;
  schema:sameAs    <http://ddwiki.reso.org/display/DDW/DevelopmentStatus+Field> ;
  vs:term_status   "stable"
.
reso:DirectionFaces a rdf:Property ;
  rdfs:comment     "The compass direction that the main entrance to the building faces. For example, North, South, East, West, South-West, etc. It may also be known as the building exposure." ;
  rdfs:domain      reso:Property ;
  rdfs:label       "DirectionFaces" ;
  rdfs:range       enum:DirectionFaces ;
  reso:CertificationLevel "Silver" ;
  reso:PropertyTypes "RESI","RLSE","RINC","MOBI","FARM","COMS","COML" ;
  schema:sameAs    <http://ddwiki.reso.org/display/DDW/DirectionFaces+Field> ;
  vs:term_status   "stable"
.
reso:Directions a rdf:Property ;
  rdfs:comment     "Driving directions to the property." ;
  rdfs:domain      reso:Property ;
  rdfs:label       "Directions" ;
  rdfs:range       xsd:string ;
  reso:CertificationLevel "Silver" ;
  reso:PropertyTypes "RESI","RLSE","RINC","LAND","MOBI","FARM","COMS","COML","BUSO" ;
  schema:sameAs    <http://ddwiki.reso.org/display/DDW/Directions+Field> ;
  vs:term_status   "stable"
.
reso:Disclaimer a rdf:Property ;
  rdfs:comment     "Text that serves as the negation or limitation of the rights under a warranty given by a seller to a buyer." ;
  rdfs:domain      reso:Property ;
  rdfs:label       "Disclaimer" ;
  rdfs:range       xsd:string ;
  reso:CertificationLevel "Bronze" ;
  reso:PropertyTypes "RESI","RLSE","RINC","LAND","MOBI","FARM","COMS","COML","BUSO" ;
  schema:sameAs    <http://ddwiki.reso.org/display/DDW/Disclaimer+Field> ;
  vs:term_status   "stable"
.
reso:Disclosures a rdf:Property ;
  rdfs:comment     "Legal or pertinent information that should be disclosed to potential buyer's agents." ;
  rdfs:domain      reso:Property ;
  rdfs:label       "Disclosures" ;
  rdfs:range       xsd:string ;
  reso:CertificationLevel "Bronze" ;
  reso:PropertyTypes "RESI","RLSE","RINC","LAND","MOBI","FARM","COMS","COML","BUSO" ;
  schema:sameAs    <http://ddwiki.reso.org/display/DDW/Disclosures+Field> ;
  vs:term_status   "stable"
.
reso:DistanceToBusComments a rdf:Property ;
  rdfs:comment     "A textual description of the distance to local bus stops." ;
  rdfs:domain      reso:Property ;
  rdfs:label       "DistanceToBusComments" ;
  rdfs:range       xsd:string ;
  reso:CertificationLevel "Silver" ;
  reso:PropertyTypes "LAND","FARM" ;
  schema:sameAs    <http://ddwiki.reso.org/display/DDW/DistanceToBusComments+Field> ;
  vs:term_status   "stable"
.
reso:DistanceToBusNumeric a rdf:Property ;
  rdfs:comment     "Numeric distance from the property to the nearest bus stop." ;
  rdfs:domain      reso:Property ;
  rdfs:label       "DistanceToBusNumeric" ;
  rdfs:range       xsd:decimal ;
  reso:CertificationLevel "Platinum" ;
  reso:PropertyTypes "LAND","FARM" ;
  schema:sameAs    <http://ddwiki.reso.org/display/DDW/DistanceToBusNumeric+Field> ;
  vs:term_status   "stable"
.
reso:DistanceToBusUnits a rdf:Property ;
  rdfs:comment     "A pick list of the unit linear measurement.  i.e. feed, meters, yards, kilometers, miles, etc." ;
  rdfs:domain      reso:Property ;
  rdfs:label       "DistanceToBusUnits" ;
  rdfs:range       enum:LinearUnits ;
  reso:CertificationLevel "Platinum" ;
  reso:PropertyTypes "LAND","FARM" ;
  schema:sameAs    <http://ddwiki.reso.org/display/DDW/DistanceToBusUnits+Field> ;
  vs:term_status   "stable"
.
reso:DistanceToElectricComments a rdf:Property ;
  rdfs:comment     "If the property does not currently have electrical utility, is service available and if so, what is the distance." ;
  rdfs:domain      reso:Property ;
  rdfs:label       "DistanceToElectricComments" ;
  rdfs:range       xsd:string ;
  reso:CertificationLevel "Bronze" ;
  reso:PropertyTypes "LAND","FARM" ;
  schema:sameAs    <http://ddwiki.reso.org/display/DDW/DistanceToElectricComments+Field> ;
  vs:term_status   "stable"
.
reso:DistanceToElectricNumeric a rdf:Property ;
  rdfs:comment     "Numeric distance from the property to the electrical utility." ;
  rdfs:domain      reso:Property ;
  rdfs:label       "DistanceToElectricNumeric" ;
  rdfs:range       xsd:decimal ;
  reso:CertificationLevel "Platinum" ;
  reso:PropertyTypes "LAND","FARM" ;
  schema:sameAs    <http://ddwiki.reso.org/display/DDW/DistanceToElectricNumeric+Field> ;
  vs:term_status   "stable"
.
reso:DistanceToElectricUnits a rdf:Property ;
  rdfs:comment     "A pick list of the unit linear measurement.  i.e. feed, meters, yards, kilometers, miles, etc." ;
  rdfs:domain      reso:Property ;
  rdfs:label       "DistanceToElectricUnits" ;
  rdfs:range       enum:LinearUnits ;
  reso:CertificationLevel "Platinum" ;
  reso:PropertyTypes "LAND","FARM" ;
  schema:sameAs    <http://ddwiki.reso.org/display/DDW/DistanceToElectricUnits+Field> ;
  vs:term_status   "stable"
.
reso:DistanceToFreewayComments a rdf:Property ;
  rdfs:comment     "A textual description of the distance to freeways." ;
  rdfs:domain      reso:Property ;
  rdfs:label       "DistanceToFreewayComments" ;
  rdfs:range       xsd:string ;
  reso:CertificationLevel "Silver" ;
  reso:PropertyTypes "LAND","FARM" ;
  schema:sameAs    <http://ddwiki.reso.org/display/DDW/DistanceToFreewayComments+Field> ;
  vs:term_status   "stable"
.
reso:DistanceToFreewayNumeric a rdf:Property ;
  rdfs:comment     "Numeric distance from the property to the nearest freeway." ;
  rdfs:domain      reso:Property ;
  rdfs:label       "DistanceToFreewayNumeric" ;
  rdfs:range       xsd:decimal ;
  reso:CertificationLevel "Platinum" ;
  reso:PropertyTypes "LAND","FARM" ;
  schema:sameAs    <http://ddwiki.reso.org/display/DDW/DistanceToFreewayNumeric+Field> ;
  vs:term_status   "stable"
.
reso:DistanceToFreewayUnits a rdf:Property ;
  rdfs:comment     "A pick list of the unit linear measurement.  i.e. feed, meters, yards, kilometers, miles, etc." ;
  rdfs:domain      reso:Property ;
  rdfs:label       "DistanceToFreewayUnits" ;
  rdfs:range       enum:LinearUnits ;
  reso:CertificationLevel "Platinum" ;
  reso:PropertyTypes "LAND","FARM" ;
  schema:sameAs    <http://ddwiki.reso.org/display/DDW/DistanceToFreewayUnits+Field> ;
  vs:term_status   "stable"
.
reso:DistanceToGasComments a rdf:Property ;
  rdfs:comment     "If the property does not currently have natural gas utility, is service available and if so, what is the distance." ;
  rdfs:domain      reso:Property ;
  rdfs:label       "DistanceToGasComments" ;
  rdfs:range       xsd:string ;
  reso:CertificationLevel "Silver" ;
  reso:PropertyTypes "LAND","FARM" ;
  schema:sameAs    <http://ddwiki.reso.org/display/DDW/DistanceToGasComments+Field> ;
  vs:term_status   "stable"
.
reso:DistanceToGasNumeric a rdf:Property ;
  rdfs:comment     "Numeric distance from the property to the gas utility." ;
  rdfs:domain      reso:Property ;
  rdfs:label       "DistanceToGasNumeric" ;
  rdfs:range       xsd:decimal ;
  reso:CertificationLevel "Platinum" ;
  reso:PropertyTypes "LAND","FARM" ;
  schema:sameAs    <http://ddwiki.reso.org/display/DDW/DistanceToGasNumeric+Field> ;
  vs:term_status   "stable"
.
reso:DistanceToGasUnits a rdf:Property ;
  rdfs:comment     "A pick list of the unit linear measurement.  i.e. feed, meters, yards, kilometers, miles, etc." ;
  rdfs:domain      reso:Property ;
  rdfs:label       "DistanceToGasUnits" ;
  rdfs:range       enum:LinearUnits ;
  reso:CertificationLevel "Platinum" ;
  reso:PropertyTypes "LAND","FARM" ;
  schema:sameAs    <http://ddwiki.reso.org/display/DDW/DistanceToGasUnits+Field> ;
  vs:term_status   "stable"
.
reso:DistanceToPhoneServiceComments a rdf:Property ;
  rdfs:comment     "If the property does not currently have phone service, is service available and if so, what is the distance." ;
  rdfs:domain      reso:Property ;
  rdfs:label       "DistanceToPhoneServiceComments" ;
  rdfs:range       xsd:string ;
  reso:CertificationLevel "Silver" ;
  reso:PropertyTypes "LAND","FARM" ;
  schema:sameAs    <http://ddwiki.reso.org/display/DDW/DistanceToPhoneServiceComments+Field> ;
  vs:term_status   "stable"
.
reso:DistanceToPhoneServiceNumeric a rdf:Property ;
  rdfs:comment     "Numeric distance from the property to the phone utility." ;
  rdfs:domain      reso:Property ;
  rdfs:label       "DistanceToPhoneServiceNumeric" ;
  rdfs:range       xsd:decimal ;
  reso:CertificationLevel "Platinum" ;
  reso:PropertyTypes "LAND","FARM" ;
  schema:sameAs    <http://ddwiki.reso.org/display/DDW/DistanceToPhoneServiceNumeric+Field> ;
  vs:term_status   "stable"
.
reso:DistanceToPhoneServiceUnits a rdf:Property ;
  rdfs:comment     "A pick list of the unit linear measurement.  i.e. feed, meters, yards, kilometers, miles, etc." ;
  rdfs:domain      reso:Property ;
  rdfs:label       "DistanceToPhoneServiceUnits" ;
  rdfs:range       enum:LinearUnits ;
  reso:CertificationLevel "Platinum" ;
  reso:PropertyTypes "LAND","FARM" ;
  schema:sameAs    <http://ddwiki.reso.org/display/DDW/DistanceToPhoneServiceUnits+Field> ;
  vs:term_status   "stable"
.
reso:DistanceToPlaceofWorshipComments a rdf:Property ;
  rdfs:comment     "A textual description of the distance to local places of worship." ;
  rdfs:domain      reso:Property ;
  rdfs:label       "DistanceToPlaceofWorshipComments" ;
  rdfs:range       xsd:string ;
  reso:CertificationLevel "Silver" ;
  reso:PropertyTypes "LAND","FARM" ;
  schema:sameAs    <http://ddwiki.reso.org/display/DDW/DistanceToPlaceofWorshipComments+Field> ;
  vs:term_status   "stable"
.
reso:DistanceToPlaceofWorshipNumeric a rdf:Property ;
  rdfs:comment     "Numeric distance from the property to the nearest place of worship." ;
  rdfs:domain      reso:Property ;
  rdfs:label       "DistanceToPlaceofWorshipNumeric" ;
  rdfs:range       xsd:decimal ;
  reso:CertificationLevel "Platinum" ;
  reso:PropertyTypes "LAND","FARM" ;
  schema:sameAs    <http://ddwiki.reso.org/display/DDW/DistanceToPlaceofWorshipNumeric+Field> ;
  vs:term_status   "stable"
.
reso:DistanceToPlaceofWorshipUnits a rdf:Property ;
  rdfs:comment     "A pick list of the unit linear measurement.  i.e. feed, meters, yards, kilometers, miles, etc." ;
  rdfs:domain      reso:Property ;
  rdfs:label       "DistanceToPlaceofWorshipUnits" ;
  rdfs:range       enum:LinearUnits ;
  reso:CertificationLevel "Platinum" ;
  reso:PropertyTypes "LAND","FARM" ;
  schema:sameAs    <http://ddwiki.reso.org/display/DDW/DistanceToPlaceofWorshipUnits+Field> ;
  vs:term_status   "stable"
.
reso:DistanceToSchoolBusComments a rdf:Property ;
  rdfs:comment     "Distance from the property to the nearest school bus pickup point." ;
  rdfs:domain      reso:Property ;
  rdfs:label       "DistanceToSchoolBusComments" ;
  rdfs:range       xsd:string ;
  reso:CertificationLevel "Silver" ;
  reso:PropertyTypes "LAND","FARM" ;
  schema:sameAs    <http://ddwiki.reso.org/display/DDW/DistanceToSchoolBusComments+Field> ;
  vs:term_status   "stable"
.
reso:DistanceToSchoolBusNumeric a rdf:Property ;
  rdfs:comment     "Numeric distance from the property to the nearest school bus pickup point." ;
  rdfs:domain      reso:Property ;
  rdfs:label       "DistanceToSchoolBusNumeric" ;
  rdfs:range       xsd:decimal ;
  reso:CertificationLevel "Platinum" ;
  reso:PropertyTypes "LAND","FARM" ;
  schema:sameAs    <http://ddwiki.reso.org/display/DDW/DistanceToSchoolBusNumeric+Field> ;
  vs:term_status   "stable"
.
reso:DistanceToSchoolBusUnits a rdf:Property ;
  rdfs:comment     "A pick list of the unit linear measurement.  i.e. feed, meters, yards, kilometers, miles, etc." ;
  rdfs:domain      reso:Property ;
  rdfs:label       "DistanceToSchoolBusUnits" ;
  rdfs:range       enum:LinearUnits ;
  reso:CertificationLevel "Platinum" ;
  reso:PropertyTypes "LAND","FARM" ;
  schema:sameAs    <http://ddwiki.reso.org/display/DDW/DistanceToSchoolBusUnits+Field> ;
  vs:term_status   "stable"
.
reso:DistanceToSchoolsComments a rdf:Property ;
  rdfs:comment     "A textual description of the distance to local schools." ;
  rdfs:domain      reso:Property ;
  rdfs:label       "DistanceToSchoolsComments" ;
  rdfs:range       xsd:string ;
  reso:CertificationLevel "Silver" ;
  reso:PropertyTypes "LAND","FARM" ;
  schema:sameAs    <http://ddwiki.reso.org/display/DDW/DistanceToSchoolsComments+Field> ;
  vs:term_status   "stable"
.
reso:DistanceToSchoolsNumeric a rdf:Property ;
  rdfs:comment     "Numeric distance from the property to the nearest school." ;
  rdfs:domain      reso:Property ;
  rdfs:label       "DistanceToSchoolsNumeric" ;
  rdfs:range       xsd:decimal ;
  reso:CertificationLevel "Platinum" ;
  reso:PropertyTypes "LAND","FARM" ;
  schema:sameAs    <http://ddwiki.reso.org/display/DDW/DistanceToSchoolsNumeric+Field> ;
  vs:term_status   "stable"
.
reso:DistanceToSchoolsUnits a rdf:Property ;
  rdfs:comment     "A pick list of the unit linear measurement.  i.e. feed, meters, yards, kilometers, miles, etc." ;
  rdfs:domain      reso:Property ;
  rdfs:label       "DistanceToSchoolsUnits" ;
  rdfs:range       enum:LinearUnits ;
  reso:CertificationLevel "Platinum" ;
  reso:PropertyTypes "LAND","FARM" ;
  schema:sameAs    <http://ddwiki.reso.org/display/DDW/DistanceToSchoolsUnits+Field> ;
  vs:term_status   "stable"
.
reso:DistanceToSewerComments a rdf:Property ;
  rdfs:comment     "If the property does not currently have sewer or septic, is sewer service available and if so, what is the distance." ;
  rdfs:domain      reso:Property ;
  rdfs:label       "DistanceToSewerComments" ;
  rdfs:range       xsd:string ;
  reso:CertificationLevel "Silver" ;
  reso:PropertyTypes "LAND","FARM" ;
  schema:sameAs    <http://ddwiki.reso.org/display/DDW/DistanceToSewerComments+Field> ;
  vs:term_status   "stable"
.
reso:DistanceToSewerNumeric a rdf:Property ;
  rdfs:comment     "Numeric distance from the property to the sewer utility." ;
  rdfs:domain      reso:Property ;
  rdfs:label       "DistanceToSewerNumeric" ;
  rdfs:range       xsd:decimal ;
  reso:CertificationLevel "Platinum" ;
  reso:PropertyTypes "LAND","FARM" ;
  schema:sameAs    <http://ddwiki.reso.org/display/DDW/DistanceToSewerNumeric+Field> ;
  vs:term_status   "stable"
.
reso:DistanceToSewerUnits a rdf:Property ;
  rdfs:comment     "A pick list of the unit linear measurement.  i.e. feed, meters, yards, kilometers, miles, etc." ;
  rdfs:domain      reso:Property ;
  rdfs:label       "DistanceToSewerUnits" ;
  rdfs:range       enum:LinearUnits ;
  reso:CertificationLevel "Platinum" ;
  reso:PropertyTypes "LAND","FARM" ;
  schema:sameAs    <http://ddwiki.reso.org/display/DDW/DistanceToSewerUnits+Field> ;
  vs:term_status   "stable"
.
reso:DistanceToShoppingComments a rdf:Property ;
  rdfs:comment     "A description of the distance to primary shopping sources such as groceries, gasoline, clothing or department stores." ;
  rdfs:domain      reso:Property ;
  rdfs:label       "DistanceToShoppingComments" ;
  rdfs:range       xsd:string ;
  reso:CertificationLevel "Silver" ;
  reso:PropertyTypes "LAND","FARM" ;
  schema:sameAs    <http://ddwiki.reso.org/display/DDW/DistanceToShoppingComments+Field> ;
  vs:term_status   "stable"
.
reso:DistanceToShoppingNumeric a rdf:Property ;
  rdfs:comment     "Numeric distance from the property to the nearest shopping." ;
  rdfs:domain      reso:Property ;
  rdfs:label       "DistanceToShoppingNumeric" ;
  rdfs:range       xsd:decimal ;
  reso:CertificationLevel "Platinum" ;
  reso:PropertyTypes "LAND","FARM" ;
  schema:sameAs    <http://ddwiki.reso.org/display/DDW/DistanceToShoppingNumeric+Field> ;
  vs:term_status   "stable"
.
reso:DistanceToShoppingUnits a rdf:Property ;
  rdfs:comment     "A pick list of the unit linear measurement.  i.e. feed, meters, yards, kilometers, miles, etc." ;
  rdfs:domain      reso:Property ;
  rdfs:label       "DistanceToShoppingUnits" ;
  rdfs:range       enum:LinearUnits ;
  reso:CertificationLevel "Platinum" ;
  reso:PropertyTypes "LAND","FARM" ;
  schema:sameAs    <http://ddwiki.reso.org/display/DDW/DistanceToShoppingUnits+Field> ;
  vs:term_status   "stable"
.
reso:DistanceToStreetComments a rdf:Property ;
  rdfs:comment     "If the property does not have a maintained road or street adjacent to the lot, what are the conditions of access and distance to a maintained road." ;
  rdfs:domain      reso:Property ;
  rdfs:label       "DistanceToStreetComments" ;
  rdfs:range       xsd:string ;
  reso:CertificationLevel "Silver" ;
  reso:PropertyTypes "LAND","FARM" ;
  schema:sameAs    <http://ddwiki.reso.org/display/DDW/DistanceToStreetComments+Field> ;
  vs:term_status   "stable"
.
reso:DistanceToStreetNumeric a rdf:Property ;
  rdfs:comment     "Numeric distance from the property to the street." ;
  rdfs:domain      reso:Property ;
  rdfs:label       "DistanceToStreetNumeric" ;
  rdfs:range       xsd:decimal ;
  reso:CertificationLevel "Platinum" ;
  reso:PropertyTypes "LAND","FARM" ;
  schema:sameAs    <http://ddwiki.reso.org/display/DDW/DistanceToStreetNumeric+Field> ;
  vs:term_status   "stable"
.
reso:DistanceToStreetUnits a rdf:Property ;
  rdfs:comment     "A pick list of the unit linear measurement.  i.e. feed, meters, yards, kilometers, miles, etc." ;
  rdfs:domain      reso:Property ;
  rdfs:label       "DistanceToStreetUnits" ;
  rdfs:range       enum:LinearUnits ;
  reso:CertificationLevel "Platinum" ;
  reso:PropertyTypes "LAND","FARM" ;
  schema:sameAs    <http://ddwiki.reso.org/display/DDW/DistanceToStreetUnits+Field> ;
  vs:term_status   "stable"
.
reso:DistanceToWaterComments a rdf:Property ;
  rdfs:comment     "If the property does not currently have water utility, is service available and if so, what is the distance." ;
  rdfs:domain      reso:Property ;
  rdfs:label       "DistanceToWaterComments" ;
  rdfs:range       xsd:string ;
  reso:CertificationLevel "Silver" ;
  reso:PropertyTypes "LAND","FARM" ;
  schema:sameAs    <http://ddwiki.reso.org/display/DDW/DistanceToWaterComments+Field> ;
  vs:term_status   "stable"
.
reso:DistanceToWaterNumeric a rdf:Property ;
  rdfs:comment     "Numeric distance from the property to the water utility." ;
  rdfs:domain      reso:Property ;
  rdfs:label       "DistanceToWaterNumeric" ;
  rdfs:range       xsd:decimal ;
  reso:CertificationLevel "Platinum" ;
  reso:PropertyTypes "LAND","FARM" ;
  schema:sameAs    <http://ddwiki.reso.org/display/DDW/DistanceToWaterNumeric+Field> ;
  vs:term_status   "stable"
.
reso:DistanceToWaterUnits a rdf:Property ;
  rdfs:comment     "A pick list of the unit linear measurement.  i.e. feed, meters, yards, kilometers, miles, etc." ;
  rdfs:domain      reso:Property ;
  rdfs:label       "DistanceToWaterUnits" ;
  rdfs:range       enum:LinearUnits ;
  reso:CertificationLevel "Platinum" ;
  reso:PropertyTypes "LAND","FARM" ;
  schema:sameAs    <http://ddwiki.reso.org/display/DDW/DistanceToWaterUnits+Field> ;
  vs:term_status   "stable"
.
reso:DocumentsAvailable a rdf:Property ;
  rdfs:comment     "A list of the Documents available for the property.  Knowing what documents are available for the property is valuable information." ;
  rdfs:domain      reso:Property ;
  rdfs:label       "DocumentsAvailable" ;
  rdfs:range       xsd:string ;
  reso:CertificationLevel "Bronze" ;
  reso:PropertyTypes "RESI","RLSE","RINC","LAND","MOBI","FARM","BUSO" ;
  schema:sameAs    <http://ddwiki.reso.org/display/DDW/DocumentsAvailable+Field> ;
  vs:term_status   "stable"
.
reso:DocumentsChangeTimestamp a rdf:Property ;
  rdfs:comment     "System generated timestamp of when the last update or change to the documents for this listing was made." ;
  rdfs:domain      reso:Property ;
  rdfs:label       "DocumentsChangeTimestamp" ;
  rdfs:range       xsd:dateTime ;
  reso:CertificationLevel "Bronze" ;
  reso:PropertyTypes "RESI","RLSE","RINC","LAND","MOBI","FARM","COMS","COML","BUSO" ;
  schema:sameAs    <http://ddwiki.reso.org/display/DDW/DocumentsChangeTimestamp+Field> ;
  vs:term_status   "stable"
.
reso:DocumentsCount a rdf:Property ;
  rdfs:comment     "The total number of documents or supplements included with the listings." ;
  rdfs:domain      reso:Property ;
  rdfs:label       "DocumentsCount" ;
  rdfs:range       xsd:decimal ;
  reso:CertificationLevel "Bronze" ;
  reso:PropertyTypes "RESI","RLSE","RINC","LAND","MOBI","FARM","COMS","COML","BUSO" ;
  schema:sameAs    <http://ddwiki.reso.org/display/DDW/DocumentsCount+Field> ;
  vs:term_status   "stable"
.
reso:DoorFeatures a rdf:Property ;
  rdfs:comment     "A list of features or description of the doors included in the sale/lease." ;
  rdfs:domain      reso:Property ;
  rdfs:label       "DoorFeatures" ;
  rdfs:range       xsd:string ;
  reso:CertificationLevel "Platinum" ;
  reso:PropertyTypes "RESI","RLSE","RINC","MOBI","FARM" ;
  schema:sameAs    <http://ddwiki.reso.org/display/DDW/DoorFeatures+Field> ;
  vs:term_status   "stable"
.
reso:DualVariableCompensationYN a rdf:Property ;
  rdfs:domain      reso:Property ;
  rdfs:label       "DualVariableCompensationYN" ;
  rdfs:range       xsd:boolean ;
  reso:CertificationLevel "Core" ;
  reso:PropertyTypes "RESI","RLSE","RINC","LAND","MOBI","FARM","COMS","COML","BUSO" ;
  schema:sameAs    <http://ddwiki.reso.org/display/DDW/DualVariableCompensationYN+Field> ;
  vs:term_status   "stable"
.
reso:Electric a rdf:Property ;
  rdfs:domain      reso:Property ;
  rdfs:label       "Electric" ;
  rdfs:range       enum:Electric ;
  reso:CertificationLevel "Bronze" ;
  reso:PropertyTypes "RESI","RLSE","RINC","LAND","MOBI","FARM" ;
  schema:sameAs    <http://ddwiki.reso.org/display/DDW/Electric+Field> ;
  vs:term_status   "stable"
.
reso:ElectricExpense a rdf:Property ;
  rdfs:comment     "The annual expense that is not paid directly by the tenant and is included in the Operating Expense calculations." ;
  rdfs:domain      reso:Property ;
  rdfs:label       "ElectricExpense" ;
  rdfs:range       xsd:decimal ;
  reso:CertificationLevel "Silver" ;
  reso:PropertyTypes "RINC","COMS","COML" ;
  schema:sameAs    <http://ddwiki.reso.org/display/DDW/ElectricExpense+Field> ;
  vs:term_status   "stable"
.
reso:ElectricOnPropertyYN a rdf:Property ;
  rdfs:comment     "Does the property currently have electrical utility available on the property." ;
  rdfs:domain      reso:Property ;
  rdfs:label       "ElectricOnPropertyYN" ;
  rdfs:range       xsd:boolean ;
  reso:CertificationLevel "Bronze" ;
  reso:PropertyTypes "LAND","FARM" ;
  schema:sameAs    <http://ddwiki.reso.org/display/DDW/ElectricOnPropertyYN+Field> ;
  vs:term_status   "stable"
.
reso:ElementarySchool a rdf:Property ;
  rdfs:comment     "The name of the primary school having a catchment area that includes the associated property." ;
  rdfs:domain      reso:Property ;
  rdfs:label       "ElementarySchool" ;
  rdfs:range       xsd:string ;
  reso:CertificationLevel "Silver" ;
  reso:PropertyTypes "RESI","RLSE","RINC","LAND","MOBI","FARM","COMS","COML","BUSO" ;
  schema:sameAs    <http://ddwiki.reso.org/display/DDW/ElementarySchool+Field> ;
  vs:term_status   "stable"
.
reso:ElementarySchoolDistrict a rdf:Property ;
  rdfs:comment     "The name of the elementary school district having a catchment area that includes the associated property." ;
  rdfs:domain      reso:Property ;
  rdfs:label       "ElementarySchoolDistrict" ;
  rdfs:range       xsd:string ;
  reso:CertificationLevel "Bronze" ;
  reso:PropertyTypes "RESI","RLSE","RINC","LAND","MOBI","FARM","COMS","COML","BUSO" ;
  schema:sameAs    <http://ddwiki.reso.org/display/DDW/ElementarySchoolDistrict+Field> ;
  vs:term_status   "stable"
.
reso:Elevation a rdf:Property ;
  rdfs:comment     "The elevation of the property in relation to sea level.  Use the Elevation Units field to communicate the unit of measurement.  i.e. Feet or Meters." ;
  rdfs:domain      reso:Property ;
  rdfs:label       "Elevation" ;
  rdfs:range       xsd:decimal ;
  reso:CertificationLevel "Bronze" ;
  reso:PropertyTypes "RESI","RLSE","RINC","LAND","MOBI","FARM","COMS","COML" ;
  schema:sameAs    <http://ddwiki.reso.org/display/DDW/Elevation+Field> ;
  vs:term_status   "stable"
.
reso:ElevationUnits a rdf:Property ;
  rdfs:comment     "A pick list of the unit of measurement used in the Elevation field.  i.e. Feet, Meters." ;
  rdfs:domain      reso:Property ;
  rdfs:label       "ElevationUnits" ;
  rdfs:range       enum:LinearUnits ;
  reso:CertificationLevel "Bronze" ;
  reso:PropertyTypes "RESI","RLSE","RINC","LAND","MOBI","FARM" ;
  schema:sameAs    <http://ddwiki.reso.org/display/DDW/ElevationUnits+Field> ;
  vs:term_status   "stable"
.
reso:EntryLevel a rdf:Property ;
  rdfs:comment     "A numeric field that describes the level within the structure, SFR or a unit in a building, where the main entry to the dwelling is located.  When a unit has one floor it is implicit that this is also the level of the unit itself." ;
  rdfs:domain      reso:Property ;
  rdfs:label       "EntryLevel" ;
  rdfs:range       xsd:decimal ;
  reso:CertificationLevel "Silver" ;
  reso:PropertyTypes "RESI","RLSE","RINC","MOBI","FARM","COMS","COML" ;
  schema:sameAs    <http://ddwiki.reso.org/display/DDW/EntryLevel+Field> ;
  vs:term_status   "stable"
.
reso:EntryLocation a rdf:Property ;
  rdfs:comment     "A description of the main entry way to the property.  i.e. Elevator, Ground Level w/ Steps, Ground Level w/o Steps, Mid Level, Top Level, etc." ;
  rdfs:domain      reso:Property ;
  rdfs:label       "EntryLocation" ;
  rdfs:range       xsd:string ;
  reso:CertificationLevel "Silver" ;
  reso:PropertyTypes "RESI","RLSE","RINC","MOBI","FARM" ;
  schema:sameAs    <http://ddwiki.reso.org/display/DDW/EntryLocation+Field> ;
  vs:term_status   "stable"
.
reso:Exclusions a rdf:Property ;
  rdfs:comment     "Elements of the property that will not be included in the sale.  i.e. Chandeliers will be removed prior to close." ;
  rdfs:domain      reso:Property ;
  rdfs:label       "Exclusions" ;
  rdfs:range       xsd:string ;
  reso:CertificationLevel "Bronze" ;
  reso:PropertyTypes "RESI","RLSE","RINC","LAND","MOBI","FARM","COMS","COML","BUSO" ;
  schema:sameAs    <http://ddwiki.reso.org/display/DDW/Exclusions+Field> ;
  vs:term_status   "stable"
.
reso:ExistingLeaseType a rdf:Property ;
  rdfs:comment     "Information about the status of the existing lease on the property.  i.e. Net, NNN, NN, Gross, Absolute Net, Escalation Clause, Ground Lease, etc." ;
  rdfs:domain      reso:Property ;
  rdfs:label       "ExistingLeaseType" ;
  rdfs:range       enum:ExistingLeaseType ;
  reso:CertificationLevel "Bronze" ;
  reso:PropertyTypes "RINC","COML" ;
  schema:sameAs    <http://ddwiki.reso.org/display/DDW/ExistingLeaseType+Field> ;
  vs:term_status   "stable"
.
reso:ExpirationDate a rdf:Property ;
  rdfs:comment     "The date when the listing agreement will expire.  This is the date entered by the agent reflecting when the change occurred, or will occur, contractually, not a timestamp of when the change was made in the MLS.  The expiration date of listings, prior to their expiration, cancellation, sale or lease, is confidential information and should be restricted to the agent and their managers, partners or broker." ;
  rdfs:domain      reso:Property ;
  rdfs:label       "ExpirationDate" ;
  rdfs:range       xsd:date ;
  reso:CertificationLevel "Core" ;
  reso:PropertyTypes "RESI","RLSE","RINC","LAND","MOBI","FARM","COMS","COML","BUSO" ;
  schema:sameAs    <http://ddwiki.reso.org/display/DDW/ExpirationDate+Field> ;
  vs:term_status   "stable"
.
reso:ExteriorFeatures a rdf:Property ;
  rdfs:comment     "A list of features or description of the exterior of the property included in the sale/lease." ;
  rdfs:domain      reso:Property ;
  rdfs:label       "ExteriorFeatures" ;
  rdfs:range       xsd:string ;
  reso:CertificationLevel "Platinum" ;
  reso:PropertyTypes "RESI","RLSE","RINC","MOBI","FARM" ;
  schema:sameAs    <http://ddwiki.reso.org/display/DDW/ExteriorFeatures+Field> ;
  vs:term_status   "stable"
.
reso:FarmCreditServiceInclYN a rdf:Property ;
  rdfs:comment     "Specifies whether or not Farm Credit Service shares are included in the price of the property." ;
  rdfs:domain      reso:Property ;
  rdfs:label       "FarmCreditServiceInclYN" ;
  rdfs:range       xsd:boolean ;
  reso:CertificationLevel "Gold" ;
  reso:PropertyTypes "FARM" ;
  schema:sameAs    <http://ddwiki.reso.org/display/DDW/FarmCreditServiceInclYN+Field> ;
  vs:term_status   "stable"
.
reso:FarmLandAreaSource a rdf:Property ;
  rdfs:comment     "The source of the measurements. This may be a pick list of options showing the source of the measurement. i.e. Agent, Assessor, Estimate, etc. This field applies to all farm area fields (Cultivated, Pasture, Range, Wooded)" ;
  rdfs:domain      reso:Property ;
  rdfs:label       "FarmLandAreaSource" ;
  rdfs:range       enum:AreaSource ;
  reso:CertificationLevel "Gold" ;
  reso:PropertyTypes "FARM" ;
  schema:sameAs    <http://ddwiki.reso.org/display/DDW/FarmLandAreaSource+Field> ;
  vs:term_status   "stable"
.
reso:FarmLandAreaUnits a rdf:Property ;
  rdfs:comment     "A pick list of the unit of measurement for the area.  i.e. Square Feet, Square Meters, Acres, etc.  This field applies to all farm area fields (Cultivated, Pasture, Range, Wooded)" ;
  rdfs:domain      reso:Property ;
  rdfs:label       "FarmLandAreaUnits" ;
  rdfs:range       enum:AreaUnits ;
  reso:CertificationLevel "Gold" ;
  reso:PropertyTypes "FARM" ;
  schema:sameAs    <http://ddwiki.reso.org/display/DDW/FarmLandAreaUnits+Field> ;
  vs:term_status   "stable"
.
reso:Fencing a rdf:Property ;
  rdfs:comment     "A list of types of fencing found at the property being sold." ;
  rdfs:domain      reso:Property ;
  rdfs:label       "Fencing" ;
  rdfs:range       xsd:string ;
  reso:CertificationLevel "Gold" ;
  reso:PropertyTypes "RESI","RLSE","RINC","LAND","MOBI","FARM","COMS","COML" ;
  schema:sameAs    <http://ddwiki.reso.org/display/DDW/Fencing+Field> ;
  vs:term_status   "stable"
.
reso:FinancialDataSource a rdf:Property ;
  rdfs:comment     "The source of the Rental information. For example Accountant, Owner, etc." ;
  rdfs:domain      reso:Property ;
  rdfs:label       "FinancialDataSource" ;
  rdfs:range       enum:FinancialDataSource ;
  reso:CertificationLevel "Bronze" ;
  reso:PropertyTypes "RINC" ;
  schema:sameAs    <http://ddwiki.reso.org/display/DDW/FinancialDataSource+Field> ;
  vs:term_status   "stable"
.
reso:FireplaceFeatures a rdf:Property ;
  rdfs:comment     "A list of features or description of the fireplace(s) included in the sale/lease." ;
  rdfs:domain      reso:Property ;
  rdfs:label       "FireplaceFeatures" ;
  rdfs:range       xsd:string ;
  reso:CertificationLevel "Platinum" ;
  reso:PropertyTypes "RESI","RLSE","RINC","MOBI","FARM" ;
  schema:sameAs    <http://ddwiki.reso.org/display/DDW/FireplaceFeatures+Field> ;
  vs:term_status   "stable"
.
reso:FireplaceYN a rdf:Property ;
  rdfs:comment     "Does the property include a fireplace." ;
  rdfs:domain      reso:Property ;
  rdfs:label       "FireplaceYN" ;
  rdfs:range       xsd:boolean ;
  reso:CertificationLevel "Platinum" ;
  reso:PropertyTypes "RESI","RLSE","RINC","MOBI","FARM" ;
  schema:sameAs    <http://ddwiki.reso.org/display/DDW/FireplaceYN+Field> ;
  vs:term_status   "stable"
.
reso:FireplacesTotal a rdf:Property ;
  rdfs:comment     "The total number of fireplaces included in the property." ;
  rdfs:domain      reso:Property ;
  rdfs:label       "FireplacesTotal" ;
  rdfs:range       xsd:decimal ;
  reso:CertificationLevel "Platinum" ;
  reso:PropertyTypes "RESI","RLSE","RINC","MOBI","FARM" ;
  schema:sameAs    <http://ddwiki.reso.org/display/DDW/FireplacesTotal+Field> ;
  vs:term_status   "stable"
.
reso:Flooring a rdf:Property ;
  rdfs:comment     "A list of the type(s) of flooring found within the property." ;
  rdfs:domain      reso:Property ;
  rdfs:label       "Flooring" ;
  rdfs:range       xsd:string ;
  reso:CertificationLevel "Platinum" ;
  reso:PropertyTypes "RESI","RLSE","RINC","MOBI","FARM","COMS","COML" ;
  schema:sameAs    <http://ddwiki.reso.org/display/DDW/Flooring+Field> ;
  vs:term_status   "stable"
.
reso:FoundationArea a rdf:Property ;
  rdfs:comment     "The area or dimensions of the footprint of the structure on the lot." ;
  rdfs:domain      reso:Property ;
  rdfs:label       "FoundationArea" ;
  rdfs:range       xsd:decimal ;
  reso:CertificationLevel "Silver" ;
  reso:PropertyTypes "RESI","RLSE","RINC","MOBI","FARM","COMS","COML" ;
  schema:sameAs    <http://ddwiki.reso.org/display/DDW/FoundationArea+Field> ;
  vs:term_status   "stable"
.
reso:FoundationDetails a rdf:Property ;
  rdfs:comment     "A list of the type(s) of foundation on which the property sits." ;
  rdfs:domain      reso:Property ;
  rdfs:label       "FoundationDetails" ;
  rdfs:range       enum:FoundationDetails ;
  reso:CertificationLevel "Silver" ;
  reso:PropertyTypes "RESI","RLSE","RINC","MOBI","FARM","COMS","COML" ;
  schema:sameAs    <http://ddwiki.reso.org/display/DDW/FoundationDetails+Field> ;
  vs:term_status   "stable"
.
reso:FrontageLength a rdf:Property ;
  rdfs:comment     "Textual description of the length of the frontages selected in the Frontage Type field." ;
  rdfs:domain      reso:Property ;
  rdfs:label       "FrontageLength" ;
  rdfs:range       xsd:string ;
  reso:CertificationLevel "Gold" ;
  reso:PropertyTypes "RESI","RLSE","RINC","LAND","MOBI","FARM","COMS","COML","BUSO" ;
  schema:sameAs    <http://ddwiki.reso.org/display/DDW/FrontageLength+Field> ;
  vs:term_status   "stable"
.
reso:FrontageType a rdf:Property ;
  rdfs:comment     "Pick list of types of frontage.  i.e. Oceanfront, Lakefront, Golf course&#x2026;etc.&#x2026;.  Information about roads or road frontage should be located in the Road Frontage Type and Road Surface Type fields." ;
  rdfs:domain      reso:Property ;
  rdfs:label       "FrontageType" ;
  rdfs:range       xsd:string ;
  reso:CertificationLevel "Gold" ;
  reso:PropertyTypes "RESI","RLSE","RINC","LAND","MOBI","FARM","COMS","COML","BUSO" ;
  schema:sameAs    <http://ddwiki.reso.org/display/DDW/FrontageType+Field> ;
  vs:term_status   "stable"
.
reso:FuelExpense a rdf:Property ;
  rdfs:comment     "The annual expense that is not paid directly by the tenant and is included in the Operating Expense calculations." ;
  rdfs:domain      reso:Property ;
  rdfs:label       "FuelExpense" ;
  rdfs:range       xsd:decimal ;
  reso:CertificationLevel "Silver" ;
  reso:PropertyTypes "RINC","COMS","COML" ;
  schema:sameAs    <http://ddwiki.reso.org/display/DDW/FuelExpense+Field> ;
  vs:term_status   "stable"
.
reso:Furnished a rdf:Property ;
  rdfs:comment     "The property being leased is furnished, unfurnished or partially furnished." ;
  rdfs:domain      reso:Property ;
  rdfs:label       "Furnished" ;
  rdfs:range       enum:Furnished ;
  reso:CertificationLevel "Bronze" ;
  reso:PropertyTypes "RLSE" ;
  schema:sameAs    <http://ddwiki.reso.org/display/DDW/Furnished+Field> ;
  vs:term_status   "stable"
.
reso:FurnitureReplacementExpense a rdf:Property ;
  rdfs:comment     "The annual expense that is not paid directly by the tenant and is included in the Operating Expense calculations." ;
  rdfs:domain      reso:Property ;
  rdfs:label       "FurnitureReplacementExpense" ;
  rdfs:range       xsd:decimal ;
  reso:CertificationLevel "Silver" ;
  reso:PropertyTypes "RINC" ;
  schema:sameAs    <http://ddwiki.reso.org/display/DDW/FurnitureReplacementExpense+Field> ;
  vs:term_status   "stable"
.
reso:GarageSpaces a rdf:Property ;
  rdfs:comment     "The number of spaces in the garage(s)." ;
  rdfs:domain      reso:Property ;
  rdfs:label       "GarageSpaces" ;
  rdfs:range       xsd:decimal ;
  reso:CertificationLevel "Core" ;
  reso:PropertyTypes "RESI","RLSE","RINC","MOBI","FARM" ;
  schema:sameAs    <http://ddwiki.reso.org/display/DDW/GarageSpaces+Field> ;
  vs:term_status   "stable"
.
reso:GarageYN a rdf:Property ;
  rdfs:comment     "A flag indicating that the listing has a garage. This flag may be T/F, Y/N or other true, false or unknown indicator. As with all flags, the field may be null." ;
  rdfs:domain      reso:Property ;
  rdfs:label       "GarageYN" ;
  rdfs:range       xsd:boolean ;
  reso:CertificationLevel "Core" ;
  reso:PropertyTypes "RESI","RLSE","RINC","MOBI","FARM" ;
  schema:sameAs    <http://ddwiki.reso.org/display/DDW/GarageYN+Field> ;
  vs:term_status   "stable"
.
reso:GardnerExpense a rdf:Property ;
  rdfs:comment     "The annual expense that is not paid directly by the tenant and is included in the Operating Expense calculations." ;
  rdfs:domain      reso:Property ;
  rdfs:label       "GardnerExpense" ;
  rdfs:range       xsd:decimal ;
  reso:CertificationLevel "Silver" ;
  reso:PropertyTypes "RINC" ;
  schema:sameAs    <http://ddwiki.reso.org/display/DDW/GardnerExpense+Field> ;
  vs:term_status   "stable"
.
reso:Gas a rdf:Property ;
  rdfs:domain      reso:Property ;
  rdfs:label       "Gas" ;
  rdfs:range       xsd:string ;
  reso:CertificationLevel "Bronze" ;
  reso:PropertyTypes "RESI","RLSE","RINC","LAND","MOBI","FARM" ;
  schema:sameAs    <http://ddwiki.reso.org/display/DDW/Gas+Field> ;
  vs:term_status   "stable"
.
reso:GrazingPermitsBlmYN a rdf:Property ;
  rdfs:comment     "Specifies whether or not the property owner has grazing permits from the Bureau of Land Management." ;
  rdfs:domain      reso:Property ;
  rdfs:label       "GrazingPermitsBlmYN" ;
  rdfs:range       xsd:boolean ;
  reso:CertificationLevel "Gold" ;
  reso:PropertyTypes "FARM" ;
  schema:sameAs    <http://ddwiki.reso.org/display/DDW/GrazingPermitsBlmYN+Field> ;
  vs:term_status   "stable"
.
reso:GrazingPermitsForestServiceYN a rdf:Property ;
  rdfs:comment     "Specifies whether or not the property owner has grazing permits from the Forestry Service." ;
  rdfs:domain      reso:Property ;
  rdfs:label       "GrazingPermitsForestServiceYN" ;
  rdfs:range       xsd:boolean ;
  reso:CertificationLevel "Gold" ;
  reso:PropertyTypes "FARM" ;
  schema:sameAs    <http://ddwiki.reso.org/display/DDW/GrazingPermitsForestServiceYN+Field> ;
  vs:term_status   "stable"
.
reso:GrazingPermitsPrivateYN a rdf:Property ;
  rdfs:comment     "Specifies whether or not the property owner has private grazing permits." ;
  rdfs:domain      reso:Property ;
  rdfs:label       "GrazingPermitsPrivateYN" ;
  rdfs:range       xsd:boolean ;
  reso:CertificationLevel "Gold" ;
  reso:PropertyTypes "FARM" ;
  schema:sameAs    <http://ddwiki.reso.org/display/DDW/GrazingPermitsPrivateYN+Field> ;
  vs:term_status   "stable"
.
reso:GreenBuildingVerificationType a rdf:Property ;
  rdfs:domain      reso:Property ;
  rdfs:label       "GreenBuildingVerificationType" ;
  rdfs:range       enum:GreenBuildingVerificationType ;
  reso:CertificationLevel "Silver" ;
  reso:PropertyTypes "RESI","RLSE","RINC","MOBI","FARM","COMS","COML" ;
  schema:sameAs    <http://ddwiki.reso.org/display/DDW/GreenBuildingVerificationType+Field> ;
  vs:term_status   "stable"
.
reso:GreenEnergyEfficient a rdf:Property ;
  rdfs:comment     "Pick list of general green attributes such as energy efficient doors, or appliances without naming specific elements with ratings that may wane over time." ;
  rdfs:domain      reso:Property ;
  rdfs:label       "GreenEnergyEfficient" ;
  rdfs:range       enum:GreenEnergyEfficient ;
  reso:CertificationLevel "Silver" ;
  reso:PropertyTypes "RESI","RLSE","RINC","MOBI","FARM","COMS","COML" ;
  schema:sameAs    <http://ddwiki.reso.org/display/DDW/GreenEnergyEfficient+Field> ;
  vs:term_status   "stable"
.
reso:GreenEnergyGeneration a rdf:Property ;
  rdfs:comment     "Methods of generating power that are included in the sale or lease." ;
  rdfs:domain      reso:Property ;
  rdfs:label       "GreenEnergyGeneration" ;
  rdfs:range       enum:GreenEnergyGeneration ;
  reso:CertificationLevel "Silver" ;
  reso:PropertyTypes "RESI","RLSE","RINC","MOBI","FARM","COMS","COML" ;
  schema:sameAs    <http://ddwiki.reso.org/display/DDW/GreenEnergyGeneration+Field> ;
  vs:term_status   "stable"
.
reso:GreenIndoorAirQuality a rdf:Property ;
  rdfs:comment     "Pick list of indoor air quality measures without naming specific elements with ratings that may wane over time." ;
  rdfs:domain      reso:Property ;
  rdfs:label       "GreenIndoorAirQuality" ;
  rdfs:range       enum:GreenIndoorAirQuality ;
  reso:CertificationLevel "Silver" ;
  reso:PropertyTypes "RESI","RLSE","RINC","MOBI","FARM","COMS","COML" ;
  schema:sameAs    <http://ddwiki.reso.org/display/DDW/GreenIndoorAirQuality+Field> ;
  vs:term_status   "stable"
.
reso:GreenLocation a rdf:Property ;
  rdfs:comment     "Pick list describing efficiencies involved with the property's location such as walkability or transportation proximity without naming specific elements with ratings that may wane over time." ;
  rdfs:domain      reso:Property ;
  rdfs:label       "GreenLocation" ;
  rdfs:range       xsd:string ;
  reso:CertificationLevel "Silver" ;
  reso:PropertyTypes "RESI","RLSE","RINC","MOBI","FARM","COMS","COML" ;
  schema:sameAs    <http://ddwiki.reso.org/display/DDW/GreenLocation+Field> ;
  vs:term_status   "stable"
.
reso:GreenSustainability a rdf:Property ;
  rdfs:comment     "Pick list of sustainable elements used in the construction of the structure without naming specific elements with ratings that may wane over time." ;
  rdfs:domain      reso:Property ;
  rdfs:label       "GreenSustainability" ;
  rdfs:range       enum:GreenSustainability ;
  reso:CertificationLevel "Silver" ;
  reso:PropertyTypes "RESI","RLSE","RINC","MOBI","FARM","COMS","COML" ;
  schema:sameAs    <http://ddwiki.reso.org/display/DDW/GreenSustainability+Field> ;
  vs:term_status   "stable"
.
reso:GreenVerification a rdf:Property ;
  rdfs:comment     "The name of the body or group providing the verification/certification/rating named in the GreenBuildingVerificationType field.  There is almost always a direct correlation between bodies and programs. This is a repeating element.  If desired replace [Type] with the name of the certification from the GreenBuildingVerificationType list." ;
  rdfs:domain      reso:Property ;
  rdfs:label       "GreenVerification" ;
  rdfs:range       xsd:string ;
  reso:CertificationLevel "Silver" ;
  reso:PropertyTypes "RESI","RLSE","RINC","MOBI","FARM","COMS","COML" ;
  schema:sameAs    <http://ddwiki.reso.org/display/DDW/GreenVerification%5BType%5DBody+Field> ;
  vs:term_status   "stable"
.
reso:GreenVerification a rdf:Property ;
  rdfs:comment     "The name of the body or group providing the verification/certification/rating named in the GreenBuildingVerificationType field.  There is almost always a direct correlation between bodies and programs. This is a repeating element.  If desired replace [Type] with the name of the certification from the GreenBuildingVerificationType list.","A final score indicating the performance of energy efficiency design and measures in the home as tested by a third-party rater.  Points achieved to earn a certification in the GreenVerification[Type]Rating field do not apply to this field.  HERS Index is most common with new homes and runs with a lower number being more efficient. A net-zero home uses zero energy and has a HERS score of 0.  A home that produces more energy than it uses has a negative score.  Home Energy Score is a tool more common for existing homes and runs with a higher number being more efficient.   It takes square footage into account and caps with 10 as the highest number of points. This is a repeating element.  If desired replace [Type] with the name of the certification from the GreenBuildingVerificationType list." ;
  rdfs:domain      reso:Property ;
  rdfs:label       "GreenVerification" ;
  rdfs:range       xsd:string,xsd:decimal ;
  reso:CertificationLevel "Silver" ;
  reso:PropertyTypes "RESI","RLSE","RINC","MOBI","FARM","COMS","COML" ;
  schema:sameAs    <http://ddwiki.reso.org/display/DDW/GreenVerification%5BType%5DBody+Field>,<http://ddwiki.reso.org/display/DDW/GreenVerification%5BType%5DMetric+Field> ;
  vs:term_status   "stable"
.
reso:GreenVerification a rdf:Property ;
  rdfs:comment     "The name of the body or group providing the verification/certification/rating named in the GreenBuildingVerificationType field.  There is almost always a direct correlation between bodies and programs. This is a repeating element.  If desired replace [Type] with the name of the certification from the GreenBuildingVerificationType list.","A final score indicating the performance of energy efficiency design and measures in the home as tested by a third-party rater.  Points achieved to earn a certification in the GreenVerification[Type]Rating field do not apply to this field.  HERS Index is most common with new homes and runs with a lower number being more efficient. A net-zero home uses zero energy and has a HERS score of 0.  A home that produces more energy than it uses has a negative score.  Home Energy Score is a tool more common for existing homes and runs with a higher number being more efficient.   It takes square footage into account and caps with 10 as the highest number of points. This is a repeating element.  If desired replace [Type] with the name of the certification from the GreenBuildingVerificationType list.","Many verifications or certifications have a rating system that provides an indication of the structure's level of energy efficiency.  When expressed in a numeric value, please use the GreenVerificationMetric field. Verifications and Certifications can also be a name, such as Gold or Silver, which is the purpose of this field. This is a repeating element.  If desired replace [Type] with the name of the certification from the GreenBuildingVerificationType list." ;
  rdfs:domain      reso:Property ;
  rdfs:label       "GreenVerification" ;
  rdfs:range       xsd:string,xsd:decimal ;
  reso:CertificationLevel "Silver" ;
  reso:PropertyTypes "RESI","RLSE","RINC","MOBI","FARM","COMS","COML" ;
  schema:sameAs    <http://ddwiki.reso.org/display/DDW/GreenVerification%5BType%5DBody+Field>,<http://ddwiki.reso.org/display/DDW/GreenVerification%5BType%5DMetric+Field>,<http://ddwiki.reso.org/display/DDW/GreenVerification%5BType%5DRating+Field> ;
  vs:term_status   "stable"
.
reso:GreenVerification a rdf:Property ;
  rdfs:comment     "The name of the body or group providing the verification/certification/rating named in the GreenBuildingVerificationType field.  There is almost always a direct correlation between bodies and programs. This is a repeating element.  If desired replace [Type] with the name of the certification from the GreenBuildingVerificationType list.","A final score indicating the performance of energy efficiency design and measures in the home as tested by a third-party rater.  Points achieved to earn a certification in the GreenVerification[Type]Rating field do not apply to this field.  HERS Index is most common with new homes and runs with a lower number being more efficient. A net-zero home uses zero energy and has a HERS score of 0.  A home that produces more energy than it uses has a negative score.  Home Energy Score is a tool more common for existing homes and runs with a higher number being more efficient.   It takes square footage into account and caps with 10 as the highest number of points. This is a repeating element.  If desired replace [Type] with the name of the certification from the GreenBuildingVerificationType list.","Many verifications or certifications have a rating system that provides an indication of the structure's level of energy efficiency.  When expressed in a numeric value, please use the GreenVerificationMetric field. Verifications and Certifications can also be a name, such as Gold or Silver, which is the purpose of this field. This is a repeating element.  If desired replace [Type] with the name of the certification from the GreenBuildingVerificationType list.","The source of the green data. May address photovoltaic characteristics, or a verified score, certification, label, etc. This may be a pick list of options showing the source. i.e. Program Sponsor, Program Verifier, Public Record, Assessor,  etc." ;
  rdfs:domain      reso:Property ;
  rdfs:label       "GreenVerification" ;
  rdfs:range       xsd:string,xsd:decimal,enum:GreenVerificationSource ;
  reso:CertificationLevel "Silver" ;
  reso:PropertyTypes "RESI","RLSE","RINC","MOBI","FARM","COMS","COML" ;
  schema:sameAs    <http://ddwiki.reso.org/display/DDW/GreenVerification%5BType%5DBody+Field>,<http://ddwiki.reso.org/display/DDW/GreenVerification%5BType%5DMetric+Field>,<http://ddwiki.reso.org/display/DDW/GreenVerification%5BType%5DRating+Field>,<http://ddwiki.reso.org/display/DDW/GreenVerification%5BType%5DSource+Field> ;
  vs:term_status   "stable"
.
reso:GreenVerification a rdf:Property ;
  rdfs:comment     "The name of the body or group providing the verification/certification/rating named in the GreenBuildingVerificationType field.  There is almost always a direct correlation between bodies and programs. This is a repeating element.  If desired replace [Type] with the name of the certification from the GreenBuildingVerificationType list.","A final score indicating the performance of energy efficiency design and measures in the home as tested by a third-party rater.  Points achieved to earn a certification in the GreenVerification[Type]Rating field do not apply to this field.  HERS Index is most common with new homes and runs with a lower number being more efficient. A net-zero home uses zero energy and has a HERS score of 0.  A home that produces more energy than it uses has a negative score.  Home Energy Score is a tool more common for existing homes and runs with a higher number being more efficient.   It takes square footage into account and caps with 10 as the highest number of points. This is a repeating element.  If desired replace [Type] with the name of the certification from the GreenBuildingVerificationType list.","Many verifications or certifications have a rating system that provides an indication of the structure's level of energy efficiency.  When expressed in a numeric value, please use the GreenVerificationMetric field. Verifications and Certifications can also be a name, such as Gold or Silver, which is the purpose of this field. This is a repeating element.  If desired replace [Type] with the name of the certification from the GreenBuildingVerificationType list.","The source of the green data. May address photovoltaic characteristics, or a verified score, certification, label, etc. This may be a pick list of options showing the source. i.e. Program Sponsor, Program Verifier, Public Record, Assessor,  etc.","Many verification programs include a multi-step process that may begin with plans and specs, involve testing and/or submission of building specifications along the way and include a final verification step.&#xa0; When ratings are involved it is not uncommon for the final rating to be either higher or lower than the target preliminary rating.&#xa0; Sometimes the final approval is not available until after sale and occupancy.&#xa0; Status indicates what the target was at the time of listing and may be updated when verification is complete.&#xa0; To limit liability concerns this field reflects information that was available at the time of listing or updated later and should be confirmed by the buyer." ;
  rdfs:domain      reso:Property ;
  rdfs:label       "GreenVerification" ;
  rdfs:range       xsd:string,xsd:decimal,enum:GreenVerificationSource ;
  reso:CertificationLevel "Silver" ;
  reso:PropertyTypes "RESI","RLSE","RINC","MOBI","FARM","COMS","COML" ;
  schema:sameAs    <http://ddwiki.reso.org/display/DDW/GreenVerification%5BType%5DBody+Field>,<http://ddwiki.reso.org/display/DDW/GreenVerification%5BType%5DMetric+Field>,<http://ddwiki.reso.org/display/DDW/GreenVerification%5BType%5DRating+Field>,<http://ddwiki.reso.org/display/DDW/GreenVerification%5BType%5DSource+Field>,<http://ddwiki.reso.org/display/DDW/GreenVerification%5BType%5DStatus+Field> ;
  vs:term_status   "stable"
.
reso:GreenVerification a rdf:Property ;
  rdfs:comment     "The name of the body or group providing the verification/certification/rating named in the GreenBuildingVerificationType field.  There is almost always a direct correlation between bodies and programs. This is a repeating element.  If desired replace [Type] with the name of the certification from the GreenBuildingVerificationType list.","A final score indicating the performance of energy efficiency design and measures in the home as tested by a third-party rater.  Points achieved to earn a certification in the GreenVerification[Type]Rating field do not apply to this field.  HERS Index is most common with new homes and runs with a lower number being more efficient. A net-zero home uses zero energy and has a HERS score of 0.  A home that produces more energy than it uses has a negative score.  Home Energy Score is a tool more common for existing homes and runs with a higher number being more efficient.   It takes square footage into account and caps with 10 as the highest number of points. This is a repeating element.  If desired replace [Type] with the name of the certification from the GreenBuildingVerificationType list.","Many verifications or certifications have a rating system that provides an indication of the structure's level of energy efficiency.  When expressed in a numeric value, please use the GreenVerificationMetric field. Verifications and Certifications can also be a name, such as Gold or Silver, which is the purpose of this field. This is a repeating element.  If desired replace [Type] with the name of the certification from the GreenBuildingVerificationType list.","The source of the green data. May address photovoltaic characteristics, or a verified score, certification, label, etc. This may be a pick list of options showing the source. i.e. Program Sponsor, Program Verifier, Public Record, Assessor,  etc.","Many verification programs include a multi-step process that may begin with plans and specs, involve testing and/or submission of building specifications along the way and include a final verification step.&#xa0; When ratings are involved it is not uncommon for the final rating to be either higher or lower than the target preliminary rating.&#xa0; Sometimes the final approval is not available until after sale and occupancy.&#xa0; Status indicates what the target was at the time of listing and may be updated when verification is complete.&#xa0; To limit liability concerns this field reflects information that was available at the time of listing or updated later and should be confirmed by the buyer.","Provides a link to the specific property&#x2019;s high-performance rating or scoring details directly from and hosted by the sponsoring body of the program.   Typically provides thorough details, for example, which points where achieved and how, or in the case of a score what specifically was tested and the results. This is a repeating element.  If desired replace [Type] with the name of the certification from the GreenBuildingVerificationType list." ;
  rdfs:domain      reso:Property ;
  rdfs:label       "GreenVerification" ;
  rdfs:range       xsd:string,xsd:decimal,enum:GreenVerificationSource ;
  reso:CertificationLevel "Silver" ;
  reso:PropertyTypes "RESI","RLSE","RINC","MOBI","FARM","COMS","COML" ;
  schema:sameAs    <http://ddwiki.reso.org/display/DDW/GreenVerification%5BType%5DBody+Field>,<http://ddwiki.reso.org/display/DDW/GreenVerification%5BType%5DMetric+Field>,<http://ddwiki.reso.org/display/DDW/GreenVerification%5BType%5DRating+Field>,<http://ddwiki.reso.org/display/DDW/GreenVerification%5BType%5DSource+Field>,<http://ddwiki.reso.org/display/DDW/GreenVerification%5BType%5DStatus+Field>,<http://ddwiki.reso.org/display/DDW/GreenVerification%5BType%5DURL+Field> ;
  vs:term_status   "stable"
.
reso:GreenVerification a rdf:Property ;
  rdfs:comment     "The name of the body or group providing the verification/certification/rating named in the GreenBuildingVerificationType field.  There is almost always a direct correlation between bodies and programs. This is a repeating element.  If desired replace [Type] with the name of the certification from the GreenBuildingVerificationType list.","A final score indicating the performance of energy efficiency design and measures in the home as tested by a third-party rater.  Points achieved to earn a certification in the GreenVerification[Type]Rating field do not apply to this field.  HERS Index is most common with new homes and runs with a lower number being more efficient. A net-zero home uses zero energy and has a HERS score of 0.  A home that produces more energy than it uses has a negative score.  Home Energy Score is a tool more common for existing homes and runs with a higher number being more efficient.   It takes square footage into account and caps with 10 as the highest number of points. This is a repeating element.  If desired replace [Type] with the name of the certification from the GreenBuildingVerificationType list.","Many verifications or certifications have a rating system that provides an indication of the structure's level of energy efficiency.  When expressed in a numeric value, please use the GreenVerificationMetric field. Verifications and Certifications can also be a name, such as Gold or Silver, which is the purpose of this field. This is a repeating element.  If desired replace [Type] with the name of the certification from the GreenBuildingVerificationType list.","The source of the green data. May address photovoltaic characteristics, or a verified score, certification, label, etc. This may be a pick list of options showing the source. i.e. Program Sponsor, Program Verifier, Public Record, Assessor,  etc.","Many verification programs include a multi-step process that may begin with plans and specs, involve testing and/or submission of building specifications along the way and include a final verification step.&#xa0; When ratings are involved it is not uncommon for the final rating to be either higher or lower than the target preliminary rating.&#xa0; Sometimes the final approval is not available until after sale and occupancy.&#xa0; Status indicates what the target was at the time of listing and may be updated when verification is complete.&#xa0; To limit liability concerns this field reflects information that was available at the time of listing or updated later and should be confirmed by the buyer.","Provides a link to the specific property&#x2019;s high-performance rating or scoring details directly from and hosted by the sponsoring body of the program.   Typically provides thorough details, for example, which points where achieved and how, or in the case of a score what specifically was tested and the results. This is a repeating element.  If desired replace [Type] with the name of the certification from the GreenBuildingVerificationType list.","The version of the certification or verification that was awarded.  Some rating programs have a year, a version, or possibly both.  This is a repeating element.  If desired replace [Type] with the name of the certification from the GreenBuildingVerificationType list." ;
  rdfs:domain      reso:Property ;
  rdfs:label       "GreenVerification" ;
  rdfs:range       xsd:string,xsd:decimal,enum:GreenVerificationSource ;
  reso:CertificationLevel "Silver" ;
  reso:PropertyTypes "RESI","RLSE","RINC","MOBI","FARM","COMS","COML" ;
  schema:sameAs    <http://ddwiki.reso.org/display/DDW/GreenVerification%5BType%5DBody+Field>,<http://ddwiki.reso.org/display/DDW/GreenVerification%5BType%5DMetric+Field>,<http://ddwiki.reso.org/display/DDW/GreenVerification%5BType%5DRating+Field>,<http://ddwiki.reso.org/display/DDW/GreenVerification%5BType%5DSource+Field>,<http://ddwiki.reso.org/display/DDW/GreenVerification%5BType%5DStatus+Field>,<http://ddwiki.reso.org/display/DDW/GreenVerification%5BType%5DURL+Field>,<http://ddwiki.reso.org/display/DDW/GreenVerification%5BType%5DVersion+Field> ;
  vs:term_status   "stable"
.
reso:GreenVerification a rdf:Property ;
  rdfs:comment     "The name of the body or group providing the verification/certification/rating named in the GreenBuildingVerificationType field.  There is almost always a direct correlation between bodies and programs. This is a repeating element.  If desired replace [Type] with the name of the certification from the GreenBuildingVerificationType list.","A final score indicating the performance of energy efficiency design and measures in the home as tested by a third-party rater.  Points achieved to earn a certification in the GreenVerification[Type]Rating field do not apply to this field.  HERS Index is most common with new homes and runs with a lower number being more efficient. A net-zero home uses zero energy and has a HERS score of 0.  A home that produces more energy than it uses has a negative score.  Home Energy Score is a tool more common for existing homes and runs with a higher number being more efficient.   It takes square footage into account and caps with 10 as the highest number of points. This is a repeating element.  If desired replace [Type] with the name of the certification from the GreenBuildingVerificationType list.","Many verifications or certifications have a rating system that provides an indication of the structure's level of energy efficiency.  When expressed in a numeric value, please use the GreenVerificationMetric field. Verifications and Certifications can also be a name, such as Gold or Silver, which is the purpose of this field. This is a repeating element.  If desired replace [Type] with the name of the certification from the GreenBuildingVerificationType list.","The source of the green data. May address photovoltaic characteristics, or a verified score, certification, label, etc. This may be a pick list of options showing the source. i.e. Program Sponsor, Program Verifier, Public Record, Assessor,  etc.","Many verification programs include a multi-step process that may begin with plans and specs, involve testing and/or submission of building specifications along the way and include a final verification step.&#xa0; When ratings are involved it is not uncommon for the final rating to be either higher or lower than the target preliminary rating.&#xa0; Sometimes the final approval is not available until after sale and occupancy.&#xa0; Status indicates what the target was at the time of listing and may be updated when verification is complete.&#xa0; To limit liability concerns this field reflects information that was available at the time of listing or updated later and should be confirmed by the buyer.","Provides a link to the specific property&#x2019;s high-performance rating or scoring details directly from and hosted by the sponsoring body of the program.   Typically provides thorough details, for example, which points where achieved and how, or in the case of a score what specifically was tested and the results. This is a repeating element.  If desired replace [Type] with the name of the certification from the GreenBuildingVerificationType list.","The version of the certification or verification that was awarded.  Some rating programs have a year, a version, or possibly both.  This is a repeating element.  If desired replace [Type] with the name of the certification from the GreenBuildingVerificationType list.","The year the certification or verification was awarded.  This is a repeating element.  If desired replace [Type] with the name of the certification from the GreenBuildingVerificationType list." ;
  rdfs:domain      reso:Property ;
  rdfs:label       "GreenVerification" ;
  rdfs:range       xsd:string,xsd:decimal,enum:GreenVerificationSource ;
  reso:CertificationLevel "Silver" ;
  reso:PropertyTypes "RESI","RLSE","RINC","MOBI","FARM","COMS","COML" ;
  schema:sameAs    <http://ddwiki.reso.org/display/DDW/GreenVerification%5BType%5DBody+Field>,<http://ddwiki.reso.org/display/DDW/GreenVerification%5BType%5DMetric+Field>,<http://ddwiki.reso.org/display/DDW/GreenVerification%5BType%5DRating+Field>,<http://ddwiki.reso.org/display/DDW/GreenVerification%5BType%5DSource+Field>,<http://ddwiki.reso.org/display/DDW/GreenVerification%5BType%5DStatus+Field>,<http://ddwiki.reso.org/display/DDW/GreenVerification%5BType%5DURL+Field>,<http://ddwiki.reso.org/display/DDW/GreenVerification%5BType%5DVersion+Field>,<http://ddwiki.reso.org/display/DDW/GreenVerification%5BType%5DYear+Field> ;
  vs:term_status   "stable"
.
reso:GreenWaterConservation a rdf:Property ;
  rdfs:comment     "Pick list of general water conserving attributes of the property such as landscaping or reclamation without naming specific elements with ratings that may wane over time." ;
  rdfs:domain      reso:Property ;
  rdfs:label       "GreenWaterConservation" ;
  rdfs:range       enum:GreenWaterConservation ;
  reso:CertificationLevel "Silver" ;
  reso:PropertyTypes "RESI","RLSE","RINC","MOBI","FARM","COMS","COML" ;
  schema:sameAs    <http://ddwiki.reso.org/display/DDW/GreenWaterConservation+Field> ;
  vs:term_status   "stable"
.
reso:GrossIncome a rdf:Property ;
  rdfs:comment     "The actual current income from rent and all other revenue generating sources." ;
  rdfs:domain      reso:Property ;
  rdfs:label       "GrossIncome" ;
  rdfs:range       xsd:decimal ;
  reso:CertificationLevel "Core" ;
  reso:PropertyTypes "RINC","COMS","COML","BUSO" ;
  schema:sameAs    <http://ddwiki.reso.org/display/DDW/GrossIncome+Field> ;
  vs:term_status   "stable"
.
reso:GrossScheduledIncome a rdf:Property ;
  rdfs:comment     "The maximum amount of annual rent collected if the property were 100% occupied all year and all tenants paid their rent." ;
  rdfs:domain      reso:Property ;
  rdfs:label       "GrossScheduledIncome" ;
  rdfs:range       xsd:decimal ;
  reso:CertificationLevel "Core" ;
  reso:PropertyTypes "RINC","COMS","COML","BUSO" ;
  schema:sameAs    <http://ddwiki.reso.org/display/DDW/GrossScheduledIncome+Field> ;
  vs:term_status   "stable"
.
reso:HabitableResidenceYN a rdf:Property ;
  rdfs:comment     "Does the property include a structure that can be lived in." ;
  rdfs:domain      reso:Property ;
  rdfs:label       "HabitableResidenceYN" ;
  rdfs:range       xsd:boolean ;
  reso:CertificationLevel "Gold" ;
  reso:PropertyTypes "FARM" ;
  schema:sameAs    <http://ddwiki.reso.org/display/DDW/HabitableResidenceYN+Field> ;
  vs:term_status   "stable"
.
reso:Heating a rdf:Property ;
  rdfs:comment     "A list describing the heating features of the property." ;
  rdfs:domain      reso:Property ;
  rdfs:label       "Heating" ;
  rdfs:range       xsd:string ;
  reso:CertificationLevel "Platinum" ;
  reso:PropertyTypes "RESI","RLSE","RINC","MOBI","FARM","COMS","COML" ;
  schema:sameAs    <http://ddwiki.reso.org/display/DDW/Heating+Field> ;
  vs:term_status   "stable"
.
reso:HeatingYN a rdf:Property ;
  rdfs:comment     "The property has heating." ;
  rdfs:domain      reso:Property ;
  rdfs:label       "HeatingYN" ;
  rdfs:range       xsd:boolean ;
  reso:CertificationLevel "Platinum" ;
  reso:PropertyTypes "RESI","RLSE","RINC","LAND","MOBI","FARM","COMS","COML" ;
  schema:sameAs    <http://ddwiki.reso.org/display/DDW/HeatingYN+Field> ;
  vs:term_status   "stable"
.
reso:HighSchool a rdf:Property ;
  rdfs:comment     "The name of the high school having a catchment area that includes the associated property." ;
  rdfs:domain      reso:Property ;
  rdfs:label       "HighSchool" ;
  rdfs:range       xsd:string ;
  reso:CertificationLevel "Silver" ;
  reso:PropertyTypes "RESI","RLSE","RINC","LAND","MOBI","FARM","COMS","COML","BUSO" ;
  schema:sameAs    <http://ddwiki.reso.org/display/DDW/HighSchool+Field> ;
  vs:term_status   "stable"
.
reso:HighSchoolDistrict a rdf:Property ;
  rdfs:comment     "The name of the high school district having a catchment area that includes the associated property.  When only one school district is used, this field should be used over the Junior or Elementary Districts." ;
  rdfs:domain      reso:Property ;
  rdfs:label       "HighSchoolDistrict" ;
  rdfs:range       xsd:string ;
  reso:CertificationLevel "Bronze" ;
  reso:PropertyTypes "RESI","RLSE","RINC","LAND","MOBI","FARM","COMS","COML","BUSO" ;
  schema:sameAs    <http://ddwiki.reso.org/display/DDW/HighSchoolDistrict+Field> ;
  vs:term_status   "stable"
.
reso:HomeWarrantyYN a rdf:Property ;
  rdfs:comment     "Is a home warranty included in the sale of the property?  Single select." ;
  rdfs:domain      reso:Property ;
  rdfs:label       "HomeWarrantyYN" ;
  rdfs:range       xsd:boolean ;
  reso:CertificationLevel "Silver" ;
  reso:PropertyTypes "RESI","RLSE","RINC","MOBI","FARM" ;
  schema:sameAs    <http://ddwiki.reso.org/display/DDW/HomeWarrantyYN+Field> ;
  vs:term_status   "stable"
.
reso:HorseAmenities a rdf:Property ;
  rdfs:comment     "A list of horse amenities on the lot or in the community." ;
  rdfs:domain      reso:Property ;
  rdfs:label       "HorseAmenities" ;
  rdfs:range       xsd:string ;
  reso:CertificationLevel "Platinum" ;
  reso:PropertyTypes "RESI","RLSE","LAND" ;
  schema:sameAs    <http://ddwiki.reso.org/display/DDW/HorseAmenities+Field> ;
  vs:term_status   "stable"
.
reso:HorseYN a rdf:Property ;
  rdfs:comment     "The Property is allowed to raise horses." ;
  rdfs:domain      reso:Property ;
  rdfs:label       "HorseYN" ;
  rdfs:range       xsd:boolean ;
  reso:CertificationLevel "Platinum" ;
  reso:PropertyTypes "RESI","RLSE","LAND" ;
  schema:sameAs    <http://ddwiki.reso.org/display/DDW/HorseYN+Field> ;
  vs:term_status   "stable"
.
reso:HoursDaysOfOperation a rdf:Property ;
  rdfs:comment     "A simplified enumerated list of the days and hours of operation of the business being sold.  i.e. Open 24 Hours or Open 7 Days.  For more detailed descriptions use the HoursDaysofOperationDescription field." ;
  rdfs:domain      reso:Property ;
  rdfs:label       "HoursDaysOfOperation" ;
  rdfs:range       enum:HoursDaysOfOperation ;
  reso:CertificationLevel "Silver" ;
  reso:PropertyTypes "BUSO" ;
  schema:sameAs    <http://ddwiki.reso.org/display/DDW/HoursDaysOfOperation+Field> ;
  vs:term_status   "stable"
.
reso:HoursDaysofOperationDescription a rdf:Property ;
  rdfs:comment     "A detailed description of the hours and days the business being sold is open for business.  For a specific list of simplified times the business is open, use the HoursDaysofOperation enumerated field." ;
  rdfs:domain      reso:Property ;
  rdfs:label       "HoursDaysofOperationDescription" ;
  rdfs:range       xsd:string ;
  reso:CertificationLevel "Silver" ;
  reso:PropertyTypes "BUSO" ;
  schema:sameAs    <http://ddwiki.reso.org/display/DDW/HoursDaysofOperationDescription+Field> ;
  vs:term_status   "stable"
.
reso:Inclusions a rdf:Property ;
  rdfs:comment     "Portable elements of the property that will be included in the sale." ;
  rdfs:domain      reso:Property ;
  rdfs:label       "Inclusions" ;
  rdfs:range       xsd:string ;
  reso:CertificationLevel "Bronze" ;
  reso:PropertyTypes "RESI","RLSE","RINC","LAND","MOBI","FARM","COMS","COML","BUSO" ;
  schema:sameAs    <http://ddwiki.reso.org/display/DDW/Inclusions+Field> ;
  vs:term_status   "stable"
.
reso:IncomeIncludes a rdf:Property ;
  rdfs:comment     "A list of income sources included in the GrossScheduledIncome and GrossIncome.  i.e. Laundry, Parking, Recreation, Storage, etc." ;
  rdfs:domain      reso:Property ;
  rdfs:label       "IncomeIncludes" ;
  rdfs:range       enum:IncomeIncludes ;
  reso:CertificationLevel "Bronze" ;
  reso:PropertyTypes "RINC","LAND" ;
  schema:sameAs    <http://ddwiki.reso.org/display/DDW/IncomeIncludes+Field> ;
  vs:term_status   "stable"
.
reso:InsuranceExpense a rdf:Property ;
  rdfs:comment     "The annual expense that is not paid directly by the tenant and is included in the Operating Expense calculations." ;
  rdfs:domain      reso:Property ;
  rdfs:label       "InsuranceExpense" ;
  rdfs:range       xsd:decimal ;
  reso:CertificationLevel "Silver" ;
  reso:PropertyTypes "RINC","COMS","COML" ;
  schema:sameAs    <http://ddwiki.reso.org/display/DDW/InsuranceExpense+Field> ;
  vs:term_status   "stable"
.
reso:InteriorFeatures a rdf:Property ;
  rdfs:comment     "A list of features or description of the interior of the property included in the sale/lease." ;
  rdfs:domain      reso:Property ;
  rdfs:label       "InteriorFeatures" ;
  rdfs:range       xsd:string ;
  reso:CertificationLevel "Platinum" ;
  reso:PropertyTypes "RESI","RLSE","RINC","MOBI","FARM" ;
  schema:sameAs    <http://ddwiki.reso.org/display/DDW/InteriorFeatures+Field> ;
  vs:term_status   "stable"
.
reso:InternetAddressDisplayYN a rdf:Property ;
  rdfs:comment     "A yes/no field that states the seller has allowed the listing address to be displayed on Internet sites." ;
  rdfs:domain      reso:Property ;
  rdfs:label       "InternetAddressDisplayYN" ;
  rdfs:range       xsd:boolean ;
  reso:CertificationLevel "Core" ;
  reso:PropertyTypes "RESI","RLSE","RINC","LAND","MOBI","FARM","COMS","COML","BUSO" ;
  schema:sameAs    <http://ddwiki.reso.org/display/DDW/InternetAddressDisplayYN+Field> ;
  vs:term_status   "stable"
.
reso:InternetAutomatedValuationDisplayYN a rdf:Property ;
  rdfs:comment     "A yes/no field that states the seller allows the listing can be displayed with an AVM on Internet sites." ;
  rdfs:domain      reso:Property ;
  rdfs:label       "InternetAutomatedValuationDisplayYN" ;
  rdfs:range       xsd:boolean ;
  reso:CertificationLevel "Core" ;
  reso:PropertyTypes "RESI","RLSE","RINC","LAND","MOBI","FARM","COMS","COML","BUSO" ;
  schema:sameAs    <http://ddwiki.reso.org/display/DDW/InternetAutomatedValuationDisplayYN+Field> ;
  vs:term_status   "stable"
.
reso:InternetConsumerCommentYN a rdf:Property ;
  rdfs:comment     "A yes/no field that states the seller allows a comment or blog system to be attached to the listing on Internet sites." ;
  rdfs:domain      reso:Property ;
  rdfs:label       "InternetConsumerCommentYN" ;
  rdfs:range       xsd:boolean ;
  reso:CertificationLevel "Core" ;
  reso:PropertyTypes "RESI","RLSE","RINC","LAND","MOBI","FARM","COMS","COML","BUSO" ;
  schema:sameAs    <http://ddwiki.reso.org/display/DDW/InternetConsumerCommentYN+Field> ;
  vs:term_status   "stable"
.
reso:InternetEntireListingDisplayYN a rdf:Property ;
  rdfs:comment     "A yes/no field that states the seller has allowed the listing to be displayed on Internet sites." ;
  rdfs:domain      reso:Property ;
  rdfs:label       "InternetEntireListingDisplayYN" ;
  rdfs:range       xsd:boolean ;
  reso:CertificationLevel "Core" ;
  reso:PropertyTypes "RESI","RLSE","RINC","LAND","MOBI","FARM","COMS","COML","BUSO" ;
  schema:sameAs    <http://ddwiki.reso.org/display/DDW/InternetEntireListingDisplayYN+Field> ;
  vs:term_status   "stable"
.
reso:IrrigationSource a rdf:Property ;
  rdfs:comment     "The source which the property receives its water for irrigation." ;
  rdfs:domain      reso:Property ;
  rdfs:label       "IrrigationSource" ;
  rdfs:range       xsd:string ;
  reso:CertificationLevel "Bronze" ;
  reso:PropertyTypes "LAND","FARM" ;
  schema:sameAs    <http://ddwiki.reso.org/display/DDW/IrrigationSource+Field> ;
  vs:term_status   "stable"
.
reso:IrrigationWaterRightsAcres a rdf:Property ;
  rdfs:comment     "The number of acres allowed under the property's water rights." ;
  rdfs:domain      reso:Property ;
  rdfs:label       "IrrigationWaterRightsAcres" ;
  rdfs:range       xsd:decimal ;
  reso:CertificationLevel "Bronze" ;
  reso:PropertyTypes "FARM" ;
  schema:sameAs    <http://ddwiki.reso.org/display/DDW/IrrigationWaterRightsAcres+Field> ;
  vs:term_status   "stable"
.
reso:IrrigationWaterRightsYN a rdf:Property ;
  rdfs:comment     "Does the property include water rights for irrigation?  A Boolean or Yes / No field." ;
  rdfs:domain      reso:Property ;
  rdfs:label       "IrrigationWaterRightsYN" ;
  rdfs:range       xsd:boolean ;
  reso:CertificationLevel "Bronze" ;
  reso:PropertyTypes "FARM" ;
  schema:sameAs    <http://ddwiki.reso.org/display/DDW/IrrigationWaterRightsYN+Field> ;
  vs:term_status   "stable"
.
reso:LaborInformation a rdf:Property ;
  rdfs:comment     "Information about labor laws that are applicable to the business being sold. i.e. Union, Non-Union, Employee License Required." ;
  rdfs:domain      reso:Property ;
  rdfs:label       "LaborInformation" ;
  rdfs:range       xsd:string ;
  reso:CertificationLevel "Silver" ;
  reso:PropertyTypes "BUSO" ;
  schema:sameAs    <http://ddwiki.reso.org/display/DDW/LaborInformation+Field> ;
  vs:term_status   "stable"
.
reso:LandLeaseAmount a rdf:Property ;
  rdfs:comment     "When the land is not included in the sale, but is leased, the amount of the lease.  This is the Space Rent for Mobile homes in a Park." ;
  rdfs:domain      reso:Property ;
  rdfs:label       "LandLeaseAmount" ;
  rdfs:range       xsd:decimal ;
  reso:CertificationLevel "Bronze" ;
  reso:PropertyTypes "RESI","RINC","LAND","MOBI","FARM","COMS","COML","BUSO" ;
  schema:sameAs    <http://ddwiki.reso.org/display/DDW/LandLeaseAmount+Field> ;
  vs:term_status   "stable"
.
reso:LandLeaseAmountFrequency a rdf:Property ;
  rdfs:comment     "When the land is not included in the sale, but is leased, the frequency the Land Lease Fee is paid." ;
  rdfs:domain      reso:Property ;
  rdfs:label       "LandLeaseAmountFrequency" ;
  rdfs:range       enum:FeeFrequency ;
  reso:CertificationLevel "Bronze" ;
  reso:PropertyTypes "RESI","RINC","LAND","MOBI","FARM","COMS","COML","BUSO" ;
  schema:sameAs    <http://ddwiki.reso.org/display/DDW/LandLeaseAmountFrequency+Field> ;
  vs:term_status   "stable"
.
reso:LandLeaseExpirationDate a rdf:Property ;
  rdfs:comment     "When the land is not included in the sale, but is leased, the expiration date of the Land Lease." ;
  rdfs:domain      reso:Property ;
  rdfs:label       "LandLeaseExpirationDate" ;
  rdfs:range       xsd:date ;
  reso:CertificationLevel "Bronze" ;
  reso:PropertyTypes "RESI","RINC","LAND","MOBI","FARM","COMS","COML","BUSO" ;
  schema:sameAs    <http://ddwiki.reso.org/display/DDW/LandLeaseExpirationDate+Field> ;
  vs:term_status   "stable"
.
reso:LandLeaseYN a rdf:Property ;
  rdfs:comment     "The land is not included in the sale and a lease exists." ;
  rdfs:domain      reso:Property ;
  rdfs:label       "LandLeaseYN" ;
  rdfs:range       xsd:boolean ;
  reso:CertificationLevel "Core" ;
  reso:PropertyTypes "RESI","RINC","LAND","MOBI","FARM","COMS","COML","BUSO" ;
  schema:sameAs    <http://ddwiki.reso.org/display/DDW/LandLeaseYN+Field> ;
  vs:term_status   "stable"
.
reso:Latitude a rdf:Property ;
  rdfs:comment     "The geographic latitude of some reference point on the property, specified in degrees and decimal parts.  Positive numbers must not include the plus symbol." ;
  rdfs:domain      reso:Property ;
  rdfs:label       "Latitude" ;
  rdfs:range       xsd:decimal ;
  reso:CertificationLevel "Core" ;
  reso:PropertyTypes "RESI","RLSE","RINC","LAND","MOBI","FARM","COMS","COML","BUSO" ;
  schema:sameAs    <http://ddwiki.reso.org/display/DDW/Latitude+Field> ;
  vs:term_status   "stable"
.
reso:LaundryFeatures a rdf:Property ;
  rdfs:comment     "Add this pick list of features and locations where the laundry is located in the property being sold.  i.e. Gas Dryer Hookup, In Kitchen, In Garage, etc.  CRMLS sees over 50% utilization of this field which has a dozen enumerations making it too long to fold into other fields such as rooms or Interior Features." ;
  rdfs:domain      reso:Property ;
  rdfs:label       "LaundryFeatures" ;
  rdfs:range       xsd:string ;
  reso:CertificationLevel "Platinum" ;
  reso:PropertyTypes "RESI","RLSE","RINC","MOBI","FARM","COMS","COML" ;
  schema:sameAs    <http://ddwiki.reso.org/display/DDW/LaundryFeatures+Field> ;
  vs:term_status   "stable"
.
reso:LeasableArea a rdf:Property ;
  rdfs:comment     "The area that may be leased within the commercial property." ;
  rdfs:domain      reso:Property ;
  rdfs:label       "LeasableArea" ;
  rdfs:range       xsd:decimal ;
  reso:CertificationLevel "Silver" ;
  reso:PropertyTypes "COMS","COML" ;
  schema:sameAs    <http://ddwiki.reso.org/display/DDW/LeasableArea+Field> ;
  vs:term_status   "stable"
.
reso:LeasableAreaUnits a rdf:Property ;
  rdfs:comment     "A pick list of the unit of measurement for the area.  i.e. Square Feet, Square Meters, Acres, etc." ;
  rdfs:domain      reso:Property ;
  rdfs:label       "LeasableAreaUnits" ;
  rdfs:range       enum:AreaUnits ;
  reso:CertificationLevel "Silver" ;
  reso:PropertyTypes "COMS","COML" ;
  schema:sameAs    <http://ddwiki.reso.org/display/DDW/LeasableAreaUnits+Field> ;
  vs:term_status   "stable"
.
reso:LeaseAmount a rdf:Property ;
  rdfs:comment     "The amount of any lease the business pays for it's current location." ;
  rdfs:domain      reso:Property ;
  rdfs:label       "LeaseAmount" ;
  rdfs:range       xsd:decimal ;
  reso:CertificationLevel "Bronze" ;
  reso:PropertyTypes "BUSO" ;
  schema:sameAs    <http://ddwiki.reso.org/display/DDW/LeaseAmount+Field> ;
  vs:term_status   "stable"
.
reso:LeaseAmountFrequency a rdf:Property ;
  rdfs:comment     "The frequency of the LeaseAmount is paid.  Monthly, weekly, annual, etc." ;
  rdfs:domain      reso:Property ;
  rdfs:label       "LeaseAmountFrequency" ;
  rdfs:range       enum:FeeFrequency ;
  reso:CertificationLevel "Bronze" ;
  reso:PropertyTypes "BUSO" ;
  schema:sameAs    <http://ddwiki.reso.org/display/DDW/LeaseAmountFrequency+Field> ;
  vs:term_status   "stable"
.
reso:LeaseAssignableYN a rdf:Property ;
  rdfs:comment     "Can the lease at the business' current location be assigned to another party." ;
  rdfs:domain      reso:Property ;
  rdfs:label       "LeaseAssignableYN" ;
  rdfs:range       xsd:boolean ;
  reso:CertificationLevel "Bronze" ;
  reso:PropertyTypes "BUSO" ;
  schema:sameAs    <http://ddwiki.reso.org/display/DDW/LeaseAssignableYN+Field> ;
  vs:term_status   "stable"
.
reso:LeaseConsideredYN a rdf:Property ;
  rdfs:comment     "Will the seller consider leasing the property instead of selling?  Single select." ;
  rdfs:domain      reso:Property ;
  rdfs:label       "LeaseConsideredYN" ;
  rdfs:range       xsd:boolean ;
  reso:CertificationLevel "Bronze" ;
  reso:PropertyTypes "RESI","RLSE","RINC","LAND","MOBI","FARM","COMS","COML" ;
  schema:sameAs    <http://ddwiki.reso.org/display/DDW/LeaseConsideredYN+Field> ;
  vs:term_status   "stable"
.
reso:LeaseExpiration a rdf:Property ;
  rdfs:comment     "The expiration date of the lease for the business' current location." ;
  rdfs:domain      reso:Property ;
  rdfs:label       "LeaseExpiration" ;
  rdfs:range       xsd:date ;
  reso:CertificationLevel "Bronze" ;
  reso:PropertyTypes "BUSO" ;
  schema:sameAs    <http://ddwiki.reso.org/display/DDW/LeaseExpiration+Field> ;
  vs:term_status   "stable"
.
reso:LeaseRenewalCompensation a rdf:Property ;
  rdfs:comment     "A list of compensations other than the original Selling Office Compensation.  i.e. Compensation Paid on Renewal, Compensation Paid on Tennant Purchase, No Renewal Commission, Call Listing Office, etc." ;
  rdfs:domain      reso:Property ;
  rdfs:label       "LeaseRenewalCompensation" ;
  rdfs:range       enum:LeaseRenewalCompensation ;
  reso:CertificationLevel "Bronze" ;
  reso:PropertyTypes "RLSE" ;
  schema:sameAs    <http://ddwiki.reso.org/display/DDW/LeaseRenewalCompensation+Field> ;
  vs:term_status   "stable"
.
reso:LeaseRenewalOptionYN a rdf:Property ;
  rdfs:comment     "Is there an option to renew the lease at the business' current location." ;
  rdfs:domain      reso:Property ;
  rdfs:label       "LeaseRenewalOptionYN" ;
  rdfs:range       xsd:boolean ;
  reso:CertificationLevel "Bronze" ;
  reso:PropertyTypes "BUSO" ;
  schema:sameAs    <http://ddwiki.reso.org/display/DDW/LeaseRenewalOptionYN+Field> ;
  vs:term_status   "stable"
.
reso:LeaseTerm a rdf:Property ;
  rdfs:comment     "A pick list of lengths that represent the length of the lease.  i.e. Weekly, Month to Month, 6 Month Lease, 12 Month Lease, 24 Month Lease." ;
  rdfs:domain      reso:Property ;
  rdfs:label       "LeaseTerm" ;
  rdfs:range       enum:LeaseTerm ;
  reso:CertificationLevel "Core" ;
  reso:PropertyTypes "RLSE" ;
  schema:sameAs    <http://ddwiki.reso.org/display/DDW/LeaseTerm+Field> ;
  vs:term_status   "stable"
.
reso:Levels a rdf:Property ;
  rdfs:comment     "The number of levels in the property being sold.  For example, One Level, Two Levels, Split Level, Three or More Levels, Multi Level, Loft.    A discreet horizontal plane of interior living space (excluding basements)." ;
  rdfs:domain      reso:Property ;
  rdfs:label       "Levels" ;
  rdfs:range       enum:Levels ;
  reso:CertificationLevel "Core" ;
  reso:PropertyTypes "RESI","RLSE","RINC","MOBI","FARM" ;
  schema:sameAs    <http://ddwiki.reso.org/display/DDW/Levels+Field> ;
  vs:term_status   "stable"
.
reso:License1 a rdf:Property ;
  rdfs:comment     "License number of the mobile or manufactured home.  Also known as the Department of Housing label/insignia number. For the first or only unit/section use License 1 over License 2 or 3." ;
  rdfs:domain      reso:Property ;
  rdfs:label       "License1" ;
  rdfs:range       xsd:string ;
  reso:CertificationLevel "Silver" ;
  reso:PropertyTypes "RESI","RLSE","MOBI" ;
  schema:sameAs    <http://ddwiki.reso.org/display/DDW/License1+Field> ;
  vs:term_status   "stable"
.
reso:License2 a rdf:Property ;
  rdfs:comment     "License number of the mobile or manufactured home.  Also known as the Department of Housing label/insignia number. For two units/sections use License 1 and 2 over License 3." ;
  rdfs:domain      reso:Property ;
  rdfs:label       "License2" ;
  rdfs:range       xsd:string ;
  reso:CertificationLevel "Silver" ;
  reso:PropertyTypes "RESI","RLSE","MOBI" ;
  schema:sameAs    <http://ddwiki.reso.org/display/DDW/License2+Field> ;
  vs:term_status   "stable"
.
reso:License3 a rdf:Property ;
  rdfs:comment     "License number of the mobile or manufactured home.  Also known as the Department of Housing label/insignia number. For two units/sections use License 1 and 2 over License 3." ;
  rdfs:domain      reso:Property ;
  rdfs:label       "License3" ;
  rdfs:range       xsd:string ;
  reso:CertificationLevel "Silver" ;
  reso:PropertyTypes "RESI","RLSE","MOBI" ;
  schema:sameAs    <http://ddwiki.reso.org/display/DDW/License3+Field> ;
  vs:term_status   "stable"
.
reso:LicensesExpense a rdf:Property ;
  rdfs:comment     "The annual expense that is not paid directly by the tenant and is included in the Operating Expense calculations." ;
  rdfs:domain      reso:Property ;
  rdfs:label       "LicensesExpense" ;
  rdfs:range       xsd:decimal ;
  reso:CertificationLevel "Silver" ;
  reso:PropertyTypes "RINC" ;
  schema:sameAs    <http://ddwiki.reso.org/display/DDW/LicensesExpense+Field> ;
  vs:term_status   "stable"
.
reso:ListAOR a rdf:Property ;
  rdfs:comment     "The responsible Board or Association of REALTORS for this listing." ;
  rdfs:domain      reso:Property ;
  rdfs:label       "ListAOR" ;
  rdfs:range       xsd:string ;
  reso:CertificationLevel "Bronze" ;
  reso:PropertyTypes "RESI","RLSE","RINC","LAND","MOBI","FARM","COMS","COML","BUSO" ;
  schema:sameAs    <http://ddwiki.reso.org/display/DDW/ListAOR+Field> ;
  vs:term_status   "stable"
.
reso:ListAgentAOR a rdf:Property ;
  rdfs:comment     "The Listing Agent's Board or Association of REALTORS." ;
  rdfs:domain      reso:Property ;
  rdfs:label       "ListAgentAOR" ;
  rdfs:range       xsd:string ;
  reso:CertificationLevel "Bronze" ;
  reso:PropertyTypes "RESI","RLSE","RINC","LAND","MOBI","FARM","COMS","COML","BUSO" ;
  schema:sameAs    <http://ddwiki.reso.org/display/DDW/ListAgentAOR+Field> ;
  vs:term_status   "stable"
.
reso:ListAgentCellPhone a rdf:Property ;
  rdfs:comment     "North American 10 digit phone numbers should be in the format of ###-###-#### (separated by hyphens).  Other conventions should use the common local standard.  International numbers should be preceded by a plus symbol." ;
  rdfs:domain      reso:Property ;
  rdfs:label       "ListAgentCellPhone" ;
  rdfs:range       xsd:string ;
  reso:CertificationLevel "Core" ;
  reso:PropertyTypes "RESI","RLSE","RINC","LAND","MOBI","FARM","COMS","COML","BUSO" ;
  schema:sameAs    <http://ddwiki.reso.org/display/DDW/ListAgentCellPhone+Field> ;
  vs:term_status   "stable"
.
reso:ListAgentDesignation a rdf:Property ;
  rdfs:comment     "Designations and certifications acknowledging experience and expertise in various real estate sectors are awarded by NAR and each affiliated group upon completion of required courses." ;
  rdfs:domain      reso:Property ;
  rdfs:label       "ListAgentDesignation" ;
  rdfs:range       xsd:string ;
  reso:CertificationLevel "Bronze" ;
  reso:PropertyTypes "RESI","RLSE","RINC","LAND","MOBI","FARM","COMS","COML","BUSO" ;
  schema:sameAs    <http://ddwiki.reso.org/display/DDW/ListAgentDesignation+Field> ;
  vs:term_status   "stable"
.
reso:ListAgentDirectPhone a rdf:Property ;
  rdfs:comment     "North American 10 digit phone numbers should be in the format of ###-###-#### (separated by hyphens).  Other conventions should use the common local standard.  International numbers should be preceded by a plus symbol." ;
  rdfs:domain      reso:Property ;
  rdfs:label       "ListAgentDirectPhone" ;
  rdfs:range       xsd:string ;
  reso:CertificationLevel "Bronze" ;
  reso:PropertyTypes "RESI","RLSE","RINC","LAND","MOBI","FARM","COMS","COML","BUSO" ;
  schema:sameAs    <http://ddwiki.reso.org/display/DDW/ListAgentDirectPhone+Field> ;
  vs:term_status   "stable"
.
reso:ListAgentEmail a rdf:Property ;
  rdfs:comment     "The email address of the Listing Agent." ;
  rdfs:domain      reso:Property ;
  rdfs:label       "ListAgentEmail" ;
  rdfs:range       xsd:string ;
  reso:CertificationLevel "Core" ;
  reso:PropertyTypes "RESI","RLSE","RINC","LAND","MOBI","FARM","COMS","COML","BUSO" ;
  schema:sameAs    <http://ddwiki.reso.org/display/DDW/ListAgentEmail+Field> ;
  vs:term_status   "stable"
.
reso:ListAgentFax a rdf:Property ;
  rdfs:comment     "North American 10 digit phone numbers should be in the format of ###-###-#### (separated by hyphens).  Other conventions should use the common local standard.  International numbers should be preceded by a plus symbol." ;
  rdfs:domain      reso:Property ;
  rdfs:label       "ListAgentFax" ;
  rdfs:range       xsd:string ;
  reso:CertificationLevel "Bronze" ;
  reso:PropertyTypes "RESI","RLSE","RINC","LAND","MOBI","FARM","COMS","COML","BUSO" ;
  schema:sameAs    <http://ddwiki.reso.org/display/DDW/ListAgentFax+Field> ;
  vs:term_status   "stable"
.
reso:ListAgentFirstName a rdf:Property ;
  rdfs:comment     "The first name of the listing agent." ;
  rdfs:domain      reso:Property ;
  rdfs:label       "ListAgentFirstName" ;
  rdfs:range       xsd:string ;
  reso:CertificationLevel "Core" ;
  reso:PropertyTypes "RESI","RLSE","RINC","LAND","MOBI","FARM","COMS","COML","BUSO" ;
  schema:sameAs    <http://ddwiki.reso.org/display/DDW/ListAgentFirstName+Field> ;
  vs:term_status   "stable"
.
reso:ListAgentFullName a rdf:Property ;
  rdfs:comment     "The full name of the listing agent. (First Middle Last)" ;
  rdfs:domain      reso:Property ;
  rdfs:label       "ListAgentFullName" ;
  rdfs:range       xsd:string ;
  reso:CertificationLevel "Bronze" ;
  reso:PropertyTypes "RESI","RLSE","RINC","LAND","MOBI","FARM","COMS","COML","BUSO" ;
  schema:sameAs    <http://ddwiki.reso.org/display/DDW/ListAgentFullName+Field> ;
  vs:term_status   "stable"
.
reso:ListAgentHomePhone a rdf:Property ;
  rdfs:comment     "North American 10 digit phone numbers should be in the format of ###-###-#### (separated by hyphens).  Other conventions should use the common local standard.  International numbers should be preceded by a plus symbol." ;
  rdfs:domain      reso:Property ;
  rdfs:label       "ListAgentHomePhone" ;
  rdfs:range       xsd:string ;
  reso:CertificationLevel "Bronze" ;
  reso:PropertyTypes "RESI","RLSE","RINC","LAND","MOBI","FARM","COMS","COML","BUSO" ;
  schema:sameAs    <http://ddwiki.reso.org/display/DDW/ListAgentHomePhone+Field> ;
  vs:term_status   "stable"
.
reso:ListAgentKey a rdf:Property ;
  rdfs:comment     "A system unique identifier. Specifically, in aggregation systems, the ListAgentKey is the system unique identifier from the system that the record was retrieved. This may be identical to the related xxxId. This is a foreign key relating to the Member resource's MemberKey." ;
  rdfs:domain      reso:Property ;
  rdfs:label       "ListAgentKey" ;
  rdfs:range       xsd:string ;
  reso:CertificationLevel "Core" ;
  reso:PropertyTypes "RESI","RLSE","RINC","LAND","MOBI","FARM","COMS","COML","BUSO" ;
  schema:sameAs    <http://ddwiki.reso.org/display/DDW/ListAgentKey+Field> ;
  vs:term_status   "stable"
.
reso:ListAgentKeyNumeric a rdf:Property ;
  rdfs:comment     "A system unique identifier. Specifically, in aggregation systems, the ListAgentKey is the system unique identifier from the system that the record was retrieved. This may be identical to the related xxxId. This is a foreign key relating to the Member resource's MemberKey. This is the numeric only key and used as an alternative to the ListAgentKey field." ;
  rdfs:domain      reso:Property ;
  rdfs:label       "ListAgentKeyNumeric" ;
  rdfs:range       xsd:decimal ;
  reso:CertificationLevel "Platinum" ;
  reso:PropertyTypes "RESI","RLSE","RINC","LAND","MOBI","FARM","COMS","COML","BUSO" ;
  schema:sameAs    <http://ddwiki.reso.org/display/DDW/ListAgentKeyNumeric+Field> ;
  vs:term_status   "stable"
.
reso:ListAgentLastName a rdf:Property ;
  rdfs:comment     "The last name of the listing agent." ;
  rdfs:domain      reso:Property ;
  rdfs:label       "ListAgentLastName" ;
  rdfs:range       xsd:string ;
  reso:CertificationLevel "Core" ;
  reso:PropertyTypes "RESI","RLSE","RINC","LAND","MOBI","FARM","COMS","COML","BUSO" ;
  schema:sameAs    <http://ddwiki.reso.org/display/DDW/ListAgentLastName+Field> ;
  vs:term_status   "stable"
.
reso:ListAgentMiddleName a rdf:Property ;
  rdfs:comment     "The middle name of the listing agent." ;
  rdfs:domain      reso:Property ;
  rdfs:label       "ListAgentMiddleName" ;
  rdfs:range       xsd:string ;
  reso:CertificationLevel "Core" ;
  reso:PropertyTypes "RESI","RLSE","RINC","LAND","MOBI","FARM","COMS","COML","BUSO" ;
  schema:sameAs    <http://ddwiki.reso.org/display/DDW/ListAgentMiddleName+Field> ;
  vs:term_status   "stable"
.
reso:ListAgentMlsId a rdf:Property ;
  rdfs:comment     "The local, well-known identifier for the member. This value may not be unique, specifically in the case of aggregation systems, this value should be the identifier from the original system." ;
  rdfs:domain      reso:Property ;
  rdfs:label       "ListAgentMlsId" ;
  rdfs:range       xsd:string ;
  reso:CertificationLevel "Core" ;
  reso:PropertyTypes "RESI","RLSE","RINC","LAND","MOBI","FARM","COMS","COML","BUSO" ;
  schema:sameAs    <http://ddwiki.reso.org/display/DDW/ListAgentMlsId+Field> ;
  vs:term_status   "stable"
.
reso:ListAgentNamePrefix a rdf:Property ;
  rdfs:comment     "Prefix to the name (e.g. Dr. Mr. Ms. etc.)" ;
  rdfs:domain      reso:Property ;
  rdfs:label       "ListAgentNamePrefix" ;
  rdfs:range       xsd:string ;
  reso:CertificationLevel "Bronze" ;
  reso:PropertyTypes "RESI","RLSE","RINC","LAND","MOBI","FARM","COMS","COML","BUSO" ;
  schema:sameAs    <http://ddwiki.reso.org/display/DDW/ListAgentNamePrefix+Field> ;
  vs:term_status   "stable"
.
reso:ListAgentNameSuffix a rdf:Property ;
  rdfs:comment     "Suffix to the ListAgentLastName (e.g. Esq.,  Jr.,  III etc.)" ;
  rdfs:domain      reso:Property ;
  rdfs:label       "ListAgentNameSuffix" ;
  rdfs:range       xsd:string ;
  reso:CertificationLevel "Bronze" ;
  reso:PropertyTypes "RESI","RLSE","RINC","LAND","MOBI","FARM","COMS","COML","BUSO" ;
  schema:sameAs    <http://ddwiki.reso.org/display/DDW/ListAgentNameSuffix+Field> ;
  vs:term_status   "stable"
.
reso:ListAgentOfficePhone a rdf:Property ;
  rdfs:comment     "North American 10 digit phone numbers should be in the format of ###-###-#### (separated by hyphens).  Other conventions should use the common local standard.  International numbers should be preceded by a plus symbol." ;
  rdfs:domain      reso:Property ;
  rdfs:label       "ListAgentOfficePhone" ;
  rdfs:range       xsd:string ;
  reso:CertificationLevel "Core" ;
  reso:PropertyTypes "RESI","RLSE","RINC","LAND","MOBI","FARM","COMS","COML","BUSO" ;
  schema:sameAs    <http://ddwiki.reso.org/display/DDW/ListAgentOfficePhone+Field> ;
  vs:term_status   "stable"
.
reso:ListAgentOfficePhoneExt a rdf:Property ;
  rdfs:comment     "The extension of the given phone number (if applicable)." ;
  rdfs:domain      reso:Property ;
  rdfs:label       "ListAgentOfficePhoneExt" ;
  rdfs:range       xsd:string ;
  reso:CertificationLevel "Core" ;
  reso:PropertyTypes "RESI","RLSE","RINC","LAND","MOBI","FARM","COMS","COML","BUSO" ;
  schema:sameAs    <http://ddwiki.reso.org/display/DDW/ListAgentOfficePhoneExt+Field> ;
  vs:term_status   "stable"
.
reso:ListAgentPager a rdf:Property ;
  rdfs:comment     "North American 10 digit phone numbers should be in the format of ###-###-#### (separated by hyphens).  Other conventions should use the common local standard.  International numbers should be preceded by a plus symbol." ;
  rdfs:domain      reso:Property ;
  rdfs:label       "ListAgentPager" ;
  rdfs:range       xsd:string ;
  reso:CertificationLevel "Bronze" ;
  reso:PropertyTypes "RESI","RLSE","RINC","LAND","MOBI","FARM","COMS","COML","BUSO" ;
  schema:sameAs    <http://ddwiki.reso.org/display/DDW/ListAgentPager+Field> ;
  vs:term_status   "stable"
.
reso:ListAgentPreferredPhone a rdf:Property ;
  rdfs:comment     "North American 10 digit phone numbers should be in the format of ###-###-#### (separated by hyphens).  Other conventions should use the common local standard.  International numbers should be preceded by a plus symbol." ;
  rdfs:domain      reso:Property ;
  rdfs:label       "ListAgentPreferredPhone" ;
  rdfs:range       xsd:string ;
  reso:CertificationLevel "Core" ;
  reso:PropertyTypes "RESI","RLSE","RINC","LAND","MOBI","FARM","COMS","COML","BUSO" ;
  schema:sameAs    <http://ddwiki.reso.org/display/DDW/ListAgentPreferredPhone+Field> ;
  vs:term_status   "stable"
.
reso:ListAgentPreferredPhoneExt a rdf:Property ;
  rdfs:comment     "The extension of the given phone number (if applicable)." ;
  rdfs:domain      reso:Property ;
  rdfs:label       "ListAgentPreferredPhoneExt" ;
  rdfs:range       xsd:string ;
  reso:CertificationLevel "Core" ;
  reso:PropertyTypes "RESI","RLSE","RINC","LAND","MOBI","FARM","COMS","COML","BUSO" ;
  schema:sameAs    <http://ddwiki.reso.org/display/DDW/ListAgentPreferredPhoneExt+Field> ;
  vs:term_status   "stable"
.
reso:ListAgentStateLicense a rdf:Property ;
  rdfs:comment     "The license of the listing agent. Separate multiple licenses with a comma and space." ;
  rdfs:domain      reso:Property ;
  rdfs:label       "ListAgentStateLicense" ;
  rdfs:range       xsd:string ;
  reso:CertificationLevel "Core" ;
  reso:PropertyTypes "RESI","RLSE","RINC","LAND","MOBI","FARM","COMS","COML","BUSO" ;
  schema:sameAs    <http://ddwiki.reso.org/display/DDW/ListAgentStateLicense+Field> ;
  vs:term_status   "stable"
.
reso:ListAgentTollFreePhone a rdf:Property ;
  rdfs:comment     "North American 10 digit phone numbers should be in the format of ###-###-#### (separated by hyphens).  Other conventions should use the common local standard.  International numbers should be preceded by a plus symbol." ;
  rdfs:domain      reso:Property ;
  rdfs:label       "ListAgentTollFreePhone" ;
  rdfs:range       xsd:string ;
  reso:CertificationLevel "Bronze" ;
  reso:PropertyTypes "RESI","RLSE","RINC","LAND","MOBI","FARM","COMS","COML","BUSO" ;
  schema:sameAs    <http://ddwiki.reso.org/display/DDW/ListAgentTollFreePhone+Field> ;
  vs:term_status   "stable"
.
reso:ListAgentURL a rdf:Property ;
  rdfs:comment     "The website URI of the listing agent." ;
  rdfs:domain      reso:Property ;
  rdfs:label       "ListAgentURL" ;
  rdfs:range       xsd:string ;
  reso:CertificationLevel "Bronze" ;
  reso:PropertyTypes "RESI","RLSE","RINC","LAND","MOBI","FARM","COMS","COML","BUSO" ;
  schema:sameAs    <http://ddwiki.reso.org/display/DDW/ListAgentURL+Field> ;
  vs:term_status   "stable"
.
reso:ListAgentVoiceMail a rdf:Property ;
  rdfs:comment     "North American 10 digit phone numbers should be in the format of ###-###-#### (separated by hyphens).  Other conventions should use the common local standard.  International numbers should be preceded by a plus symbol." ;
  rdfs:domain      reso:Property ;
  rdfs:label       "ListAgentVoiceMail" ;
  rdfs:range       xsd:string ;
  reso:CertificationLevel "Bronze" ;
  reso:PropertyTypes "RESI","RLSE","RINC","LAND","MOBI","FARM","COMS","COML","BUSO" ;
  schema:sameAs    <http://ddwiki.reso.org/display/DDW/ListAgentVoiceMail+Field> ;
  vs:term_status   "stable"
.
reso:ListAgentVoiceMailExt a rdf:Property ;
  rdfs:comment     "The extension of the given phone number (if applicable)." ;
  rdfs:domain      reso:Property ;
  rdfs:label       "ListAgentVoiceMailExt" ;
  rdfs:range       xsd:string ;
  reso:CertificationLevel "Bronze" ;
  reso:PropertyTypes "RESI","RLSE","RINC","LAND","MOBI","FARM","COMS","COML","BUSO" ;
  schema:sameAs    <http://ddwiki.reso.org/display/DDW/ListAgentVoiceMailExt+Field> ;
  vs:term_status   "stable"
.
reso:ListOfficeAOR a rdf:Property ;
  rdfs:comment     "The Listing Office's Board or Association of REALTORS." ;
  rdfs:domain      reso:Property ;
  rdfs:label       "ListOfficeAOR" ;
  rdfs:range       xsd:string ;
  reso:CertificationLevel "Bronze" ;
  reso:PropertyTypes "RESI","RLSE","RINC","LAND","MOBI","FARM","COMS","COML","BUSO" ;
  schema:sameAs    <http://ddwiki.reso.org/display/DDW/ListOfficeAOR+Field> ;
  vs:term_status   "stable"
.
reso:ListOfficeEmail a rdf:Property ;
  rdfs:comment     "The email address of the Listing Office." ;
  rdfs:domain      reso:Property ;
  rdfs:label       "ListOfficeEmail" ;
  rdfs:range       xsd:string ;
  reso:CertificationLevel "Bronze" ;
  reso:PropertyTypes "RESI","RLSE","RINC","LAND","MOBI","FARM","COMS","COML","BUSO" ;
  schema:sameAs    <http://ddwiki.reso.org/display/DDW/ListOfficeEmail+Field> ;
  vs:term_status   "stable"
.
reso:ListOfficeFax a rdf:Property ;
  rdfs:comment     "North American 10 digit phone numbers should be in the format of ###-###-#### (separated by hyphens).  Other conventions should use the common local standard.  International numbers should be preceded by a plus symbol." ;
  rdfs:domain      reso:Property ;
  rdfs:label       "ListOfficeFax" ;
  rdfs:range       xsd:string ;
  reso:CertificationLevel "Bronze" ;
  reso:PropertyTypes "RESI","RLSE","RINC","LAND","MOBI","FARM","COMS","COML","BUSO" ;
  schema:sameAs    <http://ddwiki.reso.org/display/DDW/ListOfficeFax+Field> ;
  vs:term_status   "stable"
.
reso:ListOfficeKey a rdf:Property ;
  rdfs:comment     "A system unique identifier. Specifically, in aggregation systems, the Key is the system unique identifier from the system that the record was just retrieved. This may be identical to the related xxxId identifier, but the key is guaranteed unique for this record set.  This is a foreign key relating to the Office resource's OfficeKey." ;
  rdfs:domain      reso:Property ;
  rdfs:label       "ListOfficeKey" ;
  rdfs:range       xsd:string ;
  reso:CertificationLevel "Core" ;
  reso:PropertyTypes "RESI","RLSE","RINC","LAND","MOBI","FARM","COMS","COML","BUSO" ;
  schema:sameAs    <http://ddwiki.reso.org/display/DDW/ListOfficeKey+Field> ;
  vs:term_status   "stable"
.
reso:ListOfficeKeyNumeric a rdf:Property ;
  rdfs:comment     "A system unique identifier. Specifically, in aggregation systems, the Key is the system unique identifier from the system that the record was just retrieved. This may be identical to the related xxxId identifier, but the key is guaranteed unique for this record set.  This is a foreign key relating to the Office resource's OfficeKey.  This is the numeric only key and used as an alternative to the ListOfficeKey field." ;
  rdfs:domain      reso:Property ;
  rdfs:label       "ListOfficeKeyNumeric" ;
  rdfs:range       xsd:decimal ;
  reso:CertificationLevel "Platinum" ;
  reso:PropertyTypes "RESI","RLSE","RINC","LAND","MOBI","FARM","COMS","COML","BUSO" ;
  schema:sameAs    <http://ddwiki.reso.org/display/DDW/ListOfficeKeyNumeric+Field> ;
  vs:term_status   "stable"
.
reso:ListOfficeMlsId a rdf:Property ;
  rdfs:comment     "The local, well-known identifier. This value may not be unique, specifically in the case of aggregation systems, this value should be the identifier from the original system." ;
  rdfs:domain      reso:Property ;
  rdfs:label       "ListOfficeMlsId" ;
  rdfs:range       xsd:string ;
  reso:CertificationLevel "Core" ;
  reso:PropertyTypes "RESI","RLSE","RINC","LAND","MOBI","FARM","COMS","COML","BUSO" ;
  schema:sameAs    <http://ddwiki.reso.org/display/DDW/ListOfficeMlsId+Field> ;
  vs:term_status   "stable"
.
reso:ListOfficeName a rdf:Property ;
  rdfs:comment     "The legal name of the brokerage representing the seller." ;
  rdfs:domain      reso:Property ;
  rdfs:label       "ListOfficeName" ;
  rdfs:range       xsd:string ;
  reso:CertificationLevel "Core" ;
  reso:PropertyTypes "RESI","RLSE","RINC","LAND","MOBI","FARM","COMS","COML","BUSO" ;
  schema:sameAs    <http://ddwiki.reso.org/display/DDW/ListOfficeName+Field> ;
  vs:term_status   "stable"
.
reso:ListOfficePhone a rdf:Property ;
  rdfs:comment     "North American 10 digit phone numbers should be in the format of ###-###-#### (separated by hyphens).  Other conventions should use the common local standard.  International numbers should be preceded by a plus symbol." ;
  rdfs:domain      reso:Property ;
  rdfs:label       "ListOfficePhone" ;
  rdfs:range       xsd:string ;
  reso:CertificationLevel "Core" ;
  reso:PropertyTypes "RESI","RLSE","RINC","LAND","MOBI","FARM","COMS","COML","BUSO" ;
  schema:sameAs    <http://ddwiki.reso.org/display/DDW/ListOfficePhone+Field> ;
  vs:term_status   "stable"
.
reso:ListOfficePhoneExt a rdf:Property ;
  rdfs:comment     "The extension of the given phone number (if applicable)." ;
  rdfs:domain      reso:Property ;
  rdfs:label       "ListOfficePhoneExt" ;
  rdfs:range       xsd:string ;
  reso:CertificationLevel "Core" ;
  reso:PropertyTypes "RESI","RLSE","RINC","LAND","MOBI","FARM","COMS","COML","BUSO" ;
  schema:sameAs    <http://ddwiki.reso.org/display/DDW/ListOfficePhoneExt+Field> ;
  vs:term_status   "stable"
.
reso:ListOfficeURL a rdf:Property ;
  rdfs:comment     "The website URI for the listing office." ;
  rdfs:domain      reso:Property ;
  rdfs:label       "ListOfficeURL" ;
  rdfs:range       xsd:string ;
  reso:CertificationLevel "Bronze" ;
  reso:PropertyTypes "RESI","RLSE","RINC","LAND","MOBI","FARM","COMS","COML","BUSO" ;
  schema:sameAs    <http://ddwiki.reso.org/display/DDW/ListOfficeURL+Field> ;
  vs:term_status   "stable"
.
reso:ListPrice a rdf:Property ;
  rdfs:comment     "The current price of the property as determined by the seller and the seller's broker.  For auctions this is the minimum or reserve price." ;
  rdfs:domain      reso:Property ;
  rdfs:label       "ListPrice" ;
  rdfs:range       xsd:decimal ;
  reso:CertificationLevel "Core" ;
  reso:PropertyTypes "RESI","RLSE","RINC","LAND","MOBI","FARM","COMS","COML","BUSO" ;
  schema:sameAs    <http://ddwiki.reso.org/display/DDW/ListPrice+Field> ;
  vs:term_status   "stable"
.
reso:ListPriceLow a rdf:Property ;
  rdfs:comment     "The lower price used for Value Range Pricing.  The List Price must be greater than or equal to the ListPriceLow." ;
  rdfs:domain      reso:Property ;
  rdfs:label       "ListPriceLow" ;
  rdfs:range       xsd:decimal ;
  reso:CertificationLevel "Bronze" ;
  reso:PropertyTypes "RESI","RLSE","RINC","LAND","MOBI","FARM","COMS","COML","BUSO" ;
  schema:sameAs    <http://ddwiki.reso.org/display/DDW/ListPriceLow+Field> ;
  vs:term_status   "stable"
.
reso:ListTeamKey a rdf:Property ;
  rdfs:comment     "A system unique identifier. Specifically, in aggregation systems, the Key is the system unique identifier from the system that the record was just retrieved. This may be identical to the related xxxId identifier, but the key is guaranteed unique for this record set.  This is a foreign key relating to the Teams resource's TeamKey." ;
  rdfs:domain      reso:Property ;
  rdfs:label       "ListTeamKey" ;
  rdfs:range       xsd:string ;
  reso:CertificationLevel "Silver" ;
  reso:PropertyTypes "RESI","RLSE","RINC","LAND","MOBI","FARM","COMS","COML","BUSO" ;
  schema:sameAs    <http://ddwiki.reso.org/display/DDW/ListTeamKey+Field> ;
  vs:term_status   "stable"
.
reso:ListTeamKeyNumeric a rdf:Property ;
  rdfs:comment     "A system unique identifier. Specifically, in aggregation systems, the Key is the system unique identifier from the system that the record was just retrieved. This may be identical to the related xxxId identifier, but the key is guaranteed unique for this record set.  This is a foreign key relating to the Teams resource's TeamKey.  This is the numeric only key and used as an alternative to the ListTeamKey field." ;
  rdfs:domain      reso:Property ;
  rdfs:label       "ListTeamKeyNumeric" ;
  rdfs:range       xsd:decimal ;
  reso:CertificationLevel "Platinum" ;
  reso:PropertyTypes "RESI","RLSE","RINC","LAND","MOBI","FARM","COMS","COML","BUSO" ;
  schema:sameAs    <http://ddwiki.reso.org/display/DDW/ListTeamKeyNumeric+Field> ;
  vs:term_status   "stable"
.
reso:ListTeamName a rdf:Property ;
  rdfs:comment     "The name of the team representing the seller." ;
  rdfs:domain      reso:Property ;
  rdfs:label       "ListTeamName" ;
  rdfs:range       xsd:string ;
  reso:CertificationLevel "Silver" ;
  reso:PropertyTypes "RESI","RLSE","RINC","LAND","MOBI","FARM","COMS","COML","BUSO" ;
  schema:sameAs    <http://ddwiki.reso.org/display/DDW/ListTeamName+Field> ;
  vs:term_status   "stable"
.
reso:ListingAgreement a rdf:Property ;
  rdfs:comment     "The nature of the agreement between the seller and the listing agent.  Examples are Exclusive Agency, Open Listing, etc." ;
  rdfs:domain      reso:Property ;
  rdfs:label       "ListingAgreement" ;
  rdfs:range       enum:ListingAgreement ;
  reso:CertificationLevel "Core" ;
  reso:PropertyTypes "RESI","RLSE","RINC","LAND","MOBI","FARM","COMS","COML","BUSO" ;
  schema:sameAs    <http://ddwiki.reso.org/display/DDW/ListingAgreement+Field> ;
  vs:term_status   "stable"
.
reso:ListingContractDate a rdf:Property ;
  rdfs:comment     "The effective date of the agreement between the seller and the seller's broker. This is the date entered by the agent reflecting when the change occurred contractually, not a timestamp of when the change was made in the MLS." ;
  rdfs:domain      reso:Property ;
  rdfs:label       "ListingContractDate" ;
  rdfs:range       xsd:date ;
  reso:CertificationLevel "Core" ;
  reso:PropertyTypes "RESI","RLSE","RINC","LAND","MOBI","FARM","COMS","COML","BUSO" ;
  schema:sameAs    <http://ddwiki.reso.org/display/DDW/ListingContractDate+Field> ;
  vs:term_status   "stable"
.
reso:ListingId a rdf:Property ;
  rdfs:comment     "The well known identifier for the listing. The value may be identical to that of the Listing Key, but the Listing ID is intended to be the value used by a human to retrieve the information about a specific listing. In a multiple originating system or a merged system, this value may not be unique and may require the use of the provider system to create a synthetic unique value." ;
  rdfs:domain      reso:Property ;
  rdfs:label       "ListingId" ;
  rdfs:range       xsd:string ;
  reso:CertificationLevel "Core" ;
  reso:PropertyTypes "RESI","RLSE","RINC","LAND","MOBI","FARM","COMS","COML","BUSO" ;
  schema:sameAs    <http://ddwiki.reso.org/display/DDW/ListingId+Field> ;
  vs:term_status   "stable"
.
reso:ListingKey a rdf:Property ;
  rdfs:comment     "A unique identifier for this record from the immediate source. This is a string that can include URI or other forms.  Alternatively use the ListingKeyNumeric for a numeric only key field.  This is the local key of the system.  When records are received from other systems, a local key is commonly applied.  If conveying the original keys from the source or originating systems, see SourceSystemKey and OriginatingSystemKey." ;
  rdfs:domain      reso:Property ;
  rdfs:label       "ListingKey" ;
  rdfs:range       xsd:string ;
  reso:CertificationLevel "Core" ;
  reso:PropertyTypes "RESI","RLSE","RINC","LAND","MOBI","FARM","COMS","COML","BUSO" ;
  schema:sameAs    <http://ddwiki.reso.org/display/DDW/ListingKey+Field> ;
  vs:term_status   "stable"
.
reso:ListingKeyNumeric a rdf:Property ;
  rdfs:comment     "A unique identifier for this record from the immediate source. This is the numeric only key and used as an alternative to the ListingKey fields.  This is the local key of the system.  When records are received from other systems, a local key is commonly applied.  If conveying the original keys from the source or originating systems, see SourceSystemKey and OriginatingSystemKey." ;
  rdfs:domain      reso:Property ;
  rdfs:label       "ListingKeyNumeric" ;
  rdfs:range       xsd:decimal ;
  reso:CertificationLevel "Platinum" ;
  reso:PropertyTypes "RESI","RLSE","RINC","LAND","MOBI","FARM","COMS","COML","BUSO" ;
  schema:sameAs    <http://ddwiki.reso.org/display/DDW/ListingKeyNumeric+Field> ;
  vs:term_status   "stable"
.
reso:ListingService a rdf:Property ;
  rdfs:comment     "Defines the type or level of service the listing member will be providing to the selling home owner.  This will typically be a single selection.  Examples include Full Service, Limited Service or Entry Only." ;
  rdfs:domain      reso:Property ;
  rdfs:label       "ListingService" ;
  rdfs:range       enum:ListingService ;
  reso:CertificationLevel "Core" ;
  reso:PropertyTypes "RESI","RLSE","RINC","LAND","MOBI","FARM","COMS","COML","BUSO" ;
  schema:sameAs    <http://ddwiki.reso.org/display/DDW/ListingService+Field> ;
  vs:term_status   "stable"
.
reso:ListingTerms a rdf:Property ;
  rdfs:comment     "Terms of the listing such as Lien Release, Subject to Court Approval or Owner Will Carry. Also may include options that describe the financing terms that are acceptable to the seller, i.e. cash, assumable, FHA loan, etc." ;
  rdfs:domain      reso:Property ;
  rdfs:label       "ListingTerms" ;
  rdfs:range       enum:ListingTerms ;
  reso:CertificationLevel "Bronze" ;
  reso:PropertyTypes "RESI","RLSE","RINC","LAND","MOBI","FARM","COMS","COML","BUSO" ;
  schema:sameAs    <http://ddwiki.reso.org/display/DDW/ListingTerms+Field> ;
  vs:term_status   "stable"
.
reso:LivingArea a rdf:Property ;
  rdfs:comment     "The total livable area within the structure." ;
  rdfs:domain      reso:Property ;
  rdfs:label       "LivingArea" ;
  rdfs:range       xsd:decimal ;
  reso:CertificationLevel "Core" ;
  reso:PropertyTypes "RESI","RLSE","RINC","MOBI","FARM" ;
  schema:sameAs    <http://ddwiki.reso.org/display/DDW/LivingArea+Field> ;
  vs:term_status   "stable"
.
reso:LivingAreaSource a rdf:Property ;
  rdfs:comment     "The source of the measurements. This is a pick list of options showing the source of the measurement. i.e. Agent, Assessor, Estimate, etc." ;
  rdfs:domain      reso:Property ;
  rdfs:label       "LivingAreaSource" ;
  rdfs:range       enum:AreaSource ;
  reso:CertificationLevel "Bronze" ;
  reso:PropertyTypes "RESI","RLSE","RINC","MOBI","FARM" ;
  schema:sameAs    <http://ddwiki.reso.org/display/DDW/LivingAreaSource+Field> ;
  vs:term_status   "stable"
.
reso:LivingAreaUnits a rdf:Property ;
  rdfs:comment     "A pick list of the unit of measurement for the area.  i.e. Square Feet, Square Meters, Acres, etc." ;
  rdfs:domain      reso:Property ;
  rdfs:label       "LivingAreaUnits" ;
  rdfs:range       enum:AreaUnits ;
  reso:CertificationLevel "Core" ;
  reso:PropertyTypes "RESI","RLSE","RINC","MOBI","FARM" ;
  schema:sameAs    <http://ddwiki.reso.org/display/DDW/LivingAreaUnits+Field> ;
  vs:term_status   "stable"
.
reso:LockBoxLocation a rdf:Property ;
  rdfs:comment     "A field describing the location of the lock box." ;
  rdfs:domain      reso:Property ;
  rdfs:label       "LockBoxLocation" ;
  rdfs:range       xsd:string ;
  reso:CertificationLevel "Bronze" ;
  reso:PropertyTypes "RESI","RLSE","RINC","LAND","MOBI","FARM","COMS","COML","BUSO" ;
  schema:sameAs    <http://ddwiki.reso.org/display/DDW/LockBoxLocation+Field> ;
  vs:term_status   "stable"
.
reso:LockBoxSerialNumber a rdf:Property ;
  rdfs:comment     "The serial number of the lockbox placed on the property." ;
  rdfs:domain      reso:Property ;
  rdfs:label       "LockBoxSerialNumber" ;
  rdfs:range       xsd:string ;
  reso:CertificationLevel "Bronze" ;
  reso:PropertyTypes "RESI","RLSE","RINC","LAND","MOBI","FARM","COMS","COML","BUSO" ;
  schema:sameAs    <http://ddwiki.reso.org/display/DDW/LockBoxSerialNumber+Field> ;
  vs:term_status   "stable"
.
reso:LockBoxType a rdf:Property ;
  rdfs:comment     "A field describing the type of lock box." ;
  rdfs:domain      reso:Property ;
  rdfs:label       "LockBoxType" ;
  rdfs:range       enum:LockBoxType ;
  reso:CertificationLevel "Bronze" ;
  reso:PropertyTypes "RESI","RLSE","RINC","LAND","MOBI","FARM","COMS","COML","BUSO" ;
  schema:sameAs    <http://ddwiki.reso.org/display/DDW/LockBoxType+Field> ;
  vs:term_status   "stable"
.
reso:Longitude a rdf:Property ;
  rdfs:comment     "The geographic longitude of some reference point on the property, specified in degrees and decimal parts. Positive numbers must not include the plus symbol." ;
  rdfs:domain      reso:Property ;
  rdfs:label       "Longitude" ;
  rdfs:range       xsd:decimal ;
  reso:CertificationLevel "Core" ;
  reso:PropertyTypes "RESI","RLSE","RINC","LAND","MOBI","FARM","COMS","COML","BUSO" ;
  schema:sameAs    <http://ddwiki.reso.org/display/DDW/Longitude+Field> ;
  vs:term_status   "stable"
.
reso:LotDimensionsSource a rdf:Property ;
  rdfs:comment     "The source of the measurements. This may be a pick list of options showing the source of the measurement. i.e. Agent, Assessor, Estimate, etc." ;
  rdfs:domain      reso:Property ;
  rdfs:label       "LotDimensionsSource" ;
  rdfs:range       xsd:string ;
  reso:CertificationLevel "Gold" ;
  reso:PropertyTypes "RESI","RLSE","RINC","LAND","MOBI","FARM","COMS","COML","BUSO" ;
  schema:sameAs    <http://ddwiki.reso.org/display/DDW/LotDimensionsSource+Field> ;
  vs:term_status   "stable"
.
reso:LotFeatures a rdf:Property ;
  rdfs:comment     "A list of features or description of the lot included in the sale/lease." ;
  rdfs:domain      reso:Property ;
  rdfs:label       "LotFeatures" ;
  rdfs:range       xsd:string ;
  reso:CertificationLevel "Platinum" ;
  reso:PropertyTypes "RESI","RLSE","RINC","LAND","MOBI","FARM" ;
  schema:sameAs    <http://ddwiki.reso.org/display/DDW/LotFeatures+Field> ;
  vs:term_status   "stable"
.
reso:LotSizeAcres a rdf:Property ;
  rdfs:comment     "The total Acres of the lot.  This field is related to the Lot Size Area and Lot Size Units and must be in sync with the values represented in those fields.  Lot Size Source also applies to this field when used." ;
  rdfs:domain      reso:Property ;
  rdfs:label       "LotSizeAcres" ;
  rdfs:range       xsd:decimal ;
  reso:CertificationLevel "Gold" ;
  reso:PropertyTypes "RESI","RLSE","RINC","LAND","MOBI","FARM","COMS","COML","BUSO" ;
  schema:sameAs    <http://ddwiki.reso.org/display/DDW/LotSizeAcres+Field> ;
  vs:term_status   "stable"
.
reso:LotSizeArea a rdf:Property ;
  rdfs:comment     "The total area of the lot.  See Lot Size Units for the units of measurement (Square Feet, Square Meters, Acres, etc.)." ;
  rdfs:domain      reso:Property ;
  rdfs:label       "LotSizeArea" ;
  rdfs:range       xsd:decimal ;
  reso:CertificationLevel "Core" ;
  reso:PropertyTypes "RESI","RLSE","RINC","LAND","MOBI","FARM","COMS","COML","BUSO" ;
  schema:sameAs    <http://ddwiki.reso.org/display/DDW/LotSizeArea+Field> ;
  vs:term_status   "stable"
.
reso:LotSizeDimensions a rdf:Property ;
  rdfs:comment     "The dimensions of the lot minimally represented as length and width (i.e. 250 x 180) or a measurement of all sides of the polygon representing the property lines of the property.  i.e. 30 x 50 x 120 x 60 x 22." ;
  rdfs:domain      reso:Property ;
  rdfs:label       "LotSizeDimensions" ;
  rdfs:range       xsd:string ;
  reso:CertificationLevel "Gold" ;
  reso:PropertyTypes "RESI","RLSE","RINC","LAND","MOBI","FARM","COMS","COML","BUSO" ;
  schema:sameAs    <http://ddwiki.reso.org/display/DDW/LotSizeDimensions+Field> ;
  vs:term_status   "stable"
.
reso:LotSizeSource a rdf:Property ;
  rdfs:comment     "The source of the measurements. This may be a pick list of options showing the source of the measurement. i.e. Agent, Assessor, Estimate, etc." ;
  rdfs:domain      reso:Property ;
  rdfs:label       "LotSizeSource" ;
  rdfs:range       enum:LotSizeSource ;
  reso:CertificationLevel "Bronze" ;
  reso:PropertyTypes "RESI","RLSE","RINC","LAND","MOBI","FARM","COMS","COML","BUSO" ;
  schema:sameAs    <http://ddwiki.reso.org/display/DDW/LotSizeSource+Field> ;
  vs:term_status   "stable"
.
reso:LotSizeSquareFeet a rdf:Property ;
  rdfs:comment     "The total square footage of the lot.  This field is related to the Lot Size Area and Lot Size Units and must be in sync with the values represented in those fields.  Lot Size Source also applies to this field when used." ;
  rdfs:domain      reso:Property ;
  rdfs:label       "LotSizeSquareFeet" ;
  rdfs:range       xsd:decimal ;
  reso:CertificationLevel "Gold" ;
  reso:PropertyTypes "RESI","RLSE","RINC","LAND","MOBI","FARM","COMS","COML","BUSO" ;
  schema:sameAs    <http://ddwiki.reso.org/display/DDW/LotSizeSquareFeet+Field> ;
  vs:term_status   "stable"
.
reso:LotSizeUnits a rdf:Property ;
  rdfs:comment     "A pick list of the unit of measurement for the area.  i.e. Square Feet, Square Meters, Acres, etc." ;
  rdfs:domain      reso:Property ;
  rdfs:label       "LotSizeUnits" ;
  rdfs:range       enum:LotSizeUnits ;
  reso:CertificationLevel "Core" ;
  reso:PropertyTypes "RESI","RLSE","RINC","LAND","MOBI","FARM","COMS","COML","BUSO" ;
  schema:sameAs    <http://ddwiki.reso.org/display/DDW/LotSizeUnits+Field> ;
  vs:term_status   "stable"
.
reso:MLSAreaMajor a rdf:Property ;
  rdfs:comment     "The major marketing area name, as defined by the MLS or other non-governmental organization.  If there is only one MLS Area in use, it must be the MLSAreaMajor." ;
  rdfs:domain      reso:Property ;
  rdfs:label       "MLSAreaMajor" ;
  rdfs:range       xsd:string ;
  reso:CertificationLevel "Core" ;
  reso:PropertyTypes "RESI","RLSE","RINC","LAND","MOBI","FARM","COMS","COML","BUSO" ;
  schema:sameAs    <http://ddwiki.reso.org/display/DDW/MLSAreaMajor+Field> ;
  vs:term_status   "stable"
.
reso:MLSAreaMinor a rdf:Property ;
  rdfs:comment     "The minor/sub marketing area name, as defined by the MLS or other non-governmental organization.  If there is only one MLS Area in use, it must be the MLSAreaMajor." ;
  rdfs:domain      reso:Property ;
  rdfs:label       "MLSAreaMinor" ;
  rdfs:range       xsd:string ;
  reso:CertificationLevel "Bronze" ;
  reso:PropertyTypes "RESI","RLSE","RINC","LAND","MOBI","FARM","COMS","COML","BUSO" ;
  schema:sameAs    <http://ddwiki.reso.org/display/DDW/MLSAreaMinor+Field> ;
  vs:term_status   "stable"
.
reso:MainLevelBathrooms a rdf:Property ;
  rdfs:comment     "The number of bathrooms located on the main or entry level of the property." ;
  rdfs:domain      reso:Property ;
  rdfs:label       "MainLevelBathrooms" ;
  rdfs:range       xsd:decimal ;
  reso:CertificationLevel "Silver" ;
  reso:PropertyTypes "RESI","RLSE" ;
  schema:sameAs    <http://ddwiki.reso.org/display/DDW/MainLevelBathrooms+Field> ;
  vs:term_status   "stable"
.
reso:MainLevelBedrooms a rdf:Property ;
  rdfs:comment     "The number of bedrooms located on the main or entry level of the property." ;
  rdfs:domain      reso:Property ;
  rdfs:label       "MainLevelBedrooms" ;
  rdfs:range       xsd:decimal ;
  reso:CertificationLevel "Silver" ;
  reso:PropertyTypes "RESI","RLSE" ;
  schema:sameAs    <http://ddwiki.reso.org/display/DDW/MainLevelBedrooms+Field> ;
  vs:term_status   "stable"
.
reso:MaintenanceExpense a rdf:Property ;
  rdfs:comment     "The annual expense that is not paid directly by the tenant and is included in the Operating Expense calculations." ;
  rdfs:domain      reso:Property ;
  rdfs:label       "MaintenanceExpense" ;
  rdfs:range       xsd:decimal ;
  reso:CertificationLevel "Silver" ;
  reso:PropertyTypes "RINC","COMS","COML" ;
  schema:sameAs    <http://ddwiki.reso.org/display/DDW/MaintenanceExpense+Field> ;
  vs:term_status   "stable"
.
reso:MajorChangeTimestamp a rdf:Property ;
  rdfs:comment     "Timestamp of the last major change on the listing (see also MajorChangeType)." ;
  rdfs:domain      reso:Property ;
  rdfs:label       "MajorChangeTimestamp" ;
  rdfs:range       xsd:dateTime ;
  reso:CertificationLevel "Bronze" ;
  reso:PropertyTypes "RESI","RLSE","RINC","LAND","MOBI","FARM","COMS","COML","BUSO" ;
  schema:sameAs    <http://ddwiki.reso.org/display/DDW/MajorChangeTimestamp+Field> ;
  vs:term_status   "stable"
.
reso:MajorChangeType a rdf:Property ;
  rdfs:comment     "Description of the last major change on the listing, i.e. &#x201c;price reduction&#x201d;, &#x201c;back on market&#x201d;, etc.  May be used to display on a summary view of listing results to quickly identify listings that have had major changes recently." ;
  rdfs:domain      reso:Property ;
  rdfs:label       "MajorChangeType" ;
  rdfs:range       enum:ChangeType ;
  reso:CertificationLevel "Bronze" ;
  reso:PropertyTypes "RESI","RLSE","RINC","LAND","MOBI","FARM","COMS","COML","BUSO" ;
  schema:sameAs    <http://ddwiki.reso.org/display/DDW/MajorChangeType+Field> ;
  vs:term_status   "stable"
.
reso:Make a rdf:Property ;
  rdfs:comment     "Make of the mobile or manufactured home." ;
  rdfs:domain      reso:Property ;
  rdfs:label       "Make" ;
  rdfs:range       xsd:string ;
  reso:CertificationLevel "Core" ;
  reso:PropertyTypes "RESI","RLSE","MOBI" ;
  schema:sameAs    <http://ddwiki.reso.org/display/DDW/Make+Field> ;
  vs:term_status   "stable"
.
reso:ManagerExpense a rdf:Property ;
  rdfs:comment     "The annual expense that is not paid directly by the tenant and is included in the Operating Expense calculations.  This is for an individual manager.  Use ProfessionalManagementExpense for a management company." ;
  rdfs:domain      reso:Property ;
  rdfs:label       "ManagerExpense" ;
  rdfs:range       xsd:decimal ;
  reso:CertificationLevel "Silver" ;
  reso:PropertyTypes "RINC" ;
  schema:sameAs    <http://ddwiki.reso.org/display/DDW/ManagerExpense+Field> ;
  vs:term_status   "stable"
.
reso:MapCoordinate a rdf:Property ;
  rdfs:comment     "A map coordinate for the property, as determined by local custom. This is not necessarily the same as the geographic coordinate but may depend on the coordinate system used by whatever mapping service is customarily used by the listing service." ;
  rdfs:domain      reso:Property ;
  rdfs:label       "MapCoordinate" ;
  rdfs:range       xsd:string ;
  reso:CertificationLevel "Bronze" ;
  reso:PropertyTypes "RESI","RLSE","RINC","LAND","MOBI","FARM","COMS","COML","BUSO" ;
  schema:sameAs    <http://ddwiki.reso.org/display/DDW/MapCoordinate+Field> ;
  vs:term_status   "stable"
.
reso:MapCoordinateSource a rdf:Property ;
  rdfs:comment     "Name of the map or map book publisher." ;
  rdfs:domain      reso:Property ;
  rdfs:label       "MapCoordinateSource" ;
  rdfs:range       xsd:string ;
  reso:CertificationLevel "Bronze" ;
  reso:PropertyTypes "RESI","RLSE","RINC","LAND","MOBI","FARM","COMS","COML","BUSO" ;
  schema:sameAs    <http://ddwiki.reso.org/display/DDW/MapCoordinateSource+Field> ;
  vs:term_status   "stable"
.
reso:MapURL a rdf:Property ;
  rdfs:comment     "URI to a map of the property." ;
  rdfs:domain      reso:Property ;
  rdfs:label       "MapURL" ;
  rdfs:range       xsd:string ;
  reso:CertificationLevel "Bronze" ;
  reso:PropertyTypes "RESI","RLSE","RINC","LAND","MOBI","FARM","COMS","COML","BUSO" ;
  schema:sameAs    <http://ddwiki.reso.org/display/DDW/MapURL+Field> ;
  vs:term_status   "stable"
.
reso:MiddleOrJuniorSchool a rdf:Property ;
  rdfs:comment     "The name of the junior or middle school having a catchment area that includes the associated property." ;
  rdfs:domain      reso:Property ;
  rdfs:label       "MiddleOrJuniorSchool" ;
  rdfs:range       xsd:string ;
  reso:CertificationLevel "Silver" ;
  reso:PropertyTypes "RESI","RLSE","RINC","LAND","MOBI","FARM","COMS","COML","BUSO" ;
  schema:sameAs    <http://ddwiki.reso.org/display/DDW/MiddleOrJuniorSchool+Field> ;
  vs:term_status   "stable"
.
reso:MiddleOrJuniorSchoolDistrict a rdf:Property ;
  rdfs:comment     "The name of the junior or middle school district having a catchment area that includes the associated property." ;
  rdfs:domain      reso:Property ;
  rdfs:label       "MiddleOrJuniorSchoolDistrict" ;
  rdfs:range       xsd:string ;
  reso:CertificationLevel "Bronze" ;
  reso:PropertyTypes "RESI","RLSE","RINC","LAND","MOBI","FARM","COMS","COML","BUSO" ;
  schema:sameAs    <http://ddwiki.reso.org/display/DDW/MiddleOrJuniorSchoolDistrict+Field> ;
  vs:term_status   "stable"
.
reso:MlsStatus a rdf:Property ;
  rdfs:comment     "Local or regional status that are well known by business users. Each MlsStatus must map to a single StandardStatus. Multiple MlsStatus may map to a single StandardStatus." ;
  rdfs:domain      reso:Property ;
  rdfs:label       "MlsStatus" ;
  rdfs:range       xsd:string ;
  reso:CertificationLevel "Core" ;
  reso:PropertyTypes "RESI","RLSE","RINC","LAND","MOBI","FARM","COMS","COML","BUSO" ;
  schema:sameAs    <http://ddwiki.reso.org/display/DDW/MlsStatus+Field> ;
  vs:term_status   "stable"
.
reso:MobileDimUnits a rdf:Property ;
  rdfs:comment     "A pick list of the unit linear measurement.  i.e. feed, meters, yards, kilometers, miles, etc." ;
  rdfs:domain      reso:Property ;
  rdfs:label       "MobileDimUnits" ;
  rdfs:range       enum:LinearUnits ;
  reso:CertificationLevel "Silver" ;
  reso:PropertyTypes "MOBI" ;
  schema:sameAs    <http://ddwiki.reso.org/display/DDW/MobileDimUnits+Field> ;
  vs:term_status   "stable"
.
reso:MobileHomeRemainsYN a rdf:Property ;
  rdfs:comment     "Is the mobile home to remain and be included in the sale of the property." ;
  rdfs:domain      reso:Property ;
  rdfs:label       "MobileHomeRemainsYN" ;
  rdfs:range       xsd:boolean ;
  reso:CertificationLevel "Bronze" ;
  reso:PropertyTypes "MOBI" ;
  schema:sameAs    <http://ddwiki.reso.org/display/DDW/MobileHomeRemainsYN+Field> ;
  vs:term_status   "stable"
.
reso:MobileLength a rdf:Property ;
  rdfs:comment     "Length of the mobile/manufactured home." ;
  rdfs:domain      reso:Property ;
  rdfs:label       "MobileLength" ;
  rdfs:range       xsd:decimal ;
  reso:CertificationLevel "Core" ;
  reso:PropertyTypes "MOBI" ;
  schema:sameAs    <http://ddwiki.reso.org/display/DDW/MobileLength+Field> ;
  vs:term_status   "stable"
.
reso:MobileWidth a rdf:Property ;
  rdfs:comment     "Width of the mobile/manufactured home." ;
  rdfs:domain      reso:Property ;
  rdfs:label       "MobileWidth" ;
  rdfs:range       xsd:decimal ;
  reso:CertificationLevel "Core" ;
  reso:PropertyTypes "MOBI" ;
  schema:sameAs    <http://ddwiki.reso.org/display/DDW/MobileWidth+Field> ;
  vs:term_status   "stable"
.
reso:Model a rdf:Property ;
  rdfs:comment     "Model of the mobile or manufactured home." ;
  rdfs:domain      reso:Property ;
  rdfs:label       "Model" ;
  rdfs:range       xsd:string ;
  reso:CertificationLevel "Core" ;
  reso:PropertyTypes "RESI","RLSE","MOBI" ;
  schema:sameAs    <http://ddwiki.reso.org/display/DDW/Model+Field> ;
  vs:term_status   "stable"
.
reso:ModificationTimestamp a rdf:Property ;
  rdfs:comment     "The transactional timestamp automatically recorded by the MLS system representing the date/time the listing was last modified." ;
  rdfs:domain      reso:Property ;
  rdfs:label       "ModificationTimestamp" ;
  rdfs:range       xsd:dateTime ;
  reso:CertificationLevel "Core" ;
  reso:PropertyTypes "RESI","RLSE","RINC","LAND","MOBI","FARM","COMS","COML","BUSO" ;
  schema:sameAs    <http://ddwiki.reso.org/display/DDW/ModificationTimestamp+Field> ;
  vs:term_status   "stable"
.
reso:NetOperatingIncome a rdf:Property ;
  rdfs:comment     "Net operating income is the revenue from a property after operating expenses have been deducted, but before deducting income taxes and financing expenses (interest and Principal Payments).   For example, Gross Income - Operating Expenses = Net Operating Income (NOI)." ;
  rdfs:domain      reso:Property ;
  rdfs:label       "NetOperatingIncome" ;
  rdfs:range       xsd:decimal ;
  reso:CertificationLevel "Core" ;
  reso:PropertyTypes "RINC","COMS","COML","BUSO" ;
  schema:sameAs    <http://ddwiki.reso.org/display/DDW/NetOperatingIncome+Field> ;
  vs:term_status   "stable"
.
reso:NewConstructionYN a rdf:Property ;
  rdfs:comment     "Is the property newly constructed and has not been previously occupied?" ;
  rdfs:domain      reso:Property ;
  rdfs:label       "NewConstructionYN" ;
  rdfs:range       xsd:boolean ;
  reso:CertificationLevel "Silver" ;
  reso:PropertyTypes "RESI","RLSE","RINC","MOBI","FARM" ;
  schema:sameAs    <http://ddwiki.reso.org/display/DDW/NewConstructionYN+Field> ;
  vs:term_status   "stable"
.
reso:NewTaxesExpense a rdf:Property ;
  rdfs:comment     "The annual expense that is not paid directly by the tenant and is included in the Operating Expense calculations." ;
  rdfs:domain      reso:Property ;
  rdfs:label       "NewTaxesExpense" ;
  rdfs:range       xsd:decimal ;
  reso:CertificationLevel "Silver" ;
  reso:PropertyTypes "RINC" ;
  schema:sameAs    <http://ddwiki.reso.org/display/DDW/NewTaxesExpense+Field> ;
  vs:term_status   "stable"
.
reso:NumberOfBuildings a rdf:Property ;
  rdfs:comment     "Total number of separate buildings included in the income property." ;
  rdfs:domain      reso:Property ;
  rdfs:label       "NumberOfBuildings" ;
  rdfs:range       xsd:decimal ;
  reso:CertificationLevel "Bronze" ;
  reso:PropertyTypes "RINC","COMS","COML" ;
  schema:sameAs    <http://ddwiki.reso.org/display/DDW/NumberOfBuildings+Field> ;
  vs:term_status   "stable"
.
reso:NumberOfFullTimeEmployees a rdf:Property ;
  rdfs:comment     "The current number of individuals employed by the business on a full-time basis." ;
  rdfs:domain      reso:Property ;
  rdfs:label       "NumberOfFullTimeEmployees" ;
  rdfs:range       xsd:decimal ;
  reso:CertificationLevel "Bronze" ;
  reso:PropertyTypes "BUSO" ;
  schema:sameAs    <http://ddwiki.reso.org/display/DDW/NumberOfFullTimeEmployees+Field> ;
  vs:term_status   "stable"
.
reso:NumberOfLots a rdf:Property ;
  rdfs:comment     "Total number of lots on the property or included in the sale. Land properties are often sold with multiple lots. It is important to be able to describe how many lots are in the property and not in all cases do lots have separate Parcel IDs." ;
  rdfs:domain      reso:Property ;
  rdfs:label       "NumberOfLots" ;
  rdfs:range       xsd:decimal ;
  reso:CertificationLevel "Bronze" ;
  reso:PropertyTypes "LAND" ;
  schema:sameAs    <http://ddwiki.reso.org/display/DDW/NumberOfLots+Field> ;
  vs:term_status   "stable"
.
reso:NumberOfPads a rdf:Property ;
  rdfs:comment     "The number of pads or spaces in the mobile home park." ;
  rdfs:domain      reso:Property ;
  rdfs:label       "NumberOfPads" ;
  rdfs:range       xsd:decimal ;
  reso:CertificationLevel "Silver" ;
  reso:PropertyTypes "MOBI" ;
  schema:sameAs    <http://ddwiki.reso.org/display/DDW/NumberOfPads+Field> ;
  vs:term_status   "stable"
.
reso:NumberOfPartTimeEmployees a rdf:Property ;
  rdfs:comment     "The current number of individuals employed by the business on a part-time basis." ;
  rdfs:domain      reso:Property ;
  rdfs:label       "NumberOfPartTimeEmployees" ;
  rdfs:range       xsd:decimal ;
  reso:CertificationLevel "Bronze" ;
  reso:PropertyTypes "BUSO" ;
  schema:sameAs    <http://ddwiki.reso.org/display/DDW/NumberOfPartTimeEmployees+Field> ;
  vs:term_status   "stable"
.
reso:NumberOfSeparateElectricMeters a rdf:Property ;
  rdfs:comment     "Total number of separate meters on the property." ;
  rdfs:domain      reso:Property ;
  rdfs:label       "NumberOfSeparateElectricMeters" ;
  rdfs:range       xsd:decimal ;
  reso:CertificationLevel "Silver" ;
  reso:PropertyTypes "RINC","FARM" ;
  schema:sameAs    <http://ddwiki.reso.org/display/DDW/NumberOfSeparateElectricMeters+Field> ;
  vs:term_status   "stable"
.
reso:NumberOfSeparateGasMeters a rdf:Property ;
  rdfs:comment     "Total number of separate meters on the property." ;
  rdfs:domain      reso:Property ;
  rdfs:label       "NumberOfSeparateGasMeters" ;
  rdfs:range       xsd:decimal ;
  reso:CertificationLevel "Silver" ;
  reso:PropertyTypes "RINC","FARM" ;
  schema:sameAs    <http://ddwiki.reso.org/display/DDW/NumberOfSeparateGasMeters+Field> ;
  vs:term_status   "stable"
.
reso:NumberOfSeparateWaterMeters a rdf:Property ;
  rdfs:comment     "Total number of separate meters on the property." ;
  rdfs:domain      reso:Property ;
  rdfs:label       "NumberOfSeparateWaterMeters" ;
  rdfs:range       xsd:decimal ;
  reso:CertificationLevel "Silver" ;
  reso:PropertyTypes "RINC","FARM" ;
  schema:sameAs    <http://ddwiki.reso.org/display/DDW/NumberOfSeparateWaterMeters+Field> ;
  vs:term_status   "stable"
.
reso:NumberOfUnitsInCommunity a rdf:Property ;
  rdfs:comment     "The total number of units in the building, complex or community.  This is not the number of units being sold, but rather the size of the community in which the dwelling being sold is located." ;
  rdfs:domain      reso:Property ;
  rdfs:label       "NumberOfUnitsInCommunity" ;
  rdfs:range       xsd:decimal ;
  reso:CertificationLevel "Silver" ;
  reso:PropertyTypes "RESI","RLSE" ;
  schema:sameAs    <http://ddwiki.reso.org/display/DDW/NumberOfUnitsInCommunity+Field> ;
  vs:term_status   "stable"
.
reso:NumberOfUnitsLeased a rdf:Property ;
  rdfs:comment     "Total number of units currently under a lease agreement." ;
  rdfs:domain      reso:Property ;
  rdfs:label       "NumberOfUnitsLeased" ;
  rdfs:range       xsd:decimal ;
  reso:CertificationLevel "Bronze" ;
  reso:PropertyTypes "RINC","COMS","COML" ;
  schema:sameAs    <http://ddwiki.reso.org/display/DDW/NumberOfUnitsLeased+Field> ;
  vs:term_status   "stable"
.
reso:NumberOfUnitsMoMo a rdf:Property ;
  rdfs:comment     "The total number of units leasable month to month." ;
  rdfs:domain      reso:Property ;
  rdfs:label       "NumberOfUnitsMoMo" ;
  rdfs:range       xsd:decimal ;
  reso:CertificationLevel "Bronze" ;
  reso:PropertyTypes "RINC" ;
  schema:sameAs    <http://ddwiki.reso.org/display/DDW/NumberOfUnitsMoMo+Field> ;
  vs:term_status   "stable"
.
reso:NumberOfUnitsTotal a rdf:Property ;
  rdfs:comment     "Total number of units included in the income property, occupied or unoccupied." ;
  rdfs:domain      reso:Property ;
  rdfs:label       "NumberOfUnitsTotal" ;
  rdfs:range       xsd:decimal ;
  reso:CertificationLevel "Core" ;
  reso:PropertyTypes "RINC","COMS","COML" ;
  schema:sameAs    <http://ddwiki.reso.org/display/DDW/NumberOfUnitsTotal+Field> ;
  vs:term_status   "stable"
.
reso:NumberOfUnitsVacant a rdf:Property ;
  rdfs:comment     "The number of units currently vacant." ;
  rdfs:domain      reso:Property ;
  rdfs:label       "NumberOfUnitsVacant" ;
  rdfs:range       xsd:decimal ;
  reso:CertificationLevel "Bronze" ;
  reso:PropertyTypes "RINC" ;
  schema:sameAs    <http://ddwiki.reso.org/display/DDW/NumberOfUnitsVacant+Field> ;
  vs:term_status   "stable"
.
reso:OccupantName a rdf:Property ;
  rdfs:comment     "Name of the current occupant, if any, of the property being sold." ;
  rdfs:domain      reso:Property ;
  rdfs:label       "OccupantName" ;
  rdfs:range       xsd:string ;
  reso:CertificationLevel "Bronze" ;
  reso:PropertyTypes "RESI","RLSE","MOBI" ;
  schema:sameAs    <http://ddwiki.reso.org/display/DDW/OccupantName+Field> ;
  vs:term_status   "stable"
.
reso:OccupantPhone a rdf:Property ;
  rdfs:comment     "North American 10 digit phone numbers should be in the format of ###-###-#### (separated by hyphens).  Other conventions should use the common local standard.  International numbers should be preceded by a plus symbol." ;
  rdfs:domain      reso:Property ;
  rdfs:label       "OccupantPhone" ;
  rdfs:range       xsd:string ;
  reso:CertificationLevel "Bronze" ;
  reso:PropertyTypes "RESI","RLSE","MOBI" ;
  schema:sameAs    <http://ddwiki.reso.org/display/DDW/OccupantPhone+Field> ;
  vs:term_status   "stable"
.
reso:OccupantType a rdf:Property ;
  rdfs:comment     "A field that describes the type of occupant, i.e. Owner, Tenant, Vacant." ;
  rdfs:domain      reso:Property ;
  rdfs:label       "OccupantType" ;
  rdfs:range       enum:OccupantType ;
  reso:CertificationLevel "Bronze" ;
  reso:PropertyTypes "RESI","RLSE","MOBI" ;
  schema:sameAs    <http://ddwiki.reso.org/display/DDW/OccupantType+Field> ;
  vs:term_status   "stable"
.
reso:OffMarketDate a rdf:Property ;
  rdfs:comment     "The date the listing was taken off market. Where possible, this date is reflective of the date entered by the agent reflecting when the change occurred contractually, not a timestamp of when the change was made in the MLS." ;
  rdfs:domain      reso:Property ;
  rdfs:label       "OffMarketDate" ;
  rdfs:range       xsd:date ;
  reso:CertificationLevel "Core" ;
  reso:PropertyTypes "RESI","RLSE","RINC","LAND","MOBI","FARM","COMS","COML","BUSO" ;
  schema:sameAs    <http://ddwiki.reso.org/display/DDW/OffMarketDate+Field> ;
  vs:term_status   "stable"
.
reso:OffMarketTimestamp a rdf:Property ;
  rdfs:comment     "The transactional timestamp automatically recorded by the MLS system representing the most recent date/time the listing's status was set to and off market status (not Active or Backup)" ;
  rdfs:domain      reso:Property ;
  rdfs:label       "OffMarketTimestamp" ;
  rdfs:range       xsd:dateTime ;
  reso:CertificationLevel "Bronze" ;
  reso:PropertyTypes "RESI","RLSE","RINC","LAND","MOBI","FARM","COMS","COML","BUSO" ;
  schema:sameAs    <http://ddwiki.reso.org/display/DDW/OffMarketTimestamp+Field> ;
  vs:term_status   "stable"
.
reso:OnMarketDate a rdf:Property ;
  rdfs:comment     "The date the listing was placed on market. Where possible, this date is reflective of the date entered by the agent reflecting when the change occurred contractually, not a timestamp of when the change was made in the MLS." ;
  rdfs:domain      reso:Property ;
  rdfs:label       "OnMarketDate" ;
  rdfs:range       xsd:date ;
  reso:CertificationLevel "Core" ;
  reso:PropertyTypes "RESI","RLSE","RINC","LAND","MOBI","FARM","COMS","COML","BUSO" ;
  schema:sameAs    <http://ddwiki.reso.org/display/DDW/OnMarketDate+Field> ;
  vs:term_status   "stable"
.
reso:OnMarketTimestamp a rdf:Property ;
  rdfs:comment     "The transactional timestamp automatically recorded by the MLS system representing the most recent date/time the listing's status was set to Active or Backup.  This also includes initial input of the listing to Active/Backup or from a draft or approval status to Active/Backup." ;
  rdfs:domain      reso:Property ;
  rdfs:label       "OnMarketTimestamp" ;
  rdfs:range       xsd:dateTime ;
  reso:CertificationLevel "Bronze" ;
  reso:PropertyTypes "RESI","RLSE","RINC","LAND","MOBI","FARM","COMS","COML","BUSO" ;
  schema:sameAs    <http://ddwiki.reso.org/display/DDW/OnMarketTimestamp+Field> ;
  vs:term_status   "stable"
.
reso:OpenParkingSpaces a rdf:Property ;
  rdfs:comment     "The number of open or uncovered parking spaces included in the sale." ;
  rdfs:domain      reso:Property ;
  rdfs:label       "OpenParkingSpaces" ;
  rdfs:range       xsd:decimal ;
  reso:CertificationLevel "Bronze" ;
  reso:PropertyTypes "RESI","RLSE","RINC","MOBI","FARM" ;
  schema:sameAs    <http://ddwiki.reso.org/display/DDW/OpenParkingSpaces+Field> ;
  vs:term_status   "stable"
.
reso:OpenParkingYN a rdf:Property ;
  rdfs:comment     "A flag indicating that any parking spaces associated with the property are not covered by a roof." ;
  rdfs:domain      reso:Property ;
  rdfs:label       "OpenParkingYN" ;
  rdfs:range       xsd:boolean ;
  reso:CertificationLevel "Silver" ;
  reso:PropertyTypes "RESI","RLSE","RINC","MOBI","FARM" ;
  schema:sameAs    <http://ddwiki.reso.org/display/DDW/OpenParkingYN+Field> ;
  vs:term_status   "stable"
.
reso:OperatingExpense a rdf:Property ;
  rdfs:comment     "The costs associated with the operation and maintenance of an income-producing property." ;
  rdfs:domain      reso:Property ;
  rdfs:label       "OperatingExpense" ;
  rdfs:range       xsd:decimal ;
  reso:CertificationLevel "Core" ;
  reso:PropertyTypes "RINC","COMS","COML","BUSO" ;
  schema:sameAs    <http://ddwiki.reso.org/display/DDW/OperatingExpense+Field> ;
  vs:term_status   "stable"
.
reso:OperatingExpenseIncludes a rdf:Property ;
  rdfs:comment     "When individual expense fields are not used and only a total is entered, this lists the expenses that are included in the OperatingExpense field." ;
  rdfs:domain      reso:Property ;
  rdfs:label       "OperatingExpenseIncludes" ;
  rdfs:range       enum:OperatingExpenseIncludes ;
  reso:CertificationLevel "Bronze" ;
  reso:PropertyTypes "RINC" ;
  schema:sameAs    <http://ddwiki.reso.org/display/DDW/OperatingExpenseIncludes+Field> ;
  vs:term_status   "stable"
.
reso:OriginalEntryTimestamp a rdf:Property ;
  rdfs:comment     "The transactional timestamp automatically recorded by the MLS system representing the date/time the listing was entered and made visible to members of the MLS." ;
  rdfs:domain      reso:Property ;
  rdfs:label       "OriginalEntryTimestamp" ;
  rdfs:range       xsd:dateTime ;
  reso:CertificationLevel "Core" ;
  reso:PropertyTypes "RESI","RLSE","RINC","LAND","MOBI","FARM","COMS","COML","BUSO" ;
  schema:sameAs    <http://ddwiki.reso.org/display/DDW/OriginalEntryTimestamp+Field> ;
  vs:term_status   "stable"
.
reso:OriginalListPrice a rdf:Property ;
  rdfs:comment     "The original price of the property on the initial agreement between the seller and the seller's broker." ;
  rdfs:domain      reso:Property ;
  rdfs:label       "OriginalListPrice" ;
  rdfs:range       xsd:decimal ;
  reso:CertificationLevel "Core" ;
  reso:PropertyTypes "RESI","RLSE","RINC","LAND","MOBI","FARM","COMS","COML","BUSO" ;
  schema:sameAs    <http://ddwiki.reso.org/display/DDW/OriginalListPrice+Field> ;
  vs:term_status   "stable"
.
reso:OriginatingSystemID a rdf:Property ;
  rdfs:comment     "The RESO OUID's OrganizationUniqueId of the Originating record provider.  The Originating system is the system with authoritative control over the record.  For example; the name of the MLS where the listing was input.  In cases where the Originating system was not where the record originated (the authoritative system), see the Originating System fields." ;
  rdfs:domain      reso:Property ;
  rdfs:label       "OriginatingSystemID" ;
  rdfs:range       xsd:string ;
  reso:CertificationLevel "Platinum" ;
  reso:PropertyTypes "RESI","RLSE","RINC","LAND","MOBI","FARM","COMS","COML","BUSO" ;
  schema:sameAs    <http://ddwiki.reso.org/display/DDW/OriginatingSystemID+Field> ;
  vs:term_status   "stable"
.
reso:OriginatingSystemKey a rdf:Property ;
  rdfs:comment     "The system key, a unique record identifier, from the Originating system.  The Originating system is the system with authoritative control over the record.  For example, the Multiple Listing Service where the listing was input.  There may be cases where the Source System (how you received the record) is not the Originating System.  See Source System Key for more information." ;
  rdfs:domain      reso:Property ;
  rdfs:label       "OriginatingSystemKey" ;
  rdfs:range       xsd:string ;
  reso:CertificationLevel "Core" ;
  reso:PropertyTypes "RESI","RLSE","RINC","LAND","MOBI","FARM","COMS","COML","BUSO" ;
  schema:sameAs    <http://ddwiki.reso.org/display/DDW/OriginatingSystemKey+Field> ;
  vs:term_status   "stable"
.
reso:OriginatingSystemName a rdf:Property ;
  rdfs:comment     "The name of the Originating record provider.  Most commonly the name of the MLS. The place where the listing is originally input by the member.  The legal name of the company." ;
  rdfs:domain      reso:Property ;
  rdfs:label       "OriginatingSystemName" ;
  rdfs:range       xsd:string ;
  reso:CertificationLevel "Core" ;
  reso:PropertyTypes "RESI","RLSE","RINC","LAND","MOBI","FARM","COMS","COML","BUSO" ;
  schema:sameAs    <http://ddwiki.reso.org/display/DDW/OriginatingSystemName+Field> ;
  vs:term_status   "stable"
.
reso:OtherEquipment a rdf:Property ;
  rdfs:comment     "A list of other equipment that will be included in the sale of the property." ;
  rdfs:domain      reso:Property ;
  rdfs:label       "OtherEquipment" ;
  rdfs:range       xsd:string ;
  reso:CertificationLevel "Platinum" ;
  reso:PropertyTypes "RESI","RLSE","RINC","LAND","MOBI","FARM" ;
  schema:sameAs    <http://ddwiki.reso.org/display/DDW/OtherEquipment+Field> ;
  vs:term_status   "stable"
.
reso:OtherExpense a rdf:Property ;
  rdfs:comment     "The annual expense that is not paid directly by the tenant and is included in the Operating Expense calculations." ;
  rdfs:domain      reso:Property ;
  rdfs:label       "OtherExpense" ;
  rdfs:range       xsd:decimal ;
  reso:CertificationLevel "Silver" ;
  reso:PropertyTypes "RINC","COMS","COML" ;
  schema:sameAs    <http://ddwiki.reso.org/display/DDW/OtherExpense+Field> ;
  vs:term_status   "stable"
.
reso:OtherParking a rdf:Property ;
  rdfs:comment     "Other types of parking available to, or part of, the property." ;
  rdfs:domain      reso:Property ;
  rdfs:label       "OtherParking" ;
  rdfs:range       xsd:string ;
  reso:CertificationLevel "Silver" ;
  reso:PropertyTypes "RESI","RLSE","RINC","MOBI","FARM" ;
  schema:sameAs    <http://ddwiki.reso.org/display/DDW/OtherParking+Field> ;
  vs:term_status   "stable"
.
reso:OtherStructures a rdf:Property ;
  rdfs:comment     "A list of structures other than the main dwelling.  For example, Guest House, Barn, Shed, etc." ;
  rdfs:domain      reso:Property ;
  rdfs:label       "OtherStructures" ;
  rdfs:range       xsd:string ;
  reso:CertificationLevel "Gold" ;
  reso:PropertyTypes "RESI","RLSE","RINC","MOBI","FARM" ;
  schema:sameAs    <http://ddwiki.reso.org/display/DDW/OtherStructures+Field> ;
  vs:term_status   "stable"
.
reso:OwnerName a rdf:Property ;
  rdfs:comment     "Name of the owner of the property being sold." ;
  rdfs:domain      reso:Property ;
  rdfs:label       "OwnerName" ;
  rdfs:range       xsd:string ;
  reso:CertificationLevel "Bronze" ;
  reso:PropertyTypes "RESI","RLSE","RINC","LAND","MOBI","FARM","COMS","COML","BUSO" ;
  schema:sameAs    <http://ddwiki.reso.org/display/DDW/OwnerName+Field> ;
  vs:term_status   "stable"
.
reso:OwnerPays a rdf:Property ;
  rdfs:comment     "A list of expenses for the property paid for by the owner as opposed to the tenant (e.g. Water, Trash, Electric)." ;
  rdfs:domain      reso:Property ;
  rdfs:label       "OwnerPays" ;
  rdfs:range       enum:OwnerPays ;
  reso:CertificationLevel "Bronze" ;
  reso:PropertyTypes "RLSE","RINC","COMS","COML" ;
  schema:sameAs    <http://ddwiki.reso.org/display/DDW/OwnerPays+Field> ;
  vs:term_status   "stable"
.
reso:OwnerPhone a rdf:Property ;
  rdfs:comment     "North American 10 digit phone numbers should be in the format of ###-###-#### (separated by hyphens).  Other conventions should use the common local standard.  International numbers should be preceded by a plus symbol." ;
  rdfs:domain      reso:Property ;
  rdfs:label       "OwnerPhone" ;
  rdfs:range       xsd:string ;
  reso:CertificationLevel "Bronze" ;
  reso:PropertyTypes "RESI","RLSE","RINC","LAND","MOBI","FARM","COMS","COML","BUSO" ;
  schema:sameAs    <http://ddwiki.reso.org/display/DDW/OwnerPhone+Field> ;
  vs:term_status   "stable"
.
reso:Ownership a rdf:Property ;
  rdfs:comment     "A text description of the manner in which title to a property is held.  Trust, Corporation, Joint Tennant, Individual." ;
  rdfs:domain      reso:Property ;
  rdfs:label       "Ownership" ;
  rdfs:range       xsd:string ;
  reso:CertificationLevel "Silver" ;
  reso:PropertyTypes "RESI","RLSE","RINC","LAND","MOBI","FARM","COMS","COML","BUSO" ;
  schema:sameAs    <http://ddwiki.reso.org/display/DDW/Ownership+Field> ;
  vs:term_status   "stable"
.
reso:OwnershipType a rdf:Property ;
  rdfs:comment     "Current type of ownership of the business being sold.  i.e. Corporation, LLC, Sole P, Partnership, etc.," ;
  rdfs:domain      reso:Property ;
  rdfs:label       "OwnershipType" ;
  rdfs:range       enum:OwnershipType ;
  reso:CertificationLevel "Bronze" ;
  reso:PropertyTypes "BUSO" ;
  schema:sameAs    <http://ddwiki.reso.org/display/DDW/OwnershipType+Field> ;
  vs:term_status   "stable"
.
reso:ParcelNumber a rdf:Property ;
  rdfs:comment     "A number used to uniquely identify a parcel or lot.  This number is typically issued by the county or county assessor.  The AP number format varies from county to county.  It is recommended that all Parcel Numbers be transmitted without dashes or hyphens." ;
  rdfs:domain      reso:Property ;
  rdfs:label       "ParcelNumber" ;
  rdfs:range       xsd:string ;
  reso:CertificationLevel "Core" ;
  reso:PropertyTypes "RESI","RLSE","RINC","LAND","MOBI","FARM","COMS","COML" ;
  schema:sameAs    <http://ddwiki.reso.org/display/DDW/ParcelNumber+Field> ;
  vs:term_status   "stable"
.
reso:ParkManagerName a rdf:Property ;
  rdfs:comment     "Name of the manager of the mobile home park." ;
  rdfs:domain      reso:Property ;
  rdfs:label       "ParkManagerName" ;
  rdfs:range       xsd:string ;
  reso:CertificationLevel "Silver" ;
  reso:PropertyTypes "MOBI" ;
  schema:sameAs    <http://ddwiki.reso.org/display/DDW/ParkManagerName+Field> ;
  vs:term_status   "stable"
.
reso:ParkManagerPhone a rdf:Property ;
  rdfs:comment     "North American 10 digit phone numbers should be in the format of ###-###-#### (separated by hyphens).  Other conventions should use the common local standard.  International numbers should be preceded by a plus symbol." ;
  rdfs:domain      reso:Property ;
  rdfs:label       "ParkManagerPhone" ;
  rdfs:range       xsd:string ;
  reso:CertificationLevel "Silver" ;
  reso:PropertyTypes "MOBI" ;
  schema:sameAs    <http://ddwiki.reso.org/display/DDW/ParkManagerPhone+Field> ;
  vs:term_status   "stable"
.
reso:ParkName a rdf:Property ;
  rdfs:comment     "Name of the mobile home park or corporate/commercial park." ;
  rdfs:domain      reso:Property ;
  rdfs:label       "ParkName" ;
  rdfs:range       xsd:string ;
  reso:CertificationLevel "Silver" ;
  reso:PropertyTypes "MOBI","COMS","COML" ;
  schema:sameAs    <http://ddwiki.reso.org/display/DDW/ParkName+Field> ;
  vs:term_status   "stable"
.
reso:ParkingFeatures a rdf:Property ;
  rdfs:comment     "A list of features or description of the parking included in the sale/lease." ;
  rdfs:domain      reso:Property ;
  rdfs:label       "ParkingFeatures" ;
  rdfs:range       xsd:string ;
  reso:CertificationLevel "Platinum" ;
  reso:PropertyTypes "RESI","RLSE","RINC","MOBI","FARM" ;
  schema:sameAs    <http://ddwiki.reso.org/display/DDW/ParkingFeatures+Field> ;
  vs:term_status   "stable"
.
reso:ParkingTotal a rdf:Property ;
  rdfs:comment     "The total number of parking spaces included in the sale." ;
  rdfs:domain      reso:Property ;
  rdfs:label       "ParkingTotal" ;
  rdfs:range       xsd:decimal ;
  reso:CertificationLevel "Silver" ;
  reso:PropertyTypes "RESI","RLSE","RINC","MOBI","FARM","COMS","COML","BUSO" ;
  schema:sameAs    <http://ddwiki.reso.org/display/DDW/ParkingTotal+Field> ;
  vs:term_status   "stable"
.
reso:PastureArea a rdf:Property ;
  rdfs:comment     "Measurement or percentage of the property that has been allocated as pasture or grazing area." ;
  rdfs:domain      reso:Property ;
  rdfs:label       "PastureArea" ;
  rdfs:range       xsd:decimal ;
  reso:CertificationLevel "Gold" ;
  reso:PropertyTypes "FARM" ;
  schema:sameAs    <http://ddwiki.reso.org/display/DDW/PastureArea+Field> ;
  vs:term_status   "stable"
.
reso:PatioAndPorchFeatures a rdf:Property ;
  rdfs:comment     "A list of features or description of the patio or porch included in the sale/lease." ;
  rdfs:domain      reso:Property ;
  rdfs:label       "PatioAndPorchFeatures" ;
  rdfs:range       xsd:string ;
  reso:CertificationLevel "Platinum" ;
  reso:PropertyTypes "RESI","RLSE","RINC","MOBI","FARM" ;
  schema:sameAs    <http://ddwiki.reso.org/display/DDW/PatioAndPorchFeatures+Field> ;
  vs:term_status   "stable"
.
reso:PendingTimestamp a rdf:Property ;
  rdfs:comment     "The transactional timestamp automatically recorded by the MLS system representing the most recent date/time the listing's status was set to Pending." ;
  rdfs:domain      reso:Property ;
  rdfs:label       "PendingTimestamp" ;
  rdfs:range       xsd:dateTime ;
  reso:CertificationLevel "Bronze" ;
  reso:PropertyTypes "RESI","RLSE","RINC","LAND","MOBI","FARM","COMS","COML","BUSO" ;
  schema:sameAs    <http://ddwiki.reso.org/display/DDW/PendingTimestamp+Field> ;
  vs:term_status   "stable"
.
reso:PestControlExpense a rdf:Property ;
  rdfs:comment     "The annual expense that is not paid directly by the tenant and is included in the Operating Expense calculations." ;
  rdfs:domain      reso:Property ;
  rdfs:label       "PestControlExpense" ;
  rdfs:range       xsd:decimal ;
  reso:CertificationLevel "Silver" ;
  reso:PropertyTypes "RINC" ;
  schema:sameAs    <http://ddwiki.reso.org/display/DDW/PestControlExpense+Field> ;
  vs:term_status   "stable"
.
reso:PetsAllowed a rdf:Property ;
  rdfs:comment     "Are pets allowed at the property being leased?  A list of yes, no and more detailed restrictions/allowances." ;
  rdfs:domain      reso:Property ;
  rdfs:label       "PetsAllowed" ;
  rdfs:range       enum:PetsAllowed ;
  reso:CertificationLevel "Silver" ;
  reso:PropertyTypes "RLSE","MOBI" ;
  schema:sameAs    <http://ddwiki.reso.org/display/DDW/PetsAllowed+Field> ;
  vs:term_status   "stable"
.
reso:PhotosChangeTimestamp a rdf:Property ;
  rdfs:comment     "System generated timestamp of when the last update or change to the photos for this listing was made." ;
  rdfs:domain      reso:Property ;
  rdfs:label       "PhotosChangeTimestamp" ;
  rdfs:range       xsd:dateTime ;
  reso:CertificationLevel "Core" ;
  reso:PropertyTypes "RESI","RLSE","RINC","LAND","MOBI","FARM","COMS","COML","BUSO" ;
  schema:sameAs    <http://ddwiki.reso.org/display/DDW/PhotosChangeTimestamp+Field> ;
  vs:term_status   "stable"
.
reso:PhotosCount a rdf:Property ;
  rdfs:comment     "The total number of pictures or photos included with the listing." ;
  rdfs:domain      reso:Property ;
  rdfs:label       "PhotosCount" ;
  rdfs:range       xsd:decimal ;
  reso:CertificationLevel "Core" ;
  reso:PropertyTypes "RESI","RLSE","RINC","LAND","MOBI","FARM","COMS","COML","BUSO" ;
  schema:sameAs    <http://ddwiki.reso.org/display/DDW/PhotosCount+Field> ;
  vs:term_status   "stable"
.
reso:PoolExpense a rdf:Property ;
  rdfs:comment     "The annual expense that is not paid directly by the tenant and is included in the Operating Expense calculations." ;
  rdfs:domain      reso:Property ;
  rdfs:label       "PoolExpense" ;
  rdfs:range       xsd:decimal ;
  reso:CertificationLevel "Silver" ;
  reso:PropertyTypes "RINC" ;
  schema:sameAs    <http://ddwiki.reso.org/display/DDW/PoolExpense+Field> ;
  vs:term_status   "stable"
.
reso:PoolFeatures a rdf:Property ;
  rdfs:comment     "A list of features or description of the pool included in the sale/lease." ;
  rdfs:domain      reso:Property ;
  rdfs:label       "PoolFeatures" ;
  rdfs:range       xsd:string ;
  reso:CertificationLevel "Platinum" ;
  reso:PropertyTypes "RESI","RLSE","RINC","LAND","MOBI","FARM" ;
  schema:sameAs    <http://ddwiki.reso.org/display/DDW/PoolFeatures+Field> ;
  vs:term_status   "stable"
.
reso:PoolPrivateYN a rdf:Property ;
  rdfs:comment     "The property has a privately owned pool that is included in the sale/lease." ;
  rdfs:domain      reso:Property ;
  rdfs:label       "PoolPrivateYN" ;
  rdfs:range       xsd:boolean ;
  reso:CertificationLevel "Platinum" ;
  reso:PropertyTypes "RESI","RLSE","RINC","LAND","MOBI","FARM" ;
  schema:sameAs    <http://ddwiki.reso.org/display/DDW/PoolPrivateYN+Field> ;
  vs:term_status   "stable"
.
reso:Possession a rdf:Property ;
  rdfs:comment     "A list defining when possession will occur.  i.e. COE, COE+1, etc." ;
  rdfs:domain      reso:Property ;
  rdfs:label       "Possession" ;
  rdfs:range       enum:Possession ;
  reso:CertificationLevel "Bronze" ;
  reso:PropertyTypes "RESI","RLSE","RINC","LAND","MOBI","FARM","COMS","COML","BUSO" ;
  schema:sameAs    <http://ddwiki.reso.org/display/DDW/Possession+Field> ;
  vs:term_status   "stable"
.
reso:PossibleUse a rdf:Property ;
  rdfs:comment     "A list of the type(s) of possible or best uses of the property.  Probable use gives a good indication of what the best use or potential use of the property could be.i.e. Primary, Vacation, Investment, Rental, Retirement" ;
  rdfs:domain      reso:Property ;
  rdfs:label       "PossibleUse" ;
  rdfs:range       xsd:string ;
  reso:CertificationLevel "Gold" ;
  reso:PropertyTypes "LAND" ;
  schema:sameAs    <http://ddwiki.reso.org/display/DDW/PossibleUse+Field> ;
  vs:term_status   "stable"
.
reso:PostalCity a rdf:Property ;
  rdfs:comment     "The official city per the USPS.  May be different from the \"City\"." ;
  rdfs:domain      reso:Property ;
  rdfs:label       "PostalCity" ;
  rdfs:range       xsd:string ;
  reso:CertificationLevel "Core" ;
  reso:PropertyTypes "RESI","RLSE","RINC","LAND","MOBI","FARM","COMS","COML","BUSO" ;
  schema:sameAs    <http://ddwiki.reso.org/display/DDW/PostalCity+Field> ;
  vs:term_status   "stable"
.
reso:PostalCode a rdf:Property ;
  rdfs:comment     "The postal code portion of a street or mailing address." ;
  rdfs:domain      reso:Property ;
  rdfs:label       "PostalCode" ;
  rdfs:range       xsd:string ;
  reso:CertificationLevel "Core" ;
  reso:PropertyTypes "RESI","RLSE","RINC","LAND","MOBI","FARM","COMS","COML","BUSO" ;
  schema:sameAs    <http://ddwiki.reso.org/display/DDW/PostalCode+Field> ;
  vs:term_status   "stable"
.
reso:PostalCodePlus4 a rdf:Property ;
  rdfs:comment     "The postal code +4 portion of a street or mailing address." ;
  rdfs:domain      reso:Property ;
  rdfs:label       "PostalCodePlus4" ;
  rdfs:range       xsd:string ;
  reso:CertificationLevel "Core" ;
  reso:PropertyTypes "RESI","RLSE","RINC","LAND","MOBI","FARM","COMS","COML","BUSO" ;
  schema:sameAs    <http://ddwiki.reso.org/display/DDW/PostalCodePlus4+Field> ;
  vs:term_status   "stable"
.
reso:PowerProductionType a rdf:Property ;
  rdfs:domain      reso:Property ;
  rdfs:label       "PowerProductionType" ;
  rdfs:range       enum:PowerProductionType ;
  reso:CertificationLevel "Silver" ;
  reso:PropertyTypes "RESI","RLSE","RINC","LAND","MOBI","FARM","COMS","COML" ;
  schema:sameAs    <http://ddwiki.reso.org/display/DDW/PowerProductionType+Field> ;
  vs:term_status   "stable"
.
reso:PowerProduction a rdf:Property ;
  rdfs:comment     "The most important metric of a renewables system is the amount of power it produces per year.  This number can be actual or estimated. Annual production for systems producing electricity like wind or solar are measured in kilowatt hours (kWh) per year.  A kWh is like a measure of the distance traveled per hour for a car &#x2013; how far did it go over a certain period of time. Annual production is influenced by the size of the system, the conditions (How shady are the trees? How many cloudy days?, and the installation.  Sellers typically have access to software that provides historical production totals." ;
  rdfs:domain      reso:Property ;
  rdfs:label       "PowerProduction" ;
  rdfs:range       xsd:decimal ;
  reso:CertificationLevel "Silver" ;
  reso:PropertyTypes "RESI","RLSE","RINC","LAND","MOBI","FARM","COMS","COML" ;
  schema:sameAs    <http://ddwiki.reso.org/display/DDW/PowerProduction%5BType%5D+Annual+Field> ;
  vs:term_status   "stable"
.
reso:PowerProduction a rdf:Property ;
  rdfs:comment     "The most important metric of a renewables system is the amount of power it produces per year.  This number can be actual or estimated. Annual production for systems producing electricity like wind or solar are measured in kilowatt hours (kWh) per year.  A kWh is like a measure of the distance traveled per hour for a car &#x2013; how far did it go over a certain period of time. Annual production is influenced by the size of the system, the conditions (How shady are the trees? How many cloudy days?, and the installation.  Sellers typically have access to software that provides historical production totals.","The most important metric of a renewables system is the amount of power it produces per year.  This number can be actual or estimated, or a combination if less than 12 months of actual data is available (any missing months of actual data is extrapolated).  This field allows the status of the number shown in the PowerProducationAnnual[Type] to be clarified." ;
  rdfs:domain      reso:Property ;
  rdfs:label       "PowerProduction" ;
  rdfs:range       xsd:decimal,enum:PowerProductionAnnualStatus ;
  reso:CertificationLevel "Silver" ;
  reso:PropertyTypes "RESI","RLSE","RINC","LAND","MOBI","FARM","COMS","COML" ;
  schema:sameAs    <http://ddwiki.reso.org/display/DDW/PowerProduction%5BType%5D+Annual+Field>,<http://ddwiki.reso.org/display/DDW/PowerProduction%5BType%5DAnnualStatus++Field> ;
  vs:term_status   "stable"
.
reso:PowerProduction a rdf:Property ;
  rdfs:comment     "The most important metric of a renewables system is the amount of power it produces per year.  This number can be actual or estimated. Annual production for systems producing electricity like wind or solar are measured in kilowatt hours (kWh) per year.  A kWh is like a measure of the distance traveled per hour for a car &#x2013; how far did it go over a certain period of time. Annual production is influenced by the size of the system, the conditions (How shady are the trees? How many cloudy days?, and the installation.  Sellers typically have access to software that provides historical production totals.","The most important metric of a renewables system is the amount of power it produces per year.  This number can be actual or estimated, or a combination if less than 12 months of actual data is available (any missing months of actual data is extrapolated).  This field allows the status of the number shown in the PowerProducationAnnual[Type] to be clarified.","The &#x201c;capacity&#x201d; of a renewables system. Size is measured in kilowatts (kW) DC (referring to direct current).  A kW indicates how much power the system can produce under standard conditions, like the size of a car engine. Renewables systems are sized when they are installed to cover all or a portion of the power needs of the property. Therefore, a system designed to produce 50% of the power needs will be sized smaller than a system on the exact same property designed to produce 100%. Size may be influenced by available space at the property, orientation, landscaping, etc." ;
  rdfs:domain      reso:Property ;
  rdfs:label       "PowerProduction" ;
  rdfs:range       xsd:decimal,enum:PowerProductionAnnualStatus ;
  reso:CertificationLevel "Silver" ;
  reso:PropertyTypes "RESI","RLSE","RINC","LAND","MOBI","FARM","COMS","COML" ;
  schema:sameAs    <http://ddwiki.reso.org/display/DDW/PowerProduction%5BType%5D+Annual+Field>,<http://ddwiki.reso.org/display/DDW/PowerProduction%5BType%5DAnnualStatus++Field>,<http://ddwiki.reso.org/display/DDW/PowerProduction%5BType%5DSize+Field> ;
  vs:term_status   "stable"
.
reso:PowerProduction a rdf:Property ;
  rdfs:comment     "The most important metric of a renewables system is the amount of power it produces per year.  This number can be actual or estimated. Annual production for systems producing electricity like wind or solar are measured in kilowatt hours (kWh) per year.  A kWh is like a measure of the distance traveled per hour for a car &#x2013; how far did it go over a certain period of time. Annual production is influenced by the size of the system, the conditions (How shady are the trees? How many cloudy days?, and the installation.  Sellers typically have access to software that provides historical production totals.","The most important metric of a renewables system is the amount of power it produces per year.  This number can be actual or estimated, or a combination if less than 12 months of actual data is available (any missing months of actual data is extrapolated).  This field allows the status of the number shown in the PowerProducationAnnual[Type] to be clarified.","The &#x201c;capacity&#x201d; of a renewables system. Size is measured in kilowatts (kW) DC (referring to direct current).  A kW indicates how much power the system can produce under standard conditions, like the size of a car engine. Renewables systems are sized when they are installed to cover all or a portion of the power needs of the property. Therefore, a system designed to produce 50% of the power needs will be sized smaller than a system on the exact same property designed to produce 100%. Size may be influenced by available space at the property, orientation, landscaping, etc.","The year a renewables system was installed.  Ideally this should be the year the system was interconnected with the grid and began producing power.  Renewables systems have a limited lifespan and year installed helps buyers and appraisers determine remaining useful life of the system." ;
  rdfs:domain      reso:Property ;
  rdfs:label       "PowerProduction" ;
  rdfs:range       xsd:decimal,enum:PowerProductionAnnualStatus ;
  reso:CertificationLevel "Silver" ;
  reso:PropertyTypes "RESI","RLSE","RINC","LAND","MOBI","FARM","COMS","COML" ;
  schema:sameAs    <http://ddwiki.reso.org/display/DDW/PowerProduction%5BType%5D+Annual+Field>,<http://ddwiki.reso.org/display/DDW/PowerProduction%5BType%5DAnnualStatus++Field>,<http://ddwiki.reso.org/display/DDW/PowerProduction%5BType%5DSize+Field>,<http://ddwiki.reso.org/display/DDW/PowerProduction%5BType%5DYearInstall+Field> ;
  vs:term_status   "stable"
.
reso:PreviousListPrice a rdf:Property ;
  rdfs:comment     "The most recent previous ListPrice of the listing." ;
  rdfs:domain      reso:Property ;
  rdfs:label       "PreviousListPrice" ;
  rdfs:range       xsd:decimal ;
  reso:CertificationLevel "Bronze" ;
  reso:PropertyTypes "RESI","RLSE","RINC","LAND","MOBI","FARM","COMS","COML","BUSO" ;
  schema:sameAs    <http://ddwiki.reso.org/display/DDW/PreviousListPrice+Field> ;
  vs:term_status   "stable"
.
reso:PriceChangeTimestamp a rdf:Property ;
  rdfs:comment     "The transactional timestamp automatically recorded by the MLS system representing the date/time the listing's price was last changed." ;
  rdfs:domain      reso:Property ;
  rdfs:label       "PriceChangeTimestamp" ;
  rdfs:range       xsd:dateTime ;
  reso:CertificationLevel "Bronze" ;
  reso:PropertyTypes "RESI","RLSE","RINC","LAND","MOBI","FARM","COMS","COML","BUSO" ;
  schema:sameAs    <http://ddwiki.reso.org/display/DDW/PriceChangeTimestamp+Field> ;
  vs:term_status   "stable"
.
reso:PrivateOfficeRemarks a rdf:Property ;
  rdfs:comment     "A remarks field that is only visible to members of the same offices as the listing agent." ;
  rdfs:domain      reso:Property ;
  rdfs:label       "PrivateOfficeRemarks" ;
  rdfs:range       xsd:string ;
  reso:CertificationLevel "Bronze" ;
  reso:PropertyTypes "RESI","RLSE","RINC","LAND","MOBI","FARM","COMS","COML","BUSO" ;
  schema:sameAs    <http://ddwiki.reso.org/display/DDW/PrivateOfficeRemarks+Field> ;
  vs:term_status   "stable"
.
reso:PrivateRemarks a rdf:Property ;
  rdfs:comment     "Remarks that may contain security or proprietary information and should be restricted from public view." ;
  rdfs:domain      reso:Property ;
  rdfs:label       "PrivateRemarks" ;
  rdfs:range       xsd:string ;
  reso:CertificationLevel "Core" ;
  reso:PropertyTypes "RESI","RLSE","RINC","LAND","MOBI","FARM","COMS","COML","BUSO" ;
  schema:sameAs    <http://ddwiki.reso.org/display/DDW/PrivateRemarks+Field> ;
  vs:term_status   "stable"
.
reso:ProfessionalManagementExpense a rdf:Property ;
  rdfs:comment     "The annual expense that is not paid directly by the tenant and is included in the Operating Expense calculations.  This is for a management company.  Use ManagerExpense for a individual manager." ;
  rdfs:domain      reso:Property ;
  rdfs:label       "ProfessionalManagementExpense" ;
  rdfs:range       xsd:decimal ;
  reso:CertificationLevel "Silver" ;
  reso:PropertyTypes "RINC","COMS","COML" ;
  schema:sameAs    <http://ddwiki.reso.org/display/DDW/ProfessionalManagementExpense+Field> ;
  vs:term_status   "stable"
.
reso:PropertyAttachedYN a rdf:Property ;
  rdfs:comment     "A flag indicating that the primary structure is attached to another structure that is not included in the sale.  i.e. one unit of a duplex. This flag may be T/F, Y/N or a list of attached or detached. As with all flags, the field may be null.  In some systems this information may be part of the Property Sub Type." ;
  rdfs:domain      reso:Property ;
  rdfs:label       "PropertyAttachedYN" ;
  rdfs:range       xsd:boolean ;
  reso:CertificationLevel "Core" ;
  reso:PropertyTypes "RESI","RLSE","RINC","MOBI","FARM" ;
  schema:sameAs    <http://ddwiki.reso.org/display/DDW/PropertyAttachedYN+Field> ;
  vs:term_status   "stable"
.
reso:PropertyCondition a rdf:Property ;
  rdfs:comment     "A list describing the condition of the property and any structures included in the sale." ;
  rdfs:domain      reso:Property ;
  rdfs:label       "PropertyCondition" ;
  rdfs:range       enum:PropertyCondition ;
  reso:CertificationLevel "Silver" ;
  reso:PropertyTypes "RESI","RLSE","RINC","MOBI","FARM" ;
  schema:sameAs    <http://ddwiki.reso.org/display/DDW/PropertyCondition+Field> ;
  vs:term_status   "stable"
.
reso:PropertySubType a rdf:Property ;
  rdfs:comment     "A list of types of residential and residential lease properties, i.e. SFR, Condo, etc. Or a list of Sub Types for Mobile, such as Expando, Manufactured, Modular, etc." ;
  rdfs:domain      reso:Property ;
  rdfs:label       "PropertySubType" ;
  rdfs:range       enum:PropertySubType ;
  reso:CertificationLevel "Core" ;
  reso:PropertyTypes "RESI","RLSE","MOBI","COMS","COML","BUSO" ;
  schema:sameAs    <http://ddwiki.reso.org/display/DDW/PropertySubType+Field> ;
  vs:term_status   "stable"
.
reso:PropertyType a rdf:Property ;
  rdfs:comment     "A list of types of properties such as Residential, Lease, Income, Land, Mobile, Commercial Sale, etc..." ;
  rdfs:domain      reso:Property ;
  rdfs:label       "PropertyType" ;
  rdfs:range       enum:PropertyType ;
  reso:CertificationLevel "Core" ;
  reso:PropertyTypes "RESI","RLSE","RINC","LAND","MOBI","FARM","COMS","COML","BUSO" ;
  schema:sameAs    <http://ddwiki.reso.org/display/DDW/PropertyType+Field> ;
  vs:term_status   "stable"
.
reso:PublicRemarks a rdf:Property ;
  rdfs:domain      reso:Property ;
  rdfs:label       "PublicRemarks" ;
  rdfs:range       xsd:string ;
  reso:CertificationLevel "Core" ;
  reso:PropertyTypes "RESI","RLSE","RINC","LAND","MOBI","FARM","COMS","COML","BUSO" ;
  schema:sameAs    <http://ddwiki.reso.org/display/DDW/PublicRemarks+Field> ;
  vs:term_status   "stable"
.
reso:PublicSurveyRange a rdf:Property ;
  rdfs:comment     "This field specifically identifies the Range identified by the Public Land Survey System (PLSS)." ;
  rdfs:domain      reso:Property ;
  rdfs:label       "PublicSurveyRange" ;
  rdfs:range       xsd:string ;
  reso:CertificationLevel "Gold" ;
  reso:PropertyTypes "RESI","RLSE","RINC","LAND","MOBI","FARM" ;
  schema:sameAs    <http://ddwiki.reso.org/display/DDW/PublicSurveyRange+Field> ;
  vs:term_status   "stable"
.
reso:PublicSurveySection a rdf:Property ;
  rdfs:comment     "This field specifically identifies the Section identified by the Public Land Survey System (PLSS)." ;
  rdfs:domain      reso:Property ;
  rdfs:label       "PublicSurveySection" ;
  rdfs:range       xsd:string ;
  reso:CertificationLevel "Gold" ;
  reso:PropertyTypes "RESI","RLSE","RINC","LAND","MOBI","FARM" ;
  schema:sameAs    <http://ddwiki.reso.org/display/DDW/PublicSurveySection+Field> ;
  vs:term_status   "stable"
.
reso:PublicSurveyTownship a rdf:Property ;
  rdfs:comment     "This field specifically identifies the Township identified by the Public Land Survey System (PLSS)." ;
  rdfs:domain      reso:Property ;
  rdfs:label       "PublicSurveyTownship" ;
  rdfs:range       xsd:string ;
  reso:CertificationLevel "Gold" ;
  reso:PropertyTypes "RESI","RLSE","RINC","LAND","MOBI","FARM" ;
  schema:sameAs    <http://ddwiki.reso.org/display/DDW/PublicSurveyTownship+Field> ;
  vs:term_status   "stable"
.
reso:PurchaseContractDate a rdf:Property ;
  rdfs:comment     "With for-sale listings, the date an offer was accepted and the listing was no longer on market.  This is the date entered by the agent reflecting when the change occurred contractually, not a timestamp of when the change was made in the MLS.  With lease listings this may represent a meeting of the minds to lease, but some contractual requirements are yet to be fulfilled, such as contract signing or receipt of the deposit." ;
  rdfs:domain      reso:Property ;
  rdfs:label       "PurchaseContractDate" ;
  rdfs:range       xsd:date ;
  reso:CertificationLevel "Core" ;
  reso:PropertyTypes "RESI","RLSE","RINC","LAND","MOBI","FARM","COMS","COML","BUSO" ;
  schema:sameAs    <http://ddwiki.reso.org/display/DDW/PurchaseContractDate+Field> ;
  vs:term_status   "stable"
.
reso:RVParkingDimensions a rdf:Property ;
  rdfs:comment     "The dimensions of the RV parking area minimally represented as length and width (i.e. 25 x 18) or a measurement of all sides of the polygon representing the usable RV parking space.  i.e. 33 x 15 x 12 x 60." ;
  rdfs:domain      reso:Property ;
  rdfs:label       "RVParkingDimensions" ;
  rdfs:range       xsd:string ;
  reso:CertificationLevel "Silver" ;
  reso:PropertyTypes "RESI","RLSE","RINC","MOBI","FARM" ;
  schema:sameAs    <http://ddwiki.reso.org/display/DDW/RVParkingDimensions+Field> ;
  vs:term_status   "stable"
.
reso:RangeArea a rdf:Property ;
  rdfs:comment     "Measurement or percentage of the property that has been allocated as range." ;
  rdfs:domain      reso:Property ;
  rdfs:label       "RangeArea" ;
  rdfs:range       xsd:decimal ;
  reso:CertificationLevel "Gold" ;
  reso:PropertyTypes "FARM" ;
  schema:sameAs    <http://ddwiki.reso.org/display/DDW/RangeArea+Field> ;
  vs:term_status   "stable"
.
reso:RentControlYN a rdf:Property ;
  rdfs:comment     "Is the property in a rent control area?" ;
  rdfs:domain      reso:Property ;
  rdfs:label       "RentControlYN" ;
  rdfs:range       xsd:boolean ;
  reso:CertificationLevel "Bronze" ;
  reso:PropertyTypes "RINC","COMS","COML" ;
  schema:sameAs    <http://ddwiki.reso.org/display/DDW/RentControlYN+Field> ;
  vs:term_status   "stable"
.
reso:RentIncludes a rdf:Property ;
  rdfs:comment     "A list of services or items that the tenant is not responsible to pay." ;
  rdfs:domain      reso:Property ;
  rdfs:label       "RentIncludes" ;
  rdfs:range       enum:RentIncludes ;
  reso:CertificationLevel "Bronze" ;
  reso:PropertyTypes "RLSE","MOBI" ;
  schema:sameAs    <http://ddwiki.reso.org/display/DDW/RentIncludes+Field> ;
  vs:term_status   "stable"
.
reso:RoadFrontageType a rdf:Property ;
  rdfs:comment     "Pick list of types of Road frontage.  i.e. Freeway frontage, No Road Frontage, etc. The road frontage of the property is an important factor in determining value of the property and it&#x2019;s appropriateness for intended use." ;
  rdfs:domain      reso:Property ;
  rdfs:label       "RoadFrontageType" ;
  rdfs:range       xsd:string ;
  reso:CertificationLevel "Gold" ;
  reso:PropertyTypes "RESI","RLSE","RINC","LAND","MOBI","FARM" ;
  schema:sameAs    <http://ddwiki.reso.org/display/DDW/RoadFrontageType+Field> ;
  vs:term_status   "stable"
.
reso:RoadResponsibility a rdf:Property ;
  rdfs:comment     "The person or entity responsible for road maintenance (e.g., City, County, Private)." ;
  rdfs:domain      reso:Property ;
  rdfs:label       "RoadResponsibility" ;
  rdfs:range       xsd:string ;
  reso:CertificationLevel "Gold" ;
  reso:PropertyTypes "RESI","RLSE","RINC","LAND","MOBI","FARM" ;
  schema:sameAs    <http://ddwiki.reso.org/display/DDW/RoadResponsibility+Field> ;
  vs:term_status   "stable"
.
reso:RoadSurfaceType a rdf:Property ;
  rdfs:comment     "Pick list of types of surface of the Road to access the property.  The surface of the road(s) for access to the property is an important factor in determining value of the property and it&#x2019;s appropriateness for intended use." ;
  rdfs:domain      reso:Property ;
  rdfs:label       "RoadSurfaceType" ;
  rdfs:range       xsd:string ;
  reso:CertificationLevel "Gold" ;
  reso:PropertyTypes "RESI","RLSE","RINC","LAND","MOBI","FARM" ;
  schema:sameAs    <http://ddwiki.reso.org/display/DDW/RoadSurfaceType+Field> ;
  vs:term_status   "stable"
.
reso:Roof a rdf:Property ;
  rdfs:comment     "A list describing the type or style of roof.  For example Spanish Tile, Composite, Shake, etc." ;
  rdfs:domain      reso:Property ;
  rdfs:label       "Roof" ;
  rdfs:range       enum:Roof ;
  reso:CertificationLevel "Silver" ;
  reso:PropertyTypes "RESI","RLSE","RINC","MOBI","FARM","COMS","COML" ;
  schema:sameAs    <http://ddwiki.reso.org/display/DDW/Roof+Field> ;
  vs:term_status   "stable"
.
reso:RoomType a rdf:Property ;
  rdfs:comment     "This field is a list of the types used in the rooms repeating elements.  The Type is a list of possible room types.  i.e. Bedroom, Bathroom, Living Room, Workshop, etc.  Each selected are expected to appear as the \"[type]\" in the related rooms fields in a flattened implementation (RETS 1.x only) of the room fields.  A relational implementation of rooms must omit the type from the field name and use RoomType to create a vertical representation of the various rooms.  **Note that Garage or Basement should not be added as a room type and are represented by the ParkingFeatures and Basement fields respectively." ;
  rdfs:domain      reso:Property ;
  rdfs:label       "RoomType" ;
  rdfs:range       enum:RoomType ;
  reso:CertificationLevel "Gold" ;
  reso:PropertyTypes "RESI","RLSE","MOBI","FARM" ;
  schema:sameAs    <http://ddwiki.reso.org/display/DDW/RoomType+Field> ;
  vs:term_status   "stable"
.
reso:Room a rdf:Property ;
  rdfs:comment     "[type] This field is a repeating element for each type of room selected in the RoomType field.  For every RoomType there are two possible implementations.  For a flat implementation (RETS 1.x only), each RoomType used is expected to appear as the \"[type]\" in the related rooms field name.  i.e. RoomKitchenArea.  A relational implementation of rooms must omit the type from the field name and use RoomType to create a vertical representation of the various rooms.  i.e. RoomArea with Kitchen in the relational table's RoomType field." ;
  rdfs:domain      reso:Property ;
  rdfs:label       "Room" ;
  rdfs:range       xsd:decimal ;
  reso:CertificationLevel "Gold" ;
  reso:PropertyTypes "RESI","RLSE","MOBI","FARM" ;
  schema:sameAs    <http://ddwiki.reso.org/display/DDW/Room%5Btype%5DArea+Field> ;
  vs:term_status   "stable"
.
reso:Room a rdf:Property ;
  rdfs:comment     "[type] This field is a repeating element for each type of room selected in the RoomType field.  For every RoomType there are two possible implementations.  For a flat implementation (RETS 1.x only), each RoomType used is expected to appear as the \"[type]\" in the related rooms field name.  i.e. RoomKitchenArea.  A relational implementation of rooms must omit the type from the field name and use RoomType to create a vertical representation of the various rooms.  i.e. RoomArea with Kitchen in the relational table's RoomType field.","[type] This field is a repeating element for each type of room selected in the RoomType field.  For every RoomType there are two possible implementations.  For a flat implementation (RETS 1.x only), each RoomType used is expected to appear as the \"[type]\" in the related rooms field name.  i.e. RoomKitchenAreaSource.  A relational implementation of rooms must omit the type from the field name and use RoomType to create a vertical representation of the various rooms.  i.e. RoomAreaSource." ;
  rdfs:domain      reso:Property ;
  rdfs:label       "Room" ;
  rdfs:range       xsd:decimal,enum:AreaSource ;
  reso:CertificationLevel "Gold" ;
  reso:PropertyTypes "RESI","RLSE","MOBI","FARM" ;
  schema:sameAs    <http://ddwiki.reso.org/display/DDW/Room%5Btype%5DArea+Field>,<http://ddwiki.reso.org/display/DDW/Room%5Btype%5DAreaSource+Field> ;
  vs:term_status   "stable"
.
reso:Room a rdf:Property ;
  rdfs:comment     "[type] This field is a repeating element for each type of room selected in the RoomType field.  For every RoomType there are two possible implementations.  For a flat implementation (RETS 1.x only), each RoomType used is expected to appear as the \"[type]\" in the related rooms field name.  i.e. RoomKitchenArea.  A relational implementation of rooms must omit the type from the field name and use RoomType to create a vertical representation of the various rooms.  i.e. RoomArea with Kitchen in the relational table's RoomType field.","[type] This field is a repeating element for each type of room selected in the RoomType field.  For every RoomType there are two possible implementations.  For a flat implementation (RETS 1.x only), each RoomType used is expected to appear as the \"[type]\" in the related rooms field name.  i.e. RoomKitchenAreaSource.  A relational implementation of rooms must omit the type from the field name and use RoomType to create a vertical representation of the various rooms.  i.e. RoomAreaSource.","[type] This field is a repeating element for each type of room selected in the RoomType field.  For every RoomType there are two possible implementations.  For a flat implementation (RETS 1.x only), each RoomType used is expected to appear as the \"[type]\" in the related rooms field name.  i.e. RoomKitchenAreaUnits.  A relational implementation of rooms must omit the type from the field name and use RoomType to create a vertical representation of the various rooms.  i.e. RoomAreaUnits with Kitchen in the relational table's RoomType field." ;
  rdfs:domain      reso:Property ;
  rdfs:label       "Room" ;
  rdfs:range       xsd:decimal,enum:AreaSource,enum:AreaUnits ;
  reso:CertificationLevel "Gold" ;
  reso:PropertyTypes "RESI","RLSE","MOBI","FARM" ;
  schema:sameAs    <http://ddwiki.reso.org/display/DDW/Room%5Btype%5DArea+Field>,<http://ddwiki.reso.org/display/DDW/Room%5Btype%5DAreaSource+Field>,<http://ddwiki.reso.org/display/DDW/Room%5Btype%5DAreaUnits+Field> ;
  vs:term_status   "stable"
.
reso:Room a rdf:Property ;
  rdfs:comment     "[type] This field is a repeating element for each type of room selected in the RoomType field.  For every RoomType there are two possible implementations.  For a flat implementation (RETS 1.x only), each RoomType used is expected to appear as the \"[type]\" in the related rooms field name.  i.e. RoomKitchenArea.  A relational implementation of rooms must omit the type from the field name and use RoomType to create a vertical representation of the various rooms.  i.e. RoomArea with Kitchen in the relational table's RoomType field.","[type] This field is a repeating element for each type of room selected in the RoomType field.  For every RoomType there are two possible implementations.  For a flat implementation (RETS 1.x only), each RoomType used is expected to appear as the \"[type]\" in the related rooms field name.  i.e. RoomKitchenAreaSource.  A relational implementation of rooms must omit the type from the field name and use RoomType to create a vertical representation of the various rooms.  i.e. RoomAreaSource.","[type] This field is a repeating element for each type of room selected in the RoomType field.  For every RoomType there are two possible implementations.  For a flat implementation (RETS 1.x only), each RoomType used is expected to appear as the \"[type]\" in the related rooms field name.  i.e. RoomKitchenAreaUnits.  A relational implementation of rooms must omit the type from the field name and use RoomType to create a vertical representation of the various rooms.  i.e. RoomAreaUnits with Kitchen in the relational table's RoomType field.","[type] This field is a repeating element for each type of room selected in the RoomType field.  For every RoomType there are two possible implementations.  For a flat implementation (RETS 1.x only), each RoomType used is expected to appear as the \"[type]\" in the related rooms field name.  i.e. RoomKitchenDescription.  A relational implementation of rooms must omit the type from the field name and use RoomType to create a vertical representation of the various rooms.  i.e. RoomDescription with Kitchen in the relational table's RoomType field." ;
  rdfs:domain      reso:Property ;
  rdfs:label       "Room" ;
  rdfs:range       xsd:decimal,enum:AreaSource,enum:AreaUnits,xsd:string ;
  reso:CertificationLevel "Gold" ;
  reso:PropertyTypes "RESI","RLSE","MOBI","FARM" ;
  schema:sameAs    <http://ddwiki.reso.org/display/DDW/Room%5Btype%5DArea+Field>,<http://ddwiki.reso.org/display/DDW/Room%5Btype%5DAreaSource+Field>,<http://ddwiki.reso.org/display/DDW/Room%5Btype%5DAreaUnits+Field>,<http://ddwiki.reso.org/display/DDW/Room%5Btype%5DDescription+Field> ;
  vs:term_status   "stable"
.
reso:Room a rdf:Property ;
  rdfs:comment     "[type] This field is a repeating element for each type of room selected in the RoomType field.  For every RoomType there are two possible implementations.  For a flat implementation (RETS 1.x only), each RoomType used is expected to appear as the \"[type]\" in the related rooms field name.  i.e. RoomKitchenArea.  A relational implementation of rooms must omit the type from the field name and use RoomType to create a vertical representation of the various rooms.  i.e. RoomArea with Kitchen in the relational table's RoomType field.","[type] This field is a repeating element for each type of room selected in the RoomType field.  For every RoomType there are two possible implementations.  For a flat implementation (RETS 1.x only), each RoomType used is expected to appear as the \"[type]\" in the related rooms field name.  i.e. RoomKitchenAreaSource.  A relational implementation of rooms must omit the type from the field name and use RoomType to create a vertical representation of the various rooms.  i.e. RoomAreaSource.","[type] This field is a repeating element for each type of room selected in the RoomType field.  For every RoomType there are two possible implementations.  For a flat implementation (RETS 1.x only), each RoomType used is expected to appear as the \"[type]\" in the related rooms field name.  i.e. RoomKitchenAreaUnits.  A relational implementation of rooms must omit the type from the field name and use RoomType to create a vertical representation of the various rooms.  i.e. RoomAreaUnits with Kitchen in the relational table's RoomType field.","[type] This field is a repeating element for each type of room selected in the RoomType field.  For every RoomType there are two possible implementations.  For a flat implementation (RETS 1.x only), each RoomType used is expected to appear as the \"[type]\" in the related rooms field name.  i.e. RoomKitchenDescription.  A relational implementation of rooms must omit the type from the field name and use RoomType to create a vertical representation of the various rooms.  i.e. RoomDescription with Kitchen in the relational table's RoomType field.","[type] This field is a repeating element for each type of room selected in the RoomType field.  For every RoomType there are two possible implementations.  For a flat implementation (RETS 1.x only), each RoomType used is expected to appear as the \"[type]\" in the related rooms field name.  i.e. RoomKitchenDimensions.  A relational implementation of rooms must omit the type from the field name and use RoomType to create a vertical representation of the various rooms.  i.e. RoomDimensions with Kitchen in the relational table's RoomType field." ;
  rdfs:domain      reso:Property ;
  rdfs:label       "Room" ;
  rdfs:range       xsd:decimal,enum:AreaSource,enum:AreaUnits,xsd:string ;
  reso:CertificationLevel "Gold" ;
  reso:PropertyTypes "RESI","RLSE","MOBI","FARM" ;
  schema:sameAs    <http://ddwiki.reso.org/display/DDW/Room%5Btype%5DArea+Field>,<http://ddwiki.reso.org/display/DDW/Room%5Btype%5DAreaSource+Field>,<http://ddwiki.reso.org/display/DDW/Room%5Btype%5DAreaUnits+Field>,<http://ddwiki.reso.org/display/DDW/Room%5Btype%5DDescription+Field>,<http://ddwiki.reso.org/display/DDW/Room%5Btype%5DDimensions+Field> ;
  vs:term_status   "stable"
.
reso:Room a rdf:Property ;
  rdfs:comment     "[type] This field is a repeating element for each type of room selected in the RoomType field.  For every RoomType there are two possible implementations.  For a flat implementation (RETS 1.x only), each RoomType used is expected to appear as the \"[type]\" in the related rooms field name.  i.e. RoomKitchenArea.  A relational implementation of rooms must omit the type from the field name and use RoomType to create a vertical representation of the various rooms.  i.e. RoomArea with Kitchen in the relational table's RoomType field.","[type] This field is a repeating element for each type of room selected in the RoomType field.  For every RoomType there are two possible implementations.  For a flat implementation (RETS 1.x only), each RoomType used is expected to appear as the \"[type]\" in the related rooms field name.  i.e. RoomKitchenAreaSource.  A relational implementation of rooms must omit the type from the field name and use RoomType to create a vertical representation of the various rooms.  i.e. RoomAreaSource.","[type] This field is a repeating element for each type of room selected in the RoomType field.  For every RoomType there are two possible implementations.  For a flat implementation (RETS 1.x only), each RoomType used is expected to appear as the \"[type]\" in the related rooms field name.  i.e. RoomKitchenAreaUnits.  A relational implementation of rooms must omit the type from the field name and use RoomType to create a vertical representation of the various rooms.  i.e. RoomAreaUnits with Kitchen in the relational table's RoomType field.","[type] This field is a repeating element for each type of room selected in the RoomType field.  For every RoomType there are two possible implementations.  For a flat implementation (RETS 1.x only), each RoomType used is expected to appear as the \"[type]\" in the related rooms field name.  i.e. RoomKitchenDescription.  A relational implementation of rooms must omit the type from the field name and use RoomType to create a vertical representation of the various rooms.  i.e. RoomDescription with Kitchen in the relational table's RoomType field.","[type] This field is a repeating element for each type of room selected in the RoomType field.  For every RoomType there are two possible implementations.  For a flat implementation (RETS 1.x only), each RoomType used is expected to appear as the \"[type]\" in the related rooms field name.  i.e. RoomKitchenDimensions.  A relational implementation of rooms must omit the type from the field name and use RoomType to create a vertical representation of the various rooms.  i.e. RoomDimensions with Kitchen in the relational table's RoomType field.","[type] This field is a repeating element for each type of room selected in the RoomType field.  For every RoomType there are two possible implementations.  For a flat implementation (RETS 1.x only), each RoomType used is expected to appear as the \"[type]\" in the related rooms field name.  i.e. RoomKitchenFeatures.  A relational implementation of rooms must omit the type from the field name and use RoomType to create a vertical representation of the various rooms.  i.e. RoomFeatures with Kitchen in the relational table's RoomType field." ;
  rdfs:domain      reso:Property ;
  rdfs:label       "Room" ;
  rdfs:range       xsd:decimal,enum:AreaSource,enum:AreaUnits,xsd:string ;
  reso:CertificationLevel "Gold" ;
  reso:PropertyTypes "RESI","RLSE","MOBI","FARM" ;
  schema:sameAs    <http://ddwiki.reso.org/display/DDW/Room%5Btype%5DArea+Field>,<http://ddwiki.reso.org/display/DDW/Room%5Btype%5DAreaSource+Field>,<http://ddwiki.reso.org/display/DDW/Room%5Btype%5DAreaUnits+Field>,<http://ddwiki.reso.org/display/DDW/Room%5Btype%5DDescription+Field>,<http://ddwiki.reso.org/display/DDW/Room%5Btype%5DDimensions+Field>,<http://ddwiki.reso.org/display/DDW/Room%5Btype%5DFeatures+Field> ;
  vs:term_status   "stable"
.
reso:Room a rdf:Property ;
  rdfs:comment     "[type] This field is a repeating element for each type of room selected in the RoomType field.  For every RoomType there are two possible implementations.  For a flat implementation (RETS 1.x only), each RoomType used is expected to appear as the \"[type]\" in the related rooms field name.  i.e. RoomKitchenArea.  A relational implementation of rooms must omit the type from the field name and use RoomType to create a vertical representation of the various rooms.  i.e. RoomArea with Kitchen in the relational table's RoomType field.","[type] This field is a repeating element for each type of room selected in the RoomType field.  For every RoomType there are two possible implementations.  For a flat implementation (RETS 1.x only), each RoomType used is expected to appear as the \"[type]\" in the related rooms field name.  i.e. RoomKitchenAreaSource.  A relational implementation of rooms must omit the type from the field name and use RoomType to create a vertical representation of the various rooms.  i.e. RoomAreaSource.","[type] This field is a repeating element for each type of room selected in the RoomType field.  For every RoomType there are two possible implementations.  For a flat implementation (RETS 1.x only), each RoomType used is expected to appear as the \"[type]\" in the related rooms field name.  i.e. RoomKitchenAreaUnits.  A relational implementation of rooms must omit the type from the field name and use RoomType to create a vertical representation of the various rooms.  i.e. RoomAreaUnits with Kitchen in the relational table's RoomType field.","[type] This field is a repeating element for each type of room selected in the RoomType field.  For every RoomType there are two possible implementations.  For a flat implementation (RETS 1.x only), each RoomType used is expected to appear as the \"[type]\" in the related rooms field name.  i.e. RoomKitchenDescription.  A relational implementation of rooms must omit the type from the field name and use RoomType to create a vertical representation of the various rooms.  i.e. RoomDescription with Kitchen in the relational table's RoomType field.","[type] This field is a repeating element for each type of room selected in the RoomType field.  For every RoomType there are two possible implementations.  For a flat implementation (RETS 1.x only), each RoomType used is expected to appear as the \"[type]\" in the related rooms field name.  i.e. RoomKitchenDimensions.  A relational implementation of rooms must omit the type from the field name and use RoomType to create a vertical representation of the various rooms.  i.e. RoomDimensions with Kitchen in the relational table's RoomType field.","[type] This field is a repeating element for each type of room selected in the RoomType field.  For every RoomType there are two possible implementations.  For a flat implementation (RETS 1.x only), each RoomType used is expected to appear as the \"[type]\" in the related rooms field name.  i.e. RoomKitchenFeatures.  A relational implementation of rooms must omit the type from the field name and use RoomType to create a vertical representation of the various rooms.  i.e. RoomFeatures with Kitchen in the relational table's RoomType field.","[type] This field is a repeating element for each type of room selected in the RoomType field.  For every RoomType there are two possible implementations.  For a flat implementation (RETS 1.x only), each RoomType used is expected to appear as the \"[type]\" in the related rooms field name.  i.e. RoomKitchenLength.  A relational implementation of rooms must omit the type from the field name and use RoomType to create a vertical representation of the various rooms.  i.e. RoomLength with Kitchen in the relational table's RoomType field." ;
  rdfs:domain      reso:Property ;
  rdfs:label       "Room" ;
  rdfs:range       xsd:decimal,enum:AreaSource,enum:AreaUnits,xsd:string ;
  reso:CertificationLevel "Gold" ;
  reso:PropertyTypes "RESI","RLSE","MOBI","FARM" ;
  schema:sameAs    <http://ddwiki.reso.org/display/DDW/Room%5Btype%5DArea+Field>,<http://ddwiki.reso.org/display/DDW/Room%5Btype%5DAreaSource+Field>,<http://ddwiki.reso.org/display/DDW/Room%5Btype%5DAreaUnits+Field>,<http://ddwiki.reso.org/display/DDW/Room%5Btype%5DDescription+Field>,<http://ddwiki.reso.org/display/DDW/Room%5Btype%5DDimensions+Field>,<http://ddwiki.reso.org/display/DDW/Room%5Btype%5DFeatures+Field>,<http://ddwiki.reso.org/display/DDW/Room%5Btype%5DLength+Field> ;
  vs:term_status   "stable"
.
reso:Room a rdf:Property ;
  rdfs:comment     "[type] This field is a repeating element for each type of room selected in the RoomType field.  For every RoomType there are two possible implementations.  For a flat implementation (RETS 1.x only), each RoomType used is expected to appear as the \"[type]\" in the related rooms field name.  i.e. RoomKitchenArea.  A relational implementation of rooms must omit the type from the field name and use RoomType to create a vertical representation of the various rooms.  i.e. RoomArea with Kitchen in the relational table's RoomType field.","[type] This field is a repeating element for each type of room selected in the RoomType field.  For every RoomType there are two possible implementations.  For a flat implementation (RETS 1.x only), each RoomType used is expected to appear as the \"[type]\" in the related rooms field name.  i.e. RoomKitchenAreaSource.  A relational implementation of rooms must omit the type from the field name and use RoomType to create a vertical representation of the various rooms.  i.e. RoomAreaSource.","[type] This field is a repeating element for each type of room selected in the RoomType field.  For every RoomType there are two possible implementations.  For a flat implementation (RETS 1.x only), each RoomType used is expected to appear as the \"[type]\" in the related rooms field name.  i.e. RoomKitchenAreaUnits.  A relational implementation of rooms must omit the type from the field name and use RoomType to create a vertical representation of the various rooms.  i.e. RoomAreaUnits with Kitchen in the relational table's RoomType field.","[type] This field is a repeating element for each type of room selected in the RoomType field.  For every RoomType there are two possible implementations.  For a flat implementation (RETS 1.x only), each RoomType used is expected to appear as the \"[type]\" in the related rooms field name.  i.e. RoomKitchenDescription.  A relational implementation of rooms must omit the type from the field name and use RoomType to create a vertical representation of the various rooms.  i.e. RoomDescription with Kitchen in the relational table's RoomType field.","[type] This field is a repeating element for each type of room selected in the RoomType field.  For every RoomType there are two possible implementations.  For a flat implementation (RETS 1.x only), each RoomType used is expected to appear as the \"[type]\" in the related rooms field name.  i.e. RoomKitchenDimensions.  A relational implementation of rooms must omit the type from the field name and use RoomType to create a vertical representation of the various rooms.  i.e. RoomDimensions with Kitchen in the relational table's RoomType field.","[type] This field is a repeating element for each type of room selected in the RoomType field.  For every RoomType there are two possible implementations.  For a flat implementation (RETS 1.x only), each RoomType used is expected to appear as the \"[type]\" in the related rooms field name.  i.e. RoomKitchenFeatures.  A relational implementation of rooms must omit the type from the field name and use RoomType to create a vertical representation of the various rooms.  i.e. RoomFeatures with Kitchen in the relational table's RoomType field.","[type] This field is a repeating element for each type of room selected in the RoomType field.  For every RoomType there are two possible implementations.  For a flat implementation (RETS 1.x only), each RoomType used is expected to appear as the \"[type]\" in the related rooms field name.  i.e. RoomKitchenLength.  A relational implementation of rooms must omit the type from the field name and use RoomType to create a vertical representation of the various rooms.  i.e. RoomLength with Kitchen in the relational table's RoomType field.","[type] This field is a repeating element for each type of room selected in the RoomType field.  For every RoomType there are two possible implementations.  For a flat implementation (RETS 1.x only), each RoomType used is expected to appear as the \"[type]\" in the related rooms field name.  i.e. RoomKitchenWidthSource.  A relational implementation of rooms must omit the type from the field name and use RoomType to create a vertical representation of the various rooms.  i.e. RoomWidthSource with Kitchen in the relational table's RoomType field." ;
  rdfs:domain      reso:Property ;
  rdfs:label       "Room" ;
  rdfs:range       xsd:decimal,enum:AreaSource,enum:AreaUnits,xsd:string ;
  reso:CertificationLevel "Gold" ;
  reso:PropertyTypes "RESI","RLSE","MOBI","FARM" ;
  schema:sameAs    <http://ddwiki.reso.org/display/DDW/Room%5Btype%5DArea+Field>,<http://ddwiki.reso.org/display/DDW/Room%5Btype%5DAreaSource+Field>,<http://ddwiki.reso.org/display/DDW/Room%5Btype%5DAreaUnits+Field>,<http://ddwiki.reso.org/display/DDW/Room%5Btype%5DDescription+Field>,<http://ddwiki.reso.org/display/DDW/Room%5Btype%5DDimensions+Field>,<http://ddwiki.reso.org/display/DDW/Room%5Btype%5DFeatures+Field>,<http://ddwiki.reso.org/display/DDW/Room%5Btype%5DLength+Field>,<http://ddwiki.reso.org/display/DDW/Room%5Btype%5DLengthWidthSource+Field> ;
  vs:term_status   "stable"
.
reso:Room a rdf:Property ;
  rdfs:comment     "[type] This field is a repeating element for each type of room selected in the RoomType field.  For every RoomType there are two possible implementations.  For a flat implementation (RETS 1.x only), each RoomType used is expected to appear as the \"[type]\" in the related rooms field name.  i.e. RoomKitchenArea.  A relational implementation of rooms must omit the type from the field name and use RoomType to create a vertical representation of the various rooms.  i.e. RoomArea with Kitchen in the relational table's RoomType field.","[type] This field is a repeating element for each type of room selected in the RoomType field.  For every RoomType there are two possible implementations.  For a flat implementation (RETS 1.x only), each RoomType used is expected to appear as the \"[type]\" in the related rooms field name.  i.e. RoomKitchenAreaSource.  A relational implementation of rooms must omit the type from the field name and use RoomType to create a vertical representation of the various rooms.  i.e. RoomAreaSource.","[type] This field is a repeating element for each type of room selected in the RoomType field.  For every RoomType there are two possible implementations.  For a flat implementation (RETS 1.x only), each RoomType used is expected to appear as the \"[type]\" in the related rooms field name.  i.e. RoomKitchenAreaUnits.  A relational implementation of rooms must omit the type from the field name and use RoomType to create a vertical representation of the various rooms.  i.e. RoomAreaUnits with Kitchen in the relational table's RoomType field.","[type] This field is a repeating element for each type of room selected in the RoomType field.  For every RoomType there are two possible implementations.  For a flat implementation (RETS 1.x only), each RoomType used is expected to appear as the \"[type]\" in the related rooms field name.  i.e. RoomKitchenDescription.  A relational implementation of rooms must omit the type from the field name and use RoomType to create a vertical representation of the various rooms.  i.e. RoomDescription with Kitchen in the relational table's RoomType field.","[type] This field is a repeating element for each type of room selected in the RoomType field.  For every RoomType there are two possible implementations.  For a flat implementation (RETS 1.x only), each RoomType used is expected to appear as the \"[type]\" in the related rooms field name.  i.e. RoomKitchenDimensions.  A relational implementation of rooms must omit the type from the field name and use RoomType to create a vertical representation of the various rooms.  i.e. RoomDimensions with Kitchen in the relational table's RoomType field.","[type] This field is a repeating element for each type of room selected in the RoomType field.  For every RoomType there are two possible implementations.  For a flat implementation (RETS 1.x only), each RoomType used is expected to appear as the \"[type]\" in the related rooms field name.  i.e. RoomKitchenFeatures.  A relational implementation of rooms must omit the type from the field name and use RoomType to create a vertical representation of the various rooms.  i.e. RoomFeatures with Kitchen in the relational table's RoomType field.","[type] This field is a repeating element for each type of room selected in the RoomType field.  For every RoomType there are two possible implementations.  For a flat implementation (RETS 1.x only), each RoomType used is expected to appear as the \"[type]\" in the related rooms field name.  i.e. RoomKitchenLength.  A relational implementation of rooms must omit the type from the field name and use RoomType to create a vertical representation of the various rooms.  i.e. RoomLength with Kitchen in the relational table's RoomType field.","[type] This field is a repeating element for each type of room selected in the RoomType field.  For every RoomType there are two possible implementations.  For a flat implementation (RETS 1.x only), each RoomType used is expected to appear as the \"[type]\" in the related rooms field name.  i.e. RoomKitchenWidthSource.  A relational implementation of rooms must omit the type from the field name and use RoomType to create a vertical representation of the various rooms.  i.e. RoomWidthSource with Kitchen in the relational table's RoomType field.","[type] This field is a repeating element for each type of room selected in the RoomType field.  For every RoomType there are two possible implementations.  For a flat implementation (RETS 1.x only), each RoomType used is expected to appear as the \"[type]\" in the related rooms field name.  i.e. RoomKitchenWidthUnits.  A relational implementation of rooms must omit the type from the field name and use RoomType to create a vertical representation of the various rooms.  i.e. RoomWidthUnits with Kitchen in the relational table's RoomType field." ;
  rdfs:domain      reso:Property ;
  rdfs:label       "Room" ;
  rdfs:range       xsd:decimal,enum:AreaSource,enum:AreaUnits,xsd:string,enum:LinearUnits ;
  reso:CertificationLevel "Gold" ;
  reso:PropertyTypes "RESI","RLSE","MOBI","FARM" ;
  schema:sameAs    <http://ddwiki.reso.org/display/DDW/Room%5Btype%5DArea+Field>,<http://ddwiki.reso.org/display/DDW/Room%5Btype%5DAreaSource+Field>,<http://ddwiki.reso.org/display/DDW/Room%5Btype%5DAreaUnits+Field>,<http://ddwiki.reso.org/display/DDW/Room%5Btype%5DDescription+Field>,<http://ddwiki.reso.org/display/DDW/Room%5Btype%5DDimensions+Field>,<http://ddwiki.reso.org/display/DDW/Room%5Btype%5DFeatures+Field>,<http://ddwiki.reso.org/display/DDW/Room%5Btype%5DLength+Field>,<http://ddwiki.reso.org/display/DDW/Room%5Btype%5DLengthWidthSource+Field>,<http://ddwiki.reso.org/display/DDW/Room%5Btype%5DLengthWidthUnits+Field> ;
  vs:term_status   "stable"
.
reso:Room a rdf:Property ;
  rdfs:comment     "[type] This field is a repeating element for each type of room selected in the RoomType field.  For every RoomType there are two possible implementations.  For a flat implementation (RETS 1.x only), each RoomType used is expected to appear as the \"[type]\" in the related rooms field name.  i.e. RoomKitchenArea.  A relational implementation of rooms must omit the type from the field name and use RoomType to create a vertical representation of the various rooms.  i.e. RoomArea with Kitchen in the relational table's RoomType field.","[type] This field is a repeating element for each type of room selected in the RoomType field.  For every RoomType there are two possible implementations.  For a flat implementation (RETS 1.x only), each RoomType used is expected to appear as the \"[type]\" in the related rooms field name.  i.e. RoomKitchenAreaSource.  A relational implementation of rooms must omit the type from the field name and use RoomType to create a vertical representation of the various rooms.  i.e. RoomAreaSource.","[type] This field is a repeating element for each type of room selected in the RoomType field.  For every RoomType there are two possible implementations.  For a flat implementation (RETS 1.x only), each RoomType used is expected to appear as the \"[type]\" in the related rooms field name.  i.e. RoomKitchenAreaUnits.  A relational implementation of rooms must omit the type from the field name and use RoomType to create a vertical representation of the various rooms.  i.e. RoomAreaUnits with Kitchen in the relational table's RoomType field.","[type] This field is a repeating element for each type of room selected in the RoomType field.  For every RoomType there are two possible implementations.  For a flat implementation (RETS 1.x only), each RoomType used is expected to appear as the \"[type]\" in the related rooms field name.  i.e. RoomKitchenDescription.  A relational implementation of rooms must omit the type from the field name and use RoomType to create a vertical representation of the various rooms.  i.e. RoomDescription with Kitchen in the relational table's RoomType field.","[type] This field is a repeating element for each type of room selected in the RoomType field.  For every RoomType there are two possible implementations.  For a flat implementation (RETS 1.x only), each RoomType used is expected to appear as the \"[type]\" in the related rooms field name.  i.e. RoomKitchenDimensions.  A relational implementation of rooms must omit the type from the field name and use RoomType to create a vertical representation of the various rooms.  i.e. RoomDimensions with Kitchen in the relational table's RoomType field.","[type] This field is a repeating element for each type of room selected in the RoomType field.  For every RoomType there are two possible implementations.  For a flat implementation (RETS 1.x only), each RoomType used is expected to appear as the \"[type]\" in the related rooms field name.  i.e. RoomKitchenFeatures.  A relational implementation of rooms must omit the type from the field name and use RoomType to create a vertical representation of the various rooms.  i.e. RoomFeatures with Kitchen in the relational table's RoomType field.","[type] This field is a repeating element for each type of room selected in the RoomType field.  For every RoomType there are two possible implementations.  For a flat implementation (RETS 1.x only), each RoomType used is expected to appear as the \"[type]\" in the related rooms field name.  i.e. RoomKitchenLength.  A relational implementation of rooms must omit the type from the field name and use RoomType to create a vertical representation of the various rooms.  i.e. RoomLength with Kitchen in the relational table's RoomType field.","[type] This field is a repeating element for each type of room selected in the RoomType field.  For every RoomType there are two possible implementations.  For a flat implementation (RETS 1.x only), each RoomType used is expected to appear as the \"[type]\" in the related rooms field name.  i.e. RoomKitchenWidthSource.  A relational implementation of rooms must omit the type from the field name and use RoomType to create a vertical representation of the various rooms.  i.e. RoomWidthSource with Kitchen in the relational table's RoomType field.","[type] This field is a repeating element for each type of room selected in the RoomType field.  For every RoomType there are two possible implementations.  For a flat implementation (RETS 1.x only), each RoomType used is expected to appear as the \"[type]\" in the related rooms field name.  i.e. RoomKitchenWidthUnits.  A relational implementation of rooms must omit the type from the field name and use RoomType to create a vertical representation of the various rooms.  i.e. RoomWidthUnits with Kitchen in the relational table's RoomType field.","[type] This field is a repeating element for each type of room selected in the RoomType field.  For every RoomType there are two possible implementations.  For a flat implementation (RETS 1.x only), each RoomType used is expected to appear as the \"[type]\" in the related rooms field name.  i.e. RoomKitchenLevel.  A relational implementation of rooms must omit the type from the field name and use RoomType to create a vertical representation of the various rooms.  i.e. RoomLevel with Kitchen in the relational table's RoomType field." ;
  rdfs:domain      reso:Property ;
  rdfs:label       "Room" ;
  rdfs:range       xsd:decimal,enum:AreaSource,enum:AreaUnits,xsd:string,enum:LinearUnits ;
  reso:CertificationLevel "Gold" ;
  reso:PropertyTypes "RESI","RLSE","MOBI","FARM" ;
  schema:sameAs    <http://ddwiki.reso.org/display/DDW/Room%5Btype%5DArea+Field>,<http://ddwiki.reso.org/display/DDW/Room%5Btype%5DAreaSource+Field>,<http://ddwiki.reso.org/display/DDW/Room%5Btype%5DAreaUnits+Field>,<http://ddwiki.reso.org/display/DDW/Room%5Btype%5DDescription+Field>,<http://ddwiki.reso.org/display/DDW/Room%5Btype%5DDimensions+Field>,<http://ddwiki.reso.org/display/DDW/Room%5Btype%5DFeatures+Field>,<http://ddwiki.reso.org/display/DDW/Room%5Btype%5DLength+Field>,<http://ddwiki.reso.org/display/DDW/Room%5Btype%5DLengthWidthSource+Field>,<http://ddwiki.reso.org/display/DDW/Room%5Btype%5DLengthWidthUnits+Field>,<http://ddwiki.reso.org/display/DDW/Room%5Btype%5DLevel+Field> ;
  vs:term_status   "stable"
.
reso:Room a rdf:Property ;
  rdfs:comment     "[type] This field is a repeating element for each type of room selected in the RoomType field.  For every RoomType there are two possible implementations.  For a flat implementation (RETS 1.x only), each RoomType used is expected to appear as the \"[type]\" in the related rooms field name.  i.e. RoomKitchenArea.  A relational implementation of rooms must omit the type from the field name and use RoomType to create a vertical representation of the various rooms.  i.e. RoomArea with Kitchen in the relational table's RoomType field.","[type] This field is a repeating element for each type of room selected in the RoomType field.  For every RoomType there are two possible implementations.  For a flat implementation (RETS 1.x only), each RoomType used is expected to appear as the \"[type]\" in the related rooms field name.  i.e. RoomKitchenAreaSource.  A relational implementation of rooms must omit the type from the field name and use RoomType to create a vertical representation of the various rooms.  i.e. RoomAreaSource.","[type] This field is a repeating element for each type of room selected in the RoomType field.  For every RoomType there are two possible implementations.  For a flat implementation (RETS 1.x only), each RoomType used is expected to appear as the \"[type]\" in the related rooms field name.  i.e. RoomKitchenAreaUnits.  A relational implementation of rooms must omit the type from the field name and use RoomType to create a vertical representation of the various rooms.  i.e. RoomAreaUnits with Kitchen in the relational table's RoomType field.","[type] This field is a repeating element for each type of room selected in the RoomType field.  For every RoomType there are two possible implementations.  For a flat implementation (RETS 1.x only), each RoomType used is expected to appear as the \"[type]\" in the related rooms field name.  i.e. RoomKitchenDescription.  A relational implementation of rooms must omit the type from the field name and use RoomType to create a vertical representation of the various rooms.  i.e. RoomDescription with Kitchen in the relational table's RoomType field.","[type] This field is a repeating element for each type of room selected in the RoomType field.  For every RoomType there are two possible implementations.  For a flat implementation (RETS 1.x only), each RoomType used is expected to appear as the \"[type]\" in the related rooms field name.  i.e. RoomKitchenDimensions.  A relational implementation of rooms must omit the type from the field name and use RoomType to create a vertical representation of the various rooms.  i.e. RoomDimensions with Kitchen in the relational table's RoomType field.","[type] This field is a repeating element for each type of room selected in the RoomType field.  For every RoomType there are two possible implementations.  For a flat implementation (RETS 1.x only), each RoomType used is expected to appear as the \"[type]\" in the related rooms field name.  i.e. RoomKitchenFeatures.  A relational implementation of rooms must omit the type from the field name and use RoomType to create a vertical representation of the various rooms.  i.e. RoomFeatures with Kitchen in the relational table's RoomType field.","[type] This field is a repeating element for each type of room selected in the RoomType field.  For every RoomType there are two possible implementations.  For a flat implementation (RETS 1.x only), each RoomType used is expected to appear as the \"[type]\" in the related rooms field name.  i.e. RoomKitchenLength.  A relational implementation of rooms must omit the type from the field name and use RoomType to create a vertical representation of the various rooms.  i.e. RoomLength with Kitchen in the relational table's RoomType field.","[type] This field is a repeating element for each type of room selected in the RoomType field.  For every RoomType there are two possible implementations.  For a flat implementation (RETS 1.x only), each RoomType used is expected to appear as the \"[type]\" in the related rooms field name.  i.e. RoomKitchenWidthSource.  A relational implementation of rooms must omit the type from the field name and use RoomType to create a vertical representation of the various rooms.  i.e. RoomWidthSource with Kitchen in the relational table's RoomType field.","[type] This field is a repeating element for each type of room selected in the RoomType field.  For every RoomType there are two possible implementations.  For a flat implementation (RETS 1.x only), each RoomType used is expected to appear as the \"[type]\" in the related rooms field name.  i.e. RoomKitchenWidthUnits.  A relational implementation of rooms must omit the type from the field name and use RoomType to create a vertical representation of the various rooms.  i.e. RoomWidthUnits with Kitchen in the relational table's RoomType field.","[type] This field is a repeating element for each type of room selected in the RoomType field.  For every RoomType there are two possible implementations.  For a flat implementation (RETS 1.x only), each RoomType used is expected to appear as the \"[type]\" in the related rooms field name.  i.e. RoomKitchenLevel.  A relational implementation of rooms must omit the type from the field name and use RoomType to create a vertical representation of the various rooms.  i.e. RoomLevel with Kitchen in the relational table's RoomType field.","[type] This field is a repeating element for each type of room selected in the RoomType field.  For every RoomType there are two possible implementations.  For a flat implementation (RETS 1.x only), each RoomType used is expected to appear as the \"[type]\" in the related rooms field name.  i.e. RoomKitchenWidth.  A relational implementation of rooms must omit the type from the field name and use RoomType to create a vertical representation of the various rooms.  i.e. RoomWidth with Kitchen in the relational table's RoomType field." ;
  rdfs:domain      reso:Property ;
  rdfs:label       "Room" ;
  rdfs:range       xsd:decimal,enum:AreaSource,enum:AreaUnits,xsd:string,enum:LinearUnits ;
  reso:CertificationLevel "Gold" ;
  reso:PropertyTypes "RESI","RLSE","MOBI","FARM" ;
  schema:sameAs    <http://ddwiki.reso.org/display/DDW/Room%5Btype%5DArea+Field>,<http://ddwiki.reso.org/display/DDW/Room%5Btype%5DAreaSource+Field>,<http://ddwiki.reso.org/display/DDW/Room%5Btype%5DAreaUnits+Field>,<http://ddwiki.reso.org/display/DDW/Room%5Btype%5DDescription+Field>,<http://ddwiki.reso.org/display/DDW/Room%5Btype%5DDimensions+Field>,<http://ddwiki.reso.org/display/DDW/Room%5Btype%5DFeatures+Field>,<http://ddwiki.reso.org/display/DDW/Room%5Btype%5DLength+Field>,<http://ddwiki.reso.org/display/DDW/Room%5Btype%5DLengthWidthSource+Field>,<http://ddwiki.reso.org/display/DDW/Room%5Btype%5DLengthWidthUnits+Field>,<http://ddwiki.reso.org/display/DDW/Room%5Btype%5DLevel+Field>,<http://ddwiki.reso.org/display/DDW/Room%5Btype%5DWidth+Field> ;
  vs:term_status   "stable"
.
reso:RoomsTotal a rdf:Property ;
  rdfs:comment     "The number of rooms in the dwelling." ;
  rdfs:domain      reso:Property ;
  rdfs:label       "RoomsTotal" ;
  rdfs:range       xsd:decimal ;
  reso:CertificationLevel "Gold" ;
  reso:PropertyTypes "RESI","RLSE","RINC","MOBI","FARM" ;
  schema:sameAs    <http://ddwiki.reso.org/display/DDW/RoomsTotal+Field> ;
  vs:term_status   "stable"
.
reso:SeatingCapacity a rdf:Property ;
  rdfs:comment     "The seating capacity of the business being sold." ;
  rdfs:domain      reso:Property ;
  rdfs:label       "SeatingCapacity" ;
  rdfs:range       xsd:decimal ;
  reso:CertificationLevel "Silver" ;
  reso:PropertyTypes "BUSO" ;
  schema:sameAs    <http://ddwiki.reso.org/display/DDW/SeatingCapacity+Field> ;
  vs:term_status   "stable"
.
reso:SecurityFeatures a rdf:Property ;
  rdfs:comment     "A list describing the security features included in the sale/lease." ;
  rdfs:domain      reso:Property ;
  rdfs:label       "SecurityFeatures" ;
  rdfs:range       xsd:string ;
  reso:CertificationLevel "Platinum" ;
  reso:PropertyTypes "RESI","RLSE","RINC","MOBI","FARM","COMS","COML" ;
  schema:sameAs    <http://ddwiki.reso.org/display/DDW/SecurityFeatures+Field> ;
  vs:term_status   "stable"
.
reso:SeniorCommunityYN a rdf:Property ;
  rdfs:comment     "The community is a senior community." ;
  rdfs:domain      reso:Property ;
  rdfs:label       "SeniorCommunityYN" ;
  rdfs:range       xsd:boolean ;
  reso:CertificationLevel "Platinum" ;
  reso:PropertyTypes "RESI","RLSE","RINC","LAND","MOBI","FARM" ;
  schema:sameAs    <http://ddwiki.reso.org/display/DDW/SeniorCommunityYN+Field> ;
  vs:term_status   "stable"
.
reso:SerialU a rdf:Property ;
  rdfs:comment     "Serial number of the mobile or manufactured home.  For the first or only unit/section use Serial U over Serial X or Serial XX." ;
  rdfs:domain      reso:Property ;
  rdfs:label       "SerialU" ;
  rdfs:range       xsd:string ;
  reso:CertificationLevel "Silver" ;
  reso:PropertyTypes "RESI","RLSE","MOBI" ;
  schema:sameAs    <http://ddwiki.reso.org/display/DDW/SerialU+Field> ;
  vs:term_status   "stable"
.
reso:SerialX a rdf:Property ;
  rdfs:comment     "Serial number of the mobile or manufactured home.  For two units/sections, Serial U should be used first, Serial X second over or Serial XX." ;
  rdfs:domain      reso:Property ;
  rdfs:label       "SerialX" ;
  rdfs:range       xsd:string ;
  reso:CertificationLevel "Silver" ;
  reso:PropertyTypes "RESI","RLSE","MOBI" ;
  schema:sameAs    <http://ddwiki.reso.org/display/DDW/SerialX+Field> ;
  vs:term_status   "stable"
.
reso:SerialXX a rdf:Property ;
  rdfs:comment     "Serial number of the mobile or manufactured home.  For two units/sections, Serial U should be used first, Serial X second over or Serial XX." ;
  rdfs:domain      reso:Property ;
  rdfs:label       "SerialXX" ;
  rdfs:range       xsd:string ;
  reso:CertificationLevel "Silver" ;
  reso:PropertyTypes "RESI","RLSE","MOBI" ;
  schema:sameAs    <http://ddwiki.reso.org/display/DDW/SerialXX+Field> ;
  vs:term_status   "stable"
.
reso:Sewer a rdf:Property ;
  rdfs:comment     "A list describing the sewer or septic features of the property." ;
  rdfs:domain      reso:Property ;
  rdfs:label       "Sewer" ;
  rdfs:range       enum:Sewer ;
  reso:CertificationLevel "Bronze" ;
  reso:PropertyTypes "RESI","RLSE","RINC","LAND","MOBI","FARM","COMS","COML" ;
  schema:sameAs    <http://ddwiki.reso.org/display/DDW/Sewer+Field> ;
  vs:term_status   "stable"
.
reso:ShowingContactName a rdf:Property ;
  rdfs:comment     "The name of the contact for the showing of the listed property." ;
  rdfs:domain      reso:Property ;
  rdfs:label       "ShowingContactName" ;
  rdfs:range       xsd:string ;
  reso:CertificationLevel "Bronze" ;
  reso:PropertyTypes "RESI","RLSE","RINC","LAND","MOBI","FARM","COMS","COML","BUSO" ;
  schema:sameAs    <http://ddwiki.reso.org/display/DDW/ShowingContactName+Field> ;
  vs:term_status   "stable"
.
reso:ShowingContactPhone a rdf:Property ;
  rdfs:comment     "A telephone number that should be called to arrange showing the property." ;
  rdfs:domain      reso:Property ;
  rdfs:label       "ShowingContactPhone" ;
  rdfs:range       xsd:string ;
  reso:CertificationLevel "Core" ;
  reso:PropertyTypes "RESI","RLSE","RINC","LAND","MOBI","FARM","COMS","COML","BUSO" ;
  schema:sameAs    <http://ddwiki.reso.org/display/DDW/ShowingContactPhone+Field> ;
  vs:term_status   "stable"
.
reso:ShowingContactPhoneExt a rdf:Property ;
  rdfs:comment     "The extension of the given phone number (if applicable)." ;
  rdfs:domain      reso:Property ;
  rdfs:label       "ShowingContactPhoneExt" ;
  rdfs:range       xsd:string ;
  reso:CertificationLevel "Core" ;
  reso:PropertyTypes "RESI","RLSE","RINC","LAND","MOBI","FARM","COMS","COML","BUSO" ;
  schema:sameAs    <http://ddwiki.reso.org/display/DDW/ShowingContactPhoneExt+Field> ;
  vs:term_status   "stable"
.
reso:ShowingContactType a rdf:Property ;
  rdfs:comment     "The type of contact for the showing.  i.e. Agent, Broker, Seller." ;
  rdfs:domain      reso:Property ;
  rdfs:label       "ShowingContactType" ;
  rdfs:range       enum:ShowingContactType ;
  reso:CertificationLevel "Bronze" ;
  reso:PropertyTypes "RESI","RLSE","RINC","LAND","MOBI","FARM","COMS","COML","BUSO" ;
  schema:sameAs    <http://ddwiki.reso.org/display/DDW/ShowingContactType+Field> ;
  vs:term_status   "stable"
.
reso:ShowingInstructions a rdf:Property ;
  rdfs:domain      reso:Property ;
  rdfs:label       "ShowingInstructions" ;
  rdfs:range       xsd:string ;
  reso:CertificationLevel "Core" ;
  reso:PropertyTypes "RESI","RLSE","RINC","LAND","MOBI","FARM","COMS","COML","BUSO" ;
  schema:sameAs    <http://ddwiki.reso.org/display/DDW/ShowingInstructions+Field> ;
  vs:term_status   "stable"
.
reso:SignOnPropertyYN a rdf:Property ;
  rdfs:comment     "Is there a sign on the property." ;
  rdfs:domain      reso:Property ;
  rdfs:label       "SignOnPropertyYN" ;
  rdfs:range       xsd:boolean ;
  reso:CertificationLevel "Bronze" ;
  reso:PropertyTypes "RESI","RLSE","RINC","LAND","MOBI","FARM","COMS","COML","BUSO" ;
  schema:sameAs    <http://ddwiki.reso.org/display/DDW/SignOnPropertyYN+Field> ;
  vs:term_status   "stable"
.
reso:Skirt a rdf:Property ;
  rdfs:comment     "A list of types of mobile home skirting." ;
  rdfs:domain      reso:Property ;
  rdfs:label       "Skirt" ;
  rdfs:range       enum:Skirt ;
  reso:CertificationLevel "Silver" ;
  reso:PropertyTypes "MOBI" ;
  schema:sameAs    <http://ddwiki.reso.org/display/DDW/Skirt+Field> ;
  vs:term_status   "stable"
.
reso:SourceSystemID a rdf:Property ;
  rdfs:comment     "The RESO OUID's OrganizationUniqueId of the Source record provider. The source system is the system from which the record was directly received. In cases where the source system was not where the record originated (the authoritative system), see the Originating System fields." ;
  rdfs:domain      reso:Property ;
  rdfs:label       "SourceSystemID" ;
  rdfs:range       xsd:string ;
  reso:CertificationLevel "Platinum" ;
  reso:PropertyTypes "RESI","RLSE","RINC","LAND","MOBI","FARM","COMS","COML","BUSO" ;
  schema:sameAs    <http://ddwiki.reso.org/display/DDW/SourceSystemID+Field> ;
  vs:term_status   "stable"
.
reso:SourceSystemKey a rdf:Property ;
  rdfs:comment     "The system key, a unique record identifier, from the Source System. The Source System is the system from which the record was directly received. In cases where the Source System was not where the record originated (the authoritative system), see the Originating System fields." ;
  rdfs:domain      reso:Property ;
  rdfs:label       "SourceSystemKey" ;
  rdfs:range       xsd:string ;
  reso:CertificationLevel "Core" ;
  reso:PropertyTypes "RESI","RLSE","RINC","LAND","MOBI","FARM","COMS","COML","BUSO" ;
  schema:sameAs    <http://ddwiki.reso.org/display/DDW/SourceSystemKey+Field> ;
  vs:term_status   "stable"
.
reso:SourceSystemName a rdf:Property ;
  rdfs:comment     "The name of the immediate record provider. The system from which the record was directly received. The legal name of the company." ;
  rdfs:domain      reso:Property ;
  rdfs:label       "SourceSystemName" ;
  rdfs:range       xsd:string ;
  reso:CertificationLevel "Core" ;
  reso:PropertyTypes "RESI","RLSE","RINC","LAND","MOBI","FARM","COMS","COML","BUSO" ;
  schema:sameAs    <http://ddwiki.reso.org/display/DDW/SourceSystemName+Field> ;
  vs:term_status   "stable"
.
reso:SpaFeatures a rdf:Property ;
  rdfs:comment     "A list of features or description of the spa included in the sale/lease." ;
  rdfs:domain      reso:Property ;
  rdfs:label       "SpaFeatures" ;
  rdfs:range       xsd:string ;
  reso:CertificationLevel "Platinum" ;
  reso:PropertyTypes "RESI","RLSE","RINC","LAND","MOBI","FARM" ;
  schema:sameAs    <http://ddwiki.reso.org/display/DDW/SpaFeatures+Field> ;
  vs:term_status   "stable"
.
reso:SpaYN a rdf:Property ;
  rdfs:comment     "The property has a spa." ;
  rdfs:domain      reso:Property ;
  rdfs:label       "SpaYN" ;
  rdfs:range       xsd:boolean ;
  reso:CertificationLevel "Platinum" ;
  reso:PropertyTypes "RESI","RLSE","RINC","LAND","MOBI","FARM" ;
  schema:sameAs    <http://ddwiki.reso.org/display/DDW/SpaYN+Field> ;
  vs:term_status   "stable"
.
reso:SpecialLicenses a rdf:Property ;
  rdfs:comment     "Special licenses required/used by the business being sold.  i.e. Beer/Wine, Class H, Professional, Gambling, None." ;
  rdfs:domain      reso:Property ;
  rdfs:label       "SpecialLicenses" ;
  rdfs:range       enum:SpecialLicenses ;
  reso:CertificationLevel "Bronze" ;
  reso:PropertyTypes "BUSO" ;
  schema:sameAs    <http://ddwiki.reso.org/display/DDW/SpecialLicenses+Field> ;
  vs:term_status   "stable"
.
reso:SpecialListingConditions a rdf:Property ;
  rdfs:comment     "A list of options that describe the type of sale.  i.e. Standard, REO, Short Sale, Probate, Auction, NOD, etc., at the time of listing." ;
  rdfs:domain      reso:Property ;
  rdfs:label       "SpecialListingConditions" ;
  rdfs:range       enum:SpecialListingConditions ;
  reso:CertificationLevel "Bronze" ;
  reso:PropertyTypes "RESI","RLSE","RINC","LAND","MOBI","FARM","COMS","COML","BUSO" ;
  schema:sameAs    <http://ddwiki.reso.org/display/DDW/SpecialListingConditions+Field> ;
  vs:term_status   "stable"
.
reso:StandardStatus a rdf:Property ;
  rdfs:comment     "The status of the listing as it reflects the state of the contract between the listing agent and seller or an agreement with a buyer. (Active, Backup, Canceled, Closed, Expired, Pending, Withdrawn).  Single Select" ;
  rdfs:domain      reso:Property ;
  rdfs:label       "StandardStatus" ;
  rdfs:range       enum:StandardStatus ;
  reso:CertificationLevel "Core" ;
  reso:PropertyTypes "RESI","RLSE","RINC","LAND","MOBI","FARM","COMS","COML","BUSO" ;
  schema:sameAs    <http://ddwiki.reso.org/display/DDW/StandardStatus+Field> ;
  vs:term_status   "stable"
.
reso:StateOrProvince a rdf:Property ;
  rdfs:comment     "Text field containing the accepted postal abbreviation for the state or province." ;
  rdfs:domain      reso:Property ;
  rdfs:label       "StateOrProvince" ;
  rdfs:range       enum:StateOrProvince ;
  reso:CertificationLevel "Core" ;
  reso:PropertyTypes "RESI","RLSE","RINC","LAND","MOBI","FARM","COMS","COML","BUSO" ;
  schema:sameAs    <http://ddwiki.reso.org/display/DDW/StateOrProvince+Field> ;
  vs:term_status   "stable"
.
reso:StateRegion a rdf:Property ;
  rdfs:comment     "A sub-section or area of a defined state or province.  Examples would be the Keys in FL or Hudson Valley in NY." ;
  rdfs:domain      reso:Property ;
  rdfs:label       "StateRegion" ;
  rdfs:range       xsd:string ;
  reso:CertificationLevel "Platinum" ;
  reso:PropertyTypes "RESI","RLSE","RINC","LAND","MOBI","FARM","COMS","COML","BUSO" ;
  schema:sameAs    <http://ddwiki.reso.org/display/DDW/StateRegion+Field> ;
  vs:term_status   "stable"
.
reso:StatusChangeTimestamp a rdf:Property ;
  rdfs:comment     "The transactional timestamp automatically recorded by the MLS system representing the date/time the listing's status was last changed." ;
  rdfs:domain      reso:Property ;
  rdfs:label       "StatusChangeTimestamp" ;
  rdfs:range       xsd:dateTime ;
  reso:CertificationLevel "Core" ;
  reso:PropertyTypes "RESI","RLSE","RINC","LAND","MOBI","FARM","COMS","COML","BUSO" ;
  schema:sameAs    <http://ddwiki.reso.org/display/DDW/StatusChangeTimestamp+Field> ;
  vs:term_status   "stable"
.
reso:Stories a rdf:Property ;
  rdfs:comment     "The number of floors in the property being sold." ;
  rdfs:domain      reso:Property ;
  rdfs:label       "Stories" ;
  rdfs:range       xsd:decimal ;
  reso:CertificationLevel "Core" ;
  reso:PropertyTypes "RESI","RLSE","RINC","MOBI","FARM","COMS","COML" ;
  schema:sameAs    <http://ddwiki.reso.org/display/DDW/Stories+Field> ;
  vs:term_status   "stable"
.
reso:StoriesTotal a rdf:Property ;
  rdfs:comment     "The total number of floors in the building.  In the case of multi-dwelling structures, this is the entire structure and not the individual dwelling being sold." ;
  rdfs:domain      reso:Property ;
  rdfs:label       "StoriesTotal" ;
  rdfs:range       xsd:decimal ;
  reso:CertificationLevel "Core" ;
  reso:PropertyTypes "RESI","RLSE","RINC","MOBI","FARM","COMS","COML" ;
  schema:sameAs    <http://ddwiki.reso.org/display/DDW/StoriesTotal+Field> ;
  vs:term_status   "stable"
.
reso:StreetAdditionalInfo a rdf:Property ;
  rdfs:comment     "Information other than a prefix or suffix for the street portion of a postal address." ;
  rdfs:domain      reso:Property ;
  rdfs:label       "StreetAdditionalInfo" ;
  rdfs:range       xsd:string ;
  reso:CertificationLevel "Core" ;
  reso:PropertyTypes "RESI","RLSE","RINC","LAND","MOBI","FARM","COMS","COML","BUSO" ;
  schema:sameAs    <http://ddwiki.reso.org/display/DDW/StreetAdditionalInfo+Field> ;
  vs:term_status   "stable"
.
reso:StreetDirPrefix a rdf:Property ;
  rdfs:comment     "The direction indicator that precedes the listed property's street name." ;
  rdfs:domain      reso:Property ;
  rdfs:label       "StreetDirPrefix" ;
  rdfs:range       enum:StreetDirection ;
  reso:CertificationLevel "Core" ;
  reso:PropertyTypes "RESI","RLSE","RINC","LAND","MOBI","FARM","COMS","COML","BUSO" ;
  schema:sameAs    <http://ddwiki.reso.org/display/DDW/StreetDirPrefix+Field> ;
  vs:term_status   "stable"
.
reso:StreetDirSuffix a rdf:Property ;
  rdfs:comment     "The direction indicator that follows a listed property's street address." ;
  rdfs:domain      reso:Property ;
  rdfs:label       "StreetDirSuffix" ;
  rdfs:range       enum:StreetDirection ;
  reso:CertificationLevel "Core" ;
  reso:PropertyTypes "RESI","RLSE","RINC","LAND","MOBI","FARM","COMS","COML","BUSO" ;
  schema:sameAs    <http://ddwiki.reso.org/display/DDW/StreetDirSuffix+Field> ;
  vs:term_status   "stable"
.
reso:StreetName a rdf:Property ;
  rdfs:comment     "The street name portion of a listed property's street address." ;
  rdfs:domain      reso:Property ;
  rdfs:label       "StreetName" ;
  rdfs:range       xsd:string ;
  reso:CertificationLevel "Core" ;
  reso:PropertyTypes "RESI","RLSE","RINC","LAND","MOBI","FARM","COMS","COML","BUSO" ;
  schema:sameAs    <http://ddwiki.reso.org/display/DDW/StreetName+Field> ;
  vs:term_status   "stable"
.
reso:StreetNumber a rdf:Property ;
  rdfs:comment     "The street number portion of a listed property's street address.  In some areas the street number may contain non-numeric characters.  This field can also contain extensions and modifiers to the street number, such as \"1/2\" or \"-B\".  This street number field should not include Prefixes, Direction or Suffixes." ;
  rdfs:domain      reso:Property ;
  rdfs:label       "StreetNumber" ;
  rdfs:range       xsd:string ;
  reso:CertificationLevel "Core" ;
  reso:PropertyTypes "RESI","RLSE","RINC","LAND","MOBI","FARM","COMS","COML","BUSO" ;
  schema:sameAs    <http://ddwiki.reso.org/display/DDW/StreetNumber+Field> ;
  vs:term_status   "stable"
.
reso:StreetNumberNumeric a rdf:Property ;
  rdfs:comment     "The integer portion of the street number." ;
  rdfs:domain      reso:Property ;
  rdfs:label       "StreetNumberNumeric" ;
  rdfs:range       xsd:decimal ;
  reso:CertificationLevel "Core" ;
  reso:PropertyTypes "RESI","RLSE","RINC","LAND","MOBI","FARM","COMS","COML","BUSO" ;
  schema:sameAs    <http://ddwiki.reso.org/display/DDW/StreetNumberNumeric+Field> ;
  vs:term_status   "stable"
.
reso:StreetSuffix a rdf:Property ;
  rdfs:comment     "The suffix portion of a listed property's street address." ;
  rdfs:domain      reso:Property ;
  rdfs:label       "StreetSuffix" ;
  rdfs:range       xsd:string ;
  reso:CertificationLevel "Core" ;
  reso:PropertyTypes "RESI","RLSE","RINC","LAND","MOBI","FARM","COMS","COML","BUSO" ;
  schema:sameAs    <http://ddwiki.reso.org/display/DDW/StreetSuffix+Field> ;
  vs:term_status   "stable"
.
reso:StreetSuffixModifier a rdf:Property ;
  rdfs:comment     "The Street Suffix Modifier allows the member to enter a unique Street Suffix that was not found in the Street Suffix pick list or to extend or prefix the suffix." ;
  rdfs:domain      reso:Property ;
  rdfs:label       "StreetSuffixModifier" ;
  rdfs:range       xsd:string ;
  reso:CertificationLevel "Core" ;
  reso:PropertyTypes "RESI","RLSE","RINC","LAND","MOBI","FARM","COMS","COML","BUSO" ;
  schema:sameAs    <http://ddwiki.reso.org/display/DDW/StreetSuffixModifier+Field> ;
  vs:term_status   "stable"
.
reso:StructureType a rdf:Property ;
  rdfs:comment     "The type of structure." ;
  rdfs:domain      reso:Property ;
  rdfs:label       "StructureType" ;
  rdfs:range       enum:StructureType ;
  reso:CertificationLevel "Platinum" ;
  reso:PropertyTypes "RESI","RLSE","RINC","MOBI","FARM" ;
  schema:sameAs    <http://ddwiki.reso.org/display/DDW/StructureType+Field> ;
  vs:term_status   "stable"
.
reso:SubAgencyCompensation a rdf:Property ;
  rdfs:comment     "The total commission to be paid to the Sub Agency, expressed as either a percentage or a constant currency amount." ;
  rdfs:domain      reso:Property ;
  rdfs:label       "SubAgencyCompensation" ;
  rdfs:range       xsd:string ;
  reso:CertificationLevel "Bronze" ;
  reso:PropertyTypes "RESI","RLSE","RINC","LAND","MOBI","FARM","COMS","COML","BUSO" ;
  schema:sameAs    <http://ddwiki.reso.org/display/DDW/SubAgencyCompensation+Field> ;
  vs:term_status   "stable"
.
reso:SubAgencyCompensationType a rdf:Property ;
  rdfs:comment     "A list of types to clarify the value entered in the SubAgencyCompensation field.  For example $, % or some other clarification of the SubAgencyCompensation." ;
  rdfs:domain      reso:Property ;
  rdfs:label       "SubAgencyCompensationType" ;
  rdfs:range       enum:CompensationType ;
  reso:CertificationLevel "Bronze" ;
  reso:PropertyTypes "RESI","RLSE","RINC","LAND","MOBI","FARM","COMS","COML","BUSO" ;
  schema:sameAs    <http://ddwiki.reso.org/display/DDW/SubAgencyCompensationType+Field> ;
  vs:term_status   "stable"
.
reso:SubdivisionName a rdf:Property ;
  rdfs:comment     "A neighborhood, community, complex or builder tract." ;
  rdfs:domain      reso:Property ;
  rdfs:label       "SubdivisionName" ;
  rdfs:range       xsd:string ;
  reso:CertificationLevel "Core" ;
  reso:PropertyTypes "RESI","RLSE","RINC","LAND","MOBI","FARM","COMS","COML","BUSO" ;
  schema:sameAs    <http://ddwiki.reso.org/display/DDW/SubdivisionName+Field> ;
  vs:term_status   "stable"
.
reso:SuppliesExpense a rdf:Property ;
  rdfs:comment     "The annual expense that is not paid directly by the tenant and is included in the Operating Expense calculations." ;
  rdfs:domain      reso:Property ;
  rdfs:label       "SuppliesExpense" ;
  rdfs:range       xsd:decimal ;
  reso:CertificationLevel "Silver" ;
  reso:PropertyTypes "RINC" ;
  schema:sameAs    <http://ddwiki.reso.org/display/DDW/SuppliesExpense+Field> ;
  vs:term_status   "stable"
.
reso:SyndicateTo a rdf:Property ;
  rdfs:comment     "When permitted by the broker, the options made by the agent on behalf of the seller, where they would like their listings syndicated.  i.e. Zillow, Trulia, Homes.com, etc." ;
  rdfs:domain      reso:Property ;
  rdfs:label       "SyndicateTo" ;
  rdfs:range       xsd:string ;
  reso:CertificationLevel "Gold" ;
  reso:PropertyTypes "RESI","RLSE","RINC","LAND","MOBI","FARM","COMS","COML","BUSO" ;
  schema:sameAs    <http://ddwiki.reso.org/display/DDW/SyndicateTo+Field> ;
  vs:term_status   "stable"
.
reso:SyndicationRemarks a rdf:Property ;
  rdfs:comment     "Becoming more common in the industry, MLS's are hosting a separate \"Public Remarks\" for syndication purposes.  This field should be defaulted to containing the Public Remarks, but upon broker decision, modified to include contact and other information denied by IDX rules, but allowed under local and national regulations." ;
  rdfs:domain      reso:Property ;
  rdfs:label       "SyndicationRemarks" ;
  rdfs:range       xsd:string ;
  reso:CertificationLevel "Core" ;
  reso:PropertyTypes "RESI","RLSE","RINC","LAND","MOBI","FARM","COMS","COML","BUSO" ;
  schema:sameAs    <http://ddwiki.reso.org/display/DDW/SyndicationRemarks+Field> ;
  vs:term_status   "stable"
.
reso:TaxAnnualAmount a rdf:Property ;
  rdfs:comment     "The annual property tax amount as of the last assessment made by the taxing authority." ;
  rdfs:domain      reso:Property ;
  rdfs:label       "TaxAnnualAmount" ;
  rdfs:range       xsd:decimal ;
  reso:CertificationLevel "Silver" ;
  reso:PropertyTypes "RESI","RINC","LAND","MOBI","FARM","COMS","COML" ;
  schema:sameAs    <http://ddwiki.reso.org/display/DDW/TaxAnnualAmount+Field> ;
  vs:term_status   "stable"
.
reso:TaxAssessedValue a rdf:Property ;
  rdfs:comment     "The property value as of the last assessment made by the taxing authority." ;
  rdfs:domain      reso:Property ;
  rdfs:label       "TaxAssessedValue" ;
  rdfs:range       xsd:decimal ;
  reso:CertificationLevel "Silver" ;
  reso:PropertyTypes "RESI","RINC","LAND","MOBI","FARM" ;
  schema:sameAs    <http://ddwiki.reso.org/display/DDW/TaxAssessedValue+Field> ;
  vs:term_status   "stable"
.
reso:TaxBlock a rdf:Property ;
  rdfs:comment     "A type of legal description for land in developed areas where streets or other rights-of-ways delineate large parcels of land referred to as divided into lots on which homes or other types of developments are built.  An example would read \"Lot 12 of Block 45 of Tract 3002 of the City of San Dunes, Desert County.\" Such a description would also reference an official plat filed with the clerk or recorder for that area which shows the location of the block and often the dimensions of the lots therein." ;
  rdfs:domain      reso:Property ;
  rdfs:label       "TaxBlock" ;
  rdfs:range       xsd:string ;
  reso:CertificationLevel "Bronze" ;
  reso:PropertyTypes "RESI","RINC","LAND","MOBI","FARM","COMS","COML" ;
  schema:sameAs    <http://ddwiki.reso.org/display/DDW/TaxBlock+Field> ;
  vs:term_status   "stable"
.
reso:TaxBookNumber a rdf:Property ;
  rdfs:comment     "Some systems of parcel identification incorporate a method which utilizes a county identifier, a tax book number, a tax map number and a parcel identification number." ;
  rdfs:domain      reso:Property ;
  rdfs:label       "TaxBookNumber" ;
  rdfs:range       xsd:string ;
  reso:CertificationLevel "Bronze" ;
  reso:PropertyTypes "RESI","RINC","LAND","MOBI","FARM" ;
  schema:sameAs    <http://ddwiki.reso.org/display/DDW/TaxBookNumber+Field> ;
  vs:term_status   "stable"
.
reso:TaxExemptions a rdf:Property ;
  rdfs:comment     "A list of tax exemptions as they relate to the property." ;
  rdfs:domain      reso:Property ;
  rdfs:label       "TaxExemptions" ;
  rdfs:range       xsd:string ;
  reso:CertificationLevel "Silver" ;
  reso:PropertyTypes "RESI","RINC","LAND","MOBI","FARM" ;
  schema:sameAs    <http://ddwiki.reso.org/display/DDW/TaxExemptions+Field> ;
  vs:term_status   "stable"
.
reso:TaxLegalDescription a rdf:Property ;
  rdfs:comment     "A type of legal description for land in developed areas where streets or other rights-of-ways delineate large parcels of land referred to as divided into lots on which homes or other types of developments are built.  An example would read \"Lot 12 of Block 45 of Tract 3002 of the City of San Dunes, Desert County.\" Such a description would also reference an official plat filed with the clerk or recorder for that area which shows the location of the block and often the dimensions of the lots therein. The text here is also an index into the property as described by the County Recorder." ;
  rdfs:domain      reso:Property ;
  rdfs:label       "TaxLegalDescription" ;
  rdfs:range       xsd:string ;
  reso:CertificationLevel "Bronze" ;
  reso:PropertyTypes "RESI","RINC","LAND","MOBI","FARM","COMS","COML" ;
  schema:sameAs    <http://ddwiki.reso.org/display/DDW/TaxLegalDescription+Field> ;
  vs:term_status   "stable"
.
reso:TaxLot a rdf:Property ;
  rdfs:comment     "A type of legal description for land in developed areas where streets or other rights-of-ways delineate large parcels of land referred to as divided into lots on which homes or other types of developments are built.  An example would read \"Lot 12 of Block 45 of Tract 3002 of the City of San Dunes, Desert County.\" Such a description would also reference an official plat filed with the clerk or recorder for that area which shows the location of the block and often the dimensions of the lots therein." ;
  rdfs:domain      reso:Property ;
  rdfs:label       "TaxLot" ;
  rdfs:range       xsd:string ;
  reso:CertificationLevel "Bronze" ;
  reso:PropertyTypes "RESI","RINC","LAND","MOBI","FARM","COMS","COML" ;
  schema:sameAs    <http://ddwiki.reso.org/display/DDW/TaxLot+Field> ;
  vs:term_status   "stable"
.
reso:TaxMapNumber a rdf:Property ;
  rdfs:comment     "Some systems of parcel identification incorporate a method which utilizes a county identifier, a tax book number, a tax map number and a parcel identification number." ;
  rdfs:domain      reso:Property ;
  rdfs:label       "TaxMapNumber" ;
  rdfs:range       xsd:string ;
  reso:CertificationLevel "Bronze" ;
  reso:PropertyTypes "RESI","RINC","LAND","MOBI","FARM" ;
  schema:sameAs    <http://ddwiki.reso.org/display/DDW/TaxMapNumber+Field> ;
  vs:term_status   "stable"
.
reso:TaxOtherAnnualAssessmentAmount a rdf:Property ;
  rdfs:comment     "Any other annual taxes, not including the tax reported in the TaxAmount field, as of the last assessment made by the taxing authority." ;
  rdfs:domain      reso:Property ;
  rdfs:label       "TaxOtherAnnualAssessmentAmount" ;
  rdfs:range       xsd:decimal ;
  reso:CertificationLevel "Silver" ;
  reso:PropertyTypes "RESI","RINC","LAND","MOBI","FARM","COMS","COML" ;
  schema:sameAs    <http://ddwiki.reso.org/display/DDW/TaxOtherAnnualAssessmentAmount+Field> ;
  vs:term_status   "stable"
.
reso:TaxParcelLetter a rdf:Property ;
  rdfs:comment     "Some systems of parcel identification incorporate a method which utilizes a county identifier, a tax book number, a tax map number and a parcel identification number." ;
  rdfs:domain      reso:Property ;
  rdfs:label       "TaxParcelLetter" ;
  rdfs:range       xsd:string ;
  reso:CertificationLevel "Bronze" ;
  reso:PropertyTypes "RESI","RLSE","RINC","LAND","MOBI","FARM" ;
  schema:sameAs    <http://ddwiki.reso.org/display/DDW/TaxParcelLetter+Field> ;
  vs:term_status   "stable"
.
reso:TaxStatusCurrent a rdf:Property ;
  rdfs:comment     "The current tax status of the mobile home in cases where the land or space is included in the sale." ;
  rdfs:domain      reso:Property ;
  rdfs:label       "TaxStatusCurrent" ;
  rdfs:range       xsd:string ;
  reso:CertificationLevel "Silver" ;
  reso:PropertyTypes "MOBI" ;
  schema:sameAs    <http://ddwiki.reso.org/display/DDW/TaxStatusCurrent+Field> ;
  vs:term_status   "stable"
.
reso:TaxTract a rdf:Property ;
  rdfs:comment     "A type of legal description for land in developed areas where streets or other rights-of-ways delineate large parcels of land referred to as divided into lots on which homes or other types of developments are built.  An example would read \"Lot 12 of Block 45 of Tract 3002 of the City of San Dunes, Desert County.\" Such a description would also reference an official plat filed with the clerk or recorder for that area which shows the location of the block and often the dimensions of the lots therein." ;
  rdfs:domain      reso:Property ;
  rdfs:label       "TaxTract" ;
  rdfs:range       xsd:string ;
  reso:CertificationLevel "Bronze" ;
  reso:PropertyTypes "RESI","RINC","LAND","MOBI","FARM","COMS","COML" ;
  schema:sameAs    <http://ddwiki.reso.org/display/DDW/TaxTract+Field> ;
  vs:term_status   "stable"
.
reso:TaxYear a rdf:Property ;
  rdfs:comment     "The year in with the last assessment of the property value/tax was made." ;
  rdfs:domain      reso:Property ;
  rdfs:label       "TaxYear" ;
  rdfs:range       xsd:decimal ;
  reso:CertificationLevel "Silver" ;
  reso:PropertyTypes "RESI","RINC","LAND","MOBI","FARM","COMS","COML" ;
  schema:sameAs    <http://ddwiki.reso.org/display/DDW/TaxYear+Field> ;
  vs:term_status   "stable"
.
reso:Telephone a rdf:Property ;
  rdfs:domain      reso:Property ;
  rdfs:label       "Telephone" ;
  rdfs:range       xsd:string ;
  reso:CertificationLevel "Bronze" ;
  reso:PropertyTypes "RESI","RLSE","RINC","LAND","MOBI","FARM" ;
  schema:sameAs    <http://ddwiki.reso.org/display/DDW/Telephone+Field> ;
  vs:term_status   "stable"
.
reso:TenantPays a rdf:Property ;
  rdfs:comment     "A list of services or items that the tenant is responsible to pay." ;
  rdfs:domain      reso:Property ;
  rdfs:label       "TenantPays" ;
  rdfs:range       enum:TenantPays ;
  reso:CertificationLevel "Bronze" ;
  reso:PropertyTypes "RLSE","RINC","COMS","COML" ;
  schema:sameAs    <http://ddwiki.reso.org/display/DDW/TenantPays+Field> ;
  vs:term_status   "stable"
.
reso:Topography a rdf:Property ;
  rdfs:comment     "The state of the surface of the land included with the property.  i.e. flat, rolling, etc." ;
  rdfs:domain      reso:Property ;
  rdfs:label       "Topography" ;
  rdfs:range       xsd:string ;
  reso:CertificationLevel "Platinum" ;
  reso:PropertyTypes "LAND","COMS","COML" ;
  schema:sameAs    <http://ddwiki.reso.org/display/DDW/Topography+Field> ;
  vs:term_status   "stable"
.
reso:TotalActualRent a rdf:Property ;
  rdfs:comment     "Total actual rent currently being collected from tenants of the income property." ;
  rdfs:domain      reso:Property ;
  rdfs:label       "TotalActualRent" ;
  rdfs:range       xsd:decimal ;
  reso:CertificationLevel "Bronze" ;
  reso:PropertyTypes "RINC","COMS","COML" ;
  schema:sameAs    <http://ddwiki.reso.org/display/DDW/TotalActualRent+Field> ;
  vs:term_status   "stable"
.
reso:Township a rdf:Property ;
  rdfs:comment     "A subdivision of the county." ;
  rdfs:domain      reso:Property ;
  rdfs:label       "Township" ;
  rdfs:range       xsd:string ;
  reso:CertificationLevel "Core" ;
  reso:PropertyTypes "RESI","RLSE","RINC","LAND","MOBI","FARM","COMS","COML","BUSO" ;
  schema:sameAs    <http://ddwiki.reso.org/display/DDW/Township+Field> ;
  vs:term_status   "stable"
.
reso:TransactionBrokerCompensation a rdf:Property ;
  rdfs:comment     "The total commission to be paid to the transaction facilitator, expressed as either a percentage or a constant currency amount." ;
  rdfs:domain      reso:Property ;
  rdfs:label       "TransactionBrokerCompensation" ;
  rdfs:range       xsd:string ;
  reso:CertificationLevel "Bronze" ;
  reso:PropertyTypes "RESI","RLSE","RINC","LAND","MOBI","FARM","COMS","COML","BUSO" ;
  schema:sameAs    <http://ddwiki.reso.org/display/DDW/TransactionBrokerCompensation+Field> ;
  vs:term_status   "stable"
.
reso:TransactionBrokerCompensationType a rdf:Property ;
  rdfs:comment     "A list of types to clarify the value entered in the TransactionBrokerCompensation field.  For example $, % or some other clarification of the TransactionBrokerCompensation." ;
  rdfs:domain      reso:Property ;
  rdfs:label       "TransactionBrokerCompensationType" ;
  rdfs:range       enum:CompensationType ;
  reso:CertificationLevel "Bronze" ;
  reso:PropertyTypes "RESI","RLSE","RINC","LAND","MOBI","FARM","COMS","COML","BUSO" ;
  schema:sameAs    <http://ddwiki.reso.org/display/DDW/TransactionBrokerCompensationType+Field> ;
  vs:term_status   "stable"
.
reso:TrashExpense a rdf:Property ;
  rdfs:comment     "The annual expense that is not paid directly by the tenant and is included in the Operating Expense calculations." ;
  rdfs:domain      reso:Property ;
  rdfs:label       "TrashExpense" ;
  rdfs:range       xsd:decimal ;
  reso:CertificationLevel "Silver" ;
  reso:PropertyTypes "RINC","COMS","COML" ;
  schema:sameAs    <http://ddwiki.reso.org/display/DDW/TrashExpense+Field> ;
  vs:term_status   "stable"
.
reso:UnitNumber a rdf:Property ;
  rdfs:domain      reso:Property ;
  rdfs:label       "UnitNumber" ;
  rdfs:range       xsd:string ;
  reso:CertificationLevel "Core" ;
  reso:PropertyTypes "RESI","RLSE","RINC","MOBI","FARM","COMS","COML","BUSO" ;
  schema:sameAs    <http://ddwiki.reso.org/display/DDW/UnitNumber+Field> ;
  vs:term_status   "stable"
.
reso:UnitTypeType a rdf:Property ;
  rdfs:comment     "This field is a list of the types used in the Unit Type repeating elements. The Type is a list of possible Unit Types. i.e. 1, 2, 3 or 2 Bed, Studio, Special Loft, etc. Each selected are expected to appear as the \"[type]\" in the related UnitType fields in a flattened implementation (RETS 1.x only) of the room fields. A relational implementation of UnitTypes must omit the type from the field name and use UnitTypeType to create a vertical representation of the various unit types. The fact that the field repeats the word \"type\" is intentional." ;
  rdfs:domain      reso:Property ;
  rdfs:label       "UnitTypeType" ;
  rdfs:range       xsd:string ;
  reso:CertificationLevel "Gold" ;
  reso:PropertyTypes "RINC","COMS","COML" ;
  schema:sameAs    <http://ddwiki.reso.org/display/DDW/UnitTypeType+Field> ;
  vs:term_status   "stable"
.
reso:UnitType a rdf:Property ;
  rdfs:comment     "[type] This field is a repeating element for each type of unit selected in the UnitType field. For every UnitType there are two possible implementations. For a flat implementation (RETS 1.x only), each UnitTypeType used is expected to appear as the \"[type]\" in the related rooms field name. i.e. UnitTypeStudioActualRent. A relational implementation of UnitType must omit the type from the field name and use UnitTypeType to create a vertical representation of the various rooms. i.e. UnitTypeActualRent with Studio in the relational table's UnitType field." ;
  rdfs:domain      reso:Property ;
  rdfs:label       "UnitType" ;
  rdfs:range       xsd:decimal ;
  reso:CertificationLevel "Gold" ;
  reso:PropertyTypes "RINC","COMS","COML" ;
  schema:sameAs    <http://ddwiki.reso.org/display/DDW/UnitType%5Btype%5DActualRent+Field> ;
  vs:term_status   "stable"
.
reso:UnitType a rdf:Property ;
  rdfs:comment     "[type] This field is a repeating element for each type of unit selected in the UnitType field. For every UnitType there are two possible implementations. For a flat implementation (RETS 1.x only), each UnitTypeType used is expected to appear as the \"[type]\" in the related rooms field name. i.e. UnitTypeStudioActualRent. A relational implementation of UnitType must omit the type from the field name and use UnitTypeType to create a vertical representation of the various rooms. i.e. UnitTypeActualRent with Studio in the relational table's UnitType field.","[type] This field is a repeating element for each type of unit selected in the UnitType field. For every UnitType there are two possible implementations. For a flat implementation (RETS 1.x only), each UnitTypeType used is expected to appear as the \"[type]\" in the related rooms field name. i.e. UnitTypeStudioBathsTotal. A relational implementation of UnitType must omit the type from the field name and use UnitTypeType to create a vertical representation of the various rooms. i.e. UnitTypeBathsTotal with Studio in the relational table's UnitType field." ;
  rdfs:domain      reso:Property ;
  rdfs:label       "UnitType" ;
  rdfs:range       xsd:decimal ;
  reso:CertificationLevel "Gold" ;
  reso:PropertyTypes "RINC","COMS","COML" ;
  schema:sameAs    <http://ddwiki.reso.org/display/DDW/UnitType%5Btype%5DActualRent+Field>,<http://ddwiki.reso.org/display/DDW/UnitType%5Btype%5DBathsTotal+Field> ;
  vs:term_status   "stable"
.
reso:UnitType a rdf:Property ;
  rdfs:comment     "[type] This field is a repeating element for each type of unit selected in the UnitType field. For every UnitType there are two possible implementations. For a flat implementation (RETS 1.x only), each UnitTypeType used is expected to appear as the \"[type]\" in the related rooms field name. i.e. UnitTypeStudioActualRent. A relational implementation of UnitType must omit the type from the field name and use UnitTypeType to create a vertical representation of the various rooms. i.e. UnitTypeActualRent with Studio in the relational table's UnitType field.","[type] This field is a repeating element for each type of unit selected in the UnitType field. For every UnitType there are two possible implementations. For a flat implementation (RETS 1.x only), each UnitTypeType used is expected to appear as the \"[type]\" in the related rooms field name. i.e. UnitTypeStudioBathsTotal. A relational implementation of UnitType must omit the type from the field name and use UnitTypeType to create a vertical representation of the various rooms. i.e. UnitTypeBathsTotal with Studio in the relational table's UnitType field.","[type] This field is a repeating element for each type of unit selected in the UnitType field. For every UnitType there are two possible implementations. For a flat implementation (RETS 1.x only), each UnitTypeType used is expected to appear as the \"[type]\" in the related rooms field name. i.e. UnitTypeStudioBedsTotal. A relational implementation of UnitType must omit the type from the field name and use UnitTypeType to create a vertical representation of the various rooms. i.e. UnitTypeBedsTotal with Studio in the relational table's UnitType field." ;
  rdfs:domain      reso:Property ;
  rdfs:label       "UnitType" ;
  rdfs:range       xsd:decimal ;
  reso:CertificationLevel "Gold" ;
  reso:PropertyTypes "RINC","COMS","COML" ;
  schema:sameAs    <http://ddwiki.reso.org/display/DDW/UnitType%5Btype%5DActualRent+Field>,<http://ddwiki.reso.org/display/DDW/UnitType%5Btype%5DBathsTotal+Field>,<http://ddwiki.reso.org/display/DDW/UnitType%5Btype%5DBedsTotal+Field> ;
  vs:term_status   "stable"
.
reso:UnitType a rdf:Property ;
  rdfs:comment     "[type] This field is a repeating element for each type of unit selected in the UnitType field. For every UnitType there are two possible implementations. For a flat implementation (RETS 1.x only), each UnitTypeType used is expected to appear as the \"[type]\" in the related rooms field name. i.e. UnitTypeStudioActualRent. A relational implementation of UnitType must omit the type from the field name and use UnitTypeType to create a vertical representation of the various rooms. i.e. UnitTypeActualRent with Studio in the relational table's UnitType field.","[type] This field is a repeating element for each type of unit selected in the UnitType field. For every UnitType there are two possible implementations. For a flat implementation (RETS 1.x only), each UnitTypeType used is expected to appear as the \"[type]\" in the related rooms field name. i.e. UnitTypeStudioBathsTotal. A relational implementation of UnitType must omit the type from the field name and use UnitTypeType to create a vertical representation of the various rooms. i.e. UnitTypeBathsTotal with Studio in the relational table's UnitType field.","[type] This field is a repeating element for each type of unit selected in the UnitType field. For every UnitType there are two possible implementations. For a flat implementation (RETS 1.x only), each UnitTypeType used is expected to appear as the \"[type]\" in the related rooms field name. i.e. UnitTypeStudioBedsTotal. A relational implementation of UnitType must omit the type from the field name and use UnitTypeType to create a vertical representation of the various rooms. i.e. UnitTypeBedsTotal with Studio in the relational table's UnitType field.","[type] This field is a repeating element for each type of unit selected in the UnitType field. For every UnitType there are two possible implementations. For a flat implementation (RETS 1.x only), each UnitTypeType used is expected to appear as the \"[type]\" in the related rooms field name. i.e. UnitTypeStudioDescription. A relational implementation of UnitType must omit the type from the field name and use UnitTypeType to create a vertical representation of the various rooms. i.e. UnitTypeDescription with Studio in the relational table's UnitType field." ;
  rdfs:domain      reso:Property ;
  rdfs:label       "UnitType" ;
  rdfs:range       xsd:decimal,xsd:string ;
  reso:CertificationLevel "Gold" ;
  reso:PropertyTypes "RINC","COMS","COML" ;
  schema:sameAs    <http://ddwiki.reso.org/display/DDW/UnitType%5Btype%5DActualRent+Field>,<http://ddwiki.reso.org/display/DDW/UnitType%5Btype%5DBathsTotal+Field>,<http://ddwiki.reso.org/display/DDW/UnitType%5Btype%5DBedsTotal+Field>,<http://ddwiki.reso.org/display/DDW/UnitType%5Btype%5DDescription+Field> ;
  vs:term_status   "stable"
.
reso:UnitType a rdf:Property ;
  rdfs:comment     "[type] This field is a repeating element for each type of unit selected in the UnitType field. For every UnitType there are two possible implementations. For a flat implementation (RETS 1.x only), each UnitTypeType used is expected to appear as the \"[type]\" in the related rooms field name. i.e. UnitTypeStudioActualRent. A relational implementation of UnitType must omit the type from the field name and use UnitTypeType to create a vertical representation of the various rooms. i.e. UnitTypeActualRent with Studio in the relational table's UnitType field.","[type] This field is a repeating element for each type of unit selected in the UnitType field. For every UnitType there are two possible implementations. For a flat implementation (RETS 1.x only), each UnitTypeType used is expected to appear as the \"[type]\" in the related rooms field name. i.e. UnitTypeStudioBathsTotal. A relational implementation of UnitType must omit the type from the field name and use UnitTypeType to create a vertical representation of the various rooms. i.e. UnitTypeBathsTotal with Studio in the relational table's UnitType field.","[type] This field is a repeating element for each type of unit selected in the UnitType field. For every UnitType there are two possible implementations. For a flat implementation (RETS 1.x only), each UnitTypeType used is expected to appear as the \"[type]\" in the related rooms field name. i.e. UnitTypeStudioBedsTotal. A relational implementation of UnitType must omit the type from the field name and use UnitTypeType to create a vertical representation of the various rooms. i.e. UnitTypeBedsTotal with Studio in the relational table's UnitType field.","[type] This field is a repeating element for each type of unit selected in the UnitType field. For every UnitType there are two possible implementations. For a flat implementation (RETS 1.x only), each UnitTypeType used is expected to appear as the \"[type]\" in the related rooms field name. i.e. UnitTypeStudioDescription. A relational implementation of UnitType must omit the type from the field name and use UnitTypeType to create a vertical representation of the various rooms. i.e. UnitTypeDescription with Studio in the relational table's UnitType field.","[type] This field is a repeating element for each type of unit selected in the UnitType field. For every UnitType there are two possible implementations. For a flat implementation (RETS 1.x only), each UnitTypeType used is expected to appear as the \"[type]\" in the related rooms field name. i.e. UnitTypeStudioFurnished. A relational implementation of UnitType must omit the type from the field name and use UnitTypeType to create a vertical representation of the various rooms. i.e. UnitTypeFurnished with Studio in the relational table's UnitType field." ;
  rdfs:domain      reso:Property ;
  rdfs:label       "UnitType" ;
  rdfs:range       xsd:decimal,xsd:string ;
  reso:CertificationLevel "Gold" ;
  reso:PropertyTypes "RINC","COMS","COML" ;
  schema:sameAs    <http://ddwiki.reso.org/display/DDW/UnitType%5Btype%5DActualRent+Field>,<http://ddwiki.reso.org/display/DDW/UnitType%5Btype%5DBathsTotal+Field>,<http://ddwiki.reso.org/display/DDW/UnitType%5Btype%5DBedsTotal+Field>,<http://ddwiki.reso.org/display/DDW/UnitType%5Btype%5DDescription+Field>,<http://ddwiki.reso.org/display/DDW/UnitType%5Btype%5DFurnished+Field> ;
  vs:term_status   "stable"
.
reso:UnitType a rdf:Property ;
  rdfs:comment     "[type] This field is a repeating element for each type of unit selected in the UnitType field. For every UnitType there are two possible implementations. For a flat implementation (RETS 1.x only), each UnitTypeType used is expected to appear as the \"[type]\" in the related rooms field name. i.e. UnitTypeStudioActualRent. A relational implementation of UnitType must omit the type from the field name and use UnitTypeType to create a vertical representation of the various rooms. i.e. UnitTypeActualRent with Studio in the relational table's UnitType field.","[type] This field is a repeating element for each type of unit selected in the UnitType field. For every UnitType there are two possible implementations. For a flat implementation (RETS 1.x only), each UnitTypeType used is expected to appear as the \"[type]\" in the related rooms field name. i.e. UnitTypeStudioBathsTotal. A relational implementation of UnitType must omit the type from the field name and use UnitTypeType to create a vertical representation of the various rooms. i.e. UnitTypeBathsTotal with Studio in the relational table's UnitType field.","[type] This field is a repeating element for each type of unit selected in the UnitType field. For every UnitType there are two possible implementations. For a flat implementation (RETS 1.x only), each UnitTypeType used is expected to appear as the \"[type]\" in the related rooms field name. i.e. UnitTypeStudioBedsTotal. A relational implementation of UnitType must omit the type from the field name and use UnitTypeType to create a vertical representation of the various rooms. i.e. UnitTypeBedsTotal with Studio in the relational table's UnitType field.","[type] This field is a repeating element for each type of unit selected in the UnitType field. For every UnitType there are two possible implementations. For a flat implementation (RETS 1.x only), each UnitTypeType used is expected to appear as the \"[type]\" in the related rooms field name. i.e. UnitTypeStudioDescription. A relational implementation of UnitType must omit the type from the field name and use UnitTypeType to create a vertical representation of the various rooms. i.e. UnitTypeDescription with Studio in the relational table's UnitType field.","[type] This field is a repeating element for each type of unit selected in the UnitType field. For every UnitType there are two possible implementations. For a flat implementation (RETS 1.x only), each UnitTypeType used is expected to appear as the \"[type]\" in the related rooms field name. i.e. UnitTypeStudioFurnished. A relational implementation of UnitType must omit the type from the field name and use UnitTypeType to create a vertical representation of the various rooms. i.e. UnitTypeFurnished with Studio in the relational table's UnitType field.","[type] This field is a repeating element for each type of unit selected in the UnitType field. For every UnitType there are two possible implementations. For a flat implementation (RETS 1.x only), each UnitTypeType used is expected to appear as the \"[type]\" in the related rooms field name. i.e. UnitTypeStudioGarageAttachedYN. A relational implementation of UnitType must omit the type from the field name and use UnitTypeType to create a vertical representation of the various rooms. i.e. UnitTypeGarageAttachedYN with Studio in the relational table's UnitType field." ;
  rdfs:domain      reso:Property ;
  rdfs:label       "UnitType" ;
  rdfs:range       xsd:decimal,xsd:string,xsd:boolean ;
  reso:CertificationLevel "Gold" ;
  reso:PropertyTypes "RINC","COMS","COML" ;
  schema:sameAs    <http://ddwiki.reso.org/display/DDW/UnitType%5Btype%5DActualRent+Field>,<http://ddwiki.reso.org/display/DDW/UnitType%5Btype%5DBathsTotal+Field>,<http://ddwiki.reso.org/display/DDW/UnitType%5Btype%5DBedsTotal+Field>,<http://ddwiki.reso.org/display/DDW/UnitType%5Btype%5DDescription+Field>,<http://ddwiki.reso.org/display/DDW/UnitType%5Btype%5DFurnished+Field>,<http://ddwiki.reso.org/display/DDW/UnitType%5Btype%5DGarageAttachedYN+Field> ;
  vs:term_status   "stable"
.
reso:UnitType a rdf:Property ;
  rdfs:comment     "[type] This field is a repeating element for each type of unit selected in the UnitType field. For every UnitType there are two possible implementations. For a flat implementation (RETS 1.x only), each UnitTypeType used is expected to appear as the \"[type]\" in the related rooms field name. i.e. UnitTypeStudioActualRent. A relational implementation of UnitType must omit the type from the field name and use UnitTypeType to create a vertical representation of the various rooms. i.e. UnitTypeActualRent with Studio in the relational table's UnitType field.","[type] This field is a repeating element for each type of unit selected in the UnitType field. For every UnitType there are two possible implementations. For a flat implementation (RETS 1.x only), each UnitTypeType used is expected to appear as the \"[type]\" in the related rooms field name. i.e. UnitTypeStudioBathsTotal. A relational implementation of UnitType must omit the type from the field name and use UnitTypeType to create a vertical representation of the various rooms. i.e. UnitTypeBathsTotal with Studio in the relational table's UnitType field.","[type] This field is a repeating element for each type of unit selected in the UnitType field. For every UnitType there are two possible implementations. For a flat implementation (RETS 1.x only), each UnitTypeType used is expected to appear as the \"[type]\" in the related rooms field name. i.e. UnitTypeStudioBedsTotal. A relational implementation of UnitType must omit the type from the field name and use UnitTypeType to create a vertical representation of the various rooms. i.e. UnitTypeBedsTotal with Studio in the relational table's UnitType field.","[type] This field is a repeating element for each type of unit selected in the UnitType field. For every UnitType there are two possible implementations. For a flat implementation (RETS 1.x only), each UnitTypeType used is expected to appear as the \"[type]\" in the related rooms field name. i.e. UnitTypeStudioDescription. A relational implementation of UnitType must omit the type from the field name and use UnitTypeType to create a vertical representation of the various rooms. i.e. UnitTypeDescription with Studio in the relational table's UnitType field.","[type] This field is a repeating element for each type of unit selected in the UnitType field. For every UnitType there are two possible implementations. For a flat implementation (RETS 1.x only), each UnitTypeType used is expected to appear as the \"[type]\" in the related rooms field name. i.e. UnitTypeStudioFurnished. A relational implementation of UnitType must omit the type from the field name and use UnitTypeType to create a vertical representation of the various rooms. i.e. UnitTypeFurnished with Studio in the relational table's UnitType field.","[type] This field is a repeating element for each type of unit selected in the UnitType field. For every UnitType there are two possible implementations. For a flat implementation (RETS 1.x only), each UnitTypeType used is expected to appear as the \"[type]\" in the related rooms field name. i.e. UnitTypeStudioGarageAttachedYN. A relational implementation of UnitType must omit the type from the field name and use UnitTypeType to create a vertical representation of the various rooms. i.e. UnitTypeGarageAttachedYN with Studio in the relational table's UnitType field.","[type] This field is a repeating element for each type of unit selected in the UnitType field. For every UnitType there are two possible implementations. For a flat implementation (RETS 1.x only), each UnitTypeType used is expected to appear as the \"[type]\" in the related rooms field name. i.e. UnitTypeStudioGarageSpaces. A relational implementation of UnitType must omit the type from the field name and use UnitTypeType to create a vertical representation of the various rooms. i.e. UnitTypeGarageSpaces with Studio in the relational table's UnitType field." ;
  rdfs:domain      reso:Property ;
  rdfs:label       "UnitType" ;
  rdfs:range       xsd:decimal,xsd:string,xsd:boolean ;
  reso:CertificationLevel "Gold" ;
  reso:PropertyTypes "RINC","COMS","COML" ;
  schema:sameAs    <http://ddwiki.reso.org/display/DDW/UnitType%5Btype%5DActualRent+Field>,<http://ddwiki.reso.org/display/DDW/UnitType%5Btype%5DBathsTotal+Field>,<http://ddwiki.reso.org/display/DDW/UnitType%5Btype%5DBedsTotal+Field>,<http://ddwiki.reso.org/display/DDW/UnitType%5Btype%5DDescription+Field>,<http://ddwiki.reso.org/display/DDW/UnitType%5Btype%5DFurnished+Field>,<http://ddwiki.reso.org/display/DDW/UnitType%5Btype%5DGarageAttachedYN+Field>,<http://ddwiki.reso.org/display/DDW/UnitType%5Btype%5DGarageSpaces+Field> ;
  vs:term_status   "stable"
.
reso:UnitType a rdf:Property ;
  rdfs:comment     "[type] This field is a repeating element for each type of unit selected in the UnitType field. For every UnitType there are two possible implementations. For a flat implementation (RETS 1.x only), each UnitTypeType used is expected to appear as the \"[type]\" in the related rooms field name. i.e. UnitTypeStudioActualRent. A relational implementation of UnitType must omit the type from the field name and use UnitTypeType to create a vertical representation of the various rooms. i.e. UnitTypeActualRent with Studio in the relational table's UnitType field.","[type] This field is a repeating element for each type of unit selected in the UnitType field. For every UnitType there are two possible implementations. For a flat implementation (RETS 1.x only), each UnitTypeType used is expected to appear as the \"[type]\" in the related rooms field name. i.e. UnitTypeStudioBathsTotal. A relational implementation of UnitType must omit the type from the field name and use UnitTypeType to create a vertical representation of the various rooms. i.e. UnitTypeBathsTotal with Studio in the relational table's UnitType field.","[type] This field is a repeating element for each type of unit selected in the UnitType field. For every UnitType there are two possible implementations. For a flat implementation (RETS 1.x only), each UnitTypeType used is expected to appear as the \"[type]\" in the related rooms field name. i.e. UnitTypeStudioBedsTotal. A relational implementation of UnitType must omit the type from the field name and use UnitTypeType to create a vertical representation of the various rooms. i.e. UnitTypeBedsTotal with Studio in the relational table's UnitType field.","[type] This field is a repeating element for each type of unit selected in the UnitType field. For every UnitType there are two possible implementations. For a flat implementation (RETS 1.x only), each UnitTypeType used is expected to appear as the \"[type]\" in the related rooms field name. i.e. UnitTypeStudioDescription. A relational implementation of UnitType must omit the type from the field name and use UnitTypeType to create a vertical representation of the various rooms. i.e. UnitTypeDescription with Studio in the relational table's UnitType field.","[type] This field is a repeating element for each type of unit selected in the UnitType field. For every UnitType there are two possible implementations. For a flat implementation (RETS 1.x only), each UnitTypeType used is expected to appear as the \"[type]\" in the related rooms field name. i.e. UnitTypeStudioFurnished. A relational implementation of UnitType must omit the type from the field name and use UnitTypeType to create a vertical representation of the various rooms. i.e. UnitTypeFurnished with Studio in the relational table's UnitType field.","[type] This field is a repeating element for each type of unit selected in the UnitType field. For every UnitType there are two possible implementations. For a flat implementation (RETS 1.x only), each UnitTypeType used is expected to appear as the \"[type]\" in the related rooms field name. i.e. UnitTypeStudioGarageAttachedYN. A relational implementation of UnitType must omit the type from the field name and use UnitTypeType to create a vertical representation of the various rooms. i.e. UnitTypeGarageAttachedYN with Studio in the relational table's UnitType field.","[type] This field is a repeating element for each type of unit selected in the UnitType field. For every UnitType there are two possible implementations. For a flat implementation (RETS 1.x only), each UnitTypeType used is expected to appear as the \"[type]\" in the related rooms field name. i.e. UnitTypeStudioGarageSpaces. A relational implementation of UnitType must omit the type from the field name and use UnitTypeType to create a vertical representation of the various rooms. i.e. UnitTypeGarageSpaces with Studio in the relational table's UnitType field.","[type] This field is a repeating element for each type of unit selected in the UnitType field. For every UnitType there are two possible implementations. For a flat implementation (RETS 1.x only), each UnitTypeType used is expected to appear as the \"[type]\" in the related rooms field name. i.e. UnitTypeStudioProForma. A relational implementation of UnitType must omit the type from the field name and use UnitTypeType to create a vertical representation of the various rooms. i.e. UnitTypeProForma with Studio in the relational table's UnitType field." ;
  rdfs:domain      reso:Property ;
  rdfs:label       "UnitType" ;
  rdfs:range       xsd:decimal,xsd:string,xsd:boolean ;
  reso:CertificationLevel "Gold" ;
  reso:PropertyTypes "RINC","COMS","COML" ;
  schema:sameAs    <http://ddwiki.reso.org/display/DDW/UnitType%5Btype%5DActualRent+Field>,<http://ddwiki.reso.org/display/DDW/UnitType%5Btype%5DBathsTotal+Field>,<http://ddwiki.reso.org/display/DDW/UnitType%5Btype%5DBedsTotal+Field>,<http://ddwiki.reso.org/display/DDW/UnitType%5Btype%5DDescription+Field>,<http://ddwiki.reso.org/display/DDW/UnitType%5Btype%5DFurnished+Field>,<http://ddwiki.reso.org/display/DDW/UnitType%5Btype%5DGarageAttachedYN+Field>,<http://ddwiki.reso.org/display/DDW/UnitType%5Btype%5DGarageSpaces+Field>,<http://ddwiki.reso.org/display/DDW/UnitType%5Btype%5DProForma+Field> ;
  vs:term_status   "stable"
.
reso:UnitType a rdf:Property ;
  rdfs:comment     "[type] This field is a repeating element for each type of unit selected in the UnitType field. For every UnitType there are two possible implementations. For a flat implementation (RETS 1.x only), each UnitTypeType used is expected to appear as the \"[type]\" in the related rooms field name. i.e. UnitTypeStudioActualRent. A relational implementation of UnitType must omit the type from the field name and use UnitTypeType to create a vertical representation of the various rooms. i.e. UnitTypeActualRent with Studio in the relational table's UnitType field.","[type] This field is a repeating element for each type of unit selected in the UnitType field. For every UnitType there are two possible implementations. For a flat implementation (RETS 1.x only), each UnitTypeType used is expected to appear as the \"[type]\" in the related rooms field name. i.e. UnitTypeStudioBathsTotal. A relational implementation of UnitType must omit the type from the field name and use UnitTypeType to create a vertical representation of the various rooms. i.e. UnitTypeBathsTotal with Studio in the relational table's UnitType field.","[type] This field is a repeating element for each type of unit selected in the UnitType field. For every UnitType there are two possible implementations. For a flat implementation (RETS 1.x only), each UnitTypeType used is expected to appear as the \"[type]\" in the related rooms field name. i.e. UnitTypeStudioBedsTotal. A relational implementation of UnitType must omit the type from the field name and use UnitTypeType to create a vertical representation of the various rooms. i.e. UnitTypeBedsTotal with Studio in the relational table's UnitType field.","[type] This field is a repeating element for each type of unit selected in the UnitType field. For every UnitType there are two possible implementations. For a flat implementation (RETS 1.x only), each UnitTypeType used is expected to appear as the \"[type]\" in the related rooms field name. i.e. UnitTypeStudioDescription. A relational implementation of UnitType must omit the type from the field name and use UnitTypeType to create a vertical representation of the various rooms. i.e. UnitTypeDescription with Studio in the relational table's UnitType field.","[type] This field is a repeating element for each type of unit selected in the UnitType field. For every UnitType there are two possible implementations. For a flat implementation (RETS 1.x only), each UnitTypeType used is expected to appear as the \"[type]\" in the related rooms field name. i.e. UnitTypeStudioFurnished. A relational implementation of UnitType must omit the type from the field name and use UnitTypeType to create a vertical representation of the various rooms. i.e. UnitTypeFurnished with Studio in the relational table's UnitType field.","[type] This field is a repeating element for each type of unit selected in the UnitType field. For every UnitType there are two possible implementations. For a flat implementation (RETS 1.x only), each UnitTypeType used is expected to appear as the \"[type]\" in the related rooms field name. i.e. UnitTypeStudioGarageAttachedYN. A relational implementation of UnitType must omit the type from the field name and use UnitTypeType to create a vertical representation of the various rooms. i.e. UnitTypeGarageAttachedYN with Studio in the relational table's UnitType field.","[type] This field is a repeating element for each type of unit selected in the UnitType field. For every UnitType there are two possible implementations. For a flat implementation (RETS 1.x only), each UnitTypeType used is expected to appear as the \"[type]\" in the related rooms field name. i.e. UnitTypeStudioGarageSpaces. A relational implementation of UnitType must omit the type from the field name and use UnitTypeType to create a vertical representation of the various rooms. i.e. UnitTypeGarageSpaces with Studio in the relational table's UnitType field.","[type] This field is a repeating element for each type of unit selected in the UnitType field. For every UnitType there are two possible implementations. For a flat implementation (RETS 1.x only), each UnitTypeType used is expected to appear as the \"[type]\" in the related rooms field name. i.e. UnitTypeStudioProForma. A relational implementation of UnitType must omit the type from the field name and use UnitTypeType to create a vertical representation of the various rooms. i.e. UnitTypeProForma with Studio in the relational table's UnitType field.","[type] This field is a repeating element for each type of unit selected in the UnitType field. For every UnitType there are two possible implementations. For a flat implementation (RETS 1.x only), each UnitTypeType used is expected to appear as the \"[type]\" in the related rooms field name. i.e. UnitTypeStudioTotalRent. A relational implementation of UnitType must omit the type from the field name and use UnitTypeType to create a vertical representation of the various rooms. i.e. UnitTypeTotalRent with Studio in the relational table's UnitType field." ;
  rdfs:domain      reso:Property ;
  rdfs:label       "UnitType" ;
  rdfs:range       xsd:decimal,xsd:string,xsd:boolean ;
  reso:CertificationLevel "Gold" ;
  reso:PropertyTypes "RINC","COMS","COML" ;
  schema:sameAs    <http://ddwiki.reso.org/display/DDW/UnitType%5Btype%5DActualRent+Field>,<http://ddwiki.reso.org/display/DDW/UnitType%5Btype%5DBathsTotal+Field>,<http://ddwiki.reso.org/display/DDW/UnitType%5Btype%5DBedsTotal+Field>,<http://ddwiki.reso.org/display/DDW/UnitType%5Btype%5DDescription+Field>,<http://ddwiki.reso.org/display/DDW/UnitType%5Btype%5DFurnished+Field>,<http://ddwiki.reso.org/display/DDW/UnitType%5Btype%5DGarageAttachedYN+Field>,<http://ddwiki.reso.org/display/DDW/UnitType%5Btype%5DGarageSpaces+Field>,<http://ddwiki.reso.org/display/DDW/UnitType%5Btype%5DProForma+Field>,<http://ddwiki.reso.org/display/DDW/UnitType%5Btype%5DTotalRent+Field> ;
  vs:term_status   "stable"
.
reso:UnitType a rdf:Property ;
  rdfs:comment     "[type] This field is a repeating element for each type of unit selected in the UnitType field. For every UnitType there are two possible implementations. For a flat implementation (RETS 1.x only), each UnitTypeType used is expected to appear as the \"[type]\" in the related rooms field name. i.e. UnitTypeStudioActualRent. A relational implementation of UnitType must omit the type from the field name and use UnitTypeType to create a vertical representation of the various rooms. i.e. UnitTypeActualRent with Studio in the relational table's UnitType field.","[type] This field is a repeating element for each type of unit selected in the UnitType field. For every UnitType there are two possible implementations. For a flat implementation (RETS 1.x only), each UnitTypeType used is expected to appear as the \"[type]\" in the related rooms field name. i.e. UnitTypeStudioBathsTotal. A relational implementation of UnitType must omit the type from the field name and use UnitTypeType to create a vertical representation of the various rooms. i.e. UnitTypeBathsTotal with Studio in the relational table's UnitType field.","[type] This field is a repeating element for each type of unit selected in the UnitType field. For every UnitType there are two possible implementations. For a flat implementation (RETS 1.x only), each UnitTypeType used is expected to appear as the \"[type]\" in the related rooms field name. i.e. UnitTypeStudioBedsTotal. A relational implementation of UnitType must omit the type from the field name and use UnitTypeType to create a vertical representation of the various rooms. i.e. UnitTypeBedsTotal with Studio in the relational table's UnitType field.","[type] This field is a repeating element for each type of unit selected in the UnitType field. For every UnitType there are two possible implementations. For a flat implementation (RETS 1.x only), each UnitTypeType used is expected to appear as the \"[type]\" in the related rooms field name. i.e. UnitTypeStudioDescription. A relational implementation of UnitType must omit the type from the field name and use UnitTypeType to create a vertical representation of the various rooms. i.e. UnitTypeDescription with Studio in the relational table's UnitType field.","[type] This field is a repeating element for each type of unit selected in the UnitType field. For every UnitType there are two possible implementations. For a flat implementation (RETS 1.x only), each UnitTypeType used is expected to appear as the \"[type]\" in the related rooms field name. i.e. UnitTypeStudioFurnished. A relational implementation of UnitType must omit the type from the field name and use UnitTypeType to create a vertical representation of the various rooms. i.e. UnitTypeFurnished with Studio in the relational table's UnitType field.","[type] This field is a repeating element for each type of unit selected in the UnitType field. For every UnitType there are two possible implementations. For a flat implementation (RETS 1.x only), each UnitTypeType used is expected to appear as the \"[type]\" in the related rooms field name. i.e. UnitTypeStudioGarageAttachedYN. A relational implementation of UnitType must omit the type from the field name and use UnitTypeType to create a vertical representation of the various rooms. i.e. UnitTypeGarageAttachedYN with Studio in the relational table's UnitType field.","[type] This field is a repeating element for each type of unit selected in the UnitType field. For every UnitType there are two possible implementations. For a flat implementation (RETS 1.x only), each UnitTypeType used is expected to appear as the \"[type]\" in the related rooms field name. i.e. UnitTypeStudioGarageSpaces. A relational implementation of UnitType must omit the type from the field name and use UnitTypeType to create a vertical representation of the various rooms. i.e. UnitTypeGarageSpaces with Studio in the relational table's UnitType field.","[type] This field is a repeating element for each type of unit selected in the UnitType field. For every UnitType there are two possible implementations. For a flat implementation (RETS 1.x only), each UnitTypeType used is expected to appear as the \"[type]\" in the related rooms field name. i.e. UnitTypeStudioProForma. A relational implementation of UnitType must omit the type from the field name and use UnitTypeType to create a vertical representation of the various rooms. i.e. UnitTypeProForma with Studio in the relational table's UnitType field.","[type] This field is a repeating element for each type of unit selected in the UnitType field. For every UnitType there are two possible implementations. For a flat implementation (RETS 1.x only), each UnitTypeType used is expected to appear as the \"[type]\" in the related rooms field name. i.e. UnitTypeStudioTotalRent. A relational implementation of UnitType must omit the type from the field name and use UnitTypeType to create a vertical representation of the various rooms. i.e. UnitTypeTotalRent with Studio in the relational table's UnitType field.","[type] This field is a repeating element for each type of unit selected in the UnitType field. For every UnitType there are two possible implementations. For a flat implementation (RETS 1.x only), each UnitTypeType used is expected to appear as the \"[type]\" in the related rooms field name. i.e. UnitTypeStudioUnitsTotal. A relational implementation of UnitType must omit the type from the field name and use UnitTypeType to create a vertical representation of the various rooms. i.e. UnitTypeUnitsTotal with Studio in the relational table's UnitType field." ;
  rdfs:domain      reso:Property ;
  rdfs:label       "UnitType" ;
  rdfs:range       xsd:decimal,xsd:string,xsd:boolean ;
  reso:CertificationLevel "Gold" ;
  reso:PropertyTypes "RINC","COMS","COML" ;
  schema:sameAs    <http://ddwiki.reso.org/display/DDW/UnitType%5Btype%5DActualRent+Field>,<http://ddwiki.reso.org/display/DDW/UnitType%5Btype%5DBathsTotal+Field>,<http://ddwiki.reso.org/display/DDW/UnitType%5Btype%5DBedsTotal+Field>,<http://ddwiki.reso.org/display/DDW/UnitType%5Btype%5DDescription+Field>,<http://ddwiki.reso.org/display/DDW/UnitType%5Btype%5DFurnished+Field>,<http://ddwiki.reso.org/display/DDW/UnitType%5Btype%5DGarageAttachedYN+Field>,<http://ddwiki.reso.org/display/DDW/UnitType%5Btype%5DGarageSpaces+Field>,<http://ddwiki.reso.org/display/DDW/UnitType%5Btype%5DProForma+Field>,<http://ddwiki.reso.org/display/DDW/UnitType%5Btype%5DTotalRent+Field>,<http://ddwiki.reso.org/display/DDW/UnitType%5Btype%5DUnitsTotal+Field> ;
  vs:term_status   "stable"
.
reso:UnitsFurnished a rdf:Property ;
  rdfs:comment     "Are the units furnished?  i.e. All Units, Varies By Unit, None." ;
  rdfs:domain      reso:Property ;
  rdfs:label       "UnitsFurnished" ;
  rdfs:range       xsd:string ;
  reso:CertificationLevel "Bronze" ;
  reso:PropertyTypes "RINC" ;
  schema:sameAs    <http://ddwiki.reso.org/display/DDW/UnitsFurnished+Field> ;
  vs:term_status   "stable"
.
reso:UnparsedAddress a rdf:Property ;
  rdfs:comment     "The UnparsedAddress is a text representation of the address with the full civic location as a single entity. It may optionally include any of City, StateOrProvince, PostalCode and Country." ;
  rdfs:domain      reso:Property ;
  rdfs:label       "UnparsedAddress" ;
  rdfs:range       xsd:string ;
  reso:CertificationLevel "Core" ;
  reso:PropertyTypes "RESI","RLSE","RINC","LAND","MOBI","FARM","COMS","COML","BUSO" ;
  schema:sameAs    <http://ddwiki.reso.org/display/DDW/UnparsedAddress+Field> ;
  vs:term_status   "stable"
.
reso:Utilities a rdf:Property ;
  rdfs:comment     "A list of the utilities for the property being sold/leased." ;
  rdfs:domain      reso:Property ;
  rdfs:label       "Utilities" ;
  rdfs:range       enum:Utilities ;
  reso:CertificationLevel "Bronze" ;
  reso:PropertyTypes "RESI","RLSE","RINC","LAND","MOBI","FARM","COMS","COML" ;
  schema:sameAs    <http://ddwiki.reso.org/display/DDW/Utilities+Field> ;
  vs:term_status   "stable"
.
reso:VacancyAllowance a rdf:Property ;
  rdfs:comment     "An estimate of the amount of rent that may be foregone because of unoccupied units." ;
  rdfs:domain      reso:Property ;
  rdfs:label       "VacancyAllowance" ;
  rdfs:range       xsd:decimal ;
  reso:CertificationLevel "Bronze" ;
  reso:PropertyTypes "RINC","COMS","COML" ;
  schema:sameAs    <http://ddwiki.reso.org/display/DDW/VacancyAllowance+Field> ;
  vs:term_status   "stable"
.
reso:VacancyAllowanceRate a rdf:Property ;
  rdfs:comment     "An estimate of the percent of rent that may be foregone because of unoccupied units." ;
  rdfs:domain      reso:Property ;
  rdfs:label       "VacancyAllowanceRate" ;
  rdfs:range       xsd:decimal ;
  reso:CertificationLevel "Bronze" ;
  reso:PropertyTypes "COMS","COML" ;
  schema:sameAs    <http://ddwiki.reso.org/display/DDW/VacancyAllowanceRate+Field> ;
  vs:term_status   "stable"
.
reso:Vegetation a rdf:Property ;
  rdfs:comment     "A list of the type(s) of vegetation on the property.  Note that this is not for farm crops, but more residential type vegetation." ;
  rdfs:domain      reso:Property ;
  rdfs:label       "Vegetation" ;
  rdfs:range       xsd:string ;
  reso:CertificationLevel "Gold" ;
  reso:PropertyTypes "RESI","RLSE","RINC","LAND","MOBI","FARM" ;
  schema:sameAs    <http://ddwiki.reso.org/display/DDW/Vegetation+Field> ;
  vs:term_status   "stable"
.
reso:VideosChangeTimestamp a rdf:Property ;
  rdfs:comment     "System generated timestamp of when the last update or change to the videos for this listing was made." ;
  rdfs:domain      reso:Property ;
  rdfs:label       "VideosChangeTimestamp" ;
  rdfs:range       xsd:dateTime ;
  reso:CertificationLevel "Bronze" ;
  reso:PropertyTypes "RESI","RLSE","RINC","LAND","MOBI","FARM","COMS","COML","BUSO" ;
  schema:sameAs    <http://ddwiki.reso.org/display/DDW/VideosChangeTimestamp+Field> ;
  vs:term_status   "stable"
.
reso:VideosCount a rdf:Property ;
  rdfs:comment     "The total number of videos or virtual tours included with the listing." ;
  rdfs:domain      reso:Property ;
  rdfs:label       "VideosCount" ;
  rdfs:range       xsd:decimal ;
  reso:CertificationLevel "Bronze" ;
  reso:PropertyTypes "RESI","RLSE","RINC","LAND","MOBI","FARM","COMS","COML","BUSO" ;
  schema:sameAs    <http://ddwiki.reso.org/display/DDW/VideosCount+Field> ;
  vs:term_status   "stable"
.
reso:View a rdf:Property ;
  rdfs:comment     "A view as seen from the listed property." ;
  rdfs:domain      reso:Property ;
  rdfs:label       "View" ;
  rdfs:range       xsd:string ;
  reso:CertificationLevel "Platinum" ;
  reso:PropertyTypes "RESI","RLSE","RINC","LAND","MOBI","FARM" ;
  schema:sameAs    <http://ddwiki.reso.org/display/DDW/View+Field> ;
  vs:term_status   "stable"
.
reso:ViewYN a rdf:Property ;
  rdfs:comment     "The property has a view." ;
  rdfs:domain      reso:Property ;
  rdfs:label       "ViewYN" ;
  rdfs:range       xsd:boolean ;
  reso:CertificationLevel "Platinum" ;
  reso:PropertyTypes "RESI","RLSE","RINC","LAND","MOBI","FARM" ;
  schema:sameAs    <http://ddwiki.reso.org/display/DDW/ViewYN+Field> ;
  vs:term_status   "stable"
.
reso:VirtualTourURLBranded a rdf:Property ;
  rdfs:comment     "A text field that holds the URL for a branded virtual tour of the property." ;
  rdfs:domain      reso:Property ;
  rdfs:label       "VirtualTourURLBranded" ;
  rdfs:range       xsd:string ;
  reso:CertificationLevel "Bronze" ;
  reso:PropertyTypes "RESI","RLSE","RINC","LAND","MOBI","FARM","COMS","COML","BUSO" ;
  schema:sameAs    <http://ddwiki.reso.org/display/DDW/VirtualTourURLBranded+Field> ;
  vs:term_status   "stable"
.
reso:VirtualTourURLUnbranded a rdf:Property ;
  rdfs:comment     "A text field that holds the URL for an unbranded virtual tour of the property." ;
  rdfs:domain      reso:Property ;
  rdfs:label       "VirtualTourURLUnbranded" ;
  rdfs:range       xsd:string ;
  reso:CertificationLevel "Core" ;
  reso:PropertyTypes "RESI","RLSE","RINC","LAND","MOBI","FARM","COMS","COML","BUSO" ;
  schema:sameAs    <http://ddwiki.reso.org/display/DDW/VirtualTourURLUnbranded+Field> ;
  vs:term_status   "stable"
.
reso:WalkScore a rdf:Property ;
  rdfs:comment     "A walkability index based on the time to walk from a property to near by essentials such as grocery stores, schools, churches, etc.  See www.walkscore.com for more information and requirements for using WalkScore." ;
  rdfs:domain      reso:Property ;
  rdfs:label       "WalkScore" ;
  rdfs:range       xsd:decimal ;
  reso:CertificationLevel "Silver" ;
  reso:PropertyTypes "RESI","RLSE","RINC","LAND","MOBI","FARM" ;
  schema:sameAs    <http://ddwiki.reso.org/display/DDW/WalkScore+Field> ;
  vs:term_status   "stable"
.
reso:WaterBodyName a rdf:Property ;
  rdfs:comment     "The name, if known, of the body of water on which the property is located. (E.g., lake name, river name, ocean name, sea name, canal name)." ;
  rdfs:domain      reso:Property ;
  rdfs:label       "WaterBodyName" ;
  rdfs:range       xsd:string ;
  reso:CertificationLevel "Platinum" ;
  reso:PropertyTypes "RESI","RLSE","RINC","LAND","MOBI","FARM","COMS","COML","BUSO" ;
  schema:sameAs    <http://ddwiki.reso.org/display/DDW/WaterBodyName+Field> ;
  vs:term_status   "stable"
.
reso:WaterSewerExpense a rdf:Property ;
  rdfs:comment     "The annual expense that is not paid directly by the tenant and is included in the Operating Expense calculations." ;
  rdfs:domain      reso:Property ;
  rdfs:label       "WaterSewerExpense" ;
  rdfs:range       xsd:decimal ;
  reso:CertificationLevel "Silver" ;
  reso:PropertyTypes "RINC","COMS","COML" ;
  schema:sameAs    <http://ddwiki.reso.org/display/DDW/WaterSewerExpense+Field> ;
  vs:term_status   "stable"
.
reso:WaterSource a rdf:Property ;
  rdfs:comment     "A list of the source(s) of water for the property" ;
  rdfs:domain      reso:Property ;
  rdfs:label       "WaterSource" ;
  rdfs:range       enum:WaterSource ;
  reso:CertificationLevel "Bronze" ;
  reso:PropertyTypes "RESI","RLSE","RINC","LAND","MOBI","FARM","COMS","COML" ;
  schema:sameAs    <http://ddwiki.reso.org/display/DDW/WaterSource+Field> ;
  vs:term_status   "stable"
.
reso:WaterfrontFeatures a rdf:Property ;
  rdfs:comment     "Features of the waterfront on which the property is located." ;
  rdfs:domain      reso:Property ;
  rdfs:label       "WaterfrontFeatures" ;
  rdfs:range       xsd:string ;
  reso:CertificationLevel "Platinum" ;
  reso:PropertyTypes "RESI","RLSE","RINC","LAND","MOBI","FARM","COMS","COML","BUSO" ;
  schema:sameAs    <http://ddwiki.reso.org/display/DDW/WaterfrontFeatures+Field> ;
  vs:term_status   "stable"
.
reso:WaterfrontYN a rdf:Property ;
  rdfs:comment     "The property is on the waterfront." ;
  rdfs:domain      reso:Property ;
  rdfs:label       "WaterfrontYN" ;
  rdfs:range       xsd:boolean ;
  reso:CertificationLevel "Platinum" ;
  reso:PropertyTypes "RESI","RLSE","RINC","LAND","MOBI","FARM","COMS","COML","BUSO" ;
  schema:sameAs    <http://ddwiki.reso.org/display/DDW/WaterfrontYN+Field> ;
  vs:term_status   "stable"
.
reso:WindowFeatures a rdf:Property ;
  rdfs:comment     "A list of features or description of the windows included in the sale/lease." ;
  rdfs:domain      reso:Property ;
  rdfs:label       "WindowFeatures" ;
  rdfs:range       xsd:string ;
  reso:CertificationLevel "Platinum" ;
  reso:PropertyTypes "RESI","RLSE","RINC","MOBI","FARM" ;
  schema:sameAs    <http://ddwiki.reso.org/display/DDW/WindowFeatures+Field> ;
  vs:term_status   "stable"
.
reso:WithdrawnDate a rdf:Property ;
  rdfs:comment     "Date the listing was withdrawn from the market.  This is not when a listing contact was cancelled or closed, but a withdrawal from the market while the contract between the seller and listing agent is still in effect and an offer has not been accepted. This is the date entered by the agent reflecting when the change occurred contractually, not a timestamp of when the change was made in the MLS." ;
  rdfs:domain      reso:Property ;
  rdfs:label       "WithdrawnDate" ;
  rdfs:range       xsd:date ;
  reso:CertificationLevel "Core" ;
  reso:PropertyTypes "RESI","RLSE","RINC","LAND","MOBI","FARM","COMS","COML","BUSO" ;
  schema:sameAs    <http://ddwiki.reso.org/display/DDW/WithdrawnDate+Field> ;
  vs:term_status   "stable"
.
reso:WoodedArea a rdf:Property ;
  rdfs:comment     "Measurement or percentage of the property that is wooded or forest." ;
  rdfs:domain      reso:Property ;
  rdfs:label       "WoodedArea" ;
  rdfs:range       xsd:decimal ;
  reso:CertificationLevel "Gold" ;
  reso:PropertyTypes "FARM" ;
  schema:sameAs    <http://ddwiki.reso.org/display/DDW/WoodedArea+Field> ;
  vs:term_status   "stable"
.
reso:WorkmansCompensationExpense a rdf:Property ;
  rdfs:comment     "The annual expense that is not paid directly by the tenant and is included in the Operating Expense calculations." ;
  rdfs:domain      reso:Property ;
  rdfs:label       "WorkmansCompensationExpense" ;
  rdfs:range       xsd:decimal ;
  reso:CertificationLevel "Silver" ;
  reso:PropertyTypes "RINC" ;
  schema:sameAs    <http://ddwiki.reso.org/display/DDW/WorkmansCompensationExpense+Field> ;
  vs:term_status   "stable"
.
reso:YearBuilt a rdf:Property ;
  rdfs:comment     "The year that an occupancy permit is first granted for the house or other local measure of initial habitability of the build. The type definition permits an empty value with an attribute noting that it is an unknown date or that the building is new construction. While constraints have not been applied, convention at the time of adoption has this as a four (4) digit year value." ;
  rdfs:domain      reso:Property ;
  rdfs:label       "YearBuilt" ;
  rdfs:range       xsd:decimal ;
  reso:CertificationLevel "Core" ;
  reso:PropertyTypes "RESI","RLSE","RINC","MOBI","FARM","COMS","COML" ;
  schema:sameAs    <http://ddwiki.reso.org/display/DDW/YearBuilt+Field> ;
  vs:term_status   "stable"
.
reso:YearBuiltDetails a rdf:Property ;
  rdfs:comment     "A description of the details behind the year the structure was built." ;
  rdfs:domain      reso:Property ;
  rdfs:label       "YearBuiltDetails" ;
  rdfs:range       xsd:string ;
  reso:CertificationLevel "Bronze" ;
  reso:PropertyTypes "RESI","RLSE","RINC","MOBI","FARM" ;
  schema:sameAs    <http://ddwiki.reso.org/display/DDW/YearBuiltDetails+Field> ;
  vs:term_status   "stable"
.
reso:YearBuiltEffective a rdf:Property ;
  rdfs:comment     "The year a major rebuild/renovated of the structure occurred." ;
  rdfs:domain      reso:Property ;
  rdfs:label       "YearBuiltEffective" ;
  rdfs:range       xsd:decimal ;
  reso:CertificationLevel "Bronze" ;
  reso:PropertyTypes "RESI","RLSE","RINC","MOBI","FARM" ;
  schema:sameAs    <http://ddwiki.reso.org/display/DDW/YearBuiltEffective+Field> ;
  vs:term_status   "stable"
.
reso:YearBuiltSource a rdf:Property ;
  rdfs:comment     "Add a list of sources of the year built.  i.e. Appraiser, Assessor, Builder, Estimated, etc.," ;
  rdfs:domain      reso:Property ;
  rdfs:label       "YearBuiltSource" ;
  rdfs:range       enum:YearBuiltSource ;
  reso:CertificationLevel "Bronze" ;
  reso:PropertyTypes "RESI","RLSE","RINC","MOBI","FARM" ;
  schema:sameAs    <http://ddwiki.reso.org/display/DDW/YearBuiltSource+Field> ;
  vs:term_status   "stable"
.
reso:YearEstablished a rdf:Property ;
  rdfs:comment     "The year the business being sold was established." ;
  rdfs:domain      reso:Property ;
  rdfs:label       "YearEstablished" ;
  rdfs:range       xsd:decimal ;
  reso:CertificationLevel "Silver" ;
  reso:PropertyTypes "BUSO" ;
  schema:sameAs    <http://ddwiki.reso.org/display/DDW/YearEstablished+Field> ;
  vs:term_status   "stable"
.
reso:YearsCurrentOwner a rdf:Property ;
  rdfs:comment     "The number of years the current owner has had possession of the business." ;
  rdfs:domain      reso:Property ;
  rdfs:label       "YearsCurrentOwner" ;
  rdfs:range       xsd:decimal ;
  reso:CertificationLevel "Silver" ;
  reso:PropertyTypes "BUSO" ;
  schema:sameAs    <http://ddwiki.reso.org/display/DDW/YearsCurrentOwner+Field> ;
  vs:term_status   "stable"
.
reso:Zoning a rdf:Property ;
  rdfs:comment     "A division of the city or county into areas of different permissible land uses. This Zone field should be used for the short code that is commonly used.  For full textual descriptions please use the ZoningDescription field." ;
  rdfs:domain      reso:Property ;
  rdfs:label       "Zoning" ;
  rdfs:range       xsd:string ;
  reso:CertificationLevel "Bronze" ;
  reso:PropertyTypes "RESI","RINC","LAND","MOBI","FARM","COMS","COML" ;
  schema:sameAs    <http://ddwiki.reso.org/display/DDW/Zoning+Field> ;
  vs:term_status   "stable"
.
reso:ZoningDescription a rdf:Property ;
  rdfs:comment     "A list of descriptions of the zoning of the property.  The zoning codes are often non-descriptive and variant. Zoning Description is a more descriptive form of the zoning for the property,  i.e. Agricultural, Residential, Rezone Possible, etc.  Specific zone codes must be added to the Zoning field." ;
  rdfs:domain      reso:Property ;
  rdfs:label       "ZoningDescription" ;
  rdfs:range       xsd:string ;
  reso:CertificationLevel "Bronze" ;
  reso:PropertyTypes "RESI","RINC","LAND","MOBI","FARM" ;
  schema:sameAs    <http://ddwiki.reso.org/display/DDW/ZoningDescription+Field> ;
  vs:term_status   "stable"
.
reso:JobTitle a rdf:Property ;
  rdfs:comment     "The title or position of the member within their organization." ;
  rdfs:domain      reso:Member ;
  rdfs:label       "JobTitle" ;
  rdfs:range       xsd:string ;
  reso:CertificationLevel "Silver" ;
  schema:sameAs    <http://ddwiki.reso.org/display/DDW/JobTitle+Field> ;
  vs:term_status   "stable"
.
reso:LastLoginTimestamp a rdf:Property ;
  rdfs:comment     "Date/time the member last logged into the source or other system." ;
  rdfs:domain      reso:Member ;
  rdfs:label       "LastLoginTimestamp" ;
  rdfs:range       xsd:dateTime ;
  reso:CertificationLevel "Silver" ;
  schema:sameAs    <http://ddwiki.reso.org/display/DDW/LastLoginTimestamp+Field> ;
  vs:term_status   "stable"
.
reso:MemberAOR a rdf:Property ;
  rdfs:comment     "The Member's Primary Board or Association of REALTORS." ;
  rdfs:domain      reso:Member ;
  rdfs:label       "MemberAOR" ;
  rdfs:range       xsd:string ;
  reso:CertificationLevel "Core" ;
  schema:sameAs    <http://ddwiki.reso.org/display/DDW/MemberAOR+Field> ;
  vs:term_status   "stable"
.
reso:MemberAORMlsId a rdf:Property ;
  rdfs:comment     "The local, well-known identifier for the member's Association of REALTORS. This value may not be unique, specifically in the case of aggregation systems, this value should be the identifier from the original system." ;
  rdfs:domain      reso:Member ;
  rdfs:label       "MemberAORMlsId" ;
  rdfs:range       xsd:string ;
  reso:CertificationLevel "Bronze" ;
  schema:sameAs    <http://ddwiki.reso.org/display/DDW/MemberAORMlsId+Field> ;
  vs:term_status   "stable"
.
reso:MemberAORkey a rdf:Property ;
  rdfs:comment     "A system unique identifier. Specifically, in aggregation systems, the MemberAORkey is the system unique identifier from the system that the record was retrieved. This may be identical to the related xxxId." ;
  rdfs:domain      reso:Member ;
  rdfs:label       "MemberAORkey" ;
  rdfs:range       xsd:string ;
  reso:CertificationLevel "Bronze" ;
  schema:sameAs    <http://ddwiki.reso.org/display/DDW/MemberAORkey+Field> ;
  vs:term_status   "stable"
.
reso:MemberAORkeyNumeric a rdf:Property ;
  rdfs:comment     "A system unique identifier. Specifically, in aggregation systems, the MemberAORkey is the system unique identifier from the system that the record was retrieved. This may be identical to the related xxxId.  This is the numeric only key and used as an alternative to the MemberAORkey field." ;
  rdfs:domain      reso:Member ;
  rdfs:label       "MemberAORkeyNumeric" ;
  rdfs:range       xsd:decimal ;
  reso:CertificationLevel "Platinum" ;
  schema:sameAs    <http://ddwiki.reso.org/display/DDW/MemberAORkeyNumeric+Field> ;
  vs:term_status   "stable"
.
reso:MemberAddress1 a rdf:Property ;
  rdfs:comment     "The street number, direction, name and suffix of the member." ;
  rdfs:domain      reso:Member ;
  rdfs:label       "MemberAddress1" ;
  rdfs:range       xsd:string ;
  reso:CertificationLevel "Core" ;
  schema:sameAs    <http://ddwiki.reso.org/display/DDW/MemberAddress1+Field> ;
  vs:term_status   "stable"
.
reso:MemberAddress2 a rdf:Property ;
  rdfs:comment     "The unit/suite number of the member." ;
  rdfs:domain      reso:Member ;
  rdfs:label       "MemberAddress2" ;
  rdfs:range       xsd:string ;
  reso:CertificationLevel "Core" ;
  schema:sameAs    <http://ddwiki.reso.org/display/DDW/MemberAddress2+Field> ;
  vs:term_status   "stable"
.
reso:MemberAssociationComments a rdf:Property ;
  rdfs:comment     "The association's notes regarding the member." ;
  rdfs:domain      reso:Member ;
  rdfs:label       "MemberAssociationComments" ;
  rdfs:range       xsd:string ;
  reso:CertificationLevel "Silver" ;
  schema:sameAs    <http://ddwiki.reso.org/display/DDW/MemberAssociationComments+Field> ;
  vs:term_status   "stable"
.
reso:MemberCarrierRoute a rdf:Property ;
  rdfs:domain      reso:Member ;
  rdfs:label       "MemberCarrierRoute" ;
  rdfs:range       xsd:string ;
  reso:CertificationLevel "Bronze" ;
  schema:sameAs    <http://ddwiki.reso.org/display/DDW/MemberCarrierRoute+Field> ;
  vs:term_status   "stable"
.
reso:MemberCity a rdf:Property ;
  rdfs:comment     "The city of the member." ;
  rdfs:domain      reso:Member ;
  rdfs:label       "MemberCity" ;
  rdfs:range       xsd:string ;
  reso:CertificationLevel "Core" ;
  schema:sameAs    <http://ddwiki.reso.org/display/DDW/MemberCity+Field> ;
  vs:term_status   "stable"
.
reso:MemberCountry a rdf:Property ;
  rdfs:comment     "The country abbreviation in a postal address." ;
  rdfs:domain      reso:Member ;
  rdfs:label       "MemberCountry" ;
  rdfs:range       enum:Country ;
  reso:CertificationLevel "Core" ;
  schema:sameAs    <http://ddwiki.reso.org/display/DDW/MemberCountry+Field> ;
  vs:term_status   "stable"
.
reso:MemberCountyOrParish a rdf:Property ;
  rdfs:comment     "The county or parish in which the member is addressed." ;
  rdfs:domain      reso:Member ;
  rdfs:label       "MemberCountyOrParish" ;
  rdfs:range       xsd:string ;
  reso:CertificationLevel "Core" ;
  schema:sameAs    <http://ddwiki.reso.org/display/DDW/MemberCountyOrParish+Field> ;
  vs:term_status   "stable"
.
reso:MemberDesignation a rdf:Property ;
  rdfs:comment     "Designations and certifications acknowledging experience and expertise in various real estate sectors are awarded by NAR and each affiliated group upon completion of required courses." ;
  rdfs:domain      reso:Member ;
  rdfs:label       "MemberDesignation" ;
  rdfs:range       xsd:string ;
  reso:CertificationLevel "Silver" ;
  schema:sameAs    <http://ddwiki.reso.org/display/DDW/MemberDesignation+Field> ;
  vs:term_status   "stable"
.
reso:MemberDirectPhone a rdf:Property ;
  rdfs:comment     "North American 10 digit phone numbers should be in the format of ###-###-#### (separated by hyphens).  Other conventions should use the common local standard.  International numbers should be preceded by a plus symbol." ;
  rdfs:domain      reso:Member ;
  rdfs:label       "MemberDirectPhone" ;
  rdfs:range       xsd:string ;
  reso:CertificationLevel "Bronze" ;
  schema:sameAs    <http://ddwiki.reso.org/display/DDW/MemberDirectPhone+Field> ;
  vs:term_status   "stable"
.
reso:MemberEmail a rdf:Property ;
  rdfs:comment     "The email address of the Member." ;
  rdfs:domain      reso:Member ;
  rdfs:label       "MemberEmail" ;
  rdfs:range       xsd:string ;
  reso:CertificationLevel "Core" ;
  schema:sameAs    <http://ddwiki.reso.org/display/DDW/MemberEmail+Field> ;
  vs:term_status   "stable"
.
reso:MemberFax a rdf:Property ;
  rdfs:comment     "North American 10 digit phone numbers should be in the format of ###-###-#### (separated by hyphens).  Other conventions should use the common local standard.  International numbers should be preceded by a plus symbol." ;
  rdfs:domain      reso:Member ;
  rdfs:label       "MemberFax" ;
  rdfs:range       xsd:string ;
  reso:CertificationLevel "Bronze" ;
  schema:sameAs    <http://ddwiki.reso.org/display/DDW/MemberFax+Field> ;
  vs:term_status   "stable"
.
reso:MemberFirstName a rdf:Property ;
  rdfs:comment     "The first name of the Member." ;
  rdfs:domain      reso:Member ;
  rdfs:label       "MemberFirstName" ;
  rdfs:range       xsd:string ;
  reso:CertificationLevel "Core" ;
  schema:sameAs    <http://ddwiki.reso.org/display/DDW/MemberFirstName+Field> ;
  vs:term_status   "stable"
.
reso:MemberFullName a rdf:Property ;
  rdfs:comment     "The full name of the Member. (First Middle Last) or a alternate full name." ;
  rdfs:domain      reso:Member ;
  rdfs:label       "MemberFullName" ;
  rdfs:range       xsd:string ;
  reso:CertificationLevel "Bronze" ;
  schema:sameAs    <http://ddwiki.reso.org/display/DDW/MemberFullName+Field> ;
  vs:term_status   "stable"
.
reso:MemberHomePhone a rdf:Property ;
  rdfs:comment     "North American 10 digit phone numbers should be in the format of ###-###-#### (separated by hyphens).  Other conventions should use the common local standard.  International numbers should be preceded by a plus symbol." ;
  rdfs:domain      reso:Member ;
  rdfs:label       "MemberHomePhone" ;
  rdfs:range       xsd:string ;
  reso:CertificationLevel "Bronze" ;
  schema:sameAs    <http://ddwiki.reso.org/display/DDW/MemberHomePhone+Field> ;
  vs:term_status   "stable"
.
reso:MemberIsAssistantTo a rdf:Property ;
  rdfs:comment     "The MemberMlsId of the Agent/Broker that this member is an assistant.  The typical use will be to add the agent's ID to this field when editing the member record of the assistant." ;
  rdfs:domain      reso:Member ;
  rdfs:label       "MemberIsAssistantTo" ;
  rdfs:range       xsd:string ;
  reso:CertificationLevel "Platinum" ;
  schema:sameAs    <http://ddwiki.reso.org/display/DDW/MemberIsAssistantTo+Field> ;
  vs:term_status   "stable"
.
reso:MemberKey a rdf:Property ;
  rdfs:comment     "A unique identifier for this record from the immediate source. This is a string that can include URI or other forms.  Alternatively use the MemberKeyNumeric for a numeric only key field.  This is the local key of the system.  When records are received from other systems, a local key is commonly applied.  If conveying the original keys from the source or originating systems, see SourceSystemMemberKey and OriginatingSystemMemberKey." ;
  rdfs:domain      reso:Member ;
  rdfs:label       "MemberKey" ;
  rdfs:range       xsd:string ;
  reso:CertificationLevel "Core" ;
  schema:sameAs    <http://ddwiki.reso.org/display/DDW/MemberKey+Field> ;
  vs:term_status   "stable"
.
reso:MemberKeyNumeric a rdf:Property ;
  rdfs:comment     "A unique identifier for this record from the immediate source. This is the numeric only key and used as an alternative to the MemberKey fields.  This is the local key of the system.  When records are received from other systems, a local key is commonly applied.  If conveying the original keys from the source or originating systems, see SourceSystemMemberKey and OriginatingSystemMemberKey." ;
  rdfs:domain      reso:Member ;
  rdfs:label       "MemberKeyNumeric" ;
  rdfs:range       xsd:decimal ;
  reso:CertificationLevel "Platinum" ;
  schema:sameAs    <http://ddwiki.reso.org/display/DDW/MemberKeyNumeric+Field> ;
  vs:term_status   "stable"
.
reso:MemberLanguages a rdf:Property ;
  rdfs:comment     "The languages the member speaks." ;
  rdfs:domain      reso:Member ;
  rdfs:label       "MemberLanguages" ;
  rdfs:range       enum:Languages ;
  reso:CertificationLevel "Silver" ;
  schema:sameAs    <http://ddwiki.reso.org/display/DDW/MemberLanguages+Field> ;
  vs:term_status   "stable"
.
reso:MemberLastName a rdf:Property ;
  rdfs:comment     "The last name of the Member." ;
  rdfs:domain      reso:Member ;
  rdfs:label       "MemberLastName" ;
  rdfs:range       xsd:string ;
  reso:CertificationLevel "Core" ;
  schema:sameAs    <http://ddwiki.reso.org/display/DDW/MemberLastName+Field> ;
  vs:term_status   "stable"
.
reso:MemberLoginId a rdf:Property ;
  rdfs:comment     "The ID used to logon to the MLS system." ;
  rdfs:domain      reso:Member ;
  rdfs:label       "MemberLoginId" ;
  rdfs:range       xsd:string ;
  reso:CertificationLevel "Bronze" ;
  schema:sameAs    <http://ddwiki.reso.org/display/DDW/MemberLoginId+Field> ;
  vs:term_status   "stable"
.
reso:MemberMiddleName a rdf:Property ;
  rdfs:comment     "The middle name of the Member." ;
  rdfs:domain      reso:Member ;
  rdfs:label       "MemberMiddleName" ;
  rdfs:range       xsd:string ;
  reso:CertificationLevel "Core" ;
  schema:sameAs    <http://ddwiki.reso.org/display/DDW/MemberMiddleName+Field> ;
  vs:term_status   "stable"
.
reso:MemberMlsAccessYN a rdf:Property ;
  rdfs:comment     "Does the member have access to the MLS system." ;
  rdfs:domain      reso:Member ;
  rdfs:label       "MemberMlsAccessYN" ;
  rdfs:range       xsd:boolean ;
  reso:CertificationLevel "Silver" ;
  schema:sameAs    <http://ddwiki.reso.org/display/DDW/MemberMlsAccessYN+Field> ;
  vs:term_status   "stable"
.
reso:MemberMlsId a rdf:Property ;
  rdfs:comment     "The local, well-known identifier for the member. This value may not be unique, specifically in the case of aggregation systems, this value should be the identifier from the original system." ;
  rdfs:domain      reso:Member ;
  rdfs:label       "MemberMlsId" ;
  rdfs:range       xsd:string ;
  reso:CertificationLevel "Core" ;
  schema:sameAs    <http://ddwiki.reso.org/display/DDW/MemberMlsId+Field> ;
  vs:term_status   "stable"
.
reso:MemberMlsSecurityClass a rdf:Property ;
  rdfs:comment     "The MLS security group or class given to the member." ;
  rdfs:domain      reso:Member ;
  rdfs:label       "MemberMlsSecurityClass" ;
  rdfs:range       xsd:string ;
  reso:CertificationLevel "Bronze" ;
  schema:sameAs    <http://ddwiki.reso.org/display/DDW/MemberMlsSecurityClass+Field> ;
  vs:term_status   "stable"
.
reso:MemberMobilePhone a rdf:Property ;
  rdfs:comment     "North American 10 digit phone numbers should be in the format of ###-###-#### (separated by hyphens).  Other conventions should use the common local standard.  International numbers should be preceded by a plus symbol." ;
  rdfs:domain      reso:Member ;
  rdfs:label       "MemberMobilePhone" ;
  rdfs:range       xsd:string ;
  reso:CertificationLevel "Core" ;
  schema:sameAs    <http://ddwiki.reso.org/display/DDW/MemberMobilePhone+Field> ;
  vs:term_status   "stable"
.
reso:MemberNamePrefix a rdf:Property ;
  rdfs:comment     "Prefix to the name (e.g. Dr. Mr. Ms. etc.)" ;
  rdfs:domain      reso:Member ;
  rdfs:label       "MemberNamePrefix" ;
  rdfs:range       xsd:string ;
  reso:CertificationLevel "Bronze" ;
  schema:sameAs    <http://ddwiki.reso.org/display/DDW/MemberNamePrefix+Field> ;
  vs:term_status   "stable"
.
reso:MemberNameSuffix a rdf:Property ;
  rdfs:comment     "Suffix to the surname (e.g. Esq.,  Jr.,  III etc.)" ;
  rdfs:domain      reso:Member ;
  rdfs:label       "MemberNameSuffix" ;
  rdfs:range       xsd:string ;
  reso:CertificationLevel "Bronze" ;
  schema:sameAs    <http://ddwiki.reso.org/display/DDW/MemberNameSuffix+Field> ;
  vs:term_status   "stable"
.
reso:MemberNationalAssociationId a rdf:Property ;
  rdfs:comment     "The national association ID of the member.  i.e. in the U.S. is the NRDS number." ;
  rdfs:domain      reso:Member ;
  rdfs:label       "MemberNationalAssociationId" ;
  rdfs:range       xsd:string ;
  reso:CertificationLevel "Core" ;
  schema:sameAs    <http://ddwiki.reso.org/display/DDW/MemberNationalAssociationId+Field> ;
  vs:term_status   "stable"
.
reso:MemberNickname a rdf:Property ;
  rdfs:comment     "An alternate name used by the Member, usually as a substitute for the first name." ;
  rdfs:domain      reso:Member ;
  rdfs:label       "MemberNickname" ;
  rdfs:range       xsd:string ;
  reso:CertificationLevel "Bronze" ;
  schema:sameAs    <http://ddwiki.reso.org/display/DDW/MemberNickname+Field> ;
  vs:term_status   "stable"
.
reso:MemberOfficePhone a rdf:Property ;
  rdfs:comment     "North American 10 digit phone numbers should be in the format of ###-###-#### (separated by hyphens).  Other conventions should use the common local standard.  International numbers should be preceded by a plus symbol." ;
  rdfs:domain      reso:Member ;
  rdfs:label       "MemberOfficePhone" ;
  rdfs:range       xsd:string ;
  reso:CertificationLevel "Core" ;
  schema:sameAs    <http://ddwiki.reso.org/display/DDW/MemberOfficePhone+Field> ;
  vs:term_status   "stable"
.
reso:MemberOfficePhoneExt a rdf:Property ;
  rdfs:comment     "The extension of the given phone number (if applicable)." ;
  rdfs:domain      reso:Member ;
  rdfs:label       "MemberOfficePhoneExt" ;
  rdfs:range       xsd:string ;
  reso:CertificationLevel "Core" ;
  schema:sameAs    <http://ddwiki.reso.org/display/DDW/MemberOfficePhoneExt+Field> ;
  vs:term_status   "stable"
.
reso:MemberOtherPhoneType a rdf:Property ;
  rdfs:comment     "The type of \"other\" phone.  i.e. Preferred, Office, Mobile, Direct, Home, Fax, Pager, Voicemail, Toll Free, SMS, 1, 2, 3, First, Second, Third, etc..  This is used as the list of options for the Member Other Phone repeating elements." ;
  rdfs:domain      reso:Member ;
  rdfs:label       "MemberOtherPhoneType" ;
  rdfs:range       xsd:string ;
  reso:CertificationLevel "Bronze" ;
  schema:sameAs    <http://ddwiki.reso.org/display/DDW/MemberOtherPhoneType+Field> ;
  vs:term_status   "stable"
.
reso:MemberOtherPhone a rdf:Property ;
  rdfs:comment     "The \"other\" phone option allowing members to convey additional phone numbers other than those already covered by the MemberMobilePhone, MemberFax, etc., fields.  This is a repeating element." ;
  rdfs:domain      reso:Member ;
  rdfs:label       "MemberOtherPhone" ;
  rdfs:range       xsd:string ;
  reso:CertificationLevel "Bronze" ;
  schema:sameAs    <http://ddwiki.reso.org/display/DDW/MemberOtherPhone%5BType%5DExt+Field> ;
  vs:term_status   "stable"
.
reso:MemberOtherPhone a rdf:Property ;
  rdfs:comment     "The \"other\" phone option allowing members to convey additional phone numbers other than those already covered by the MemberMobilePhone, MemberFax, etc., fields.  This is a repeating element." ;
  rdfs:domain      reso:Member ;
  rdfs:label       "MemberOtherPhone" ;
  rdfs:range       xsd:string ;
  reso:CertificationLevel "Bronze" ;
  schema:sameAs    <http://ddwiki.reso.org/display/DDW/MemberOtherPhone%5BType%5DExt+Field>,<http://ddwiki.reso.org/display/DDW/MemberOtherPhone%5BType%5DNumber+Field> ;
  vs:term_status   "stable"
.
reso:MemberPager a rdf:Property ;
  rdfs:comment     "North American 10 digit phone numbers should be in the format of ###-###-#### (separated by hyphens).  Other conventions should use the common local standard.  International numbers should be preceded by a plus symbol." ;
  rdfs:domain      reso:Member ;
  rdfs:label       "MemberPager" ;
  rdfs:range       xsd:string ;
  reso:CertificationLevel "Platinum" ;
  schema:sameAs    <http://ddwiki.reso.org/display/DDW/MemberPager+Field> ;
  vs:term_status   "stable"
.
reso:MemberPassword a rdf:Property ;
  rdfs:comment     "A password that the member whishes to share with other systems.  Normal security considerations apply and are the responsibility of the entity utilizing this field." ;
  rdfs:domain      reso:Member ;
  rdfs:label       "MemberPassword" ;
  rdfs:range       xsd:string ;
  reso:CertificationLevel "Silver" ;
  schema:sameAs    <http://ddwiki.reso.org/display/DDW/MemberPassword+Field> ;
  vs:term_status   "stable"
.
reso:MemberPhoneTTYTDD a rdf:Property ;
  rdfs:comment     "(Telecommunications Device for the Deaf/TeleTYpewriter) A user terminal with keyboard input and printer or display output used by the hearing and speech impaired. The device contains a modem and is used over a standard analog phone line. If a recipient does not have a corresponding terminal device, TDD/TTY users dial a relay service composed of operators who receive the typed messages, call the recipients and speak the messages to them. The operators also type the responses back to the TDD/TTY user." ;
  rdfs:domain      reso:Member ;
  rdfs:label       "MemberPhoneTTYTDD" ;
  rdfs:range       xsd:string ;
  reso:CertificationLevel "Platinum" ;
  schema:sameAs    <http://ddwiki.reso.org/display/DDW/MemberPhoneTTYTDD+Field> ;
  vs:term_status   "stable"
.
reso:MemberPostalCode a rdf:Property ;
  rdfs:comment     "The postal code of the member." ;
  rdfs:domain      reso:Member ;
  rdfs:label       "MemberPostalCode" ;
  rdfs:range       xsd:string ;
  reso:CertificationLevel "Core" ;
  schema:sameAs    <http://ddwiki.reso.org/display/DDW/MemberPostalCode+Field> ;
  vs:term_status   "stable"
.
reso:MemberPostalCodePlus4 a rdf:Property ;
  rdfs:comment     "The extension of the postal/zip code.  i.e. +4" ;
  rdfs:domain      reso:Member ;
  rdfs:label       "MemberPostalCodePlus4" ;
  rdfs:range       xsd:string ;
  reso:CertificationLevel "Core" ;
  schema:sameAs    <http://ddwiki.reso.org/display/DDW/MemberPostalCodePlus4+Field> ;
  vs:term_status   "stable"
.
reso:MemberPreferredPhone a rdf:Property ;
  rdfs:comment     "North American 10 digit phone numbers should be in the format of ###-###-#### (separated by hyphens).  Other conventions should use the common local standard.  International numbers should be preceded by a plus symbol." ;
  rdfs:domain      reso:Member ;
  rdfs:label       "MemberPreferredPhone" ;
  rdfs:range       xsd:string ;
  reso:CertificationLevel "Core" ;
  schema:sameAs    <http://ddwiki.reso.org/display/DDW/MemberPreferredPhone+Field> ;
  vs:term_status   "stable"
.
reso:MemberPreferredPhoneExt a rdf:Property ;
  rdfs:comment     "The extension of the given phone number (if applicable)." ;
  rdfs:domain      reso:Member ;
  rdfs:label       "MemberPreferredPhoneExt" ;
  rdfs:range       xsd:string ;
  reso:CertificationLevel "Core" ;
  schema:sameAs    <http://ddwiki.reso.org/display/DDW/MemberPreferredPhoneExt+Field> ;
  vs:term_status   "stable"
.
reso:MemberStateLicense a rdf:Property ;
  rdfs:comment     "The license of the Member. Separate multiple licenses with a comma and space." ;
  rdfs:domain      reso:Member ;
  rdfs:label       "MemberStateLicense" ;
  rdfs:range       xsd:string ;
  reso:CertificationLevel "Core" ;
  schema:sameAs    <http://ddwiki.reso.org/display/DDW/MemberStateLicense+Field> ;
  vs:term_status   "stable"
.
reso:MemberStateLicenseState a rdf:Property ;
  rdfs:comment     "The state in which the member is licensed." ;
  rdfs:domain      reso:Member ;
  rdfs:label       "MemberStateLicenseState" ;
  rdfs:range       enum:StateOrProvince ;
  reso:CertificationLevel "Bronze" ;
  schema:sameAs    <http://ddwiki.reso.org/display/DDW/MemberStateLicenseState+Field> ;
  vs:term_status   "stable"
.
reso:MemberStateOrProvince a rdf:Property ;
  rdfs:comment     "The state or province in which the member is addressed." ;
  rdfs:domain      reso:Member ;
  rdfs:label       "MemberStateOrProvince" ;
  rdfs:range       enum:StateOrProvince ;
  reso:CertificationLevel "Core" ;
  schema:sameAs    <http://ddwiki.reso.org/display/DDW/MemberStateOrProvince+Field> ;
  vs:term_status   "stable"
.
reso:MemberStatus a rdf:Property ;
  rdfs:comment     "Is the account active, inactive or under disciplinary action." ;
  rdfs:domain      reso:Member ;
  rdfs:label       "MemberStatus" ;
  rdfs:range       enum:MemberStatus ;
  reso:CertificationLevel "Core" ;
  schema:sameAs    <http://ddwiki.reso.org/display/DDW/MemberStatus+Field> ;
  vs:term_status   "stable"
.
reso:MemberTollFreePhone a rdf:Property ;
  rdfs:comment     "North American 10 digit phone numbers should be in the format of ###-###-#### (separated by hyphens).  Other conventions should use the common local standard.  International numbers should be preceded by a plus symbol." ;
  rdfs:domain      reso:Member ;
  rdfs:label       "MemberTollFreePhone" ;
  rdfs:range       xsd:string ;
  reso:CertificationLevel "Bronze" ;
  schema:sameAs    <http://ddwiki.reso.org/display/DDW/MemberTollFreePhone+Field> ;
  vs:term_status   "stable"
.
reso:MemberType a rdf:Property ;
  rdfs:comment     "The type of member.  i.e. Agent, Broker, Office Manager, Appraiser, Photographer, Assistants, MLO, Realtor, Association Staff, MLS Staff, etc." ;
  rdfs:domain      reso:Member ;
  rdfs:label       "MemberType" ;
  rdfs:range       enum:MemberType ;
  reso:CertificationLevel "Bronze" ;
  schema:sameAs    <http://ddwiki.reso.org/display/DDW/MemberType+Field> ;
  vs:term_status   "stable"
.
reso:MemberVoiceMail a rdf:Property ;
  rdfs:comment     "North American 10 digit phone numbers should be in the format of ###-###-#### (separated by hyphens).  Other conventions should use the common local standard.  International numbers should be preceded by a plus symbol." ;
  rdfs:domain      reso:Member ;
  rdfs:label       "MemberVoiceMail" ;
  rdfs:range       xsd:string ;
  reso:CertificationLevel "Bronze" ;
  schema:sameAs    <http://ddwiki.reso.org/display/DDW/MemberVoiceMail+Field> ;
  vs:term_status   "stable"
.
reso:MemberVoiceMailExt a rdf:Property ;
  rdfs:comment     "The extension of the given phone number (if applicable)." ;
  rdfs:domain      reso:Member ;
  rdfs:label       "MemberVoiceMailExt" ;
  rdfs:range       xsd:string ;
  reso:CertificationLevel "Bronze" ;
  schema:sameAs    <http://ddwiki.reso.org/display/DDW/MemberVoiceMailExt+Field> ;
  vs:term_status   "stable"
.
reso:ModificationTimestamp a rdf:Property ;
  rdfs:comment     "The transactional timestamp automatically recorded by the MLS system representing the date/time the listing was last modified.","Date/time the roster (member or office) record was last modified." ;
  rdfs:domain      reso:Property,reso:Member ;
  rdfs:label       "ModificationTimestamp" ;
  rdfs:range       xsd:dateTime ;
  reso:CertificationLevel "Core" ;
  reso:PropertyTypes "RESI","RLSE","RINC","LAND","MOBI","FARM","COMS","COML","BUSO" ;
  schema:sameAs    <http://ddwiki.reso.org/display/DDW/ModificationTimestamp+Field>,<http://ddwiki.reso.org/display/DDW/ModificationTimestamp+%28Member%29+Field> ;
  vs:term_status   "stable"
.
reso:OfficeKey a rdf:Property ;
  rdfs:comment     "A system unique identifier. Specifically, in aggregation systems, the Key is the system unique identifier from the system that the record was just retrieved. This may be identical to the related xxxId identifier, but the key is guaranteed unique for this record set. This is a foreign key relating to the Office resource's OfficeKey." ;
  rdfs:domain      reso:Member ;
  rdfs:label       "OfficeKey" ;
  rdfs:range       xsd:string ;
  reso:CertificationLevel "Core" ;
  schema:sameAs    <http://ddwiki.reso.org/display/DDW/OfficeKey+Field> ;
  vs:term_status   "stable"
.
reso:OfficeKeyNumeric a rdf:Property ;
  rdfs:comment     "A system unique identifier. Specifically, in aggregation systems, the Key is the system unique identifier from the system that the record was just retrieved. This may be identical to the related xxxId identifier, but the key is guaranteed unique for this record set. This is a foreign key relating to the Office resource's OfficeKey.  This is the numeric only key and used as an alternative to the MemberAORkey field." ;
  rdfs:domain      reso:Member ;
  rdfs:label       "OfficeKeyNumeric" ;
  rdfs:range       xsd:decimal ;
  reso:CertificationLevel "Platinum" ;
  schema:sameAs    <http://ddwiki.reso.org/display/DDW/OfficeKeyNumeric+Field> ;
  vs:term_status   "stable"
.
reso:OfficeMlsId a rdf:Property ;
  rdfs:comment     "The local, well-known identifier. This value may not be unique, specifically in the case of aggregation systems, this value should be the identifier from the original system." ;
  rdfs:domain      reso:Member ;
  rdfs:label       "OfficeMlsId" ;
  rdfs:range       xsd:string ;
  reso:CertificationLevel "Core" ;
  schema:sameAs    <http://ddwiki.reso.org/display/DDW/OfficeMlsId+Field> ;
  vs:term_status   "stable"
.
reso:OfficeName a rdf:Property ;
  rdfs:comment     "The legal name of the brokerage." ;
  rdfs:domain      reso:Member ;
  rdfs:label       "OfficeName" ;
  rdfs:range       xsd:string ;
  reso:CertificationLevel "Bronze" ;
  schema:sameAs    <http://ddwiki.reso.org/display/DDW/OfficeName+Field> ;
  vs:term_status   "stable"
.
reso:OriginalEntryTimestamp a rdf:Property ;
  rdfs:comment     "The transactional timestamp automatically recorded by the MLS system representing the date/time the listing was entered and made visible to members of the MLS.","Date/time the roster (member or office) record was originally input into the source system." ;
  rdfs:domain      reso:Property,reso:Member ;
  rdfs:label       "OriginalEntryTimestamp" ;
  rdfs:range       xsd:dateTime ;
  reso:CertificationLevel "Core" ;
  reso:PropertyTypes "RESI","RLSE","RINC","LAND","MOBI","FARM","COMS","COML","BUSO" ;
  schema:sameAs    <http://ddwiki.reso.org/display/DDW/OriginalEntryTimestamp+Field>,<http://ddwiki.reso.org/display/DDW/OriginalEntryTimestamp+%28Member%29+Field> ;
  vs:term_status   "stable"
.
reso:OriginatingSystemID a rdf:Property ;
  rdfs:comment     "The RESO OUID's OrganizationUniqueId of the Originating record provider.  The Originating system is the system with authoritative control over the record.  For example; the name of the MLS where the listing was input.  In cases where the Originating system was not where the record originated (the authoritative system), see the Originating System fields.","The RESO OUID's OrganizationUniqueId of the Originating record provider.  The Originating system is the system with authoritative control over the record.  For example; the name of the MLS where the member was input.  In cases where the Originating system was not where the record originated (the authoritative system), see the Originating System fields." ;
  rdfs:domain      reso:Property,reso:Member ;
  rdfs:label       "OriginatingSystemID" ;
  rdfs:range       xsd:string ;
  reso:CertificationLevel "Platinum" ;
  reso:PropertyTypes "RESI","RLSE","RINC","LAND","MOBI","FARM","COMS","COML","BUSO" ;
  schema:sameAs    <http://ddwiki.reso.org/display/DDW/OriginatingSystemID+Field>,<http://ddwiki.reso.org/display/DDW/OriginatingSystemID+%28Member%29+Field> ;
  vs:term_status   "stable"
.
reso:OriginatingSystemMemberKey a rdf:Property ;
  rdfs:comment     "The system key, a unique record identifier, from the Originating system.  The Originating system is the system with authoritative control over the record.  For example, the Multiple Listing Service where the member was input.  There may be cases where the Source System (how you received the record) is not the Originating System.  See Source System Key for more information." ;
  rdfs:domain      reso:Member ;
  rdfs:label       "OriginatingSystemMemberKey" ;
  rdfs:range       xsd:string ;
  reso:CertificationLevel "Core" ;
  schema:sameAs    <http://ddwiki.reso.org/display/DDW/OriginatingSystemMemberKey+Field> ;
  vs:term_status   "stable"
.
reso:OriginatingSystemName a rdf:Property ;
  rdfs:comment     "The name of the Originating record provider.  Most commonly the name of the MLS. The place where the listing is originally input by the member.  The legal name of the company.","The name of the Originating record provider.  Most commonly the name of the MLS. The place where the member is originally input by the member.  The legal name of the company." ;
  rdfs:domain      reso:Property,reso:Member ;
  rdfs:label       "OriginatingSystemName" ;
  rdfs:range       xsd:string ;
  reso:CertificationLevel "Core","Bronze" ;
  reso:PropertyTypes "RESI","RLSE","RINC","LAND","MOBI","FARM","COMS","COML","BUSO" ;
  schema:sameAs    <http://ddwiki.reso.org/display/DDW/OriginatingSystemName+Field>,<http://ddwiki.reso.org/display/DDW/OriginatingSystemName+%28Member%29+Field> ;
  vs:term_status   "stable"
.
reso:SocialMediaType a rdf:Property ;
  rdfs:comment     "A list of types of sites, blog, social media, the Member URL or ID is referring to.  i.e. Website, Blog, Facebook, Twitter, LinkedIn, Skype, etc.,  This list is used to populate the Type with repeating Social Media URL or ID types." ;
  rdfs:domain      reso:Member ;
  rdfs:label       "SocialMediaType" ;
  rdfs:range       xsd:string ;
  reso:CertificationLevel "Bronze" ;
  schema:sameAs    <http://ddwiki.reso.org/display/DDW/SocialMediaType+Field> ;
  vs:term_status   "stable"
.
reso:SocialMedia a rdf:Property ;
  rdfs:domain      reso:Member ;
  rdfs:label       "SocialMedia" ;
  rdfs:range       xsd:string ;
  reso:CertificationLevel "Bronze" ;
  schema:sameAs    <http://ddwiki.reso.org/display/DDW/SocialMedia%5BType%5DUrlOrId+Field> ;
  vs:term_status   "stable"
.
reso:SourceSystemID a rdf:Property ;
  rdfs:comment     "The RESO OUID's OrganizationUniqueId of the Source record provider. The source system is the system from which the record was directly received. In cases where the source system was not where the record originated (the authoritative system), see the Originating System fields.","The RESO OUID's OrganizationUniqueId of the Source record provider.  The source system is the system from which the record was directly received.  In cases where the source system was not where the record originated (the authoritative system), see the Originating System fields." ;
  rdfs:domain      reso:Property,reso:Member ;
  rdfs:label       "SourceSystemID" ;
  rdfs:range       xsd:string ;
  reso:CertificationLevel "Platinum" ;
  reso:PropertyTypes "RESI","RLSE","RINC","LAND","MOBI","FARM","COMS","COML","BUSO" ;
  schema:sameAs    <http://ddwiki.reso.org/display/DDW/SourceSystemID+Field>,<http://ddwiki.reso.org/display/DDW/SourceSystemID+%28Member%29+Field> ;
  vs:term_status   "stable"
.
reso:SourceSystemMemberKey a rdf:Property ;
  rdfs:comment     "The system key, a unique record identifier, from the Source System.  The Source System is the system from which the record was directly received.  In cases where the Source System was not where the record originated (the authoritative system), see the Originating System fields." ;
  rdfs:domain      reso:Member ;
  rdfs:label       "SourceSystemMemberKey" ;
  rdfs:range       xsd:string ;
  reso:CertificationLevel "Silver" ;
  schema:sameAs    <http://ddwiki.reso.org/display/DDW/SourceSystemMemberKey+Field> ;
  vs:term_status   "stable"
.
reso:SourceSystemName a rdf:Property ;
  rdfs:comment     "The name of the immediate record provider. The system from which the record was directly received. The legal name of the company.","The name of the immediate record provider.  The system from which the record was directly received.  The legal name of the company." ;
  rdfs:domain      reso:Property,reso:Member ;
  rdfs:label       "SourceSystemName" ;
  rdfs:range       xsd:string ;
  reso:CertificationLevel "Core","Silver" ;
  reso:PropertyTypes "RESI","RLSE","RINC","LAND","MOBI","FARM","COMS","COML","BUSO" ;
  schema:sameAs    <http://ddwiki.reso.org/display/DDW/SourceSystemName+Field>,<http://ddwiki.reso.org/display/DDW/SourceSystemName+%28Member%29+Field> ;
  vs:term_status   "stable"
.
reso:SyndicateTo a rdf:Property ;
  rdfs:comment     "When permitted by the broker, the options made by the agent on behalf of the seller, where they would like their listings syndicated.  i.e. Zillow, Trulia, Homes.com, etc.","When permitted by the broker, the options made by the individual agent on where they would like their listings syndicated.  i.e. Zillow, Trulia, Homes.com, etc." ;
  rdfs:domain      reso:Property,reso:Member ;
  rdfs:label       "SyndicateTo" ;
  rdfs:range       xsd:string ;
  reso:CertificationLevel "Gold" ;
  reso:PropertyTypes "RESI","RLSE","RINC","LAND","MOBI","FARM","COMS","COML","BUSO" ;
  schema:sameAs    <http://ddwiki.reso.org/display/DDW/SyndicateTo+Field>,<http://ddwiki.reso.org/display/DDW/SyndicateTo+%28Member%29+Field> ;
  vs:term_status   "stable"
.
reso:FranchiseAffiliation a rdf:Property ;
  rdfs:comment     "The name of the franchise to which the broker/office is contracted." ;
  rdfs:domain      reso:Office ;
  rdfs:label       "FranchiseAffiliation" ;
  rdfs:range       xsd:string ;
  reso:CertificationLevel "Silver" ;
  schema:sameAs    <http://ddwiki.reso.org/display/DDW/FranchiseAffiliation+Field> ;
  vs:term_status   "stable"
.
reso:IDXOfficeParticipationYN a rdf:Property ;
  rdfs:comment     "Does the Office/Broker participate in IDX." ;
  rdfs:domain      reso:Office ;
  rdfs:label       "IDXOfficeParticipationYN" ;
  rdfs:range       xsd:boolean ;
  reso:CertificationLevel "Bronze" ;
  schema:sameAs    <http://ddwiki.reso.org/display/DDW/IDXOfficeParticipationYN+Field> ;
  vs:term_status   "stable"
.
reso:MainOfficeKey a rdf:Property ;
  rdfs:comment     "OfficeKey of the Main Office in a firm/company of offices.  This is a self referencing foreign key relating to this resource's OfficeKey.  This key may be the same value as the OfficeKey for a given record if the given office is the Main Office." ;
  rdfs:domain      reso:Office ;
  rdfs:label       "MainOfficeKey" ;
  rdfs:range       xsd:string ;
  reso:CertificationLevel "Core" ;
  schema:sameAs    <http://ddwiki.reso.org/display/DDW/MainOfficeKey+Field> ;
  vs:term_status   "stable"
.
reso:MainOfficeKeyNumeric a rdf:Property ;
  rdfs:comment     "OfficeKey of the Main Office in a firm/company of offices.  This is a self referencing foreign key relating to this resource's OfficeKey.  This key may be the same value as the OfficeKey for a given record if the given office is the Main Office.  This is the numeric only key and used as an alternative to the MainOfficeKey field." ;
  rdfs:domain      reso:Office ;
  rdfs:label       "MainOfficeKeyNumeric" ;
  rdfs:range       xsd:decimal ;
  reso:CertificationLevel "Platinum" ;
  schema:sameAs    <http://ddwiki.reso.org/display/DDW/MainOfficeKeyNumeric+Field> ;
  vs:term_status   "stable"
.
reso:MainOfficeMlsId a rdf:Property ;
  rdfs:comment     "OfficeMlsId of the Main Office in a firm/company of offices." ;
  rdfs:domain      reso:Office ;
  rdfs:label       "MainOfficeMlsId" ;
  rdfs:range       xsd:string ;
  reso:CertificationLevel "Core" ;
  schema:sameAs    <http://ddwiki.reso.org/display/DDW/MainOfficeMlsId+Field> ;
  vs:term_status   "stable"
.
reso:ModificationTimestamp a rdf:Property ;
  rdfs:comment     "The transactional timestamp automatically recorded by the MLS system representing the date/time the listing was last modified.","Date/time the roster (member or office) record was last modified." ;
  rdfs:domain      reso:Property,reso:Member,reso:Office ;
  rdfs:label       "ModificationTimestamp" ;
  rdfs:range       xsd:dateTime ;
  reso:CertificationLevel "Core" ;
  reso:PropertyTypes "RESI","RLSE","RINC","LAND","MOBI","FARM","COMS","COML","BUSO" ;
  schema:sameAs    <http://ddwiki.reso.org/display/DDW/ModificationTimestamp+Field>,<http://ddwiki.reso.org/display/DDW/ModificationTimestamp+%28Member%29+Field>,<http://ddwiki.reso.org/display/DDW/ModificationTimestamp+%28Office%29+Field> ;
  vs:term_status   "stable"
.
reso:OfficeAOR a rdf:Property ;
  rdfs:comment     "The Office's Board or Association of REALTORS." ;
  rdfs:domain      reso:Office ;
  rdfs:label       "OfficeAOR" ;
  rdfs:range       xsd:string ;
  reso:CertificationLevel "Bronze" ;
  schema:sameAs    <http://ddwiki.reso.org/display/DDW/OfficeAOR+Field> ;
  vs:term_status   "stable"
.
reso:OfficeAORMlsId a rdf:Property ;
  rdfs:comment     "The local, well-known identifier for the office's Association of REALTORS. This value may not be unique, specifically in the case of aggregation systems, this value should be the identifier from the original system." ;
  rdfs:domain      reso:Office ;
  rdfs:label       "OfficeAORMlsId" ;
  rdfs:range       xsd:string ;
  reso:CertificationLevel "Bronze" ;
  schema:sameAs    <http://ddwiki.reso.org/display/DDW/OfficeAORMlsId+Field> ;
  vs:term_status   "stable"
.
reso:OfficeAORkey a rdf:Property ;
  rdfs:comment     "A system unique identifier. Specifically, in aggregation systems, the OfficeAORkey is the system unique identifier from the system that the record was retrieved. This may be identical to the related xxxId.  This is a foreign key relating to the AOR's member management system in which the record was originated." ;
  rdfs:domain      reso:Office ;
  rdfs:label       "OfficeAORkey" ;
  rdfs:range       xsd:string ;
  reso:CertificationLevel "Bronze" ;
  schema:sameAs    <http://ddwiki.reso.org/display/DDW/OfficeAORkey+Field> ;
  vs:term_status   "stable"
.
reso:OfficeAORkeyNumeric a rdf:Property ;
  rdfs:comment     "A system unique identifier. Specifically, in aggregation systems, the OfficeAORkey is the system unique identifier from the system that the record was retrieved. This may be identical to the related xxxId.  This is a foreign key relating to the AOR's member management system in which the record was originated.  This is the numeric only key and used as an alternative to the OfficeAORkey field." ;
  rdfs:domain      reso:Office ;
  rdfs:label       "OfficeAORkeyNumeric" ;
  rdfs:range       xsd:decimal ;
  reso:CertificationLevel "Platinum" ;
  schema:sameAs    <http://ddwiki.reso.org/display/DDW/OfficeAORkeyNumeric+Field> ;
  vs:term_status   "stable"
.
reso:OfficeAddress1 a rdf:Property ;
  rdfs:comment     "The street number, direction, name and suffix of the office." ;
  rdfs:domain      reso:Office ;
  rdfs:label       "OfficeAddress1" ;
  rdfs:range       xsd:string ;
  reso:CertificationLevel "Core" ;
  schema:sameAs    <http://ddwiki.reso.org/display/DDW/OfficeAddress1+Field> ;
  vs:term_status   "stable"
.
reso:OfficeAddress2 a rdf:Property ;
  rdfs:comment     "The unit/suite number of the office." ;
  rdfs:domain      reso:Office ;
  rdfs:label       "OfficeAddress2" ;
  rdfs:range       xsd:string ;
  reso:CertificationLevel "Core" ;
  schema:sameAs    <http://ddwiki.reso.org/display/DDW/OfficeAddress2+Field> ;
  vs:term_status   "stable"
.
reso:OfficeAssociationComments a rdf:Property ;
  rdfs:comment     "Notes relating to the office." ;
  rdfs:domain      reso:Office ;
  rdfs:label       "OfficeAssociationComments" ;
  rdfs:range       xsd:string ;
  reso:CertificationLevel "Silver" ;
  schema:sameAs    <http://ddwiki.reso.org/display/DDW/OfficeAssociationComments+Field> ;
  vs:term_status   "stable"
.
reso:OfficeBranchType a rdf:Property ;
  rdfs:comment     "The level of the office in the hierarchy of Main, Branch, Stand Alone, etc.," ;
  rdfs:domain      reso:Office ;
  rdfs:label       "OfficeBranchType" ;
  rdfs:range       xsd:string ;
  reso:CertificationLevel "Silver" ;
  schema:sameAs    <http://ddwiki.reso.org/display/DDW/OfficeBranchType+Field> ;
  vs:term_status   "stable"
.
reso:OfficeBrokerKey a rdf:Property ;
  rdfs:comment     "The MemberKey of the responsible/owning broker.  This is a foreign key relating to the Member resource's MemberKey." ;
  rdfs:domain      reso:Office ;
  rdfs:label       "OfficeBrokerKey" ;
  rdfs:range       xsd:string ;
  reso:CertificationLevel "Core" ;
  schema:sameAs    <http://ddwiki.reso.org/display/DDW/OfficeBrokerKey+Field> ;
  vs:term_status   "stable"
.
reso:OfficeBrokerKeyNumeric a rdf:Property ;
  rdfs:comment     "The MemberKey of the responsible/owning broker.  This is a foreign key relating to the Member resource's MemberKey.  This is the numeric only key and used as an alternative to the OfficeBrokerKey field." ;
  rdfs:domain      reso:Office ;
  rdfs:label       "OfficeBrokerKeyNumeric" ;
  rdfs:range       xsd:decimal ;
  reso:CertificationLevel "Platinum" ;
  schema:sameAs    <http://ddwiki.reso.org/display/DDW/OfficeBrokerKeyNumeric+Field> ;
  vs:term_status   "stable"
.
reso:OfficeBrokerMlsId a rdf:Property ;
  rdfs:comment     "The MemberMlsId of the responsible/owning broker." ;
  rdfs:domain      reso:Office ;
  rdfs:label       "OfficeBrokerMlsId" ;
  rdfs:range       xsd:string ;
  reso:CertificationLevel "Core" ;
  schema:sameAs    <http://ddwiki.reso.org/display/DDW/OfficeBrokerMlsId+Field> ;
  vs:term_status   "stable"
.
reso:OfficeCity a rdf:Property ;
  rdfs:comment     "The city of the office." ;
  rdfs:domain      reso:Office ;
  rdfs:label       "OfficeCity" ;
  rdfs:range       xsd:string ;
  reso:CertificationLevel "Core" ;
  schema:sameAs    <http://ddwiki.reso.org/display/DDW/OfficeCity+Field> ;
  vs:term_status   "stable"
.
reso:OfficeCorporateLicense a rdf:Property ;
  rdfs:comment     "When an office/firm is a corporation, an independent license number is issued." ;
  rdfs:domain      reso:Office ;
  rdfs:label       "OfficeCorporateLicense" ;
  rdfs:range       xsd:string ;
  reso:CertificationLevel "Bronze" ;
  schema:sameAs    <http://ddwiki.reso.org/display/DDW/OfficeCorporateLicense+Field> ;
  vs:term_status   "stable"
.
reso:OfficeCountyOrParish a rdf:Property ;
  rdfs:comment     "The county or parish in which the offices is located." ;
  rdfs:domain      reso:Office ;
  rdfs:label       "OfficeCountyOrParish" ;
  rdfs:range       xsd:string ;
  reso:CertificationLevel "Core" ;
  schema:sameAs    <http://ddwiki.reso.org/display/DDW/OfficeCountyOrParish+Field> ;
  vs:term_status   "stable"
.
reso:OfficeEmail a rdf:Property ;
  rdfs:comment     "The email address of the office" ;
  rdfs:domain      reso:Office ;
  rdfs:label       "OfficeEmail" ;
  rdfs:range       xsd:string ;
  reso:CertificationLevel "Core" ;
  schema:sameAs    <http://ddwiki.reso.org/display/DDW/OfficeEmail+Field> ;
  vs:term_status   "stable"
.
reso:OfficeFax a rdf:Property ;
  rdfs:comment     "North American 10 digit phone numbers should be in the format of ###-###-#### (separated by hyphens).  Other conventions should use the common local standard.  International numbers should be preceded by a plus symbol." ;
  rdfs:domain      reso:Office ;
  rdfs:label       "OfficeFax" ;
  rdfs:range       xsd:string ;
  reso:CertificationLevel "Bronze" ;
  schema:sameAs    <http://ddwiki.reso.org/display/DDW/OfficeFax+Field> ;
  vs:term_status   "stable"
.
reso:OfficeKey a rdf:Property ;
  rdfs:comment     "A system unique identifier. Specifically, in aggregation systems, the Key is the system unique identifier from the system that the record was just retrieved. This may be identical to the related xxxId identifier, but the key is guaranteed unique for this record set. This is a foreign key relating to the Office resource's OfficeKey.","A system unique identifier. Specifically, in aggregation systems, the Key is the system unique identifier from the system that the record was just retrieved. This may be identical to the related xxxId identifier, but the key is guaranteed unique for this record set." ;
  rdfs:domain      reso:Member,reso:Office ;
  rdfs:label       "OfficeKey" ;
  rdfs:range       xsd:string ;
  reso:CertificationLevel "Core" ;
  schema:sameAs    <http://ddwiki.reso.org/display/DDW/OfficeKey+Field>,<http://ddwiki.reso.org/display/DDW/OfficeKey+%28Office%29+Field> ;
  vs:term_status   "stable"
.
reso:OfficeKeyNumeric a rdf:Property ;
  rdfs:comment     "A system unique identifier. Specifically, in aggregation systems, the Key is the system unique identifier from the system that the record was just retrieved. This may be identical to the related xxxId identifier, but the key is guaranteed unique for this record set. This is a foreign key relating to the Office resource's OfficeKey.  This is the numeric only key and used as an alternative to the MemberAORkey field.","A unique identifier for this record from the immediate source. This is the numeric only key and used as an alternative to the OfficeKey fields.  This is the local key of the system.  When records are received from other systems, a local key is commonly applied.  If conveying the original keys from the source or originating systems, see SourceSystemOfficeKey and OriginatingSystemOfficeKey." ;
  rdfs:domain      reso:Member,reso:Office ;
  rdfs:label       "OfficeKeyNumeric" ;
  rdfs:range       xsd:decimal ;
  reso:CertificationLevel "Platinum" ;
  schema:sameAs    <http://ddwiki.reso.org/display/DDW/OfficeKeyNumeric+Field>,<http://ddwiki.reso.org/display/DDW/OfficeKeyNumeric+%28Office%29+Field> ;
  vs:term_status   "stable"
.
reso:OfficeManagerKey a rdf:Property ;
  rdfs:comment     "The lead Office Manager for the given office.  This is a foreign key relating to the Member resource's MemberKey." ;
  rdfs:domain      reso:Office ;
  rdfs:label       "OfficeManagerKey" ;
  rdfs:range       xsd:string ;
  reso:CertificationLevel "Bronze" ;
  schema:sameAs    <http://ddwiki.reso.org/display/DDW/OfficeManagerKey+Field> ;
  vs:term_status   "stable"
.
reso:OfficeManagerKeyNumeric a rdf:Property ;
  rdfs:comment     "The lead Office Manager for the given office.  This is a foreign key relating to the Member resource's MemberKey.  This is the numeric only key and used as an alternative to the OfficeManagerKey field." ;
  rdfs:domain      reso:Office ;
  rdfs:label       "OfficeManagerKeyNumeric" ;
  rdfs:range       xsd:decimal ;
  reso:CertificationLevel "Platinum" ;
  schema:sameAs    <http://ddwiki.reso.org/display/DDW/OfficeManagerKeyNumeric+Field> ;
  vs:term_status   "stable"
.
reso:OfficeManagerMlsId a rdf:Property ;
  rdfs:comment     "The lead Office Manager for the given office." ;
  rdfs:domain      reso:Office ;
  rdfs:label       "OfficeManagerMlsId" ;
  rdfs:range       xsd:string ;
  reso:CertificationLevel "Bronze" ;
  schema:sameAs    <http://ddwiki.reso.org/display/DDW/OfficeManagerMlsId+Field> ;
  vs:term_status   "stable"
.
reso:OfficeMlsId a rdf:Property ;
  rdfs:comment     "The local, well-known identifier. This value may not be unique, specifically in the case of aggregation systems, this value should be the identifier from the original system." ;
  rdfs:domain      reso:Member,reso:Office ;
  rdfs:label       "OfficeMlsId" ;
  rdfs:range       xsd:string ;
  reso:CertificationLevel "Core" ;
  schema:sameAs    <http://ddwiki.reso.org/display/DDW/OfficeMlsId+Field>,<http://ddwiki.reso.org/display/DDW/OfficeMlsId+%28Office%29+Field> ;
  vs:term_status   "stable"
.
reso:OfficeName a rdf:Property ;
  rdfs:comment     "The legal name of the brokerage." ;
  rdfs:domain      reso:Member,reso:Office ;
  rdfs:label       "OfficeName" ;
  rdfs:range       xsd:string ;
  reso:CertificationLevel "Bronze","Core" ;
  schema:sameAs    <http://ddwiki.reso.org/display/DDW/OfficeName+Field>,<http://ddwiki.reso.org/display/DDW/OfficeName+%28Office%29+Field> ;
  vs:term_status   "stable"
.
reso:OfficeNationalAssociationId a rdf:Property ;
  rdfs:comment     "The national association ID of the office.  i.e. in the U.S. is the NRDS number." ;
  rdfs:domain      reso:Office ;
  rdfs:label       "OfficeNationalAssociationId" ;
  rdfs:range       xsd:string ;
  reso:CertificationLevel "Core" ;
  schema:sameAs    <http://ddwiki.reso.org/display/DDW/OfficeNationalAssociationId+Field> ;
  vs:term_status   "stable"
.
reso:OfficePhone a rdf:Property ;
  rdfs:comment     "North American 10 digit phone numbers should be in the format of ###-###-#### (separated by hyphens).  Other conventions should use the common local standard.  International numbers should be preceded by a plus symbol." ;
  rdfs:domain      reso:Office ;
  rdfs:label       "OfficePhone" ;
  rdfs:range       xsd:string ;
  reso:CertificationLevel "Core" ;
  schema:sameAs    <http://ddwiki.reso.org/display/DDW/OfficePhone+Field> ;
  vs:term_status   "stable"
.
reso:OfficePhoneExt a rdf:Property ;
  rdfs:comment     "The extension of the given phone number (if applicable)." ;
  rdfs:domain      reso:Office ;
  rdfs:label       "OfficePhoneExt" ;
  rdfs:range       xsd:string ;
  reso:CertificationLevel "Core" ;
  schema:sameAs    <http://ddwiki.reso.org/display/DDW/OfficePhoneExt+Field> ;
  vs:term_status   "stable"
.
reso:OfficePostalCode a rdf:Property ;
  rdfs:comment     "The postal code of the office." ;
  rdfs:domain      reso:Office ;
  rdfs:label       "OfficePostalCode" ;
  rdfs:range       xsd:string ;
  reso:CertificationLevel "Core" ;
  schema:sameAs    <http://ddwiki.reso.org/display/DDW/OfficePostalCode+Field> ;
  vs:term_status   "stable"
.
reso:OfficePostalCodePlus4 a rdf:Property ;
  rdfs:comment     "The extension of the postal/zip code.  i.e. +4" ;
  rdfs:domain      reso:Office ;
  rdfs:label       "OfficePostalCodePlus4" ;
  rdfs:range       xsd:string ;
  reso:CertificationLevel "Core" ;
  schema:sameAs    <http://ddwiki.reso.org/display/DDW/OfficePostalCodePlus4+Field> ;
  vs:term_status   "stable"
.
reso:OfficeStateOrProvince a rdf:Property ;
  rdfs:comment     "The state or province in which the office is located." ;
  rdfs:domain      reso:Office ;
  rdfs:label       "OfficeStateOrProvince" ;
  rdfs:range       enum:StateOrProvince ;
  reso:CertificationLevel "Core" ;
  schema:sameAs    <http://ddwiki.reso.org/display/DDW/OfficeStateOrProvince+Field> ;
  vs:term_status   "stable"
.
reso:OfficeStatus a rdf:Property ;
  rdfs:comment     "Is the office active, inactive or under disciplinary action." ;
  rdfs:domain      reso:Office ;
  rdfs:label       "OfficeStatus" ;
  rdfs:range       enum:OfficeStatus ;
  reso:CertificationLevel "Core" ;
  schema:sameAs    <http://ddwiki.reso.org/display/DDW/OfficeStatus+Field> ;
  vs:term_status   "stable"
.
reso:OfficeType a rdf:Property ;
  rdfs:comment     "The type of business conducted by the office.  i.e. Real Estate, Appraiser, etc." ;
  rdfs:domain      reso:Office ;
  rdfs:label       "OfficeType" ;
  rdfs:range       enum:OfficeType ;
  reso:CertificationLevel "Bronze" ;
  schema:sameAs    <http://ddwiki.reso.org/display/DDW/OfficeType+Field> ;
  vs:term_status   "stable"
.
reso:OriginalEntryTimestamp a rdf:Property ;
  rdfs:comment     "The transactional timestamp automatically recorded by the MLS system representing the date/time the listing was entered and made visible to members of the MLS.","Date/time the roster (member or office) record was originally input into the source system." ;
  rdfs:domain      reso:Property,reso:Member,reso:Office ;
  rdfs:label       "OriginalEntryTimestamp" ;
  rdfs:range       xsd:dateTime ;
  reso:CertificationLevel "Core" ;
  reso:PropertyTypes "RESI","RLSE","RINC","LAND","MOBI","FARM","COMS","COML","BUSO" ;
  schema:sameAs    <http://ddwiki.reso.org/display/DDW/OriginalEntryTimestamp+Field>,<http://ddwiki.reso.org/display/DDW/OriginalEntryTimestamp+%28Member%29+Field>,<http://ddwiki.reso.org/display/DDW/OriginalEntryTimestamp+%28Office%29+Field> ;
  vs:term_status   "stable"
.
reso:OriginatingSystemID a rdf:Property ;
  rdfs:comment     "The RESO OUID's OrganizationUniqueId of the Originating record provider.  The Originating system is the system with authoritative control over the record.  For example; the name of the MLS where the listing was input.  In cases where the Originating system was not where the record originated (the authoritative system), see the Originating System fields.","The RESO OUID's OrganizationUniqueId of the Originating record provider.  The Originating system is the system with authoritative control over the record.  For example; the name of the MLS where the member was input.  In cases where the Originating system was not where the record originated (the authoritative system), see the Originating System fields.","The RESO OUID's OrganizationUniqueId of the Originating record provider.  The Originating system is the system with authoritative control over the record.  For example; the name of the MLS where the office was input.  In cases where the Originating system was not where the record originated (the authoritative system), see the Originating System fields." ;
  rdfs:domain      reso:Property,reso:Member,reso:Office ;
  rdfs:label       "OriginatingSystemID" ;
  rdfs:range       xsd:string ;
  reso:CertificationLevel "Platinum" ;
  reso:PropertyTypes "RESI","RLSE","RINC","LAND","MOBI","FARM","COMS","COML","BUSO" ;
  schema:sameAs    <http://ddwiki.reso.org/display/DDW/OriginatingSystemID+Field>,<http://ddwiki.reso.org/display/DDW/OriginatingSystemID+%28Member%29+Field>,<http://ddwiki.reso.org/display/DDW/OriginatingSystemID+%28Office%29+Field> ;
  vs:term_status   "stable"
.
reso:OriginatingSystemName a rdf:Property ;
  rdfs:comment     "The name of the Originating record provider.  Most commonly the name of the MLS. The place where the listing is originally input by the member.  The legal name of the company.","The name of the Originating record provider.  Most commonly the name of the MLS. The place where the member is originally input by the member.  The legal name of the company.","The name of the Originating record provider.  Most commonly the name of the MLS. The place where the office is originally input by the member.  The legal name of the company." ;
  rdfs:domain      reso:Property,reso:Member,reso:Office ;
  rdfs:label       "OriginatingSystemName" ;
  rdfs:range       xsd:string ;
  reso:CertificationLevel "Core","Bronze" ;
  reso:PropertyTypes "RESI","RLSE","RINC","LAND","MOBI","FARM","COMS","COML","BUSO" ;
  schema:sameAs    <http://ddwiki.reso.org/display/DDW/OriginatingSystemName+Field>,<http://ddwiki.reso.org/display/DDW/OriginatingSystemName+%28Member%29+Field>,<http://ddwiki.reso.org/display/DDW/OriginatingSystemName+%28Office%29+Field> ;
  vs:term_status   "stable"
.
reso:OriginatingSystemOfficeKey a rdf:Property ;
  rdfs:comment     "The system key, a unique record identifier, from the Originating system.  The Originating system is the system with authoritative control over the record.  For example, the Multiple Listing Service where the office was input.  There may be cases where the Source System (how you received the record) is not the Originating System.  See Source System Key for more information." ;
  rdfs:domain      reso:Office ;
  rdfs:label       "OriginatingSystemOfficeKey" ;
  rdfs:range       xsd:string ;
  reso:CertificationLevel "Core" ;
  schema:sameAs    <http://ddwiki.reso.org/display/DDW/OriginatingSystemOfficeKey+Field> ;
  vs:term_status   "stable"
.
reso:SocialMediaType a rdf:Property ;
  rdfs:comment     "A list of types of sites, blog, social media, the Member URL or ID is referring to.  i.e. Website, Blog, Facebook, Twitter, LinkedIn, Skype, etc.,  This list is used to populate the Type with repeating Social Media URL or ID types.","A list of types of sites, blog, social media, the Office URL or ID is referring to.  i.e. Website, Blog, Facebook, Twitter, LinkedIn, Skype, etc.,  This list is used to populate the Type with repeating Social Media URL or ID types." ;
  rdfs:domain      reso:Member,reso:Office ;
  rdfs:label       "SocialMediaType" ;
  rdfs:range       xsd:string ;
  reso:CertificationLevel "Bronze","Silver" ;
  schema:sameAs    <http://ddwiki.reso.org/display/DDW/SocialMediaType+Field>,<http://ddwiki.reso.org/display/DDW/SocialMediaType+%28Office%29+Field> ;
  vs:term_status   "stable"
.
reso:SocialMedia a rdf:Property ;
  rdfs:domain      reso:Member,reso:Office ;
  rdfs:label       "SocialMedia" ;
  rdfs:range       xsd:string ;
  reso:CertificationLevel "Bronze","Silver" ;
  schema:sameAs    <http://ddwiki.reso.org/display/DDW/SocialMedia%5BType%5DUrlOrId+Field>,<http://ddwiki.reso.org/display/DDW/SocialMedia%5BType%5DUrlOrId+%28Office%29+Field> ;
  vs:term_status   "stable"
.
reso:SourceSystemID a rdf:Property ;
  rdfs:comment     "The RESO OUID's OrganizationUniqueId of the Source record provider. The source system is the system from which the record was directly received. In cases where the source system was not where the record originated (the authoritative system), see the Originating System fields.","The RESO OUID's OrganizationUniqueId of the Source record provider.  The source system is the system from which the record was directly received.  In cases where the source system was not where the record originated (the authoritative system), see the Originating System fields." ;
  rdfs:domain      reso:Property,reso:Member,reso:Office ;
  rdfs:label       "SourceSystemID" ;
  rdfs:range       xsd:string ;
  reso:CertificationLevel "Platinum" ;
  reso:PropertyTypes "RESI","RLSE","RINC","LAND","MOBI","FARM","COMS","COML","BUSO" ;
  schema:sameAs    <http://ddwiki.reso.org/display/DDW/SourceSystemID+Field>,<http://ddwiki.reso.org/display/DDW/SourceSystemID+%28Member%29+Field>,<http://ddwiki.reso.org/display/DDW/SourceSystemID+%28Office%29+Field> ;
  vs:term_status   "stable"
.
reso:SourceSystemName a rdf:Property ;
  rdfs:comment     "The name of the immediate record provider. The system from which the record was directly received. The legal name of the company.","The name of the immediate record provider.  The system from which the record was directly received.  The legal name of the company." ;
  rdfs:domain      reso:Property,reso:Member,reso:Office ;
  rdfs:label       "SourceSystemName" ;
  rdfs:range       xsd:string ;
  reso:CertificationLevel "Core","Silver" ;
  reso:PropertyTypes "RESI","RLSE","RINC","LAND","MOBI","FARM","COMS","COML","BUSO" ;
  schema:sameAs    <http://ddwiki.reso.org/display/DDW/SourceSystemName+Field>,<http://ddwiki.reso.org/display/DDW/SourceSystemName+%28Member%29+Field>,<http://ddwiki.reso.org/display/DDW/SourceSystemName+%28Office%29+Field> ;
  vs:term_status   "stable"
.
reso:SourceSystemOfficeKey a rdf:Property ;
  rdfs:comment     "The system key, a unique record identifier, from the Source System.  The Source System is the system from which the record was directly received.  In cases where the Source System was not where the record originated (the authoritative system), see the Originating System fields." ;
  rdfs:domain      reso:Office ;
  rdfs:label       "SourceSystemOfficeKey" ;
  rdfs:range       xsd:string ;
  reso:CertificationLevel "Silver" ;
  schema:sameAs    <http://ddwiki.reso.org/display/DDW/SourceSystemOfficeKey+Field> ;
  vs:term_status   "stable"
.
reso:SyndicateAgentOption a rdf:Property ;
  rdfs:comment     "A list of options allowing the broker to pass the decision of syndication choice down to the listing agents.  i.e. No Agent Choice, Allow Agent Choice, Restrict Agent Choice, etc." ;
  rdfs:domain      reso:Office ;
  rdfs:label       "SyndicateAgentOption" ;
  rdfs:range       xsd:string ;
  reso:CertificationLevel "Gold" ;
  schema:sameAs    <http://ddwiki.reso.org/display/DDW/SyndicateAgentOption+Field> ;
  vs:term_status   "stable"
.
reso:SyndicateTo a rdf:Property ;
  rdfs:comment     "When permitted by the broker, the options made by the agent on behalf of the seller, where they would like their listings syndicated.  i.e. Zillow, Trulia, Homes.com, etc.","When permitted by the broker, the options made by the individual agent on where they would like their listings syndicated.  i.e. Zillow, Trulia, Homes.com, etc.","The principal broker's choice on where they would like their listings syndicated.  i.e. Zillow, Trulia, Homes.com, etc." ;
  rdfs:domain      reso:Property,reso:Member,reso:Office ;
  rdfs:label       "SyndicateTo" ;
  rdfs:range       xsd:string ;
  reso:CertificationLevel "Gold" ;
  reso:PropertyTypes "RESI","RLSE","RINC","LAND","MOBI","FARM","COMS","COML","BUSO" ;
  schema:sameAs    <http://ddwiki.reso.org/display/DDW/SyndicateTo+Field>,<http://ddwiki.reso.org/display/DDW/SyndicateTo+%28Member%29+Field>,<http://ddwiki.reso.org/display/DDW/SyndicateTo+%28Office%29+Field> ;
  vs:term_status   "stable"
.
reso:Anniversary a rdf:Property ;
  rdfs:comment     "The wedding anniversary of the contact; month, day and year." ;
  rdfs:domain      reso:Contacts ;
  rdfs:label       "Anniversary" ;
  rdfs:range       xsd:date ;
  reso:CertificationLevel "Silver" ;
  schema:sameAs    <http://ddwiki.reso.org/display/DDW/Anniversary+Field> ;
  vs:term_status   "stable"
.
reso:AssistantEmail a rdf:Property ;
  rdfs:comment     "Email address of the contact's assistant." ;
  rdfs:domain      reso:Contacts ;
  rdfs:label       "AssistantEmail" ;
  rdfs:range       xsd:string ;
  reso:CertificationLevel "Silver" ;
  schema:sameAs    <http://ddwiki.reso.org/display/DDW/AssistantEmail+Field> ;
  vs:term_status   "stable"
.
reso:AssistantName a rdf:Property ;
  rdfs:comment     "Name of the contact's assistant." ;
  rdfs:domain      reso:Contacts ;
  rdfs:label       "AssistantName" ;
  rdfs:range       xsd:string ;
  reso:CertificationLevel "Silver" ;
  schema:sameAs    <http://ddwiki.reso.org/display/DDW/AssistantName+Field> ;
  vs:term_status   "stable"
.
reso:AssistantPhone a rdf:Property ;
  rdfs:comment     "Phone number of the contact's assistant." ;
  rdfs:domain      reso:Contacts ;
  rdfs:label       "AssistantPhone" ;
  rdfs:range       xsd:string ;
  reso:CertificationLevel "Silver" ;
  schema:sameAs    <http://ddwiki.reso.org/display/DDW/AssistantPhone+Field> ;
  vs:term_status   "stable"
.
reso:AssistantPhoneExt a rdf:Property ;
  rdfs:comment     "Phone number extension of the contact's assistant." ;
  rdfs:domain      reso:Contacts ;
  rdfs:label       "AssistantPhoneExt" ;
  rdfs:range       xsd:string ;
  reso:CertificationLevel "Silver" ;
  schema:sameAs    <http://ddwiki.reso.org/display/DDW/AssistantPhoneExt+Field> ;
  vs:term_status   "stable"
.
reso:Birthdate a rdf:Property ;
  rdfs:comment     "The birthday of the contact; month, day and year." ;
  rdfs:domain      reso:Contacts ;
  rdfs:label       "Birthdate" ;
  rdfs:range       xsd:date ;
  reso:CertificationLevel "Silver" ;
  schema:sameAs    <http://ddwiki.reso.org/display/DDW/Birthdate+Field> ;
  vs:term_status   "stable"
.
reso:BusinessFax a rdf:Property ;
  rdfs:comment     "North American 10 digit phone numbers should be in the format of ###-###-#### (separated by hyphens).  Other conventions should use the common local standard.  International numbers should be preceded by a plus symbol." ;
  rdfs:domain      reso:Contacts ;
  rdfs:label       "BusinessFax" ;
  rdfs:range       xsd:string ;
  reso:CertificationLevel "Silver" ;
  schema:sameAs    <http://ddwiki.reso.org/display/DDW/BusinessFax+Field> ;
  vs:term_status   "stable"
.
reso:Children a rdf:Property ;
  rdfs:comment     "A list of the names of the contact's children in a comma separated list." ;
  rdfs:domain      reso:Contacts ;
  rdfs:label       "Children" ;
  rdfs:range       xsd:string ;
  reso:CertificationLevel "Silver" ;
  schema:sameAs    <http://ddwiki.reso.org/display/DDW/Children+Field> ;
  vs:term_status   "stable"
.
reso:Company a rdf:Property ;
  rdfs:comment     "The contact's company or employer." ;
  rdfs:domain      reso:Contacts ;
  rdfs:label       "Company" ;
  rdfs:range       xsd:string ;
  reso:CertificationLevel "Silver" ;
  schema:sameAs    <http://ddwiki.reso.org/display/DDW/Company+Field> ;
  vs:term_status   "stable"
.
reso:ContactKey a rdf:Property ;
  rdfs:comment     "A system unique identifier. Specifically, in aggregation systems, the ContactKey is the system unique identifier from the system that the record was retrieved. This may be identical to the related xxxId." ;
  rdfs:domain      reso:Contacts ;
  rdfs:label       "ContactKey" ;
  rdfs:range       xsd:string ;
  reso:CertificationLevel "Silver" ;
  schema:sameAs    <http://ddwiki.reso.org/display/DDW/ContactKey+Field> ;
  vs:term_status   "stable"
.
reso:ContactKeyNumeric a rdf:Property ;
  rdfs:comment     "A system unique identifier. Specifically, in aggregation systems, the ContactKey is the system unique identifier from the system that the record was retrieved. This may be identical to the related xxxId.  This is the numeric only key and used as an alternative to the ContactKey field." ;
  rdfs:domain      reso:Contacts ;
  rdfs:label       "ContactKeyNumeric" ;
  rdfs:range       xsd:decimal ;
  reso:CertificationLevel "Platinum" ;
  schema:sameAs    <http://ddwiki.reso.org/display/DDW/ContactKeyNumeric+Field> ;
  vs:term_status   "stable"
.
reso:ContactLoginId a rdf:Property ;
  rdfs:comment     "The local, well-known identifier for the contact. This value may not be unique, specifically in the case of aggregation systems, this value should be the identifier from the original system and is used by the Contact to logon to a client portal in that system." ;
  rdfs:domain      reso:Contacts ;
  rdfs:label       "ContactLoginId" ;
  rdfs:range       xsd:string ;
  reso:CertificationLevel "Silver" ;
  schema:sameAs    <http://ddwiki.reso.org/display/DDW/ContactLoginId+Field> ;
  vs:term_status   "stable"
.
reso:ContactPassword a rdf:Property ;
  rdfs:comment     "A client password that the member wishes to share with other systems. Normal security considerations apply and are the responsibility of the entity utilizing this field." ;
  rdfs:domain      reso:Contacts ;
  rdfs:label       "ContactPassword" ;
  rdfs:range       xsd:string ;
  reso:CertificationLevel "Silver" ;
  schema:sameAs    <http://ddwiki.reso.org/display/DDW/ContactPassword+Field> ;
  vs:term_status   "stable"
.
reso:ContactStatus a rdf:Property ;
  rdfs:comment     "The status of the contact.  Active, Inactive, On Vacation, Deleted, etc.," ;
  rdfs:domain      reso:Contacts ;
  rdfs:label       "ContactStatus" ;
  rdfs:range       xsd:string ;
  reso:CertificationLevel "Silver" ;
  schema:sameAs    <http://ddwiki.reso.org/display/DDW/ContactStatus+Field> ;
  vs:term_status   "stable"
.
reso:ContactType a rdf:Property ;
  rdfs:comment     "The type of contact.  i.e. Business, Friend, Family, Prospect, Ready to Buy, etc." ;
  rdfs:domain      reso:Contacts ;
  rdfs:label       "ContactType" ;
  rdfs:range       xsd:string ;
  reso:CertificationLevel "Silver" ;
  schema:sameAs    <http://ddwiki.reso.org/display/DDW/ContactType+Field> ;
  vs:term_status   "stable"
.
reso:Department a rdf:Property ;
  rdfs:comment     "The department in which the contact works." ;
  rdfs:domain      reso:Contacts ;
  rdfs:label       "Department" ;
  rdfs:range       xsd:string ;
  reso:CertificationLevel "Silver" ;
  schema:sameAs    <http://ddwiki.reso.org/display/DDW/Department+Field> ;
  vs:term_status   "stable"
.
reso:DirectPhone a rdf:Property ;
  rdfs:comment     "North American 10 digit phone numbers should be in the format of ###-###-#### (separated by hyphens).  Other conventions should use the common local standard.  International numbers should be preceded by a plus symbol." ;
  rdfs:domain      reso:Contacts ;
  rdfs:label       "DirectPhone" ;
  rdfs:range       xsd:string ;
  reso:CertificationLevel "Silver" ;
  schema:sameAs    <http://ddwiki.reso.org/display/DDW/DirectPhone+Field> ;
  vs:term_status   "stable"
.
reso:Email a rdf:Property ;
  rdfs:comment     "The preferred Email address of the contact." ;
  rdfs:domain      reso:Contacts ;
  rdfs:label       "Email" ;
  rdfs:range       xsd:string ;
  reso:CertificationLevel "Silver" ;
  schema:sameAs    <http://ddwiki.reso.org/display/DDW/Email+Field> ;
  vs:term_status   "stable"
.
reso:Email2 a rdf:Property ;
  rdfs:comment     "The secondary email address of the contact." ;
  rdfs:domain      reso:Contacts ;
  rdfs:label       "Email2" ;
  rdfs:range       xsd:string ;
  reso:CertificationLevel "Silver" ;
  schema:sameAs    <http://ddwiki.reso.org/display/DDW/Email2+Field> ;
  vs:term_status   "stable"
.
reso:Email3 a rdf:Property ;
  rdfs:comment     "The tertiary email address of the contact." ;
  rdfs:domain      reso:Contacts ;
  rdfs:label       "Email3" ;
  rdfs:range       xsd:string ;
  reso:CertificationLevel "Silver" ;
  schema:sameAs    <http://ddwiki.reso.org/display/DDW/Email3+Field> ;
  vs:term_status   "stable"
.
reso:FirstName a rdf:Property ;
  rdfs:comment     "The first name of the Member." ;
  rdfs:domain      reso:Contacts ;
  rdfs:label       "FirstName" ;
  rdfs:range       xsd:string ;
  reso:CertificationLevel "Silver" ;
  schema:sameAs    <http://ddwiki.reso.org/display/DDW/FirstName+Field> ;
  vs:term_status   "stable"
.
reso:FullName a rdf:Property ;
  rdfs:comment     "The full name of the Member. (First Middle Last) or a alternate full name." ;
  rdfs:domain      reso:Contacts ;
  rdfs:label       "FullName" ;
  rdfs:range       xsd:string ;
  reso:CertificationLevel "Silver" ;
  schema:sameAs    <http://ddwiki.reso.org/display/DDW/FullName+Field> ;
  vs:term_status   "stable"
.
reso:Gender a rdf:Property ;
  rdfs:comment     "The contact's gender." ;
  rdfs:domain      reso:Contacts ;
  rdfs:label       "Gender" ;
  rdfs:range       xsd:string ;
  reso:CertificationLevel "Silver" ;
  schema:sameAs    <http://ddwiki.reso.org/display/DDW/Gender+Field> ;
  vs:term_status   "stable"
.
reso:Groups a rdf:Property ;
  rdfs:comment     "Also knows as Tags, Categories, Circles," ;
  rdfs:domain      reso:Contacts ;
  rdfs:label       "Groups" ;
  rdfs:range       xsd:string ;
  reso:CertificationLevel "Silver" ;
  schema:sameAs    <http://ddwiki.reso.org/display/DDW/Groups+Field> ;
  vs:term_status   "stable"
.
reso:HomeAddress1 a rdf:Property ;
  rdfs:comment     "The street number, direction, name and suffix of the contact's home." ;
  rdfs:domain      reso:Contacts ;
  rdfs:label       "HomeAddress1" ;
  rdfs:range       xsd:string ;
  reso:CertificationLevel "Silver" ;
  schema:sameAs    <http://ddwiki.reso.org/display/DDW/HomeAddress1+Field> ;
  vs:term_status   "stable"
.
reso:HomeAddress2 a rdf:Property ;
  rdfs:comment     "The unit/suite number of the contact's home." ;
  rdfs:domain      reso:Contacts ;
  rdfs:label       "HomeAddress2" ;
  rdfs:range       xsd:string ;
  reso:CertificationLevel "Silver" ;
  schema:sameAs    <http://ddwiki.reso.org/display/DDW/HomeAddress2+Field> ;
  vs:term_status   "stable"
.
reso:HomeCarrierRoute a rdf:Property ;
  rdfs:domain      reso:Contacts ;
  rdfs:label       "HomeCarrierRoute" ;
  rdfs:range       xsd:string ;
  reso:CertificationLevel "Silver" ;
  schema:sameAs    <http://ddwiki.reso.org/display/DDW/HomeCarrierRoute+Field> ;
  vs:term_status   "stable"
.
reso:HomeCity a rdf:Property ;
  rdfs:comment     "The city of the contact's home." ;
  rdfs:domain      reso:Contacts ;
  rdfs:label       "HomeCity" ;
  rdfs:range       xsd:string ;
  reso:CertificationLevel "Silver" ;
  schema:sameAs    <http://ddwiki.reso.org/display/DDW/HomeCity+Field> ;
  vs:term_status   "stable"
.
reso:HomeCountry a rdf:Property ;
  rdfs:comment     "The country abbreviation in a postal address." ;
  rdfs:domain      reso:Contacts ;
  rdfs:label       "HomeCountry" ;
  rdfs:range       enum:Country ;
  reso:CertificationLevel "Silver" ;
  schema:sameAs    <http://ddwiki.reso.org/display/DDW/HomeCountry+Field> ;
  vs:term_status   "stable"
.
reso:HomeCountyOrParish a rdf:Property ;
  rdfs:comment     "The county or parish in which the contact's home is addressed." ;
  rdfs:domain      reso:Contacts ;
  rdfs:label       "HomeCountyOrParish" ;
  rdfs:range       xsd:string ;
  reso:CertificationLevel "Silver" ;
  schema:sameAs    <http://ddwiki.reso.org/display/DDW/HomeCountyOrParish+Field> ;
  vs:term_status   "stable"
.
reso:HomeFax a rdf:Property ;
  rdfs:comment     "North American 10 digit phone numbers should be in the format of ###-###-#### (separated by hyphens).  Other conventions should use the common local standard.  International numbers should be preceded by a plus symbol." ;
  rdfs:domain      reso:Contacts ;
  rdfs:label       "HomeFax" ;
  rdfs:range       xsd:string ;
  reso:CertificationLevel "Silver" ;
  schema:sameAs    <http://ddwiki.reso.org/display/DDW/HomeFax+Field> ;
  vs:term_status   "stable"
.
reso:HomePhone a rdf:Property ;
  rdfs:comment     "North American 10 digit phone numbers should be in the format of ###-###-#### (separated by hyphens).  Other conventions should use the common local standard.  International numbers should be preceded by a plus symbol." ;
  rdfs:domain      reso:Contacts ;
  rdfs:label       "HomePhone" ;
  rdfs:range       xsd:string ;
  reso:CertificationLevel "Silver" ;
  schema:sameAs    <http://ddwiki.reso.org/display/DDW/HomePhone+Field> ;
  vs:term_status   "stable"
.
reso:HomePostalCode a rdf:Property ;
  rdfs:comment     "The postal code of the contact's home." ;
  rdfs:domain      reso:Contacts ;
  rdfs:label       "HomePostalCode" ;
  rdfs:range       xsd:string ;
  reso:CertificationLevel "Silver" ;
  schema:sameAs    <http://ddwiki.reso.org/display/DDW/HomePostalCode+Field> ;
  vs:term_status   "stable"
.
reso:HomePostalCodePlus4 a rdf:Property ;
  rdfs:comment     "The extension of the postal/zip code.  i.e. +4" ;
  rdfs:domain      reso:Contacts ;
  rdfs:label       "HomePostalCodePlus4" ;
  rdfs:range       xsd:string ;
  reso:CertificationLevel "Silver" ;
  schema:sameAs    <http://ddwiki.reso.org/display/DDW/HomePostalCodePlus4+Field> ;
  vs:term_status   "stable"
.
reso:HomeStateOrProvince a rdf:Property ;
  rdfs:comment     "The state or province in which the contact's home is addressed." ;
  rdfs:domain      reso:Contacts ;
  rdfs:label       "HomeStateOrProvince" ;
  rdfs:range       enum:StateOrProvince ;
  reso:CertificationLevel "Silver" ;
  schema:sameAs    <http://ddwiki.reso.org/display/DDW/HomeStateOrProvince+Field> ;
  vs:term_status   "stable"
.
reso:JobTitle a rdf:Property ;
  rdfs:comment     "The title or position of the member within their organization." ;
  rdfs:domain      reso:Member,reso:Contacts ;
  rdfs:label       "JobTitle" ;
  rdfs:range       xsd:string ;
  reso:CertificationLevel "Silver" ;
  schema:sameAs    <http://ddwiki.reso.org/display/DDW/JobTitle+Field>,<http://ddwiki.reso.org/display/DDW/JobTitle+%28Contacts%29+Field> ;
  vs:term_status   "stable"
.
reso:Language a rdf:Property ;
  rdfs:comment     "The languages spoken by the contact." ;
  rdfs:domain      reso:Contacts ;
  rdfs:label       "Language" ;
  rdfs:range       enum:Languages ;
  reso:CertificationLevel "Silver" ;
  schema:sameAs    <http://ddwiki.reso.org/display/DDW/Language+Field> ;
  vs:term_status   "stable"
.
reso:LastName a rdf:Property ;
  rdfs:comment     "The last name of the Member." ;
  rdfs:domain      reso:Contacts ;
  rdfs:label       "LastName" ;
  rdfs:range       xsd:string ;
  reso:CertificationLevel "Silver" ;
  schema:sameAs    <http://ddwiki.reso.org/display/DDW/LastName+Field> ;
  vs:term_status   "stable"
.
reso:MiddleName a rdf:Property ;
  rdfs:comment     "The middle name of the Member." ;
  rdfs:domain      reso:Contacts ;
  rdfs:label       "MiddleName" ;
  rdfs:range       xsd:string ;
  reso:CertificationLevel "Silver" ;
  schema:sameAs    <http://ddwiki.reso.org/display/DDW/MiddleName+Field> ;
  vs:term_status   "stable"
.
reso:MobilePhone a rdf:Property ;
  rdfs:comment     "North American 10 digit phone numbers should be in the format of ###-###-#### (separated by hyphens).  Other conventions should use the common local standard.  International numbers should be preceded by a plus symbol." ;
  rdfs:domain      reso:Contacts ;
  rdfs:label       "MobilePhone" ;
  rdfs:range       xsd:string ;
  reso:CertificationLevel "Silver" ;
  schema:sameAs    <http://ddwiki.reso.org/display/DDW/MobilePhone+Field> ;
  vs:term_status   "stable"
.
reso:ModificationTimestamp a rdf:Property ;
  rdfs:comment     "The transactional timestamp automatically recorded by the MLS system representing the date/time the listing was last modified.","Date/time the roster (member or office) record was last modified.","Date/time the contact record was last modified." ;
  rdfs:domain      reso:Property,reso:Member,reso:Office,reso:Contacts ;
  rdfs:label       "ModificationTimestamp" ;
  rdfs:range       xsd:dateTime ;
  reso:CertificationLevel "Core","Silver" ;
  reso:PropertyTypes "RESI","RLSE","RINC","LAND","MOBI","FARM","COMS","COML","BUSO" ;
  schema:sameAs    <http://ddwiki.reso.org/display/DDW/ModificationTimestamp+Field>,<http://ddwiki.reso.org/display/DDW/ModificationTimestamp+%28Member%29+Field>,<http://ddwiki.reso.org/display/DDW/ModificationTimestamp+%28Office%29+Field>,<http://ddwiki.reso.org/display/DDW/ModificationTimestamp+%28Contacts%29+Field> ;
  vs:term_status   "stable"
.
reso:NamePrefix a rdf:Property ;
  rdfs:comment     "Prefix to the name (e.g. Dr. Mr. Ms. etc.)" ;
  rdfs:domain      reso:Contacts ;
  rdfs:label       "NamePrefix" ;
  rdfs:range       xsd:string ;
  reso:CertificationLevel "Silver" ;
  schema:sameAs    <http://ddwiki.reso.org/display/DDW/NamePrefix+Field> ;
  vs:term_status   "stable"
.
reso:NameSuffix a rdf:Property ;
  rdfs:comment     "Suffix to the surname (e.g. Esq.,  Jr.,  III etc.)" ;
  rdfs:domain      reso:Contacts ;
  rdfs:label       "NameSuffix" ;
  rdfs:range       xsd:string ;
  reso:CertificationLevel "Silver" ;
  schema:sameAs    <http://ddwiki.reso.org/display/DDW/NameSuffix+Field> ;
  vs:term_status   "stable"
.
reso:Nickname a rdf:Property ;
  rdfs:comment     "An alternate name used by the Member, usually as a substitute for the first name." ;
  rdfs:domain      reso:Contacts ;
  rdfs:label       "Nickname" ;
  rdfs:range       xsd:string ;
  reso:CertificationLevel "Silver" ;
  schema:sameAs    <http://ddwiki.reso.org/display/DDW/Nickname+Field> ;
  vs:term_status   "stable"
.
reso:Notes a rdf:Property ;
  rdfs:comment     "Notes about the client." ;
  rdfs:domain      reso:Contacts ;
  rdfs:label       "Notes" ;
  rdfs:range       xsd:string ;
  reso:CertificationLevel "Silver" ;
  schema:sameAs    <http://ddwiki.reso.org/display/DDW/Notes+Field> ;
  vs:term_status   "stable"
.
reso:OfficePhone a rdf:Property ;
  rdfs:comment     "North American 10 digit phone numbers should be in the format of ###-###-#### (separated by hyphens).  Other conventions should use the common local standard.  International numbers should be preceded by a plus symbol." ;
  rdfs:domain      reso:Office,reso:Contacts ;
  rdfs:label       "OfficePhone" ;
  rdfs:range       xsd:string ;
  reso:CertificationLevel "Core","Silver" ;
  schema:sameAs    <http://ddwiki.reso.org/display/DDW/OfficePhone+Field>,<http://ddwiki.reso.org/display/DDW/OfficePhone+%28Contacts%29+Field> ;
  vs:term_status   "stable"
.
reso:OfficePhoneExt a rdf:Property ;
  rdfs:comment     "The extension of the given phone number (if applicable)." ;
  rdfs:domain      reso:Office,reso:Contacts ;
  rdfs:label       "OfficePhoneExt" ;
  rdfs:range       xsd:string ;
  reso:CertificationLevel "Core","Silver" ;
  schema:sameAs    <http://ddwiki.reso.org/display/DDW/OfficePhoneExt+Field>,<http://ddwiki.reso.org/display/DDW/OfficePhoneExt+%28Contacts%29+Field> ;
  vs:term_status   "stable"
.
reso:OriginalEntryTimestamp a rdf:Property ;
  rdfs:comment     "The transactional timestamp automatically recorded by the MLS system representing the date/time the listing was entered and made visible to members of the MLS.","Date/time the roster (member or office) record was originally input into the source system.","Date/time the contact record was originally input into the source system." ;
  rdfs:domain      reso:Property,reso:Member,reso:Office,reso:Contacts ;
  rdfs:label       "OriginalEntryTimestamp" ;
  rdfs:range       xsd:dateTime ;
  reso:CertificationLevel "Core","Silver" ;
  reso:PropertyTypes "RESI","RLSE","RINC","LAND","MOBI","FARM","COMS","COML","BUSO" ;
  schema:sameAs    <http://ddwiki.reso.org/display/DDW/OriginalEntryTimestamp+Field>,<http://ddwiki.reso.org/display/DDW/OriginalEntryTimestamp+%28Member%29+Field>,<http://ddwiki.reso.org/display/DDW/OriginalEntryTimestamp+%28Office%29+Field>,<http://ddwiki.reso.org/display/DDW/OriginalEntryTimestamp+%28Contacts%29+Field> ;
  vs:term_status   "stable"
.
reso:OriginatingSystemContactKey a rdf:Property ;
  rdfs:comment     "The system key, a unique record identifier, from the Originating system.  The Originating system is the system with authoritative control over the record.  For example, the Multiple Listing Service where the Contact was input.  There may be cases where the Source System (how you received the record) is not the Originating System.  See Source System Key for more information." ;
  rdfs:domain      reso:Contacts ;
  rdfs:label       "OriginatingSystemContactKey" ;
  rdfs:range       xsd:string ;
  reso:CertificationLevel "Silver" ;
  schema:sameAs    <http://ddwiki.reso.org/display/DDW/OriginatingSystemContactKey+Field> ;
  vs:term_status   "stable"
.
reso:OriginatingSystemID a rdf:Property ;
  rdfs:comment     "The RESO OUID's OrganizationUniqueId of the Originating record provider.  The Originating system is the system with authoritative control over the record.  For example; the name of the MLS where the listing was input.  In cases where the Originating system was not where the record originated (the authoritative system), see the Originating System fields.","The RESO OUID's OrganizationUniqueId of the Originating record provider.  The Originating system is the system with authoritative control over the record.  For example; the name of the MLS where the member was input.  In cases where the Originating system was not where the record originated (the authoritative system), see the Originating System fields.","The RESO OUID's OrganizationUniqueId of the Originating record provider.  The Originating system is the system with authoritative control over the record.  For example; the name of the MLS where the office was input.  In cases where the Originating system was not where the record originated (the authoritative system), see the Originating System fields.","The RESO OUID's OrganizationUniqueId of the Originating record provider.  The Originating system is the system with authoritative control over the record.  For example; the name of the MLS where the Contact was input.  In cases where the Originating system was not where the record originated (the authoritative system), see the Originating System fields." ;
  rdfs:domain      reso:Property,reso:Member,reso:Office,reso:Contacts ;
  rdfs:label       "OriginatingSystemID" ;
  rdfs:range       xsd:string ;
  reso:CertificationLevel "Platinum" ;
  reso:PropertyTypes "RESI","RLSE","RINC","LAND","MOBI","FARM","COMS","COML","BUSO" ;
  schema:sameAs    <http://ddwiki.reso.org/display/DDW/OriginatingSystemID+Field>,<http://ddwiki.reso.org/display/DDW/OriginatingSystemID+%28Member%29+Field>,<http://ddwiki.reso.org/display/DDW/OriginatingSystemID+%28Office%29+Field>,<http://ddwiki.reso.org/display/DDW/OriginatingSystemID+%28Contacts%29+Field> ;
  vs:term_status   "stable"
.
reso:OriginatingSystemName a rdf:Property ;
  rdfs:comment     "The name of the Originating record provider.  Most commonly the name of the MLS. The place where the listing is originally input by the member.  The legal name of the company.","The name of the Originating record provider.  Most commonly the name of the MLS. The place where the member is originally input by the member.  The legal name of the company.","The name of the Originating record provider.  Most commonly the name of the MLS. The place where the office is originally input by the member.  The legal name of the company.","The name of the Originating record provider.  Most commonly the name of the MLS. The place where the Contact is originally input by the member.  The legal name of the company." ;
  rdfs:domain      reso:Property,reso:Member,reso:Office,reso:Contacts ;
  rdfs:label       "OriginatingSystemName" ;
  rdfs:range       xsd:string ;
  reso:CertificationLevel "Core","Bronze","Silver" ;
  reso:PropertyTypes "RESI","RLSE","RINC","LAND","MOBI","FARM","COMS","COML","BUSO" ;
  schema:sameAs    <http://ddwiki.reso.org/display/DDW/OriginatingSystemName+Field>,<http://ddwiki.reso.org/display/DDW/OriginatingSystemName+%28Member%29+Field>,<http://ddwiki.reso.org/display/DDW/OriginatingSystemName+%28Office%29+Field>,<http://ddwiki.reso.org/display/DDW/OriginatingSystemName+%28Contacts%29+Field> ;
  vs:term_status   "stable"
.
reso:OtherAddress1 a rdf:Property ;
  rdfs:comment     "The other street number, direction, name and suffix of the contact." ;
  rdfs:domain      reso:Contacts ;
  rdfs:label       "OtherAddress1" ;
  rdfs:range       xsd:string ;
  reso:CertificationLevel "Silver" ;
  schema:sameAs    <http://ddwiki.reso.org/display/DDW/OtherAddress1+Field> ;
  vs:term_status   "stable"
.
reso:OtherAddress2 a rdf:Property ;
  rdfs:comment     "The other unit/suite number of the contact." ;
  rdfs:domain      reso:Contacts ;
  rdfs:label       "OtherAddress2" ;
  rdfs:range       xsd:string ;
  reso:CertificationLevel "Silver" ;
  schema:sameAs    <http://ddwiki.reso.org/display/DDW/OtherAddress2+Field> ;
  vs:term_status   "stable"
.
reso:OtherCarrierRoute a rdf:Property ;
  rdfs:domain      reso:Contacts ;
  rdfs:label       "OtherCarrierRoute" ;
  rdfs:range       xsd:string ;
  reso:CertificationLevel "Silver" ;
  schema:sameAs    <http://ddwiki.reso.org/display/DDW/OtherCarrierRoute+Field> ;
  vs:term_status   "stable"
.
reso:OtherCity a rdf:Property ;
  rdfs:comment     "The other city of the contact." ;
  rdfs:domain      reso:Contacts ;
  rdfs:label       "OtherCity" ;
  rdfs:range       xsd:string ;
  reso:CertificationLevel "Silver" ;
  schema:sameAs    <http://ddwiki.reso.org/display/DDW/OtherCity+Field> ;
  vs:term_status   "stable"
.
reso:OtherCountry a rdf:Property ;
  rdfs:comment     "The other country abbreviation in a postal address." ;
  rdfs:domain      reso:Contacts ;
  rdfs:label       "OtherCountry" ;
  rdfs:range       enum:Country ;
  reso:CertificationLevel "Silver" ;
  schema:sameAs    <http://ddwiki.reso.org/display/DDW/OtherCountry+Field> ;
  vs:term_status   "stable"
.
reso:OtherCountyOrParish a rdf:Property ;
  rdfs:comment     "The other county or parish in which contact is addressed." ;
  rdfs:domain      reso:Contacts ;
  rdfs:label       "OtherCountyOrParish" ;
  rdfs:range       xsd:string ;
  reso:CertificationLevel "Silver" ;
  schema:sameAs    <http://ddwiki.reso.org/display/DDW/OtherCountyOrParish+Field> ;
  vs:term_status   "stable"
.
reso:OtherPhoneType a rdf:Property ;
  rdfs:comment     "The type of \"other\" phone that does not already exist in the given phone fields or if a second of any type of phone field is needed.  i.e. HomePhone2,  BrothersPhone, etc.  This is used as the list of options for the Other Phone repeating elements." ;
  rdfs:domain      reso:Contacts ;
  rdfs:label       "OtherPhoneType" ;
  rdfs:range       xsd:string ;
  reso:CertificationLevel "Silver" ;
  schema:sameAs    <http://ddwiki.reso.org/display/DDW/OtherPhoneType+Field> ;
  vs:term_status   "stable"
.
reso:OtherPhone a rdf:Property ;
  rdfs:comment     "The \"other\" phone option allowing members to convey additional phone numbers other than those already covered by the VoiceMailExt, OfficePhoneExt, etc., fields.  This is a repeating element.  Use the OtherPhoneType for a selection of additional phone types." ;
  rdfs:domain      reso:Contacts ;
  rdfs:label       "OtherPhone" ;
  rdfs:range       xsd:string ;
  reso:CertificationLevel "Silver" ;
  schema:sameAs    <http://ddwiki.reso.org/display/DDW/OtherPhone%5BType%5DExt+Field> ;
  vs:term_status   "stable"
.
reso:OtherPhone a rdf:Property ;
  rdfs:comment     "The \"other\" phone option allowing members to convey additional phone numbers other than those already covered by the VoiceMailExt, OfficePhoneExt, etc., fields.  This is a repeating element.  Use the OtherPhoneType for a selection of additional phone types.","The \"other\" phone option allowing members to convey additional phone numbers other than those already covered by the HomePhone, VoiceMail, etc., fields.  This is a repeating element.  Use the OtherPhoneType for a selection of additional phone types." ;
  rdfs:domain      reso:Contacts ;
  rdfs:label       "OtherPhone" ;
  rdfs:range       xsd:string ;
  reso:CertificationLevel "Silver" ;
  schema:sameAs    <http://ddwiki.reso.org/display/DDW/OtherPhone%5BType%5DExt+Field>,<http://ddwiki.reso.org/display/DDW/OtherPhone%5BType%5DNumber+Field> ;
  vs:term_status   "stable"
.
reso:OtherPostalCode a rdf:Property ;
  rdfs:comment     "The other postal code of the contact." ;
  rdfs:domain      reso:Contacts ;
  rdfs:label       "OtherPostalCode" ;
  rdfs:range       xsd:string ;
  reso:CertificationLevel "Silver" ;
  schema:sameAs    <http://ddwiki.reso.org/display/DDW/OtherPostalCode+Field> ;
  vs:term_status   "stable"
.
reso:OtherPostalCodePlus4 a rdf:Property ;
  rdfs:comment     "The other extension of the postal/zip code.  i.e. +4" ;
  rdfs:domain      reso:Contacts ;
  rdfs:label       "OtherPostalCodePlus4" ;
  rdfs:range       xsd:string ;
  reso:CertificationLevel "Silver" ;
  schema:sameAs    <http://ddwiki.reso.org/display/DDW/OtherPostalCodePlus4+Field> ;
  vs:term_status   "stable"
.
reso:OtherStateOrProvince a rdf:Property ;
  rdfs:comment     "The other state or province in which the contact is addressed." ;
  rdfs:domain      reso:Contacts ;
  rdfs:label       "OtherStateOrProvince" ;
  rdfs:range       enum:StateOrProvince ;
  reso:CertificationLevel "Silver" ;
  schema:sameAs    <http://ddwiki.reso.org/display/DDW/OtherStateOrProvince+Field> ;
  vs:term_status   "stable"
.
reso:OwnerMemberID a rdf:Property ;
  rdfs:comment     "The local, well-known identifier for the member owning the contact." ;
  rdfs:domain      reso:Contacts ;
  rdfs:label       "OwnerMemberID" ;
  rdfs:range       xsd:string ;
  reso:CertificationLevel "Silver" ;
  schema:sameAs    <http://ddwiki.reso.org/display/DDW/OwnerMemberID+Field> ;
  vs:term_status   "stable"
.
reso:OwnerMemberKey a rdf:Property ;
  rdfs:comment     "The unique identifier (key) of the member owning the contact. This is a foreign key relating to the Member resource's MemberKey." ;
  rdfs:domain      reso:Contacts ;
  rdfs:label       "OwnerMemberKey" ;
  rdfs:range       xsd:string ;
  reso:CertificationLevel "Silver" ;
  schema:sameAs    <http://ddwiki.reso.org/display/DDW/OwnerMemberKey+Field> ;
  vs:term_status   "stable"
.
reso:OwnerMemberKeyNumeric a rdf:Property ;
  rdfs:comment     "The unique identifier (key) of the member owning the contact. This is a foreign key relating to the Member resource's MemberKey.  This is the numeric only key and used as an alternative to the OwnerMemberKey field." ;
  rdfs:domain      reso:Contacts ;
  rdfs:label       "OwnerMemberKeyNumeric" ;
  rdfs:range       xsd:decimal ;
  reso:CertificationLevel "Platinum" ;
  schema:sameAs    <http://ddwiki.reso.org/display/DDW/OwnerMemberKeyNumeric+Field> ;
  vs:term_status   "stable"
.
reso:Pager a rdf:Property ;
  rdfs:comment     "North American 10 digit phone numbers should be in the format of ###-###-#### (separated by hyphens).  Other conventions should use the common local standard.  International numbers should be preceded by a plus symbol." ;
  rdfs:domain      reso:Contacts ;
  rdfs:label       "Pager" ;
  rdfs:range       xsd:string ;
  reso:CertificationLevel "Silver" ;
  schema:sameAs    <http://ddwiki.reso.org/display/DDW/Pager+Field> ;
  vs:term_status   "stable"
.
reso:PhoneTTYTTD a rdf:Property ;
  rdfs:comment     "North American 10 digit phone numbers should be in the format of ###-###-#### (separated by hyphens).  Other conventions should use the common local standard.  International numbers should be preceded by a plus symbol." ;
  rdfs:domain      reso:Contacts ;
  rdfs:label       "PhoneTTYTTD" ;
  rdfs:range       xsd:string ;
  reso:CertificationLevel "Silver" ;
  schema:sameAs    <http://ddwiki.reso.org/display/DDW/PhoneTTYTTD+Field> ;
  vs:term_status   "stable"
.
reso:PreferredAddress a rdf:Property ;
  rdfs:comment     "A list of the address options Home, Work and Other used to determine the address preferred by the client." ;
  rdfs:domain      reso:Contacts ;
  rdfs:label       "PreferredAddress" ;
  rdfs:range       xsd:string ;
  reso:CertificationLevel "Silver" ;
  schema:sameAs    <http://ddwiki.reso.org/display/DDW/PreferredAddress+Field> ;
  vs:term_status   "stable"
.
reso:PreferredPhone a rdf:Property ;
  rdfs:comment     "A list of the phone options Office, Mobile, Direct, Voicemail, Other used to determine the phone preferred by the client." ;
  rdfs:domain      reso:Contacts ;
  rdfs:label       "PreferredPhone" ;
  rdfs:range       xsd:string ;
  reso:CertificationLevel "Silver" ;
  schema:sameAs    <http://ddwiki.reso.org/display/DDW/PreferredPhone+Field> ;
  vs:term_status   "stable"
.
reso:ReferredBy a rdf:Property ;
  rdfs:comment     "Name of the person who referred the contact." ;
  rdfs:domain      reso:Contacts ;
  rdfs:label       "ReferredBy" ;
  rdfs:range       xsd:string ;
  reso:CertificationLevel "Silver" ;
  schema:sameAs    <http://ddwiki.reso.org/display/DDW/ReferredBy+Field> ;
  vs:term_status   "stable"
.
reso:SocialMediaType a rdf:Property ;
  rdfs:comment     "A list of types of sites, blog, social media, the Member URL or ID is referring to.  i.e. Website, Blog, Facebook, Twitter, LinkedIn, Skype, etc.,  This list is used to populate the Type with repeating Social Media URL or ID types.","A list of types of sites, blog, social media, the Office URL or ID is referring to.  i.e. Website, Blog, Facebook, Twitter, LinkedIn, Skype, etc.,  This list is used to populate the Type with repeating Social Media URL or ID types." ;
  rdfs:domain      reso:Member,reso:Office,reso:Contacts ;
  rdfs:label       "SocialMediaType" ;
  rdfs:range       xsd:string ;
  reso:CertificationLevel "Bronze","Silver" ;
  schema:sameAs    <http://ddwiki.reso.org/display/DDW/SocialMediaType+Field>,<http://ddwiki.reso.org/display/DDW/SocialMediaType+%28Office%29+Field>,<http://ddwiki.reso.org/display/DDW/SocialMediaType+%28Contacts%29+Field> ;
  vs:term_status   "stable"
.
reso:SocialMedia a rdf:Property ;
  rdfs:domain      reso:Member,reso:Office,reso:Contacts ;
  rdfs:label       "SocialMedia" ;
  rdfs:range       xsd:string ;
  reso:CertificationLevel "Bronze","Silver" ;
  schema:sameAs    <http://ddwiki.reso.org/display/DDW/SocialMedia%5BType%5DUrlOrId+Field>,<http://ddwiki.reso.org/display/DDW/SocialMedia%5BType%5DUrlOrId+%28Office%29+Field>,<http://ddwiki.reso.org/display/DDW/SocialMedia%5BType%5DUrlOrId+%28Contacts%29+Field> ;
  vs:term_status   "stable"
.
reso:SourceSystemContactKey a rdf:Property ;
  rdfs:comment     "The system key, a unique record identifier, from the Source System.  The Source System is the system from which the record was directly received.  In cases where the Source System was not where the record originated (the authoritative system), see the Originating System fields." ;
  rdfs:domain      reso:Contacts ;
  rdfs:label       "SourceSystemContactKey" ;
  rdfs:range       xsd:string ;
  reso:CertificationLevel "Silver" ;
  schema:sameAs    <http://ddwiki.reso.org/display/DDW/SourceSystemContactKey+Field> ;
  vs:term_status   "stable"
.
reso:SourceSystemID a rdf:Property ;
  rdfs:comment     "The RESO OUID's OrganizationUniqueId of the Source record provider. The source system is the system from which the record was directly received. In cases where the source system was not where the record originated (the authoritative system), see the Originating System fields.","The RESO OUID's OrganizationUniqueId of the Source record provider.  The source system is the system from which the record was directly received.  In cases where the source system was not where the record originated (the authoritative system), see the Originating System fields." ;
  rdfs:domain      reso:Property,reso:Member,reso:Office,reso:Contacts ;
  rdfs:label       "SourceSystemID" ;
  rdfs:range       xsd:string ;
  reso:CertificationLevel "Platinum" ;
  reso:PropertyTypes "RESI","RLSE","RINC","LAND","MOBI","FARM","COMS","COML","BUSO" ;
  schema:sameAs    <http://ddwiki.reso.org/display/DDW/SourceSystemID+Field>,<http://ddwiki.reso.org/display/DDW/SourceSystemID+%28Member%29+Field>,<http://ddwiki.reso.org/display/DDW/SourceSystemID+%28Office%29+Field>,<http://ddwiki.reso.org/display/DDW/SourceSystemID+%28Contacts%29+Field> ;
  vs:term_status   "stable"
.
reso:SourceSystemName a rdf:Property ;
  rdfs:comment     "The name of the immediate record provider. The system from which the record was directly received. The legal name of the company.","The name of the immediate record provider.  The system from which the record was directly received.  The legal name of the company." ;
  rdfs:domain      reso:Property,reso:Member,reso:Office,reso:Contacts ;
  rdfs:label       "SourceSystemName" ;
  rdfs:range       xsd:string ;
  reso:CertificationLevel "Core","Silver" ;
  reso:PropertyTypes "RESI","RLSE","RINC","LAND","MOBI","FARM","COMS","COML","BUSO" ;
  schema:sameAs    <http://ddwiki.reso.org/display/DDW/SourceSystemName+Field>,<http://ddwiki.reso.org/display/DDW/SourceSystemName+%28Member%29+Field>,<http://ddwiki.reso.org/display/DDW/SourceSystemName+%28Office%29+Field>,<http://ddwiki.reso.org/display/DDW/SourceSystemName+%28Contacts%29+Field> ;
  vs:term_status   "stable"
.
reso:SpousePartnerName a rdf:Property ;
  rdfs:comment     "The contact's spouse or partner." ;
  rdfs:domain      reso:Contacts ;
  rdfs:label       "SpousePartnerName" ;
  rdfs:range       xsd:string ;
  reso:CertificationLevel "Silver" ;
  schema:sameAs    <http://ddwiki.reso.org/display/DDW/SpousePartnerName+Field> ;
  vs:term_status   "stable"
.
reso:TollFreePhone a rdf:Property ;
  rdfs:comment     "North American 10 digit phone numbers should be in the format of ###-###-#### (separated by hyphens).  Other conventions should use the common local standard.  International numbers should be preceded by a plus symbol." ;
  rdfs:domain      reso:Contacts ;
  rdfs:label       "TollFreePhone" ;
  rdfs:range       xsd:string ;
  reso:CertificationLevel "Silver" ;
  schema:sameAs    <http://ddwiki.reso.org/display/DDW/TollFreePhone+Field> ;
  vs:term_status   "stable"
.
reso:UserDefinedFieldName a rdf:Property ;
  rdfs:comment     "[#] This field is a repeating element.  If this field is repeated, add 1, 2, 3, etc., to the end of the field." ;
  rdfs:domain      reso:Contacts ;
  rdfs:label       "UserDefinedFieldName" ;
  rdfs:range       xsd:string ;
  reso:CertificationLevel "Silver" ;
  schema:sameAs    <http://ddwiki.reso.org/display/DDW/UserDefinedFieldName%5B%23%5D+Field> ;
  vs:term_status   "stable"
.
reso:UserDefinedFieldValue a rdf:Property ;
  rdfs:comment     "[#] This field is a repeating element.  If this field is repeated, add 1, 2, 3, etc., to the end of the field." ;
  rdfs:domain      reso:Contacts ;
  rdfs:label       "UserDefinedFieldValue" ;
  rdfs:range       xsd:string ;
  reso:CertificationLevel "Silver" ;
  schema:sameAs    <http://ddwiki.reso.org/display/DDW/UserDefinedFieldValue%5B%23%5D+Field> ;
  vs:term_status   "stable"
.
reso:VoiceMail a rdf:Property ;
  rdfs:comment     "North American 10 digit phone numbers should be in the format of ###-###-#### (separated by hyphens).  Other conventions should use the common local standard.  International numbers should be preceded by a plus symbol." ;
  rdfs:domain      reso:Contacts ;
  rdfs:label       "VoiceMail" ;
  rdfs:range       xsd:string ;
  reso:CertificationLevel "Silver" ;
  schema:sameAs    <http://ddwiki.reso.org/display/DDW/VoiceMail+Field> ;
  vs:term_status   "stable"
.
reso:VoiceMailExt a rdf:Property ;
  rdfs:comment     "The extension of the given phone number (if applicable)." ;
  rdfs:domain      reso:Contacts ;
  rdfs:label       "VoiceMailExt" ;
  rdfs:range       xsd:string ;
  reso:CertificationLevel "Silver" ;
  schema:sameAs    <http://ddwiki.reso.org/display/DDW/VoiceMailExt+Field> ;
  vs:term_status   "stable"
.
reso:WorkAddress1 a rdf:Property ;
  rdfs:comment     "The street number, direction, name and suffix of the contact's work." ;
  rdfs:domain      reso:Contacts ;
  rdfs:label       "WorkAddress1" ;
  rdfs:range       xsd:string ;
  reso:CertificationLevel "Silver" ;
  schema:sameAs    <http://ddwiki.reso.org/display/DDW/WorkAddress1+Field> ;
  vs:term_status   "stable"
.
reso:WorkAddress2 a rdf:Property ;
  rdfs:comment     "The unit/suite number of the contact's work." ;
  rdfs:domain      reso:Contacts ;
  rdfs:label       "WorkAddress2" ;
  rdfs:range       xsd:string ;
  reso:CertificationLevel "Silver" ;
  schema:sameAs    <http://ddwiki.reso.org/display/DDW/WorkAddress2+Field> ;
  vs:term_status   "stable"
.
reso:WorkCarrierRoute a rdf:Property ;
  rdfs:domain      reso:Contacts ;
  rdfs:label       "WorkCarrierRoute" ;
  rdfs:range       xsd:string ;
  reso:CertificationLevel "Silver" ;
  schema:sameAs    <http://ddwiki.reso.org/display/DDW/WorkCarrierRoute+Field> ;
  vs:term_status   "stable"
.
reso:WorkCity a rdf:Property ;
  rdfs:comment     "The city of the contact's work." ;
  rdfs:domain      reso:Contacts ;
  rdfs:label       "WorkCity" ;
  rdfs:range       xsd:string ;
  reso:CertificationLevel "Silver" ;
  schema:sameAs    <http://ddwiki.reso.org/display/DDW/WorkCity+Field> ;
  vs:term_status   "stable"
.
reso:WorkCountry a rdf:Property ;
  rdfs:comment     "The country abbreviation in a postal address." ;
  rdfs:domain      reso:Contacts ;
  rdfs:label       "WorkCountry" ;
  rdfs:range       enum:Country ;
  reso:CertificationLevel "Silver" ;
  schema:sameAs    <http://ddwiki.reso.org/display/DDW/WorkCountry+Field> ;
  vs:term_status   "stable"
.
reso:WorkCountyOrParish a rdf:Property ;
  rdfs:comment     "The county or parish in which the contact's work is addressed." ;
  rdfs:domain      reso:Contacts ;
  rdfs:label       "WorkCountyOrParish" ;
  rdfs:range       xsd:string ;
  reso:CertificationLevel "Silver" ;
  schema:sameAs    <http://ddwiki.reso.org/display/DDW/WorkCountyOrParish+Field> ;
  vs:term_status   "stable"
.
reso:WorkPostalCode a rdf:Property ;
  rdfs:comment     "The postal code of the contact's work." ;
  rdfs:domain      reso:Contacts ;
  rdfs:label       "WorkPostalCode" ;
  rdfs:range       xsd:string ;
  reso:CertificationLevel "Silver" ;
  schema:sameAs    <http://ddwiki.reso.org/display/DDW/WorkPostalCode+Field> ;
  vs:term_status   "stable"
.
reso:WorkPostalCodePlus4 a rdf:Property ;
  rdfs:comment     "The extension of the postal/zip code.  i.e. +4" ;
  rdfs:domain      reso:Contacts ;
  rdfs:label       "WorkPostalCodePlus4" ;
  rdfs:range       xsd:string ;
  reso:CertificationLevel "Silver" ;
  schema:sameAs    <http://ddwiki.reso.org/display/DDW/WorkPostalCodePlus4+Field> ;
  vs:term_status   "stable"
.
reso:WorkStateOrProvince a rdf:Property ;
  rdfs:comment     "The state or province in which the contact's work is addressed." ;
  rdfs:domain      reso:Contacts ;
  rdfs:label       "WorkStateOrProvince" ;
  rdfs:range       enum:StateOrProvince ;
  reso:CertificationLevel "Silver" ;
  schema:sameAs    <http://ddwiki.reso.org/display/DDW/WorkStateOrProvince+Field> ;
  vs:term_status   "stable"
.
reso:ChangedByMemberID a rdf:Property ;
  rdfs:comment     "ID of the user, agent, member, etc., that uploaded the media this record refers to." ;
  rdfs:domain      reso:Media ;
  rdfs:label       "ChangedByMemberID" ;
  rdfs:range       xsd:string ;
  reso:CertificationLevel "Core" ;
  schema:sameAs    <http://ddwiki.reso.org/display/DDW/ChangedByMemberID+Field> ;
  vs:term_status   "stable"
.
reso:ChangedByMemberKey a rdf:Property ;
  rdfs:comment     "The primary key of the member who uploaded the media this record refers to.  This is a foreign key relating to the Member resource's MemberKey." ;
  rdfs:domain      reso:Media ;
  rdfs:label       "ChangedByMemberKey" ;
  rdfs:range       xsd:string ;
  reso:CertificationLevel "Core" ;
  schema:sameAs    <http://ddwiki.reso.org/display/DDW/ChangedByMemberKey+Field> ;
  vs:term_status   "stable"
.
reso:ChangedByMemberKeyNumeric a rdf:Property ;
  rdfs:comment     "The primary key of the member who uploaded the media this record refers to.  This is a foreign key relating to the Member resource's MemberKey.  This is the numeric only key and used as an alternative to the ChangedByMemberKey field." ;
  rdfs:domain      reso:Media ;
  rdfs:label       "ChangedByMemberKeyNumeric" ;
  rdfs:range       xsd:decimal ;
  reso:CertificationLevel "Platinum" ;
  schema:sameAs    <http://ddwiki.reso.org/display/DDW/ChangedByMemberKeyNumeric+Field> ;
  vs:term_status   "stable"
.
reso:ClassName a rdf:Property ;
  rdfs:comment     "The class or table of the listing or other record the media.  Residential, Lease, Agent, Office, Contact, etc." ;
  rdfs:domain      reso:Media ;
  rdfs:label       "ClassName" ;
  rdfs:range       enum:ClassName ;
  reso:CertificationLevel "Bronze" ;
  schema:sameAs    <http://ddwiki.reso.org/display/DDW/ClassName+Field> ;
  vs:term_status   "stable"
.
reso:Group a rdf:Property ;
  rdfs:comment     "A placeholder for media classification such as elevation, exterior, interior, community, view, plan, plat.  The purpose is to allow media items to be grouped." ;
  rdfs:domain      reso:Media ;
  rdfs:label       "Group" ;
  rdfs:range       xsd:string ;
  reso:CertificationLevel "Bronze" ;
  schema:sameAs    <http://ddwiki.reso.org/display/DDW/Group+Field> ;
  vs:term_status   "stable"
.
reso:ImageHeight a rdf:Property ;
  rdfs:comment     "The height of the image expressed in pixels." ;
  rdfs:domain      reso:Media ;
  rdfs:label       "ImageHeight" ;
  rdfs:range       xsd:decimal ;
  reso:CertificationLevel "Bronze" ;
  schema:sameAs    <http://ddwiki.reso.org/display/DDW/ImageHeight+Field> ;
  vs:term_status   "stable"
.
reso:ImageOf a rdf:Property ;
  rdfs:comment     "When the media is an image, a list of possible matches such as kitchen, bathroom, front of structure, etc.  This field may be used to identify a required image under association or MLS rules." ;
  rdfs:domain      reso:Media ;
  rdfs:label       "ImageOf" ;
  rdfs:range       enum:ImageOf ;
  reso:CertificationLevel "Platinum" ;
  schema:sameAs    <http://ddwiki.reso.org/display/DDW/ImageOf+Field> ;
  vs:term_status   "stable"
.
reso:ImageSizeDescription a rdf:Property ;
  rdfs:comment     "A text description of the size of the image.  i.e. Small, Thumbnail, Medium, Large, X-Large.  The largest image must be described as \"Largest\".  Thumbnail must also be included.  Pick List will remain open/extendable." ;
  rdfs:domain      reso:Media ;
  rdfs:label       "ImageSizeDescription" ;
  rdfs:range       xsd:string ;
  reso:CertificationLevel "Bronze" ;
  schema:sameAs    <http://ddwiki.reso.org/display/DDW/ImageSizeDescription+Field> ;
  vs:term_status   "stable"
.
reso:ImageWidth a rdf:Property ;
  rdfs:comment     "The width of the image expressed in pixels." ;
  rdfs:domain      reso:Media ;
  rdfs:label       "ImageWidth" ;
  rdfs:range       xsd:decimal ;
  reso:CertificationLevel "Bronze" ;
  schema:sameAs    <http://ddwiki.reso.org/display/DDW/ImageWidth+Field> ;
  vs:term_status   "stable"
.
reso:LongDescription a rdf:Property ;
  rdfs:comment     "The full robust description of the object." ;
  rdfs:domain      reso:Media ;
  rdfs:label       "LongDescription" ;
  rdfs:range       xsd:string ;
  reso:CertificationLevel "Bronze" ;
  schema:sameAs    <http://ddwiki.reso.org/display/DDW/LongDescription+Field> ;
  vs:term_status   "stable"
.
reso:MediaCategory a rdf:Property ;
  rdfs:comment     "Category describing the , Photos, Documents, Video, Unbranded Virtual Tour, Branded Virtual Tour, Floor Plan, Logo" ;
  rdfs:domain      reso:Media ;
  rdfs:label       "MediaCategory" ;
  rdfs:range       enum:MediaCategory ;
  reso:CertificationLevel "Bronze" ;
  schema:sameAs    <http://ddwiki.reso.org/display/DDW/MediaCategory+Field> ;
  vs:term_status   "stable"
.
reso:MediaHTML a rdf:Property ;
  rdfs:comment     "The JavaScript or other method to embed a video, image, virtual tour or other media." ;
  rdfs:domain      reso:Media ;
  rdfs:label       "MediaHTML" ;
  rdfs:range       xsd:string ;
  reso:CertificationLevel "Bronze" ;
  schema:sameAs    <http://ddwiki.reso.org/display/DDW/MediaHTML+Field> ;
  vs:term_status   "stable"
.
reso:MediaKey a rdf:Property ;
  rdfs:comment     "A unique identifier for this record from the immediate source. This may be a number, or string that can include URI or other forms.  This is the system you are connecting to and not necessarily the original source of the record." ;
  rdfs:domain      reso:Media ;
  rdfs:label       "MediaKey" ;
  rdfs:range       xsd:string ;
  reso:CertificationLevel "Core" ;
  schema:sameAs    <http://ddwiki.reso.org/display/DDW/MediaKey+Field> ;
  vs:term_status   "stable"
.
reso:MediaKeyNumeric a rdf:Property ;
  rdfs:comment     "A unique identifier for this record from the immediate source. This may be a number, or string that can include URI or other forms.  This is the system you are connecting to and not necessarily the original source of the record.  This is the numeric only key and used as an alternative to the MediaKey field." ;
  rdfs:domain      reso:Media ;
  rdfs:label       "MediaKeyNumeric" ;
  rdfs:range       xsd:decimal ;
  reso:CertificationLevel "Platinum" ;
  schema:sameAs    <http://ddwiki.reso.org/display/DDW/MediaKeyNumeric+Field> ;
  vs:term_status   "stable"
.
reso:MediaModificationTimestamp a rdf:Property ;
  rdfs:comment     "This timestamp is updated when a change to the object has been made, which may differ from a change to the Media Resource." ;
  rdfs:domain      reso:Media ;
  rdfs:label       "MediaModificationTimestamp" ;
  rdfs:range       xsd:dateTime ;
  reso:CertificationLevel "Bronze" ;
  schema:sameAs    <http://ddwiki.reso.org/display/DDW/MediaModificationTimestamp+Field> ;
  vs:term_status   "stable"
.
reso:MediaObjectID a rdf:Property ;
  rdfs:comment     "ID of the image, supplement or other object specified by the given media record." ;
  rdfs:domain      reso:Media ;
  rdfs:label       "MediaObjectID" ;
  rdfs:range       xsd:string ;
  reso:CertificationLevel "Core" ;
  schema:sameAs    <http://ddwiki.reso.org/display/DDW/MediaObjectID+Field> ;
  vs:term_status   "stable"
.
reso:MediaStatus a rdf:Property ;
  rdfs:comment     "The status of the media item referenced by this record.  (Updated, Deleted, etc.,_" ;
  rdfs:domain      reso:Media ;
  rdfs:label       "MediaStatus" ;
  rdfs:range       xsd:string ;
  reso:CertificationLevel "Bronze" ;
  schema:sameAs    <http://ddwiki.reso.org/display/DDW/MediaStatus+Field> ;
  vs:term_status   "stable"
.
reso:MediaType a rdf:Property ;
  rdfs:domain      reso:Media ;
  rdfs:label       "MediaType" ;
  rdfs:range       enum:MediaType ;
  reso:CertificationLevel "Bronze" ;
  schema:sameAs    <http://ddwiki.reso.org/display/DDW/MediaType+Field> ;
  vs:term_status   "stable"
.
reso:MediaURL a rdf:Property ;
  rdfs:comment     "The URI to the media file referenced by this record." ;
  rdfs:domain      reso:Media ;
  rdfs:label       "MediaURL" ;
  rdfs:range       xsd:string ;
  reso:CertificationLevel "Core" ;
  schema:sameAs    <http://ddwiki.reso.org/display/DDW/MediaURL+Field> ;
  vs:term_status   "stable"
.
reso:ModificationTimestamp a rdf:Property ;
  rdfs:comment     "The transactional timestamp automatically recorded by the MLS system representing the date/time the listing was last modified.","Date/time the roster (member or office) record was last modified.","Date/time the contact record was last modified.","The transactional timestamp automatically recorded by the MLS system representing the date/time the media record was last modified." ;
  rdfs:domain      reso:Property,reso:Member,reso:Office,reso:Contacts,reso:Media ;
  rdfs:label       "ModificationTimestamp" ;
  rdfs:range       xsd:dateTime ;
  reso:CertificationLevel "Core","Silver" ;
  reso:PropertyTypes "RESI","RLSE","RINC","LAND","MOBI","FARM","COMS","COML","BUSO" ;
  schema:sameAs    <http://ddwiki.reso.org/display/DDW/ModificationTimestamp+Field>,<http://ddwiki.reso.org/display/DDW/ModificationTimestamp+%28Member%29+Field>,<http://ddwiki.reso.org/display/DDW/ModificationTimestamp+%28Office%29+Field>,<http://ddwiki.reso.org/display/DDW/ModificationTimestamp+%28Contacts%29+Field>,<http://ddwiki.reso.org/display/DDW/ModificationTimestamp+%28Media%29+Field> ;
  vs:term_status   "stable"
.
reso:Order a rdf:Property ;
  rdfs:comment     "Only a positive integer including zero.  Element zero is the primary photo per RETS convention." ;
  rdfs:domain      reso:Media ;
  rdfs:label       "Order" ;
  rdfs:range       xsd:decimal ;
  reso:CertificationLevel "Core" ;
  schema:sameAs    <http://ddwiki.reso.org/display/DDW/Order+Field> ;
  vs:term_status   "stable"
.
reso:OriginatingSystemID a rdf:Property ;
  rdfs:comment     "The RESO OUID's OrganizationUniqueId of the Originating record provider.  The Originating system is the system with authoritative control over the record.  For example; the name of the MLS where the listing was input.  In cases where the Originating system was not where the record originated (the authoritative system), see the Originating System fields.","The RESO OUID's OrganizationUniqueId of the Originating record provider.  The Originating system is the system with authoritative control over the record.  For example; the name of the MLS where the member was input.  In cases where the Originating system was not where the record originated (the authoritative system), see the Originating System fields.","The RESO OUID's OrganizationUniqueId of the Originating record provider.  The Originating system is the system with authoritative control over the record.  For example; the name of the MLS where the office was input.  In cases where the Originating system was not where the record originated (the authoritative system), see the Originating System fields.","The RESO OUID's OrganizationUniqueId of the Originating record provider.  The Originating system is the system with authoritative control over the record.  For example; the name of the MLS where the Contact was input.  In cases where the Originating system was not where the record originated (the authoritative system), see the Originating System fields.","The RESO OUID's OrganizationUniqueId of the Originating record provider.  The Originating system is the system with authoritative control over the record.  For example; the name of the MLS where the Media was input.  In cases where the Originating system was not where the record originated (the authoritative system), see the Originating System fields." ;
  rdfs:domain      reso:Property,reso:Member,reso:Office,reso:Contacts,reso:Media ;
  rdfs:label       "OriginatingSystemID" ;
  rdfs:range       xsd:string ;
  reso:CertificationLevel "Platinum" ;
  reso:PropertyTypes "RESI","RLSE","RINC","LAND","MOBI","FARM","COMS","COML","BUSO" ;
  schema:sameAs    <http://ddwiki.reso.org/display/DDW/OriginatingSystemID+Field>,<http://ddwiki.reso.org/display/DDW/OriginatingSystemID+%28Member%29+Field>,<http://ddwiki.reso.org/display/DDW/OriginatingSystemID+%28Office%29+Field>,<http://ddwiki.reso.org/display/DDW/OriginatingSystemID+%28Contacts%29+Field>,<http://ddwiki.reso.org/display/DDW/OriginatingSystemID+%28Media%29+Field> ;
  vs:term_status   "stable"
.
reso:OriginatingSystemMediaKey a rdf:Property ;
  rdfs:comment     "The system key, a unique record identifier, from the Originating system.  The Originating system is the system with authoritative control over the record.  For example, the Multiple Listing Service where the Media was input.  There may be cases where the Source System (how you received the record) is not the Originating System.  See Source System Key for more information." ;
  rdfs:domain      reso:Media ;
  rdfs:label       "OriginatingSystemMediaKey" ;
  rdfs:range       xsd:string ;
  reso:CertificationLevel "Core" ;
  schema:sameAs    <http://ddwiki.reso.org/display/DDW/OriginatingSystemMediaKey+Field> ;
  vs:term_status   "stable"
.
reso:OriginatingSystemName a rdf:Property ;
  rdfs:comment     "The name of the Originating record provider.  Most commonly the name of the MLS. The place where the listing is originally input by the member.  The legal name of the company.","The name of the Originating record provider.  Most commonly the name of the MLS. The place where the member is originally input by the member.  The legal name of the company.","The name of the Originating record provider.  Most commonly the name of the MLS. The place where the office is originally input by the member.  The legal name of the company.","The name of the Originating record provider.  Most commonly the name of the MLS. The place where the Contact is originally input by the member.  The legal name of the company.","The name of the Originating record provider.  Most commonly the name of the MLS. The place where the Media is originally input by the member.  The legal name of the company." ;
  rdfs:domain      reso:Property,reso:Member,reso:Office,reso:Contacts,reso:Media ;
  rdfs:label       "OriginatingSystemName" ;
  rdfs:range       xsd:string ;
  reso:CertificationLevel "Core","Bronze","Silver" ;
  reso:PropertyTypes "RESI","RLSE","RINC","LAND","MOBI","FARM","COMS","COML","BUSO" ;
  schema:sameAs    <http://ddwiki.reso.org/display/DDW/OriginatingSystemName+Field>,<http://ddwiki.reso.org/display/DDW/OriginatingSystemName+%28Member%29+Field>,<http://ddwiki.reso.org/display/DDW/OriginatingSystemName+%28Office%29+Field>,<http://ddwiki.reso.org/display/DDW/OriginatingSystemName+%28Contacts%29+Field>,<http://ddwiki.reso.org/display/DDW/OriginatingSystemName+%28Media%29+Field> ;
  vs:term_status   "stable"
.
reso:Permission a rdf:Property ;
  rdfs:comment     "Public, Private, IDX, VOW, Office Only, Firm Only, Agent Only," ;
  rdfs:domain      reso:Media ;
  rdfs:label       "Permission" ;
  rdfs:range       xsd:string ;
  reso:CertificationLevel "Bronze" ;
  schema:sameAs    <http://ddwiki.reso.org/display/DDW/Permission+Field> ;
  vs:term_status   "stable"
.
reso:PreferredPhotoYN a rdf:Property ;
  rdfs:comment     "When set to true, the media record in question is the preferred photo.  This will typically mean the photo to be shown when only one of the photos is to be displayed." ;
  rdfs:domain      reso:Media ;
  rdfs:label       "PreferredPhotoYN" ;
  rdfs:range       xsd:boolean ;
  reso:CertificationLevel "Platinum" ;
  schema:sameAs    <http://ddwiki.reso.org/display/DDW/PreferredPhotoYN+Field> ;
  vs:term_status   "stable"
.
reso:ResourceName a rdf:Property ;
  rdfs:comment     "The resource or table of the listing or other record the media relates to.  i.e. Property, Member, Office, etc." ;
  rdfs:domain      reso:Media ;
  rdfs:label       "ResourceName" ;
  rdfs:range       enum:ResourceName ;
  reso:CertificationLevel "Core" ;
  schema:sameAs    <http://ddwiki.reso.org/display/DDW/ResourceName+Field> ;
  vs:term_status   "stable"
.
reso:ResourceRecordID a rdf:Property ;
  rdfs:comment     "The well known identifier of the related record from the source resource. The value may be identical to that of the Listing Key, but the Listing ID is intended to be the value used by a human to retrieve the information about a specific listing. In a multiple originating system or a merged system, this value may not be unique and may require the use of the provider system to create a synthetic unique value." ;
  rdfs:domain      reso:Media ;
  rdfs:label       "ResourceRecordID" ;
  rdfs:range       xsd:string ;
  reso:CertificationLevel "Core" ;
  schema:sameAs    <http://ddwiki.reso.org/display/DDW/ResourceRecordID+Field> ;
  vs:term_status   "stable"
.
reso:ResourceRecordKey a rdf:Property ;
  rdfs:comment     "The primary key of the related record from the source resource. For example the ListingKey, AgentKey, OfficeKey, TeamKey, etc.  This is the system you are connecting to and not necessarily the original source of the record.  This is a foreign key from the resource selected in the ResourceName field." ;
  rdfs:domain      reso:Media ;
  rdfs:label       "ResourceRecordKey" ;
  rdfs:range       xsd:string ;
  reso:CertificationLevel "Core" ;
  schema:sameAs    <http://ddwiki.reso.org/display/DDW/ResourceRecordKey+Field> ;
  vs:term_status   "stable"
.
reso:ResourceRecordKeyNumeric a rdf:Property ;
  rdfs:comment     "The primary key of the related record from the source resource. For example the ListingKey, AgentKey, OfficeKey, TeamKey, etc.  This is the system you are connecting to and not necessarily the original source of the record.  This is a foreign key from the resource selected in the ResourceName field.  This is the numeric only key and used as an alternative to the ResourceRecordKey field." ;
  rdfs:domain      reso:Media ;
  rdfs:label       "ResourceRecordKeyNumeric" ;
  rdfs:range       xsd:decimal ;
  reso:CertificationLevel "Platinum" ;
  schema:sameAs    <http://ddwiki.reso.org/display/DDW/ResourceRecordKeyNumeric+Field> ;
  vs:term_status   "stable"
.
reso:ShortDescription a rdf:Property ;
  rdfs:comment     "The short text given to summarize the object.  Commonly used as the short description displayed under a photo." ;
  rdfs:domain      reso:Media ;
  rdfs:label       "ShortDescription" ;
  rdfs:range       xsd:string ;
  reso:CertificationLevel "Bronze" ;
  schema:sameAs    <http://ddwiki.reso.org/display/DDW/ShortDescription+Field> ;
  vs:term_status   "stable"
.
reso:SourceSystemID a rdf:Property ;
  rdfs:comment     "The RESO OUID's OrganizationUniqueId of the Source record provider. The source system is the system from which the record was directly received. In cases where the source system was not where the record originated (the authoritative system), see the Originating System fields.","The RESO OUID's OrganizationUniqueId of the Source record provider.  The source system is the system from which the record was directly received.  In cases where the source system was not where the record originated (the authoritative system), see the Originating System fields." ;
  rdfs:domain      reso:Property,reso:Member,reso:Office,reso:Contacts,reso:Media ;
  rdfs:label       "SourceSystemID" ;
  rdfs:range       xsd:string ;
  reso:CertificationLevel "Platinum" ;
  reso:PropertyTypes "RESI","RLSE","RINC","LAND","MOBI","FARM","COMS","COML","BUSO" ;
  schema:sameAs    <http://ddwiki.reso.org/display/DDW/SourceSystemID+Field>,<http://ddwiki.reso.org/display/DDW/SourceSystemID+%28Member%29+Field>,<http://ddwiki.reso.org/display/DDW/SourceSystemID+%28Office%29+Field>,<http://ddwiki.reso.org/display/DDW/SourceSystemID+%28Contacts%29+Field>,<http://ddwiki.reso.org/display/DDW/SourceSystemID+%28Media%29+Field> ;
  vs:term_status   "stable"
.
reso:SourceSystemMediaKey a rdf:Property ;
  rdfs:comment     "The system key, a unique record identifier, from the Source System.  The Source System is the system from which the record was directly received.  In cases where the Source System was not where the record originated (the authoritative system), see the Originating System fields." ;
  rdfs:domain      reso:Media ;
  rdfs:label       "SourceSystemMediaKey" ;
  rdfs:range       xsd:string ;
  reso:CertificationLevel "Silver" ;
  schema:sameAs    <http://ddwiki.reso.org/display/DDW/SourceSystemMediaKey+Field> ;
  vs:term_status   "stable"
.
reso:SourceSystemName a rdf:Property ;
  rdfs:comment     "The name of the immediate record provider. The system from which the record was directly received. The legal name of the company.","The name of the immediate record provider.  The system from which the record was directly received.  The legal name of the company." ;
  rdfs:domain      reso:Property,reso:Member,reso:Office,reso:Contacts,reso:Media ;
  rdfs:label       "SourceSystemName" ;
  rdfs:range       xsd:string ;
  reso:CertificationLevel "Core","Silver" ;
  reso:PropertyTypes "RESI","RLSE","RINC","LAND","MOBI","FARM","COMS","COML","BUSO" ;
  schema:sameAs    <http://ddwiki.reso.org/display/DDW/SourceSystemName+Field>,<http://ddwiki.reso.org/display/DDW/SourceSystemName+%28Member%29+Field>,<http://ddwiki.reso.org/display/DDW/SourceSystemName+%28Office%29+Field>,<http://ddwiki.reso.org/display/DDW/SourceSystemName+%28Contacts%29+Field>,<http://ddwiki.reso.org/display/DDW/SourceSystemName+%28Media%29+Field> ;
  vs:term_status   "stable"
.
reso:ChangeType a rdf:Property ;
  rdfs:comment     "Description of the last major change on the listing, i.e. &#x201c;price reduction&#x201d;, &#x201c;back on market&#x201d;, etc.  May be used to display on a summary view of listing results to quickly identify listings that have had major changes recently." ;
  rdfs:domain      reso:HistoryTransactional ;
  rdfs:label       "ChangeType" ;
  rdfs:range       enum:ChangeType ;
  reso:CertificationLevel "Silver" ;
  schema:sameAs    <http://ddwiki.reso.org/display/DDW/ChangeType+Field> ;
  vs:term_status   "stable"
.
reso:ChangedByMemberID a rdf:Property ;
  rdfs:comment     "ID of the user, agent, member, etc., that uploaded the media this record refers to.","The local, well-know identifier of the member (user) who made the change." ;
  rdfs:domain      reso:Media,reso:HistoryTransactional ;
  rdfs:label       "ChangedByMemberID" ;
  rdfs:range       xsd:string ;
  reso:CertificationLevel "Core","Silver" ;
  schema:sameAs    <http://ddwiki.reso.org/display/DDW/ChangedByMemberID+Field>,<http://ddwiki.reso.org/display/DDW/ChangedByMemberID+%28HistoryTransactional%29+Field> ;
  vs:term_status   "stable"
.
reso:ChangedByMemberKey a rdf:Property ;
  rdfs:comment     "The primary key of the member who uploaded the media this record refers to.  This is a foreign key relating to the Member resource's MemberKey.","The unique identifier of the member (user) who made the change.  This is a foreign key relating to the Member resource's MemberKey." ;
  rdfs:domain      reso:Media,reso:HistoryTransactional ;
  rdfs:label       "ChangedByMemberKey" ;
  rdfs:range       xsd:string ;
  reso:CertificationLevel "Core","Silver" ;
  schema:sameAs    <http://ddwiki.reso.org/display/DDW/ChangedByMemberKey+Field>,<http://ddwiki.reso.org/display/DDW/ChangedByMemberKey+%28HistoryTransactional%29+Field> ;
  vs:term_status   "stable"
.
reso:ChangedByMemberKeyNumeric a rdf:Property ;
  rdfs:comment     "The primary key of the member who uploaded the media this record refers to.  This is a foreign key relating to the Member resource's MemberKey.  This is the numeric only key and used as an alternative to the ChangedByMemberKey field.","The unique identifier of the member (user) who made the change.  This is a foreign key relating to the Member resource's MemberKey.  This is the numeric only key and used as an alternative to the ChangedByMemberKey field." ;
  rdfs:domain      reso:Media,reso:HistoryTransactional ;
  rdfs:label       "ChangedByMemberKeyNumeric" ;
  rdfs:range       xsd:decimal ;
  reso:CertificationLevel "Platinum" ;
  schema:sameAs    <http://ddwiki.reso.org/display/DDW/ChangedByMemberKeyNumeric+Field>,<http://ddwiki.reso.org/display/DDW/ChangedByMemberKeyNumeric+%28HistoryTransactional%29+Field> ;
  vs:term_status   "stable"
.
reso:ClassName a rdf:Property ;
  rdfs:comment     "The class or table of the listing or other record the media.  Residential, Lease, Agent, Office, Contact, etc.","Name of the class which this history record applies." ;
  rdfs:domain      reso:Media,reso:HistoryTransactional ;
  rdfs:label       "ClassName" ;
  rdfs:range       enum:ClassName,xsd:string ;
  reso:CertificationLevel "Bronze","Silver" ;
  schema:sameAs    <http://ddwiki.reso.org/display/DDW/ClassName+Field>,<http://ddwiki.reso.org/display/DDW/ClassName+%28HistoryTransactional%29+Field> ;
  vs:term_status   "stable"
.
reso:FieldKey a rdf:Property ;
  rdfs:comment     "The unique identifier of the field whose data is being changed.  This is a foreign key relating to the field found in the resource per the ResourceName." ;
  rdfs:domain      reso:HistoryTransactional ;
  rdfs:label       "FieldKey" ;
  rdfs:range       xsd:string ;
  reso:CertificationLevel "Silver" ;
  schema:sameAs    <http://ddwiki.reso.org/display/DDW/FieldKey+Field> ;
  vs:term_status   "stable"
.
reso:FieldKeyNumeric a rdf:Property ;
  rdfs:comment     "The unique identifier of the field whose data is being changed.  This is a foreign key relating to the field found in the resource per the ResourceName.  This is the numeric only key and used as an alternative to the FieldKey field." ;
  rdfs:domain      reso:HistoryTransactional ;
  rdfs:label       "FieldKeyNumeric" ;
  rdfs:range       xsd:decimal ;
  reso:CertificationLevel "Platinum" ;
  schema:sameAs    <http://ddwiki.reso.org/display/DDW/FieldKeyNumeric+Field> ;
  vs:term_status   "stable"
.
reso:FieldName a rdf:Property ;
  rdfs:comment     "The name of the field whose data is being changed." ;
  rdfs:domain      reso:HistoryTransactional ;
  rdfs:label       "FieldName" ;
  rdfs:range       xsd:string ;
  reso:CertificationLevel "Silver" ;
  schema:sameAs    <http://ddwiki.reso.org/display/DDW/FieldName+Field> ;
  vs:term_status   "stable"
.
reso:HistoryTransactionalKey a rdf:Property ;
  rdfs:comment     "A unique identifier for this record from the immediate source. This may be a number, or string that can include URI or other forms.  This is the system you are connecting to and not necessarily the original source of the record." ;
  rdfs:domain      reso:HistoryTransactional ;
  rdfs:label       "HistoryTransactionalKey" ;
  rdfs:range       xsd:string ;
  reso:CertificationLevel "Silver" ;
  schema:sameAs    <http://ddwiki.reso.org/display/DDW/HistoryTransactionalKey+Field> ;
  vs:term_status   "stable"
.
reso:HistoryTransactionalKeyNumeric a rdf:Property ;
  rdfs:comment     "A unique identifier for this record from the immediate source. This may be a number, or string that can include URI or other forms.  This is the system you are connecting to and not necessarily the original source of the record.  This is the numeric only key and used as an alternative to the HistoryTransactionalKey field." ;
  rdfs:domain      reso:HistoryTransactional ;
  rdfs:label       "HistoryTransactionalKeyNumeric" ;
  rdfs:range       xsd:decimal ;
  reso:CertificationLevel "Platinum" ;
  schema:sameAs    <http://ddwiki.reso.org/display/DDW/HistoryTransactionalKeyNumeric+Field> ;
  vs:term_status   "stable"
.
reso:ModificationTimestamp a rdf:Property ;
  rdfs:comment     "The transactional timestamp automatically recorded by the MLS system representing the date/time the listing was last modified.","Date/time the roster (member or office) record was last modified.","Date/time the contact record was last modified.","The transactional timestamp automatically recorded by the MLS system representing the date/time the media record was last modified.","Timestamp of the last major change on the listing (see also MajorChangeType)." ;
  rdfs:domain      reso:Property,reso:Member,reso:Office,reso:Contacts,reso:Media,reso:HistoryTransactional ;
  rdfs:label       "ModificationTimestamp" ;
  rdfs:range       xsd:dateTime ;
  reso:CertificationLevel "Core","Silver" ;
  reso:PropertyTypes "RESI","RLSE","RINC","LAND","MOBI","FARM","COMS","COML","BUSO" ;
  schema:sameAs    <http://ddwiki.reso.org/display/DDW/ModificationTimestamp+Field>,<http://ddwiki.reso.org/display/DDW/ModificationTimestamp+%28Member%29+Field>,<http://ddwiki.reso.org/display/DDW/ModificationTimestamp+%28Office%29+Field>,<http://ddwiki.reso.org/display/DDW/ModificationTimestamp+%28Contacts%29+Field>,<http://ddwiki.reso.org/display/DDW/ModificationTimestamp+%28Media%29+Field>,<http://ddwiki.reso.org/display/DDW/ModificationTimestamp+%28HistoryTransactional%29+Field> ;
  vs:term_status   "stable"
.
reso:NewValue a rdf:Property ;
  rdfs:comment     "The new value applied to the named field." ;
  rdfs:domain      reso:HistoryTransactional ;
  rdfs:label       "NewValue" ;
  rdfs:range       xsd:string ;
  reso:CertificationLevel "Silver" ;
  schema:sameAs    <http://ddwiki.reso.org/display/DDW/NewValue+Field> ;
  vs:term_status   "stable"
.
reso:OriginatingSystemHistoryKey a rdf:Property ;
  rdfs:comment     "The system key, a unique record identifier, from the Originating system.  The Originating system is the system with authoritative control over the record.  For example, the Multiple Listing Service where the History was input.  There may be cases where the Source System (how you received the record) is not the Originating System.  See Source System Key for more information." ;
  rdfs:domain      reso:HistoryTransactional ;
  rdfs:label       "OriginatingSystemHistoryKey" ;
  rdfs:range       xsd:string ;
  reso:CertificationLevel "Silver" ;
  schema:sameAs    <http://ddwiki.reso.org/display/DDW/OriginatingSystemHistoryKey+Field> ;
  vs:term_status   "stable"
.
reso:OriginatingSystemID a rdf:Property ;
  rdfs:comment     "The RESO OUID's OrganizationUniqueId of the Originating record provider.  The Originating system is the system with authoritative control over the record.  For example; the name of the MLS where the listing was input.  In cases where the Originating system was not where the record originated (the authoritative system), see the Originating System fields.","The RESO OUID's OrganizationUniqueId of the Originating record provider.  The Originating system is the system with authoritative control over the record.  For example; the name of the MLS where the member was input.  In cases where the Originating system was not where the record originated (the authoritative system), see the Originating System fields.","The RESO OUID's OrganizationUniqueId of the Originating record provider.  The Originating system is the system with authoritative control over the record.  For example; the name of the MLS where the office was input.  In cases where the Originating system was not where the record originated (the authoritative system), see the Originating System fields.","The RESO OUID's OrganizationUniqueId of the Originating record provider.  The Originating system is the system with authoritative control over the record.  For example; the name of the MLS where the Contact was input.  In cases where the Originating system was not where the record originated (the authoritative system), see the Originating System fields.","The RESO OUID's OrganizationUniqueId of the Originating record provider.  The Originating system is the system with authoritative control over the record.  For example; the name of the MLS where the Media was input.  In cases where the Originating system was not where the record originated (the authoritative system), see the Originating System fields.","The RESO OUID's OrganizationUniqueId of the Originating record provider.  The Originating system is the system with authoritative control over the record.  For example; the name of the MLS where the History was input.  In cases where the Originating system was not where the record originated (the authoritative system), see the Originating System fields." ;
  rdfs:domain      reso:Property,reso:Member,reso:Office,reso:Contacts,reso:Media,reso:HistoryTransactional ;
  rdfs:label       "OriginatingSystemID" ;
  rdfs:range       xsd:string ;
  reso:CertificationLevel "Platinum" ;
  reso:PropertyTypes "RESI","RLSE","RINC","LAND","MOBI","FARM","COMS","COML","BUSO" ;
  schema:sameAs    <http://ddwiki.reso.org/display/DDW/OriginatingSystemID+Field>,<http://ddwiki.reso.org/display/DDW/OriginatingSystemID+%28Member%29+Field>,<http://ddwiki.reso.org/display/DDW/OriginatingSystemID+%28Office%29+Field>,<http://ddwiki.reso.org/display/DDW/OriginatingSystemID+%28Contacts%29+Field>,<http://ddwiki.reso.org/display/DDW/OriginatingSystemID+%28Media%29+Field>,<http://ddwiki.reso.org/display/DDW/OriginatingSystemID+%28HistoryTransactional%29+Field> ;
  vs:term_status   "stable"
.
reso:OriginatingSystemName a rdf:Property ;
  rdfs:comment     "The name of the Originating record provider.  Most commonly the name of the MLS. The place where the listing is originally input by the member.  The legal name of the company.","The name of the Originating record provider.  Most commonly the name of the MLS. The place where the member is originally input by the member.  The legal name of the company.","The name of the Originating record provider.  Most commonly the name of the MLS. The place where the office is originally input by the member.  The legal name of the company.","The name of the Originating record provider.  Most commonly the name of the MLS. The place where the Contact is originally input by the member.  The legal name of the company.","The name of the Originating record provider.  Most commonly the name of the MLS. The place where the Media is originally input by the member.  The legal name of the company.","The name of the Originating record provider.  Most commonly the name of the MLS. The place where the History is originally input.  The legal name of the company." ;
  rdfs:domain      reso:Property,reso:Member,reso:Office,reso:Contacts,reso:Media,reso:HistoryTransactional ;
  rdfs:label       "OriginatingSystemName" ;
  rdfs:range       xsd:string ;
  reso:CertificationLevel "Core","Bronze","Silver" ;
  reso:PropertyTypes "RESI","RLSE","RINC","LAND","MOBI","FARM","COMS","COML","BUSO" ;
  schema:sameAs    <http://ddwiki.reso.org/display/DDW/OriginatingSystemName+Field>,<http://ddwiki.reso.org/display/DDW/OriginatingSystemName+%28Member%29+Field>,<http://ddwiki.reso.org/display/DDW/OriginatingSystemName+%28Office%29+Field>,<http://ddwiki.reso.org/display/DDW/OriginatingSystemName+%28Contacts%29+Field>,<http://ddwiki.reso.org/display/DDW/OriginatingSystemName+%28Media%29+Field>,<http://ddwiki.reso.org/display/DDW/OriginatingSystemName+%28HistoryTransactional%29+Field> ;
  vs:term_status   "stable"
.
reso:PreviousValue a rdf:Property ;
  rdfs:comment     "The value found in the named field prior to the change represented by this record." ;
  rdfs:domain      reso:HistoryTransactional ;
  rdfs:label       "PreviousValue" ;
  rdfs:range       xsd:string ;
  reso:CertificationLevel "Silver" ;
  schema:sameAs    <http://ddwiki.reso.org/display/DDW/PreviousValue+Field> ;
  vs:term_status   "stable"
.
reso:ResourceName a rdf:Property ;
  rdfs:comment     "The resource or table of the listing or other record the media relates to.  i.e. Property, Member, Office, etc.","The name of the resource which this history record applies." ;
  rdfs:domain      reso:Media,reso:HistoryTransactional ;
  rdfs:label       "ResourceName" ;
  rdfs:range       enum:ResourceName,xsd:string ;
  reso:CertificationLevel "Core","Silver" ;
  schema:sameAs    <http://ddwiki.reso.org/display/DDW/ResourceName+Field>,<http://ddwiki.reso.org/display/DDW/ResourceName+%28HistoryTransactional%29+Field> ;
  vs:term_status   "stable"
.
reso:ResourceRecordID a rdf:Property ;
  rdfs:comment     "The well known identifier of the related record from the source resource. The value may be identical to that of the Listing Key, but the Listing ID is intended to be the value used by a human to retrieve the information about a specific listing. In a multiple originating system or a merged system, this value may not be unique and may require the use of the provider system to create a synthetic unique value." ;
  rdfs:domain      reso:Media,reso:HistoryTransactional ;
  rdfs:label       "ResourceRecordID" ;
  rdfs:range       xsd:string ;
  reso:CertificationLevel "Core","Silver" ;
  schema:sameAs    <http://ddwiki.reso.org/display/DDW/ResourceRecordID+Field>,<http://ddwiki.reso.org/display/DDW/ResourceRecordID+%28HistoryTransactional%29+Field> ;
  vs:term_status   "stable"
.
reso:ResourceRecordKey a rdf:Property ;
  rdfs:comment     "The primary key of the related record from the source resource. For example the ListingKey, AgentKey, OfficeKey, TeamKey, etc.  This is the system you are connecting to and not necessarily the original source of the record.  This is a foreign key from the resource selected in the ResourceName field.","The primary key of the related record from the source resource. For example the ListingKey, AgentKey, OfficeKey, etc.  This is the system you are connecting to and not necessarily the original source of the record.  This is a foreign key from the resource selected in the ResourceName field." ;
  rdfs:domain      reso:Media,reso:HistoryTransactional ;
  rdfs:label       "ResourceRecordKey" ;
  rdfs:range       xsd:string ;
  reso:CertificationLevel "Core","Silver" ;
  schema:sameAs    <http://ddwiki.reso.org/display/DDW/ResourceRecordKey+Field>,<http://ddwiki.reso.org/display/DDW/ResourceRecordKey+%28HistoryTransactional%29+Field> ;
  vs:term_status   "stable"
.
reso:ResourceRecordKeyNumeric a rdf:Property ;
  rdfs:comment     "The primary key of the related record from the source resource. For example the ListingKey, AgentKey, OfficeKey, TeamKey, etc.  This is the system you are connecting to and not necessarily the original source of the record.  This is a foreign key from the resource selected in the ResourceName field.  This is the numeric only key and used as an alternative to the ResourceRecordKey field.","The primary key of the related record from the source resource. For example the ListingKey, AgentKey, OfficeKey, etc.  This is the system you are connecting to and not necessarily the original source of the record.  This is a foreign key from the resource selected in the ResourceName field.  This is the numeric only key and used as an alternative to the ResourceRecordKey field." ;
  rdfs:domain      reso:Media,reso:HistoryTransactional ;
  rdfs:label       "ResourceRecordKeyNumeric" ;
  rdfs:range       xsd:decimal ;
  reso:CertificationLevel "Platinum" ;
  schema:sameAs    <http://ddwiki.reso.org/display/DDW/ResourceRecordKeyNumeric+Field>,<http://ddwiki.reso.org/display/DDW/ResourceRecordKeyNumeric+%28HistoryTransactional%29+Field> ;
  vs:term_status   "stable"
.
reso:SourceSystemHistoryKey a rdf:Property ;
  rdfs:comment     "The system key, a unique record identifier, from the Source System.  The Source System is the system from which the record was directly received.  In cases where the Source System was not where the record originated (the authoritative system), see the Originating System fields." ;
  rdfs:domain      reso:HistoryTransactional ;
  rdfs:label       "SourceSystemHistoryKey" ;
  rdfs:range       xsd:string ;
  reso:CertificationLevel "Silver" ;
  schema:sameAs    <http://ddwiki.reso.org/display/DDW/SourceSystemHistoryKey+Field> ;
  vs:term_status   "stable"
.
reso:SourceSystemID a rdf:Property ;
  rdfs:comment     "The RESO OUID's OrganizationUniqueId of the Source record provider. The source system is the system from which the record was directly received. In cases where the source system was not where the record originated (the authoritative system), see the Originating System fields.","The RESO OUID's OrganizationUniqueId of the Source record provider.  The source system is the system from which the record was directly received.  In cases where the source system was not where the record originated (the authoritative system), see the Originating System fields." ;
  rdfs:domain      reso:Property,reso:Member,reso:Office,reso:Contacts,reso:Media,reso:HistoryTransactional ;
  rdfs:label       "SourceSystemID" ;
  rdfs:range       xsd:string ;
  reso:CertificationLevel "Platinum" ;
  reso:PropertyTypes "RESI","RLSE","RINC","LAND","MOBI","FARM","COMS","COML","BUSO" ;
  schema:sameAs    <http://ddwiki.reso.org/display/DDW/SourceSystemID+Field>,<http://ddwiki.reso.org/display/DDW/SourceSystemID+%28Member%29+Field>,<http://ddwiki.reso.org/display/DDW/SourceSystemID+%28Office%29+Field>,<http://ddwiki.reso.org/display/DDW/SourceSystemID+%28Contacts%29+Field>,<http://ddwiki.reso.org/display/DDW/SourceSystemID+%28Media%29+Field>,<http://ddwiki.reso.org/display/DDW/SourceSystemID+%28HistoryTransactional%29+Field> ;
  vs:term_status   "stable"
.
reso:SourceSystemName a rdf:Property ;
  rdfs:comment     "The name of the immediate record provider. The system from which the record was directly received. The legal name of the company.","The name of the immediate record provider.  The system from which the record was directly received.  The legal name of the company.","The name of the History record provider.  The system from which the record was directly received.  The legal name of the company." ;
  rdfs:domain      reso:Property,reso:Member,reso:Office,reso:Contacts,reso:Media,reso:HistoryTransactional ;
  rdfs:label       "SourceSystemName" ;
  rdfs:range       xsd:string ;
  reso:CertificationLevel "Core","Silver" ;
  reso:PropertyTypes "RESI","RLSE","RINC","LAND","MOBI","FARM","COMS","COML","BUSO" ;
  schema:sameAs    <http://ddwiki.reso.org/display/DDW/SourceSystemName+Field>,<http://ddwiki.reso.org/display/DDW/SourceSystemName+%28Member%29+Field>,<http://ddwiki.reso.org/display/DDW/SourceSystemName+%28Office%29+Field>,<http://ddwiki.reso.org/display/DDW/SourceSystemName+%28Contacts%29+Field>,<http://ddwiki.reso.org/display/DDW/SourceSystemName+%28Media%29+Field>,<http://ddwiki.reso.org/display/DDW/SourceSystemName+%28HistoryTransactional%29+Field> ;
  vs:term_status   "stable"
.
reso:ClassName a rdf:Property ;
  rdfs:comment     "The class or table of the listing or other record the media.  Residential, Lease, Agent, Office, Contact, etc.","Name of the class which this history record applies.","The class or table to which the SearchQuery criteria refers.  i.e. Residential, Residential Lease, Income, Mobile, etc." ;
  rdfs:domain      reso:Media,reso:HistoryTransactional,reso:SavedSearch ;
  rdfs:label       "ClassName" ;
  rdfs:range       enum:ClassName,xsd:string ;
  reso:CertificationLevel "Bronze","Silver","Gold" ;
  schema:sameAs    <http://ddwiki.reso.org/display/DDW/ClassName+Field>,<http://ddwiki.reso.org/display/DDW/ClassName+%28HistoryTransactional%29+Field>,<http://ddwiki.reso.org/display/DDW/ClassName+%28SavedSearch%29+Field> ;
  vs:term_status   "stable"
.
reso:MemberKey a rdf:Property ;
  rdfs:comment     "A unique identifier for this record from the immediate source. This is a string that can include URI or other forms.  Alternatively use the MemberKeyNumeric for a numeric only key field.  This is the local key of the system.  When records are received from other systems, a local key is commonly applied.  If conveying the original keys from the source or originating systems, see SourceSystemMemberKey and OriginatingSystemMemberKey.","A system unique identifier. Specifically, in aggregation systems, the MemberKey is the system unique identifier from the system that the record was retrieved. This may be identical to the related xxxId.  This is a foreign key relating to the Member resource's MemberKey." ;
  rdfs:domain      reso:Member,reso:SavedSearch ;
  rdfs:label       "MemberKey" ;
  rdfs:range       xsd:string ;
  reso:CertificationLevel "Core","Gold" ;
  schema:sameAs    <http://ddwiki.reso.org/display/DDW/MemberKey+Field>,<http://ddwiki.reso.org/display/DDW/MemberKey+%28SavedSearch%29+Field> ;
  vs:term_status   "stable"
.
reso:MemberKeyNumeric a rdf:Property ;
  rdfs:comment     "A unique identifier for this record from the immediate source. This is the numeric only key and used as an alternative to the MemberKey fields.  This is the local key of the system.  When records are received from other systems, a local key is commonly applied.  If conveying the original keys from the source or originating systems, see SourceSystemMemberKey and OriginatingSystemMemberKey.","A system unique identifier. Specifically, in aggregation systems, the MemberKey is the system unique identifier from the system that the record was retrieved. This may be identical to the related xxxId.  This is a foreign key relating to the Member resource's MemberKey.  This is the numeric only key and used as an alternative to the MemberKey field." ;
  rdfs:domain      reso:Member,reso:SavedSearch ;
  rdfs:label       "MemberKeyNumeric" ;
  rdfs:range       xsd:decimal ;
  reso:CertificationLevel "Platinum" ;
  schema:sameAs    <http://ddwiki.reso.org/display/DDW/MemberKeyNumeric+Field>,<http://ddwiki.reso.org/display/DDW/MemberKeyNumeric+%28SavedSearch%29+Field> ;
  vs:term_status   "stable"
.
reso:MemberMlsId a rdf:Property ;
  rdfs:comment     "The local, well-known identifier for the member. This value may not be unique, specifically in the case of aggregation systems, this value should be the identifier from the original system." ;
  rdfs:domain      reso:Member,reso:SavedSearch ;
  rdfs:label       "MemberMlsId" ;
  rdfs:range       xsd:string ;
  reso:CertificationLevel "Core","Gold" ;
  schema:sameAs    <http://ddwiki.reso.org/display/DDW/MemberMlsId+Field>,<http://ddwiki.reso.org/display/DDW/MemberMlsId+%28SavedSearch%29+Field> ;
  vs:term_status   "stable"
.
reso:ModificationTimestamp a rdf:Property ;
  rdfs:comment     "The transactional timestamp automatically recorded by the MLS system representing the date/time the listing was last modified.","Date/time the roster (member or office) record was last modified.","Date/time the contact record was last modified.","The transactional timestamp automatically recorded by the MLS system representing the date/time the media record was last modified.","Timestamp of the last major change on the listing (see also MajorChangeType)." ;
  rdfs:domain      reso:Property,reso:Member,reso:Office,reso:Contacts,reso:Media,reso:HistoryTransactional,reso:SavedSearch ;
  rdfs:label       "ModificationTimestamp" ;
  rdfs:range       xsd:dateTime ;
  reso:CertificationLevel "Core","Silver","Gold" ;
  reso:PropertyTypes "RESI","RLSE","RINC","LAND","MOBI","FARM","COMS","COML","BUSO" ;
  schema:sameAs    <http://ddwiki.reso.org/display/DDW/ModificationTimestamp+Field>,<http://ddwiki.reso.org/display/DDW/ModificationTimestamp+%28Member%29+Field>,<http://ddwiki.reso.org/display/DDW/ModificationTimestamp+%28Office%29+Field>,<http://ddwiki.reso.org/display/DDW/ModificationTimestamp+%28Contacts%29+Field>,<http://ddwiki.reso.org/display/DDW/ModificationTimestamp+%28Media%29+Field>,<http://ddwiki.reso.org/display/DDW/ModificationTimestamp+%28HistoryTransactional%29+Field>,<http://ddwiki.reso.org/display/DDW/ModificationTimestamp+%28SavedSearch%29+Field> ;
  vs:term_status   "stable"
.
reso:OriginalEntryTimestamp a rdf:Property ;
  rdfs:comment     "The transactional timestamp automatically recorded by the MLS system representing the date/time the listing was entered and made visible to members of the MLS.","Date/time the roster (member or office) record was originally input into the source system.","Date/time the contact record was originally input into the source system." ;
  rdfs:domain      reso:Property,reso:Member,reso:Office,reso:Contacts,reso:SavedSearch ;
  rdfs:label       "OriginalEntryTimestamp" ;
  rdfs:range       xsd:dateTime ;
  reso:CertificationLevel "Core","Silver","Gold" ;
  reso:PropertyTypes "RESI","RLSE","RINC","LAND","MOBI","FARM","COMS","COML","BUSO" ;
  schema:sameAs    <http://ddwiki.reso.org/display/DDW/OriginalEntryTimestamp+Field>,<http://ddwiki.reso.org/display/DDW/OriginalEntryTimestamp+%28Member%29+Field>,<http://ddwiki.reso.org/display/DDW/OriginalEntryTimestamp+%28Office%29+Field>,<http://ddwiki.reso.org/display/DDW/OriginalEntryTimestamp+%28Contacts%29+Field>,<http://ddwiki.reso.org/display/DDW/OriginalEntryTimestamp+%28SavedSearch%29+Field> ;
  vs:term_status   "stable"
.
reso:OriginatingSystemID a rdf:Property ;
  rdfs:comment     "The RESO OUID's OrganizationUniqueId of the Originating record provider.  The Originating system is the system with authoritative control over the record.  For example; the name of the MLS where the listing was input.  In cases where the Originating system was not where the record originated (the authoritative system), see the Originating System fields.","The RESO OUID's OrganizationUniqueId of the Originating record provider.  The Originating system is the system with authoritative control over the record.  For example; the name of the MLS where the member was input.  In cases where the Originating system was not where the record originated (the authoritative system), see the Originating System fields.","The RESO OUID's OrganizationUniqueId of the Originating record provider.  The Originating system is the system with authoritative control over the record.  For example; the name of the MLS where the office was input.  In cases where the Originating system was not where the record originated (the authoritative system), see the Originating System fields.","The RESO OUID's OrganizationUniqueId of the Originating record provider.  The Originating system is the system with authoritative control over the record.  For example; the name of the MLS where the Contact was input.  In cases where the Originating system was not where the record originated (the authoritative system), see the Originating System fields.","The RESO OUID's OrganizationUniqueId of the Originating record provider.  The Originating system is the system with authoritative control over the record.  For example; the name of the MLS where the Media was input.  In cases where the Originating system was not where the record originated (the authoritative system), see the Originating System fields.","The RESO OUID's OrganizationUniqueId of the Originating record provider.  The Originating system is the system with authoritative control over the record.  For example; the name of the MLS where the History was input.  In cases where the Originating system was not where the record originated (the authoritative system), see the Originating System fields.","The RESO OUID's OrganizationUniqueId of the Originating record provider.  The Originating system is the system with authoritative control over the record.  For example; the name of the MLS where the Saved Search was input.  In cases where the Originating system was not where the record originated (the authoritative system), see the Originating System fields." ;
  rdfs:domain      reso:Property,reso:Member,reso:Office,reso:Contacts,reso:Media,reso:HistoryTransactional,reso:SavedSearch ;
  rdfs:label       "OriginatingSystemID" ;
  rdfs:range       xsd:string ;
  reso:CertificationLevel "Platinum" ;
  reso:PropertyTypes "RESI","RLSE","RINC","LAND","MOBI","FARM","COMS","COML","BUSO" ;
  schema:sameAs    <http://ddwiki.reso.org/display/DDW/OriginatingSystemID+Field>,<http://ddwiki.reso.org/display/DDW/OriginatingSystemID+%28Member%29+Field>,<http://ddwiki.reso.org/display/DDW/OriginatingSystemID+%28Office%29+Field>,<http://ddwiki.reso.org/display/DDW/OriginatingSystemID+%28Contacts%29+Field>,<http://ddwiki.reso.org/display/DDW/OriginatingSystemID+%28Media%29+Field>,<http://ddwiki.reso.org/display/DDW/OriginatingSystemID+%28HistoryTransactional%29+Field>,<http://ddwiki.reso.org/display/DDW/OriginatingSystemID+%28SavedSearch%29+Field> ;
  vs:term_status   "stable"
.
reso:OriginatingSystemKey a rdf:Property ;
  rdfs:comment     "The system key, a unique record identifier, from the Originating system.  The Originating system is the system with authoritative control over the record.  For example, the Multiple Listing Service where the listing was input.  There may be cases where the Source System (how you received the record) is not the Originating System.  See Source System Key for more information.","The system key, a unique record identifier, from the Originating system.  The Originating system is the system with authoritative control over the record.  For example, the Multiple Listing Service where the Saved Search was input.  There may be cases where the Source System (how you received the record) is not the Originating System.  See Source System Key for more information." ;
  rdfs:domain      reso:Property,reso:SavedSearch ;
  rdfs:label       "OriginatingSystemKey" ;
  rdfs:range       xsd:string ;
  reso:CertificationLevel "Core","Gold" ;
  reso:PropertyTypes "RESI","RLSE","RINC","LAND","MOBI","FARM","COMS","COML","BUSO" ;
  schema:sameAs    <http://ddwiki.reso.org/display/DDW/OriginatingSystemKey+Field>,<http://ddwiki.reso.org/display/DDW/OriginatingSystemKey+%28SavedSearch%29+Field> ;
  vs:term_status   "stable"
.
reso:OriginatingSystemMemberKey a rdf:Property ;
  rdfs:comment     "The system key, a unique record identifier, from the Originating system.  The Originating system is the system with authoritative control over the record.  For example, the Multiple Listing Service where the member was input.  There may be cases where the Source System (how you received the record) is not the Originating System.  See Source System Key for more information.","Unique identifier from the originating system which is commonly a key to that system.  In the case where data is passed through more than one system, this is the originating system key.  This is a foreign key relating to the system where this record was originated." ;
  rdfs:domain      reso:Member,reso:SavedSearch ;
  rdfs:label       "OriginatingSystemMemberKey" ;
  rdfs:range       xsd:string ;
  reso:CertificationLevel "Core","Gold" ;
  schema:sameAs    <http://ddwiki.reso.org/display/DDW/OriginatingSystemMemberKey+Field>,<http://ddwiki.reso.org/display/DDW/OriginatingSystemMemberKey+%28SavedSearch%29+Field> ;
  vs:term_status   "stable"
.
reso:OriginatingSystemMemberName a rdf:Property ;
  rdfs:comment     "The name of the originating record provider.  Most commonly the name of the MLS. The place where the listing is originally input by the member.  The legal name of the company.  To be used for display." ;
  rdfs:domain      reso:SavedSearch ;
  rdfs:label       "OriginatingSystemMemberName" ;
  rdfs:range       xsd:string ;
  reso:CertificationLevel "Gold" ;
  schema:sameAs    <http://ddwiki.reso.org/display/DDW/OriginatingSystemMemberName+Field> ;
  vs:term_status   "stable"
.
reso:OriginatingSystemName a rdf:Property ;
  rdfs:comment     "The name of the Originating record provider.  Most commonly the name of the MLS. The place where the listing is originally input by the member.  The legal name of the company.","The name of the Originating record provider.  Most commonly the name of the MLS. The place where the member is originally input by the member.  The legal name of the company.","The name of the Originating record provider.  Most commonly the name of the MLS. The place where the office is originally input by the member.  The legal name of the company.","The name of the Originating record provider.  Most commonly the name of the MLS. The place where the Contact is originally input by the member.  The legal name of the company.","The name of the Originating record provider.  Most commonly the name of the MLS. The place where the Media is originally input by the member.  The legal name of the company.","The name of the Originating record provider.  Most commonly the name of the MLS. The place where the History is originally input.  The legal name of the company.","The name of the Originating record provider.  Most commonly the name of the MLS. The place where the Saved Search is originally input.  The legal name of the company." ;
  rdfs:domain      reso:Property,reso:Member,reso:Office,reso:Contacts,reso:Media,reso:HistoryTransactional,reso:SavedSearch ;
  rdfs:label       "OriginatingSystemName" ;
  rdfs:range       xsd:string ;
  reso:CertificationLevel "Core","Bronze","Silver","Gold" ;
  reso:PropertyTypes "RESI","RLSE","RINC","LAND","MOBI","FARM","COMS","COML","BUSO" ;
  schema:sameAs    <http://ddwiki.reso.org/display/DDW/OriginatingSystemName+Field>,<http://ddwiki.reso.org/display/DDW/OriginatingSystemName+%28Member%29+Field>,<http://ddwiki.reso.org/display/DDW/OriginatingSystemName+%28Office%29+Field>,<http://ddwiki.reso.org/display/DDW/OriginatingSystemName+%28Contacts%29+Field>,<http://ddwiki.reso.org/display/DDW/OriginatingSystemName+%28Media%29+Field>,<http://ddwiki.reso.org/display/DDW/OriginatingSystemName+%28HistoryTransactional%29+Field>,<http://ddwiki.reso.org/display/DDW/OriginatingSystemName+%28SavedSearch%29+Field> ;
  vs:term_status   "stable"
.
reso:ResourceName a rdf:Property ;
  rdfs:comment     "The resource or table of the listing or other record the media relates to.  i.e. Property, Member, Office, etc.","The name of the resource which this history record applies.","The resource to which the SearchQuery criteria refers. i.e. Property, Open House, Agent, Office, Contact, etc." ;
  rdfs:domain      reso:Media,reso:HistoryTransactional,reso:SavedSearch ;
  rdfs:label       "ResourceName" ;
  rdfs:range       enum:ResourceName,xsd:string ;
  reso:CertificationLevel "Core","Silver","Gold" ;
  schema:sameAs    <http://ddwiki.reso.org/display/DDW/ResourceName+Field>,<http://ddwiki.reso.org/display/DDW/ResourceName+%28HistoryTransactional%29+Field>,<http://ddwiki.reso.org/display/DDW/ResourceName+%28SavedSearch%29+Field> ;
  vs:term_status   "stable"
.
reso:SavedSearchDescription a rdf:Property ;
  rdfs:comment     "A textual description of the saved search input by the member who created the saved search." ;
  rdfs:domain      reso:SavedSearch ;
  rdfs:label       "SavedSearchDescription" ;
  rdfs:range       xsd:string ;
  reso:CertificationLevel "Gold" ;
  schema:sameAs    <http://ddwiki.reso.org/display/DDW/SavedSearchDescription+Field> ;
  vs:term_status   "stable"
.
reso:SavedSearchKey a rdf:Property ;
  rdfs:comment     "A unique identifier for this record from the immediate source. This may be a number, or string that can include URI or other forms.  This is the system you are connecting to and not necessarily the original source of the record." ;
  rdfs:domain      reso:SavedSearch ;
  rdfs:label       "SavedSearchKey" ;
  rdfs:range       xsd:string ;
  reso:CertificationLevel "Gold" ;
  schema:sameAs    <http://ddwiki.reso.org/display/DDW/SavedSearchKey+Field> ;
  vs:term_status   "stable"
.
reso:SavedSearchKeyNumeric a rdf:Property ;
  rdfs:comment     "A unique identifier for this record from the immediate source. This may be a number, or string that can include URI or other forms.  This is the system you are connecting to and not necessarily the original source of the record.  This is the numeric only key and used as an alternative to the SavedSearchKey field." ;
  rdfs:domain      reso:SavedSearch ;
  rdfs:label       "SavedSearchKeyNumeric" ;
  rdfs:range       xsd:decimal ;
  reso:CertificationLevel "Platinum" ;
  schema:sameAs    <http://ddwiki.reso.org/display/DDW/SavedSearchKeyNumeric+Field> ;
  vs:term_status   "stable"
.
reso:SavedSearchName a rdf:Property ;
  rdfs:comment     "The name given to the search by the member inputting the saved search." ;
  rdfs:domain      reso:SavedSearch ;
  rdfs:label       "SavedSearchName" ;
  rdfs:range       xsd:string ;
  reso:CertificationLevel "Gold" ;
  schema:sameAs    <http://ddwiki.reso.org/display/DDW/SavedSearchName+Field> ;
  vs:term_status   "stable"
.
reso:SavedSearchType a rdf:Property ;
  rdfs:comment     "Is the saved search used to pass criteria to be stored and executed by the client or is the saved search a key to be passed to the host for execution.  i.e. Client Receives Criteria, Host Returns Listings.  This may be described at the record level with this field, or at some other level of implementation to be determined by RESO R&D." ;
  rdfs:domain      reso:SavedSearch ;
  rdfs:label       "SavedSearchType" ;
  rdfs:range       xsd:string ;
  reso:CertificationLevel "Gold" ;
  schema:sameAs    <http://ddwiki.reso.org/display/DDW/SavedSearchType+Field> ;
  vs:term_status   "stable"
.
reso:SearchQuery a rdf:Property ;
  rdfs:comment     "Textual representation of the search performed by the member that was saved.  It is required to present in ODATA's $filter format.  Additional formats are under review.  See additional documentation for specific requirements for this field." ;
  rdfs:domain      reso:SavedSearch ;
  rdfs:label       "SearchQuery" ;
  rdfs:range       xsd:string ;
  reso:CertificationLevel "Gold" ;
  schema:sameAs    <http://ddwiki.reso.org/display/DDW/SearchQuery+Field> ;
  vs:term_status   "stable"
.
reso:SearchQueryExceptionDetails a rdf:Property ;
  rdfs:comment     "A free text description used to expand on the SearchQueryExceptions selections made by the host." ;
  rdfs:domain      reso:SavedSearch ;
  rdfs:label       "SearchQueryExceptionDetails" ;
  rdfs:range       xsd:string ;
  reso:CertificationLevel "Gold" ;
  schema:sameAs    <http://ddwiki.reso.org/display/DDW/SearchQueryExceptionDetails+Field> ;
  vs:term_status   "stable"
.
reso:SearchQueryExceptions a rdf:Property ;
  rdfs:comment     "A list of exceptions or errors with the given search query during it's creation by the host.  Analogous to an error code this is the host's opportunity to describe an inability to fully express a saved search under the constraints of the given protocol.  i.e. $filter.  The client may use this information to bring attention to the user about a given saved search and a need to review or recreate the search." ;
  rdfs:domain      reso:SavedSearch ;
  rdfs:label       "SearchQueryExceptions" ;
  rdfs:range       xsd:string ;
  reso:CertificationLevel "Gold" ;
  schema:sameAs    <http://ddwiki.reso.org/display/DDW/SearchQueryExceptions+Field> ;
  vs:term_status   "stable"
.
reso:SearchQueryHumanReadable a rdf:Property ;
  rdfs:comment     "A human readable version of the search query that is commonly used for display and may not contain all actual criteria.  For actual search criteria, use the SearchQuery field." ;
  rdfs:domain      reso:SavedSearch ;
  rdfs:label       "SearchQueryHumanReadable" ;
  rdfs:range       xsd:string ;
  reso:CertificationLevel "Gold" ;
  schema:sameAs    <http://ddwiki.reso.org/display/DDW/SearchQueryHumanReadable+Field> ;
  vs:term_status   "stable"
.
reso:SearchQueryType a rdf:Property ;
  rdfs:comment     "A picklist of the type of query language used in the SearchQuery field.  i.e. DMQL2, $filter, etc." ;
  rdfs:domain      reso:SavedSearch ;
  rdfs:label       "SearchQueryType" ;
  rdfs:range       xsd:string ;
  reso:CertificationLevel "Gold" ;
  schema:sameAs    <http://ddwiki.reso.org/display/DDW/SearchQueryType+Field> ;
  vs:term_status   "stable"
.
reso:SourceSystemID a rdf:Property ;
  rdfs:comment     "The RESO OUID's OrganizationUniqueId of the Source record provider. The source system is the system from which the record was directly received. In cases where the source system was not where the record originated (the authoritative system), see the Originating System fields.","The RESO OUID's OrganizationUniqueId of the Source record provider.  The source system is the system from which the record was directly received.  In cases where the source system was not where the record originated (the authoritative system), see the Originating System fields." ;
  rdfs:domain      reso:Property,reso:Member,reso:Office,reso:Contacts,reso:Media,reso:HistoryTransactional,reso:SavedSearch ;
  rdfs:label       "SourceSystemID" ;
  rdfs:range       xsd:string ;
  reso:CertificationLevel "Platinum" ;
  reso:PropertyTypes "RESI","RLSE","RINC","LAND","MOBI","FARM","COMS","COML","BUSO" ;
  schema:sameAs    <http://ddwiki.reso.org/display/DDW/SourceSystemID+Field>,<http://ddwiki.reso.org/display/DDW/SourceSystemID+%28Member%29+Field>,<http://ddwiki.reso.org/display/DDW/SourceSystemID+%28Office%29+Field>,<http://ddwiki.reso.org/display/DDW/SourceSystemID+%28Contacts%29+Field>,<http://ddwiki.reso.org/display/DDW/SourceSystemID+%28Media%29+Field>,<http://ddwiki.reso.org/display/DDW/SourceSystemID+%28HistoryTransactional%29+Field>,<http://ddwiki.reso.org/display/DDW/SourceSystemID+%28SavedSearch%29+Field> ;
  vs:term_status   "stable"
.
reso:SourceSystemKey a rdf:Property ;
  rdfs:comment     "The system key, a unique record identifier, from the Source System. The Source System is the system from which the record was directly received. In cases where the Source System was not where the record originated (the authoritative system), see the Originating System fields.","The system key, a unique record identifier, from the Source System.  The Source System is the system from which the record was directly received.  In cases where the Source System was not where the record originated (the authoritative system), see the Originating System fields." ;
  rdfs:domain      reso:Property,reso:SavedSearch ;
  rdfs:label       "SourceSystemKey" ;
  rdfs:range       xsd:string ;
  reso:CertificationLevel "Core","Silver" ;
  reso:PropertyTypes "RESI","RLSE","RINC","LAND","MOBI","FARM","COMS","COML","BUSO" ;
  schema:sameAs    <http://ddwiki.reso.org/display/DDW/SourceSystemKey+Field>,<http://ddwiki.reso.org/display/DDW/SourceSystemKey+%28SavedSearch%29+Field> ;
  vs:term_status   "stable"
.
reso:SourceSystemName a rdf:Property ;
  rdfs:comment     "The name of the immediate record provider. The system from which the record was directly received. The legal name of the company.","The name of the immediate record provider.  The system from which the record was directly received.  The legal name of the company.","The name of the History record provider.  The system from which the record was directly received.  The legal name of the company.","The name of the Saved Search record provider.  The system from which the record was directly received.  The legal name of the company." ;
  rdfs:domain      reso:Property,reso:Member,reso:Office,reso:Contacts,reso:Media,reso:HistoryTransactional,reso:SavedSearch ;
  rdfs:label       "SourceSystemName" ;
  rdfs:range       xsd:string ;
  reso:CertificationLevel "Core","Silver" ;
  reso:PropertyTypes "RESI","RLSE","RINC","LAND","MOBI","FARM","COMS","COML","BUSO" ;
  schema:sameAs    <http://ddwiki.reso.org/display/DDW/SourceSystemName+Field>,<http://ddwiki.reso.org/display/DDW/SourceSystemName+%28Member%29+Field>,<http://ddwiki.reso.org/display/DDW/SourceSystemName+%28Office%29+Field>,<http://ddwiki.reso.org/display/DDW/SourceSystemName+%28Contacts%29+Field>,<http://ddwiki.reso.org/display/DDW/SourceSystemName+%28Media%29+Field>,<http://ddwiki.reso.org/display/DDW/SourceSystemName+%28HistoryTransactional%29+Field>,<http://ddwiki.reso.org/display/DDW/SourceSystemName+%28SavedSearch%29+Field> ;
  vs:term_status   "stable"
.
reso:AppointmentRequiredYN a rdf:Property ;
  rdfs:comment     "Indicates whether or not the OpenHouse requires an appointment." ;
  rdfs:domain      reso:OpenHouse ;
  rdfs:label       "AppointmentRequiredYN" ;
  rdfs:range       xsd:boolean ;
  reso:CertificationLevel "Bronze" ;
  schema:sameAs    <http://ddwiki.reso.org/display/DDW/AppointmentRequiredYN+Field> ;
  vs:term_status   "stable"
.
reso:ListingId a rdf:Property ;
  rdfs:comment     "The well known identifier for the listing. The value may be identical to that of the Listing Key, but the Listing ID is intended to be the value used by a human to retrieve the information about a specific listing. In a multiple originating system or a merged system, this value may not be unique and may require the use of the provider system to create a synthetic unique value.","The well known identifier for the listing related to this Open House. The value may be identical to that of the Listing Key, but the Listing ID is intended to be the value used by a human to retrieve the information about a specific listing. In a multiple originating system or a merged system, this value may not be unique and may require the use of the provider system to create a synthetic unique value." ;
  rdfs:domain      reso:Property,reso:OpenHouse ;
  rdfs:label       "ListingId" ;
  rdfs:range       xsd:string ;
  reso:CertificationLevel "Core" ;
  reso:PropertyTypes "RESI","RLSE","RINC","LAND","MOBI","FARM","COMS","COML","BUSO" ;
  schema:sameAs    <http://ddwiki.reso.org/display/DDW/ListingId+Field>,<http://ddwiki.reso.org/display/DDW/ListingId+%28OpenHouse%29+Field> ;
  vs:term_status   "stable"
.
reso:ListingKey a rdf:Property ;
  rdfs:comment     "A unique identifier for this record from the immediate source. This is a string that can include URI or other forms.  Alternatively use the ListingKeyNumeric for a numeric only key field.  This is the local key of the system.  When records are received from other systems, a local key is commonly applied.  If conveying the original keys from the source or originating systems, see SourceSystemKey and OriginatingSystemKey.","A unique identifier for the listing record related to this Open House. This may be a number, or string that can include URI or other forms.  This is the system you are connecting to and not necessarily the original source of the record.   This may be a foreign key from the resource selected in the ResourceName field." ;
  rdfs:domain      reso:Property,reso:OpenHouse ;
  rdfs:label       "ListingKey" ;
  rdfs:range       xsd:string ;
  reso:CertificationLevel "Core" ;
  reso:PropertyTypes "RESI","RLSE","RINC","LAND","MOBI","FARM","COMS","COML","BUSO" ;
  schema:sameAs    <http://ddwiki.reso.org/display/DDW/ListingKey+Field>,<http://ddwiki.reso.org/display/DDW/ListingKey+%28OpenHouse%29+Field> ;
  vs:term_status   "stable"
.
reso:ListingKeyNumeric a rdf:Property ;
  rdfs:comment     "A unique identifier for this record from the immediate source. This is the numeric only key and used as an alternative to the ListingKey fields.  This is the local key of the system.  When records are received from other systems, a local key is commonly applied.  If conveying the original keys from the source or originating systems, see SourceSystemKey and OriginatingSystemKey.","A unique identifier for the listing record related to this Open House. This may be a number, or string that can include URI or other forms.  This is the system you are connecting to and not necessarily the original source of the record.   This may be a foreign key from the resource selected in the ResourceName field.  This is the numeric only key and used as an alternative to the ListingKey field." ;
  rdfs:domain      reso:Property,reso:OpenHouse ;
  rdfs:label       "ListingKeyNumeric" ;
  rdfs:range       xsd:decimal ;
  reso:CertificationLevel "Platinum" ;
  reso:PropertyTypes "RESI","RLSE","RINC","LAND","MOBI","FARM","COMS","COML","BUSO" ;
  schema:sameAs    <http://ddwiki.reso.org/display/DDW/ListingKeyNumeric+Field>,<http://ddwiki.reso.org/display/DDW/ListingKeyNumeric+%28OpenHouse%29+Field> ;
  vs:term_status   "stable"
.
reso:ModificationTimestamp a rdf:Property ;
  rdfs:comment     "The transactional timestamp automatically recorded by the MLS system representing the date/time the listing was last modified.","Date/time the roster (member or office) record was last modified.","Date/time the contact record was last modified.","The transactional timestamp automatically recorded by the MLS system representing the date/time the media record was last modified.","Timestamp of the last major change on the listing (see also MajorChangeType).","The transactional timestamp automatically recorded by the MLS system representing the date/time the Open House was last modified." ;
  rdfs:domain      reso:Property,reso:Member,reso:Office,reso:Contacts,reso:Media,reso:HistoryTransactional,reso:SavedSearch,reso:OpenHouse ;
  rdfs:label       "ModificationTimestamp" ;
  rdfs:range       xsd:dateTime ;
  reso:CertificationLevel "Core","Silver","Gold" ;
  reso:PropertyTypes "RESI","RLSE","RINC","LAND","MOBI","FARM","COMS","COML","BUSO" ;
  schema:sameAs    <http://ddwiki.reso.org/display/DDW/ModificationTimestamp+Field>,<http://ddwiki.reso.org/display/DDW/ModificationTimestamp+%28Member%29+Field>,<http://ddwiki.reso.org/display/DDW/ModificationTimestamp+%28Office%29+Field>,<http://ddwiki.reso.org/display/DDW/ModificationTimestamp+%28Contacts%29+Field>,<http://ddwiki.reso.org/display/DDW/ModificationTimestamp+%28Media%29+Field>,<http://ddwiki.reso.org/display/DDW/ModificationTimestamp+%28HistoryTransactional%29+Field>,<http://ddwiki.reso.org/display/DDW/ModificationTimestamp+%28SavedSearch%29+Field>,<http://ddwiki.reso.org/display/DDW/ModificationTimestamp+%28OpenHouse%29+Field> ;
  vs:term_status   "stable"
.
reso:OpenHouseAttendedBy a rdf:Property ;
  rdfs:comment     "Will the open house be attended by a licensed agent?  Options are attended by agent, attended by the seller or unattended." ;
  rdfs:domain      reso:OpenHouse ;
  rdfs:label       "OpenHouseAttendedBy" ;
  rdfs:range       enum:Attended ;
  reso:CertificationLevel "Bronze" ;
  schema:sameAs    <http://ddwiki.reso.org/display/DDW/OpenHouseAttendedBy+Field> ;
  vs:term_status   "stable"
.
reso:OpenHouseDate a rdf:Property ;
  rdfs:comment     "The date on which the open house will occur." ;
  rdfs:domain      reso:OpenHouse ;
  rdfs:label       "OpenHouseDate" ;
  rdfs:range       xsd:date ;
  reso:CertificationLevel "Core" ;
  schema:sameAs    <http://ddwiki.reso.org/display/DDW/OpenHouseDate+Field> ;
  vs:term_status   "stable"
.
reso:OpenHouseEndTime a rdf:Property ;
  rdfs:comment     "The time the open house ends." ;
  rdfs:domain      reso:OpenHouse ;
  rdfs:label       "OpenHouseEndTime" ;
  rdfs:range       xsd:dateTime ;
  reso:CertificationLevel "Core" ;
  schema:sameAs    <http://ddwiki.reso.org/display/DDW/OpenHouseEndTime+Field> ;
  vs:term_status   "stable"
.
reso:OpenHouseId a rdf:Property ;
  rdfs:comment     "The well known identifier for the listing. The value may be identical to that of the Listing Key, but the Listing ID is intended to be the value used by a human to retrieve the information about a specific listing. In a multiple originating system or a merged system, this value may not be unique and may require the use of the provider system to create a synthetic unique value." ;
  rdfs:domain      reso:OpenHouse ;
  rdfs:label       "OpenHouseId" ;
  rdfs:range       xsd:string ;
  reso:CertificationLevel "Core" ;
  schema:sameAs    <http://ddwiki.reso.org/display/DDW/OpenHouseId+Field> ;
  vs:term_status   "stable"
.
reso:OpenHouseKey a rdf:Property ;
  rdfs:comment     "A unique identifier for this record from the immediate source. This may be a number, or string that can include URI or other forms.  This is the system you are connecting to and not necessarily the original source of the record." ;
  rdfs:domain      reso:OpenHouse ;
  rdfs:label       "OpenHouseKey" ;
  rdfs:range       xsd:string ;
  reso:CertificationLevel "Core" ;
  schema:sameAs    <http://ddwiki.reso.org/display/DDW/OpenHouseKey+Field> ;
  vs:term_status   "stable"
.
reso:OpenHouseKeyNumeric a rdf:Property ;
  rdfs:comment     "A unique identifier for this record from the immediate source. This may be a number, or string that can include URI or other forms.  This is the system you are connecting to and not necessarily the original source of the record.  This is the numeric only key and used as an alternative to the OpenHouseKey field." ;
  rdfs:domain      reso:OpenHouse ;
  rdfs:label       "OpenHouseKeyNumeric" ;
  rdfs:range       xsd:decimal ;
  reso:CertificationLevel "Platinum" ;
  schema:sameAs    <http://ddwiki.reso.org/display/DDW/OpenHouseKeyNumeric+Field> ;
  vs:term_status   "stable"
.
reso:OpenHouseRemarks a rdf:Property ;
  rdfs:comment     "Comments, instructions or information about the open house." ;
  rdfs:domain      reso:OpenHouse ;
  rdfs:label       "OpenHouseRemarks" ;
  rdfs:range       xsd:string ;
  reso:CertificationLevel "Core" ;
  schema:sameAs    <http://ddwiki.reso.org/display/DDW/OpenHouseRemarks+Field> ;
  vs:term_status   "stable"
.
reso:OpenHouseStartTime a rdf:Property ;
  rdfs:comment     "The time the open house begins." ;
  rdfs:domain      reso:OpenHouse ;
  rdfs:label       "OpenHouseStartTime" ;
  rdfs:range       xsd:dateTime ;
  reso:CertificationLevel "Core" ;
  schema:sameAs    <http://ddwiki.reso.org/display/DDW/OpenHouseStartTime+Field> ;
  vs:term_status   "stable"
.
reso:OpenHouseStatus a rdf:Property ;
  rdfs:comment     "Status of the open house, i.e. Active, Cancelled, Ended." ;
  rdfs:domain      reso:OpenHouse ;
  rdfs:label       "OpenHouseStatus" ;
  rdfs:range       enum:OpenHouseStatus ;
  reso:CertificationLevel "Core" ;
  schema:sameAs    <http://ddwiki.reso.org/display/DDW/OpenHouseStatus+Field> ;
  vs:term_status   "stable"
.
reso:OpenHouseType a rdf:Property ;
  rdfs:comment     "The type of open house.  i.e. Public, Broker, Office, Association, Private (invitation or targeted publication)." ;
  rdfs:domain      reso:OpenHouse ;
  rdfs:label       "OpenHouseType" ;
  rdfs:range       enum:OpenHouseType ;
  reso:CertificationLevel "Core" ;
  schema:sameAs    <http://ddwiki.reso.org/display/DDW/OpenHouseType+Field> ;
  vs:term_status   "stable"
.
reso:OriginalEntryTimestamp a rdf:Property ;
  rdfs:comment     "The transactional timestamp automatically recorded by the MLS system representing the date/time the listing was entered and made visible to members of the MLS.","Date/time the roster (member or office) record was originally input into the source system.","Date/time the contact record was originally input into the source system.","The transactional timestamp automatically recorded by the MLS system representing the date/time the Open House was entered and made visible to members of the MLS." ;
  rdfs:domain      reso:Property,reso:Member,reso:Office,reso:Contacts,reso:SavedSearch,reso:OpenHouse ;
  rdfs:label       "OriginalEntryTimestamp" ;
  rdfs:range       xsd:dateTime ;
  reso:CertificationLevel "Core","Silver","Gold","Bronze" ;
  reso:PropertyTypes "RESI","RLSE","RINC","LAND","MOBI","FARM","COMS","COML","BUSO" ;
  schema:sameAs    <http://ddwiki.reso.org/display/DDW/OriginalEntryTimestamp+Field>,<http://ddwiki.reso.org/display/DDW/OriginalEntryTimestamp+%28Member%29+Field>,<http://ddwiki.reso.org/display/DDW/OriginalEntryTimestamp+%28Office%29+Field>,<http://ddwiki.reso.org/display/DDW/OriginalEntryTimestamp+%28Contacts%29+Field>,<http://ddwiki.reso.org/display/DDW/OriginalEntryTimestamp+%28SavedSearch%29+Field>,<http://ddwiki.reso.org/display/DDW/OriginalEntryTimestamp+%28OpenHouse%29+Field> ;
  vs:term_status   "stable"
.
reso:OriginatingSystemID a rdf:Property ;
  rdfs:comment     "The RESO OUID's OrganizationUniqueId of the Originating record provider.  The Originating system is the system with authoritative control over the record.  For example; the name of the MLS where the listing was input.  In cases where the Originating system was not where the record originated (the authoritative system), see the Originating System fields.","The RESO OUID's OrganizationUniqueId of the Originating record provider.  The Originating system is the system with authoritative control over the record.  For example; the name of the MLS where the member was input.  In cases where the Originating system was not where the record originated (the authoritative system), see the Originating System fields.","The RESO OUID's OrganizationUniqueId of the Originating record provider.  The Originating system is the system with authoritative control over the record.  For example; the name of the MLS where the office was input.  In cases where the Originating system was not where the record originated (the authoritative system), see the Originating System fields.","The RESO OUID's OrganizationUniqueId of the Originating record provider.  The Originating system is the system with authoritative control over the record.  For example; the name of the MLS where the Contact was input.  In cases where the Originating system was not where the record originated (the authoritative system), see the Originating System fields.","The RESO OUID's OrganizationUniqueId of the Originating record provider.  The Originating system is the system with authoritative control over the record.  For example; the name of the MLS where the Media was input.  In cases where the Originating system was not where the record originated (the authoritative system), see the Originating System fields.","The RESO OUID's OrganizationUniqueId of the Originating record provider.  The Originating system is the system with authoritative control over the record.  For example; the name of the MLS where the History was input.  In cases where the Originating system was not where the record originated (the authoritative system), see the Originating System fields.","The RESO OUID's OrganizationUniqueId of the Originating record provider.  The Originating system is the system with authoritative control over the record.  For example; the name of the MLS where the Saved Search was input.  In cases where the Originating system was not where the record originated (the authoritative system), see the Originating System fields.","The RESO OUID's OrganizationUniqueId of the Originating record provider.  The Originating system is the system with authoritative control over the record.  For example; the name of the MLS where the Open House was input.  In cases where the Originating system was not where the record originated (the authoritative system), see the Originating System fields." ;
  rdfs:domain      reso:Property,reso:Member,reso:Office,reso:Contacts,reso:Media,reso:HistoryTransactional,reso:SavedSearch,reso:OpenHouse ;
  rdfs:label       "OriginatingSystemID" ;
  rdfs:range       xsd:string ;
  reso:CertificationLevel "Platinum" ;
  reso:PropertyTypes "RESI","RLSE","RINC","LAND","MOBI","FARM","COMS","COML","BUSO" ;
  schema:sameAs    <http://ddwiki.reso.org/display/DDW/OriginatingSystemID+Field>,<http://ddwiki.reso.org/display/DDW/OriginatingSystemID+%28Member%29+Field>,<http://ddwiki.reso.org/display/DDW/OriginatingSystemID+%28Office%29+Field>,<http://ddwiki.reso.org/display/DDW/OriginatingSystemID+%28Contacts%29+Field>,<http://ddwiki.reso.org/display/DDW/OriginatingSystemID+%28Media%29+Field>,<http://ddwiki.reso.org/display/DDW/OriginatingSystemID+%28HistoryTransactional%29+Field>,<http://ddwiki.reso.org/display/DDW/OriginatingSystemID+%28SavedSearch%29+Field>,<http://ddwiki.reso.org/display/DDW/OriginatingSystemID+%28OpenHouse%29+Field> ;
  vs:term_status   "stable"
.
reso:OriginatingSystemKey a rdf:Property ;
  rdfs:comment     "The system key, a unique record identifier, from the Originating system.  The Originating system is the system with authoritative control over the record.  For example, the Multiple Listing Service where the listing was input.  There may be cases where the Source System (how you received the record) is not the Originating System.  See Source System Key for more information.","The system key, a unique record identifier, from the Originating system.  The Originating system is the system with authoritative control over the record.  For example, the Multiple Listing Service where the Saved Search was input.  There may be cases where the Source System (how you received the record) is not the Originating System.  See Source System Key for more information.","The system key, a unique record identifier, from the Originating system.  The Originating system is the system with authoritative control over the record.  For example, the Multiple Listing Service where the Open House was input.  There may be cases where the Source System (how you received the record) is not the Originating System.  See Source System Key for more information." ;
  rdfs:domain      reso:Property,reso:SavedSearch,reso:OpenHouse ;
  rdfs:label       "OriginatingSystemKey" ;
  rdfs:range       xsd:string ;
  reso:CertificationLevel "Core","Gold" ;
  reso:PropertyTypes "RESI","RLSE","RINC","LAND","MOBI","FARM","COMS","COML","BUSO" ;
  schema:sameAs    <http://ddwiki.reso.org/display/DDW/OriginatingSystemKey+Field>,<http://ddwiki.reso.org/display/DDW/OriginatingSystemKey+%28SavedSearch%29+Field>,<http://ddwiki.reso.org/display/DDW/OriginatingSystemKey+%28OpenHouse%29+Field> ;
  vs:term_status   "stable"
.
reso:OriginatingSystemName a rdf:Property ;
  rdfs:comment     "The name of the Originating record provider.  Most commonly the name of the MLS. The place where the listing is originally input by the member.  The legal name of the company.","The name of the Originating record provider.  Most commonly the name of the MLS. The place where the member is originally input by the member.  The legal name of the company.","The name of the Originating record provider.  Most commonly the name of the MLS. The place where the office is originally input by the member.  The legal name of the company.","The name of the Originating record provider.  Most commonly the name of the MLS. The place where the Contact is originally input by the member.  The legal name of the company.","The name of the Originating record provider.  Most commonly the name of the MLS. The place where the Media is originally input by the member.  The legal name of the company.","The name of the Originating record provider.  Most commonly the name of the MLS. The place where the History is originally input.  The legal name of the company.","The name of the Originating record provider.  Most commonly the name of the MLS. The place where the Saved Search is originally input.  The legal name of the company.","The name of the Originating record provider.  Most commonly the name of the MLS. The place where the Open House is originally input.  The legal name of the company." ;
  rdfs:domain      reso:Property,reso:Member,reso:Office,reso:Contacts,reso:Media,reso:HistoryTransactional,reso:SavedSearch,reso:OpenHouse ;
  rdfs:label       "OriginatingSystemName" ;
  rdfs:range       xsd:string ;
  reso:CertificationLevel "Core","Bronze","Silver","Gold" ;
  reso:PropertyTypes "RESI","RLSE","RINC","LAND","MOBI","FARM","COMS","COML","BUSO" ;
  schema:sameAs    <http://ddwiki.reso.org/display/DDW/OriginatingSystemName+Field>,<http://ddwiki.reso.org/display/DDW/OriginatingSystemName+%28Member%29+Field>,<http://ddwiki.reso.org/display/DDW/OriginatingSystemName+%28Office%29+Field>,<http://ddwiki.reso.org/display/DDW/OriginatingSystemName+%28Contacts%29+Field>,<http://ddwiki.reso.org/display/DDW/OriginatingSystemName+%28Media%29+Field>,<http://ddwiki.reso.org/display/DDW/OriginatingSystemName+%28HistoryTransactional%29+Field>,<http://ddwiki.reso.org/display/DDW/OriginatingSystemName+%28SavedSearch%29+Field>,<http://ddwiki.reso.org/display/DDW/OriginatingSystemName+%28OpenHouse%29+Field> ;
  vs:term_status   "stable"
.
reso:Refreshments a rdf:Property ;
  rdfs:comment     "A description of the refreshments that will be served at the open house." ;
  rdfs:domain      reso:OpenHouse ;
  rdfs:label       "Refreshments" ;
  rdfs:range       xsd:string ;
  reso:CertificationLevel "Bronze" ;
  schema:sameAs    <http://ddwiki.reso.org/display/DDW/Refreshments+Field> ;
  vs:term_status   "stable"
.
reso:ShowingAgentFirstName a rdf:Property ;
  rdfs:comment     "The first name of the showing agent." ;
  rdfs:domain      reso:OpenHouse ;
  rdfs:label       "ShowingAgentFirstName" ;
  rdfs:range       xsd:string ;
  reso:CertificationLevel "Core" ;
  schema:sameAs    <http://ddwiki.reso.org/display/DDW/ShowingAgentFirstName+Field> ;
  vs:term_status   "stable"
.
reso:ShowingAgentKey a rdf:Property ;
  rdfs:comment     "A system unique identifier. Specifically, in aggregation systems, the ListAgentKey is the system unique identifier from the system that the record was retrieved. This may be identical to the related xxxId.  This is a foreign key relating to the Member resource's MemberKey." ;
  rdfs:domain      reso:OpenHouse ;
  rdfs:label       "ShowingAgentKey" ;
  rdfs:range       xsd:string ;
  reso:CertificationLevel "Core" ;
  schema:sameAs    <http://ddwiki.reso.org/display/DDW/ShowingAgentKey+Field> ;
  vs:term_status   "stable"
.
reso:ShowingAgentKeyNumeric a rdf:Property ;
  rdfs:comment     "A system unique identifier. Specifically, in aggregation systems, the ListAgentKey is the system unique identifier from the system that the record was retrieved. This may be identical to the related xxxId.  This is a foreign key relating to the Member resource's MemberKey.  This is the numeric only key and used as an alternative to the ShowingAgentKey field." ;
  rdfs:domain      reso:OpenHouse ;
  rdfs:label       "ShowingAgentKeyNumeric" ;
  rdfs:range       xsd:decimal ;
  reso:CertificationLevel "Platinum" ;
  schema:sameAs    <http://ddwiki.reso.org/display/DDW/ShowingAgentKeyNumeric+Field> ;
  vs:term_status   "stable"
.
reso:ShowingAgentLastName a rdf:Property ;
  rdfs:comment     "The last name of the showing agent." ;
  rdfs:domain      reso:OpenHouse ;
  rdfs:label       "ShowingAgentLastName" ;
  rdfs:range       xsd:string ;
  reso:CertificationLevel "Core" ;
  schema:sameAs    <http://ddwiki.reso.org/display/DDW/ShowingAgentLastName+Field> ;
  vs:term_status   "stable"
.
reso:ShowingAgentMlsID a rdf:Property ;
  rdfs:comment     "The local, well-known identifier for the member. This value may not be unique, specifically in the case of aggregation systems, this value should be the identifier from the original system." ;
  rdfs:domain      reso:OpenHouse ;
  rdfs:label       "ShowingAgentMlsID" ;
  rdfs:range       xsd:string ;
  reso:CertificationLevel "Core" ;
  schema:sameAs    <http://ddwiki.reso.org/display/DDW/ShowingAgentMlsID+Field> ;
  vs:term_status   "stable"
.
reso:SourceSystemID a rdf:Property ;
  rdfs:comment     "The RESO OUID's OrganizationUniqueId of the Source record provider. The source system is the system from which the record was directly received. In cases where the source system was not where the record originated (the authoritative system), see the Originating System fields.","The RESO OUID's OrganizationUniqueId of the Source record provider.  The source system is the system from which the record was directly received.  In cases where the source system was not where the record originated (the authoritative system), see the Originating System fields." ;
  rdfs:domain      reso:Property,reso:Member,reso:Office,reso:Contacts,reso:Media,reso:HistoryTransactional,reso:SavedSearch,reso:OpenHouse ;
  rdfs:label       "SourceSystemID" ;
  rdfs:range       xsd:string ;
  reso:CertificationLevel "Platinum" ;
  reso:PropertyTypes "RESI","RLSE","RINC","LAND","MOBI","FARM","COMS","COML","BUSO" ;
  schema:sameAs    <http://ddwiki.reso.org/display/DDW/SourceSystemID+Field>,<http://ddwiki.reso.org/display/DDW/SourceSystemID+%28Member%29+Field>,<http://ddwiki.reso.org/display/DDW/SourceSystemID+%28Office%29+Field>,<http://ddwiki.reso.org/display/DDW/SourceSystemID+%28Contacts%29+Field>,<http://ddwiki.reso.org/display/DDW/SourceSystemID+%28Media%29+Field>,<http://ddwiki.reso.org/display/DDW/SourceSystemID+%28HistoryTransactional%29+Field>,<http://ddwiki.reso.org/display/DDW/SourceSystemID+%28SavedSearch%29+Field>,<http://ddwiki.reso.org/display/DDW/SourceSystemID+%28OpenHouse%29+Field> ;
  vs:term_status   "stable"
.
reso:SourceSystemKey a rdf:Property ;
  rdfs:comment     "The system key, a unique record identifier, from the Source System. The Source System is the system from which the record was directly received. In cases where the Source System was not where the record originated (the authoritative system), see the Originating System fields.","The system key, a unique record identifier, from the Source System.  The Source System is the system from which the record was directly received.  In cases where the Source System was not where the record originated (the authoritative system), see the Originating System fields." ;
  rdfs:domain      reso:Property,reso:SavedSearch,reso:OpenHouse ;
  rdfs:label       "SourceSystemKey" ;
  rdfs:range       xsd:string ;
  reso:CertificationLevel "Core","Silver" ;
  reso:PropertyTypes "RESI","RLSE","RINC","LAND","MOBI","FARM","COMS","COML","BUSO" ;
  schema:sameAs    <http://ddwiki.reso.org/display/DDW/SourceSystemKey+Field>,<http://ddwiki.reso.org/display/DDW/SourceSystemKey+%28SavedSearch%29+Field>,<http://ddwiki.reso.org/display/DDW/SourceSystemKey+%28OpenHouse%29+Field> ;
  vs:term_status   "stable"
.
reso:SourceSystemName a rdf:Property ;
  rdfs:comment     "The name of the immediate record provider. The system from which the record was directly received. The legal name of the company.","The name of the immediate record provider.  The system from which the record was directly received.  The legal name of the company.","The name of the History record provider.  The system from which the record was directly received.  The legal name of the company.","The name of the Saved Search record provider.  The system from which the record was directly received.  The legal name of the company.","The name of the Open House record provider.  The system from which the record was directly received.  The legal name of the company." ;
  rdfs:domain      reso:Property,reso:Member,reso:Office,reso:Contacts,reso:Media,reso:HistoryTransactional,reso:SavedSearch,reso:OpenHouse ;
  rdfs:label       "SourceSystemName" ;
  rdfs:range       xsd:string ;
  reso:CertificationLevel "Core","Silver" ;
  reso:PropertyTypes "RESI","RLSE","RINC","LAND","MOBI","FARM","COMS","COML","BUSO" ;
  schema:sameAs    <http://ddwiki.reso.org/display/DDW/SourceSystemName+Field>,<http://ddwiki.reso.org/display/DDW/SourceSystemName+%28Member%29+Field>,<http://ddwiki.reso.org/display/DDW/SourceSystemName+%28Office%29+Field>,<http://ddwiki.reso.org/display/DDW/SourceSystemName+%28Contacts%29+Field>,<http://ddwiki.reso.org/display/DDW/SourceSystemName+%28Media%29+Field>,<http://ddwiki.reso.org/display/DDW/SourceSystemName+%28HistoryTransactional%29+Field>,<http://ddwiki.reso.org/display/DDW/SourceSystemName+%28SavedSearch%29+Field>,<http://ddwiki.reso.org/display/DDW/SourceSystemName+%28OpenHouse%29+Field> ;
  vs:term_status   "stable"
.
reso:ModificationTimestamp a rdf:Property ;
  rdfs:comment     "The transactional timestamp automatically recorded by the MLS system representing the date/time the listing was last modified.","Date/time the roster (member or office) record was last modified.","Date/time the contact record was last modified.","The transactional timestamp automatically recorded by the MLS system representing the date/time the media record was last modified.","Timestamp of the last major change on the listing (see also MajorChangeType).","The transactional timestamp automatically recorded by the MLS system representing the date/time the Open House was last modified.","Date/time the roster (Team or office) record was last modified." ;
  rdfs:domain      reso:Property,reso:Member,reso:Office,reso:Contacts,reso:Media,reso:HistoryTransactional,reso:SavedSearch,reso:OpenHouse,reso:Teams ;
  rdfs:label       "ModificationTimestamp" ;
  rdfs:range       xsd:dateTime ;
  reso:CertificationLevel "Core","Silver","Gold","Platinum" ;
  reso:PropertyTypes "RESI","RLSE","RINC","LAND","MOBI","FARM","COMS","COML","BUSO" ;
  schema:sameAs    <http://ddwiki.reso.org/display/DDW/ModificationTimestamp+Field>,<http://ddwiki.reso.org/display/DDW/ModificationTimestamp+%28Member%29+Field>,<http://ddwiki.reso.org/display/DDW/ModificationTimestamp+%28Office%29+Field>,<http://ddwiki.reso.org/display/DDW/ModificationTimestamp+%28Contacts%29+Field>,<http://ddwiki.reso.org/display/DDW/ModificationTimestamp+%28Media%29+Field>,<http://ddwiki.reso.org/display/DDW/ModificationTimestamp+%28HistoryTransactional%29+Field>,<http://ddwiki.reso.org/display/DDW/ModificationTimestamp+%28SavedSearch%29+Field>,<http://ddwiki.reso.org/display/DDW/ModificationTimestamp+%28OpenHouse%29+Field>,<http://ddwiki.reso.org/display/DDW/ModificationTimestamp+%28Teams%29+Field> ;
  vs:term_status   "stable"
.
reso:OriginalEntryTimestamp a rdf:Property ;
  rdfs:comment     "The transactional timestamp automatically recorded by the MLS system representing the date/time the listing was entered and made visible to members of the MLS.","Date/time the roster (member or office) record was originally input into the source system.","Date/time the contact record was originally input into the source system.","The transactional timestamp automatically recorded by the MLS system representing the date/time the Open House was entered and made visible to members of the MLS.","Date/time the roster (Team or office) record was originally input into the source system." ;
  rdfs:domain      reso:Property,reso:Member,reso:Office,reso:Contacts,reso:SavedSearch,reso:OpenHouse,reso:Teams ;
  rdfs:label       "OriginalEntryTimestamp" ;
  rdfs:range       xsd:dateTime ;
  reso:CertificationLevel "Core","Silver","Gold","Bronze","Platinum" ;
  reso:PropertyTypes "RESI","RLSE","RINC","LAND","MOBI","FARM","COMS","COML","BUSO" ;
  schema:sameAs    <http://ddwiki.reso.org/display/DDW/OriginalEntryTimestamp+Field>,<http://ddwiki.reso.org/display/DDW/OriginalEntryTimestamp+%28Member%29+Field>,<http://ddwiki.reso.org/display/DDW/OriginalEntryTimestamp+%28Office%29+Field>,<http://ddwiki.reso.org/display/DDW/OriginalEntryTimestamp+%28Contacts%29+Field>,<http://ddwiki.reso.org/display/DDW/OriginalEntryTimestamp+%28SavedSearch%29+Field>,<http://ddwiki.reso.org/display/DDW/OriginalEntryTimestamp+%28OpenHouse%29+Field>,<http://ddwiki.reso.org/display/DDW/OriginalEntryTimestamp+%28Teams%29+Field> ;
  vs:term_status   "stable"
.
reso:OriginatingSystemID a rdf:Property ;
  rdfs:comment     "The RESO OUID's OrganizationUniqueId of the Originating record provider.  The Originating system is the system with authoritative control over the record.  For example; the name of the MLS where the listing was input.  In cases where the Originating system was not where the record originated (the authoritative system), see the Originating System fields.","The RESO OUID's OrganizationUniqueId of the Originating record provider.  The Originating system is the system with authoritative control over the record.  For example; the name of the MLS where the member was input.  In cases where the Originating system was not where the record originated (the authoritative system), see the Originating System fields.","The RESO OUID's OrganizationUniqueId of the Originating record provider.  The Originating system is the system with authoritative control over the record.  For example; the name of the MLS where the office was input.  In cases where the Originating system was not where the record originated (the authoritative system), see the Originating System fields.","The RESO OUID's OrganizationUniqueId of the Originating record provider.  The Originating system is the system with authoritative control over the record.  For example; the name of the MLS where the Contact was input.  In cases where the Originating system was not where the record originated (the authoritative system), see the Originating System fields.","The RESO OUID's OrganizationUniqueId of the Originating record provider.  The Originating system is the system with authoritative control over the record.  For example; the name of the MLS where the Media was input.  In cases where the Originating system was not where the record originated (the authoritative system), see the Originating System fields.","The RESO OUID's OrganizationUniqueId of the Originating record provider.  The Originating system is the system with authoritative control over the record.  For example; the name of the MLS where the History was input.  In cases where the Originating system was not where the record originated (the authoritative system), see the Originating System fields.","The RESO OUID's OrganizationUniqueId of the Originating record provider.  The Originating system is the system with authoritative control over the record.  For example; the name of the MLS where the Saved Search was input.  In cases where the Originating system was not where the record originated (the authoritative system), see the Originating System fields.","The RESO OUID's OrganizationUniqueId of the Originating record provider.  The Originating system is the system with authoritative control over the record.  For example; the name of the MLS where the Open House was input.  In cases where the Originating system was not where the record originated (the authoritative system), see the Originating System fields.","The RESO OUID's OrganizationUniqueId of the Originating record provider.  The Originating system is the system with authoritative control over the record.  For example; the name of the MLS where the Team was input.  In cases where the Originating system was not where the record originated (the authoritative system), see the Originating System fields." ;
  rdfs:domain      reso:Property,reso:Member,reso:Office,reso:Contacts,reso:Media,reso:HistoryTransactional,reso:SavedSearch,reso:OpenHouse,reso:Teams ;
  rdfs:label       "OriginatingSystemID" ;
  rdfs:range       xsd:string ;
  reso:CertificationLevel "Platinum" ;
  reso:PropertyTypes "RESI","RLSE","RINC","LAND","MOBI","FARM","COMS","COML","BUSO" ;
  schema:sameAs    <http://ddwiki.reso.org/display/DDW/OriginatingSystemID+Field>,<http://ddwiki.reso.org/display/DDW/OriginatingSystemID+%28Member%29+Field>,<http://ddwiki.reso.org/display/DDW/OriginatingSystemID+%28Office%29+Field>,<http://ddwiki.reso.org/display/DDW/OriginatingSystemID+%28Contacts%29+Field>,<http://ddwiki.reso.org/display/DDW/OriginatingSystemID+%28Media%29+Field>,<http://ddwiki.reso.org/display/DDW/OriginatingSystemID+%28HistoryTransactional%29+Field>,<http://ddwiki.reso.org/display/DDW/OriginatingSystemID+%28SavedSearch%29+Field>,<http://ddwiki.reso.org/display/DDW/OriginatingSystemID+%28OpenHouse%29+Field>,<http://ddwiki.reso.org/display/DDW/OriginatingSystemID+%28Teams%29+Field> ;
  vs:term_status   "stable"
.
reso:OriginatingSystemKey a rdf:Property ;
  rdfs:comment     "The system key, a unique record identifier, from the Originating system.  The Originating system is the system with authoritative control over the record.  For example, the Multiple Listing Service where the listing was input.  There may be cases where the Source System (how you received the record) is not the Originating System.  See Source System Key for more information.","The system key, a unique record identifier, from the Originating system.  The Originating system is the system with authoritative control over the record.  For example, the Multiple Listing Service where the Saved Search was input.  There may be cases where the Source System (how you received the record) is not the Originating System.  See Source System Key for more information.","The system key, a unique record identifier, from the Originating system.  The Originating system is the system with authoritative control over the record.  For example, the Multiple Listing Service where the Open House was input.  There may be cases where the Source System (how you received the record) is not the Originating System.  See Source System Key for more information.","The system key, a unique record identifier, from the Originating system.  The Originating system is the system with authoritative control over the record.  For example, the Multiple Listing Service where the Team was input.  There may be cases where the Source System (how you received the record) is not the Originating System.  See Source System Key for more information." ;
  rdfs:domain      reso:Property,reso:SavedSearch,reso:OpenHouse,reso:Teams ;
  rdfs:label       "OriginatingSystemKey" ;
  rdfs:range       xsd:string ;
  reso:CertificationLevel "Core","Gold","Platinum" ;
  reso:PropertyTypes "RESI","RLSE","RINC","LAND","MOBI","FARM","COMS","COML","BUSO" ;
  schema:sameAs    <http://ddwiki.reso.org/display/DDW/OriginatingSystemKey+Field>,<http://ddwiki.reso.org/display/DDW/OriginatingSystemKey+%28SavedSearch%29+Field>,<http://ddwiki.reso.org/display/DDW/OriginatingSystemKey+%28OpenHouse%29+Field>,<http://ddwiki.reso.org/display/DDW/OriginatingSystemKey+%28Teams%29+Field> ;
  vs:term_status   "stable"
.
reso:OriginatingSystemName a rdf:Property ;
  rdfs:comment     "The name of the Originating record provider.  Most commonly the name of the MLS. The place where the listing is originally input by the member.  The legal name of the company.","The name of the Originating record provider.  Most commonly the name of the MLS. The place where the member is originally input by the member.  The legal name of the company.","The name of the Originating record provider.  Most commonly the name of the MLS. The place where the office is originally input by the member.  The legal name of the company.","The name of the Originating record provider.  Most commonly the name of the MLS. The place where the Contact is originally input by the member.  The legal name of the company.","The name of the Originating record provider.  Most commonly the name of the MLS. The place where the Media is originally input by the member.  The legal name of the company.","The name of the Originating record provider.  Most commonly the name of the MLS. The place where the History is originally input.  The legal name of the company.","The name of the Originating record provider.  Most commonly the name of the MLS. The place where the Saved Search is originally input.  The legal name of the company.","The name of the Originating record provider.  Most commonly the name of the MLS. The place where the Open House is originally input.  The legal name of the company.","The name of the Originating record provider.  Most commonly the name of the MLS. The place where the Team is originally input.  The legal name of the company." ;
  rdfs:domain      reso:Property,reso:Member,reso:Office,reso:Contacts,reso:Media,reso:HistoryTransactional,reso:SavedSearch,reso:OpenHouse,reso:Teams ;
  rdfs:label       "OriginatingSystemName" ;
  rdfs:range       xsd:string ;
  reso:CertificationLevel "Core","Bronze","Silver","Gold","Platinum" ;
  reso:PropertyTypes "RESI","RLSE","RINC","LAND","MOBI","FARM","COMS","COML","BUSO" ;
  schema:sameAs    <http://ddwiki.reso.org/display/DDW/OriginatingSystemName+Field>,<http://ddwiki.reso.org/display/DDW/OriginatingSystemName+%28Member%29+Field>,<http://ddwiki.reso.org/display/DDW/OriginatingSystemName+%28Office%29+Field>,<http://ddwiki.reso.org/display/DDW/OriginatingSystemName+%28Contacts%29+Field>,<http://ddwiki.reso.org/display/DDW/OriginatingSystemName+%28Media%29+Field>,<http://ddwiki.reso.org/display/DDW/OriginatingSystemName+%28HistoryTransactional%29+Field>,<http://ddwiki.reso.org/display/DDW/OriginatingSystemName+%28SavedSearch%29+Field>,<http://ddwiki.reso.org/display/DDW/OriginatingSystemName+%28OpenHouse%29+Field>,<http://ddwiki.reso.org/display/DDW/OriginatingSystemName+%28Teams%29+Field> ;
  vs:term_status   "stable"
.
reso:SocialMediaType a rdf:Property ;
  rdfs:comment     "A list of types of sites, blog, social media, the Member URL or ID is referring to.  i.e. Website, Blog, Facebook, Twitter, LinkedIn, Skype, etc.,  This list is used to populate the Type with repeating Social Media URL or ID types.","A list of types of sites, blog, social media, the Office URL or ID is referring to.  i.e. Website, Blog, Facebook, Twitter, LinkedIn, Skype, etc.,  This list is used to populate the Type with repeating Social Media URL or ID types.","A list of types of sites, blog, social media, the Team URL or ID is referring to.  i.e. Website, Blog, Facebook, Twitter, LinkedIn, Skype, etc.,  This list is used to populate the Type with repeating Social Media URL or ID types." ;
  rdfs:domain      reso:Member,reso:Office,reso:Contacts,reso:Teams ;
  rdfs:label       "SocialMediaType" ;
  rdfs:range       xsd:string ;
  reso:CertificationLevel "Bronze","Silver","Platinum" ;
  schema:sameAs    <http://ddwiki.reso.org/display/DDW/SocialMediaType+Field>,<http://ddwiki.reso.org/display/DDW/SocialMediaType+%28Office%29+Field>,<http://ddwiki.reso.org/display/DDW/SocialMediaType+%28Contacts%29+Field>,<http://ddwiki.reso.org/display/DDW/SocialMediaType+%28Teams%29+Field> ;
  vs:term_status   "stable"
.
reso:SocialMedia a rdf:Property ;
  rdfs:domain      reso:Member,reso:Office,reso:Contacts,reso:Teams ;
  rdfs:label       "SocialMedia" ;
  rdfs:range       xsd:string ;
  reso:CertificationLevel "Bronze","Silver","Platinum" ;
  schema:sameAs    <http://ddwiki.reso.org/display/DDW/SocialMedia%5BType%5DUrlOrId+Field>,<http://ddwiki.reso.org/display/DDW/SocialMedia%5BType%5DUrlOrId+%28Office%29+Field>,<http://ddwiki.reso.org/display/DDW/SocialMedia%5BType%5DUrlOrId+%28Contacts%29+Field>,<http://ddwiki.reso.org/display/DDW/SocialMedia%5BType%5DUrlOrId+%28Teams%29+Field> ;
  vs:term_status   "stable"
.
reso:SourceSystemID a rdf:Property ;
  rdfs:comment     "The RESO OUID's OrganizationUniqueId of the Source record provider. The source system is the system from which the record was directly received. In cases where the source system was not where the record originated (the authoritative system), see the Originating System fields.","The RESO OUID's OrganizationUniqueId of the Source record provider.  The source system is the system from which the record was directly received.  In cases where the source system was not where the record originated (the authoritative system), see the Originating System fields." ;
  rdfs:domain      reso:Property,reso:Member,reso:Office,reso:Contacts,reso:Media,reso:HistoryTransactional,reso:SavedSearch,reso:OpenHouse,reso:Teams ;
  rdfs:label       "SourceSystemID" ;
  rdfs:range       xsd:string ;
  reso:CertificationLevel "Platinum" ;
  reso:PropertyTypes "RESI","RLSE","RINC","LAND","MOBI","FARM","COMS","COML","BUSO" ;
  schema:sameAs    <http://ddwiki.reso.org/display/DDW/SourceSystemID+Field>,<http://ddwiki.reso.org/display/DDW/SourceSystemID+%28Member%29+Field>,<http://ddwiki.reso.org/display/DDW/SourceSystemID+%28Office%29+Field>,<http://ddwiki.reso.org/display/DDW/SourceSystemID+%28Contacts%29+Field>,<http://ddwiki.reso.org/display/DDW/SourceSystemID+%28Media%29+Field>,<http://ddwiki.reso.org/display/DDW/SourceSystemID+%28HistoryTransactional%29+Field>,<http://ddwiki.reso.org/display/DDW/SourceSystemID+%28SavedSearch%29+Field>,<http://ddwiki.reso.org/display/DDW/SourceSystemID+%28OpenHouse%29+Field>,<http://ddwiki.reso.org/display/DDW/SourceSystemID+%28Teams%29+Field> ;
  vs:term_status   "stable"
.
reso:SourceSystemKey a rdf:Property ;
  rdfs:comment     "The system key, a unique record identifier, from the Source System. The Source System is the system from which the record was directly received. In cases where the Source System was not where the record originated (the authoritative system), see the Originating System fields.","The system key, a unique record identifier, from the Source System.  The Source System is the system from which the record was directly received.  In cases where the Source System was not where the record originated (the authoritative system), see the Originating System fields." ;
  rdfs:domain      reso:Property,reso:SavedSearch,reso:OpenHouse,reso:Teams ;
  rdfs:label       "SourceSystemKey" ;
  rdfs:range       xsd:string ;
  reso:CertificationLevel "Core","Silver" ;
  reso:PropertyTypes "RESI","RLSE","RINC","LAND","MOBI","FARM","COMS","COML","BUSO" ;
  schema:sameAs    <http://ddwiki.reso.org/display/DDW/SourceSystemKey+Field>,<http://ddwiki.reso.org/display/DDW/SourceSystemKey+%28SavedSearch%29+Field>,<http://ddwiki.reso.org/display/DDW/SourceSystemKey+%28OpenHouse%29+Field>,<http://ddwiki.reso.org/display/DDW/SourceSystemKey+%28Teams%29+Field> ;
  vs:term_status   "stable"
.
reso:SourceSystemName a rdf:Property ;
  rdfs:comment     "The name of the immediate record provider. The system from which the record was directly received. The legal name of the company.","The name of the immediate record provider.  The system from which the record was directly received.  The legal name of the company.","The name of the History record provider.  The system from which the record was directly received.  The legal name of the company.","The name of the Saved Search record provider.  The system from which the record was directly received.  The legal name of the company.","The name of the Open House record provider.  The system from which the record was directly received.  The legal name of the company.","The name of the Team record provider.  The system from which the record was directly received.  The legal name of the company." ;
  rdfs:domain      reso:Property,reso:Member,reso:Office,reso:Contacts,reso:Media,reso:HistoryTransactional,reso:SavedSearch,reso:OpenHouse,reso:Teams ;
  rdfs:label       "SourceSystemName" ;
  rdfs:range       xsd:string ;
  reso:CertificationLevel "Core","Silver" ;
  reso:PropertyTypes "RESI","RLSE","RINC","LAND","MOBI","FARM","COMS","COML","BUSO" ;
  schema:sameAs    <http://ddwiki.reso.org/display/DDW/SourceSystemName+Field>,<http://ddwiki.reso.org/display/DDW/SourceSystemName+%28Member%29+Field>,<http://ddwiki.reso.org/display/DDW/SourceSystemName+%28Office%29+Field>,<http://ddwiki.reso.org/display/DDW/SourceSystemName+%28Contacts%29+Field>,<http://ddwiki.reso.org/display/DDW/SourceSystemName+%28Media%29+Field>,<http://ddwiki.reso.org/display/DDW/SourceSystemName+%28HistoryTransactional%29+Field>,<http://ddwiki.reso.org/display/DDW/SourceSystemName+%28SavedSearch%29+Field>,<http://ddwiki.reso.org/display/DDW/SourceSystemName+%28OpenHouse%29+Field>,<http://ddwiki.reso.org/display/DDW/SourceSystemName+%28Teams%29+Field> ;
  vs:term_status   "stable"
.
reso:TeamAddress1 a rdf:Property ;
  rdfs:comment     "The street number, direction, name and suffix of the Team." ;
  rdfs:domain      reso:Teams ;
  rdfs:label       "TeamAddress1" ;
  rdfs:range       xsd:string ;
  reso:CertificationLevel "Platinum" ;
  schema:sameAs    <http://ddwiki.reso.org/display/DDW/TeamAddress1+Field> ;
  vs:term_status   "stable"
.
reso:TeamAddress2 a rdf:Property ;
  rdfs:comment     "The unit/suite number of the Team." ;
  rdfs:domain      reso:Teams ;
  rdfs:label       "TeamAddress2" ;
  rdfs:range       xsd:string ;
  reso:CertificationLevel "Platinum" ;
  schema:sameAs    <http://ddwiki.reso.org/display/DDW/TeamAddress2+Field> ;
  vs:term_status   "stable"
.
reso:TeamCarrierRoute a rdf:Property ;
  rdfs:domain      reso:Teams ;
  rdfs:label       "TeamCarrierRoute" ;
  rdfs:range       xsd:string ;
  reso:CertificationLevel "Platinum" ;
  schema:sameAs    <http://ddwiki.reso.org/display/DDW/TeamCarrierRoute+Field> ;
  vs:term_status   "stable"
.
reso:TeamCity a rdf:Property ;
  rdfs:comment     "The city of the Team." ;
  rdfs:domain      reso:Teams ;
  rdfs:label       "TeamCity" ;
  rdfs:range       xsd:string ;
  reso:CertificationLevel "Platinum" ;
  schema:sameAs    <http://ddwiki.reso.org/display/DDW/TeamCity+Field> ;
  vs:term_status   "stable"
.
reso:TeamCountry a rdf:Property ;
  rdfs:comment     "The country abbreviation in a postal address." ;
  rdfs:domain      reso:Teams ;
  rdfs:label       "TeamCountry" ;
  rdfs:range       enum:Country ;
  reso:CertificationLevel "Platinum" ;
  schema:sameAs    <http://ddwiki.reso.org/display/DDW/TeamCountry+Field> ;
  vs:term_status   "stable"
.
reso:TeamCountyOrParish a rdf:Property ;
  rdfs:comment     "The county or parish in which the Team is addressed." ;
  rdfs:domain      reso:Teams ;
  rdfs:label       "TeamCountyOrParish" ;
  rdfs:range       xsd:string ;
  reso:CertificationLevel "Platinum" ;
  schema:sameAs    <http://ddwiki.reso.org/display/DDW/TeamCountyOrParish+Field> ;
  vs:term_status   "stable"
.
reso:TeamDescription a rdf:Property ;
  rdfs:comment     "A description or marketing information about the team." ;
  rdfs:domain      reso:Teams ;
  rdfs:label       "TeamDescription" ;
  rdfs:range       xsd:string ;
  reso:CertificationLevel "Platinum" ;
  schema:sameAs    <http://ddwiki.reso.org/display/DDW/TeamDescription+Field> ;
  vs:term_status   "stable"
.
reso:TeamDirectPhone a rdf:Property ;
  rdfs:comment     "North American 10 digit phone numbers should be in the format of ###-###-#### (separated by hyphens).  Other conventions should use the common local standard.  International numbers should be preceded by a plus symbol." ;
  rdfs:domain      reso:Teams ;
  rdfs:label       "TeamDirectPhone" ;
  rdfs:range       xsd:string ;
  reso:CertificationLevel "Platinum" ;
  schema:sameAs    <http://ddwiki.reso.org/display/DDW/TeamDirectPhone+Field> ;
  vs:term_status   "stable"
.
reso:TeamEmail a rdf:Property ;
  rdfs:comment     "The email address of the Team." ;
  rdfs:domain      reso:Teams ;
  rdfs:label       "TeamEmail" ;
  rdfs:range       xsd:string ;
  reso:CertificationLevel "Platinum" ;
  schema:sameAs    <http://ddwiki.reso.org/display/DDW/TeamEmail+Field> ;
  vs:term_status   "stable"
.
reso:TeamFax a rdf:Property ;
  rdfs:comment     "North American 10 digit phone numbers should be in the format of ###-###-#### (separated by hyphens).  Other conventions should use the common local standard.  International numbers should be preceded by a plus symbol." ;
  rdfs:domain      reso:Teams ;
  rdfs:label       "TeamFax" ;
  rdfs:range       xsd:string ;
  reso:CertificationLevel "Platinum" ;
  schema:sameAs    <http://ddwiki.reso.org/display/DDW/TeamFax+Field> ;
  vs:term_status   "stable"
.
reso:TeamKey a rdf:Property ;
  rdfs:comment     "A system unique identifier. Specifically, in aggregation systems, the TeamKey is the system unique identifier from the system that the record was retrieved." ;
  rdfs:domain      reso:Teams ;
  rdfs:label       "TeamKey" ;
  rdfs:range       xsd:string ;
  reso:CertificationLevel "Platinum" ;
  schema:sameAs    <http://ddwiki.reso.org/display/DDW/TeamKey+Field> ;
  vs:term_status   "stable"
.
reso:TeamKeyNumeric a rdf:Property ;
  rdfs:comment     "A system unique identifier. Specifically, in aggregation systems, the TeamKey is the system unique identifier from the system that the record was retrieved.  This is the numeric only key and used as an alternative to the TeamKey field." ;
  rdfs:domain      reso:Teams ;
  rdfs:label       "TeamKeyNumeric" ;
  rdfs:range       xsd:decimal ;
  reso:CertificationLevel "Platinum" ;
  schema:sameAs    <http://ddwiki.reso.org/display/DDW/TeamKeyNumeric+Field> ;
  vs:term_status   "stable"
.
reso:TeamLeadKey a rdf:Property ;
  rdfs:comment     "The unique system identifier of the team's lead member." ;
  rdfs:domain      reso:Teams ;
  rdfs:label       "TeamLeadKey" ;
  rdfs:range       xsd:string ;
  reso:CertificationLevel "Platinum" ;
  schema:sameAs    <http://ddwiki.reso.org/display/DDW/TeamLeadKey+Field> ;
  vs:term_status   "stable"
.
reso:TeamLeadKeyNumeric a rdf:Property ;
  rdfs:comment     "The unique system identifier of the team's lead member.  This is the numeric only key and used as an alternative to the TeamLeadKey field." ;
  rdfs:domain      reso:Teams ;
  rdfs:label       "TeamLeadKeyNumeric" ;
  rdfs:range       xsd:decimal ;
  reso:CertificationLevel "Platinum" ;
  schema:sameAs    <http://ddwiki.reso.org/display/DDW/TeamLeadKeyNumeric+Field> ;
  vs:term_status   "stable"
.
reso:TeamLeadLoginId a rdf:Property ;
  rdfs:comment     "The ID used to logon to the MLS system." ;
  rdfs:domain      reso:Teams ;
  rdfs:label       "TeamLeadLoginId" ;
  rdfs:range       xsd:string ;
  reso:CertificationLevel "Platinum" ;
  schema:sameAs    <http://ddwiki.reso.org/display/DDW/TeamLeadLoginId+Field> ;
  vs:term_status   "stable"
.
reso:TeamLeadMlsId a rdf:Property ;
  rdfs:comment     "The local, well-known identifier for the Team Lead. This value may not be unique, specifically in the case of aggregation systems, this value should be the identifier from the original system." ;
  rdfs:domain      reso:Teams ;
  rdfs:label       "TeamLeadMlsId" ;
  rdfs:range       xsd:string ;
  reso:CertificationLevel "Platinum" ;
  schema:sameAs    <http://ddwiki.reso.org/display/DDW/TeamLeadMlsId+Field> ;
  vs:term_status   "stable"
.
reso:TeamLeadNationalAssociationId a rdf:Property ;
  rdfs:comment     "The national association ID of the team lead.  i.e. in the U.S. is the NRDS number." ;
  rdfs:domain      reso:Teams ;
  rdfs:label       "TeamLeadNationalAssociationId" ;
  rdfs:range       xsd:string ;
  reso:CertificationLevel "Platinum" ;
  schema:sameAs    <http://ddwiki.reso.org/display/DDW/TeamLeadNationalAssociationId+Field> ;
  vs:term_status   "stable"
.
reso:TeamLeadStateLicense a rdf:Property ;
  rdfs:comment     "The license of the Team Lead. Separate multiple licenses with a comma and space." ;
  rdfs:domain      reso:Teams ;
  rdfs:label       "TeamLeadStateLicense" ;
  rdfs:range       xsd:string ;
  reso:CertificationLevel "Platinum" ;
  schema:sameAs    <http://ddwiki.reso.org/display/DDW/TeamLeadStateLicense+Field> ;
  vs:term_status   "stable"
.
reso:TeamLeadStateLicenseState a rdf:Property ;
  rdfs:comment     "The state in which the Team Lead is licensed." ;
  rdfs:domain      reso:Teams ;
  rdfs:label       "TeamLeadStateLicenseState" ;
  rdfs:range       enum:StateOrProvince ;
  reso:CertificationLevel "Platinum" ;
  schema:sameAs    <http://ddwiki.reso.org/display/DDW/TeamLeadStateLicenseState+Field> ;
  vs:term_status   "stable"
.
reso:TeamMobilePhone a rdf:Property ;
  rdfs:comment     "North American 10 digit phone numbers should be in the format of ###-###-#### (separated by hyphens).  Other conventions should use the common local standard.  International numbers should be preceded by a plus symbol." ;
  rdfs:domain      reso:Teams ;
  rdfs:label       "TeamMobilePhone" ;
  rdfs:range       xsd:string ;
  reso:CertificationLevel "Platinum" ;
  schema:sameAs    <http://ddwiki.reso.org/display/DDW/TeamMobilePhone+Field> ;
  vs:term_status   "stable"
.
reso:TeamName a rdf:Property ;
  rdfs:comment     "The name under which the team operates.  If a business this may be a DBA." ;
  rdfs:domain      reso:Teams ;
  rdfs:label       "TeamName" ;
  rdfs:range       xsd:string ;
  reso:CertificationLevel "Platinum" ;
  schema:sameAs    <http://ddwiki.reso.org/display/DDW/TeamName+Field> ;
  vs:term_status   "stable"
.
reso:TeamOfficePhone a rdf:Property ;
  rdfs:comment     "North American 10 digit phone numbers should be in the format of ###-###-#### (separated by hyphens).  Other conventions should use the common local standard.  International numbers should be preceded by a plus symbol." ;
  rdfs:domain      reso:Teams ;
  rdfs:label       "TeamOfficePhone" ;
  rdfs:range       xsd:string ;
  reso:CertificationLevel "Platinum" ;
  schema:sameAs    <http://ddwiki.reso.org/display/DDW/TeamOfficePhone+Field> ;
  vs:term_status   "stable"
.
reso:TeamOfficePhoneExt a rdf:Property ;
  rdfs:comment     "The extension of the given phone number (if applicable)." ;
  rdfs:domain      reso:Teams ;
  rdfs:label       "TeamOfficePhoneExt" ;
  rdfs:range       xsd:string ;
  reso:CertificationLevel "Platinum" ;
  schema:sameAs    <http://ddwiki.reso.org/display/DDW/TeamOfficePhoneExt+Field> ;
  vs:term_status   "stable"
.
reso:TeamPostalCode a rdf:Property ;
  rdfs:comment     "The postal code of the Team." ;
  rdfs:domain      reso:Teams ;
  rdfs:label       "TeamPostalCode" ;
  rdfs:range       xsd:string ;
  reso:CertificationLevel "Platinum" ;
  schema:sameAs    <http://ddwiki.reso.org/display/DDW/TeamPostalCode+Field> ;
  vs:term_status   "stable"
.
reso:TeamPostalCodePlus4 a rdf:Property ;
  rdfs:comment     "The extension of the postal/zip code.  i.e. +4" ;
  rdfs:domain      reso:Teams ;
  rdfs:label       "TeamPostalCodePlus4" ;
  rdfs:range       xsd:string ;
  reso:CertificationLevel "Platinum" ;
  schema:sameAs    <http://ddwiki.reso.org/display/DDW/TeamPostalCodePlus4+Field> ;
  vs:term_status   "stable"
.
reso:TeamPreferredPhone a rdf:Property ;
  rdfs:comment     "North American 10 digit phone numbers should be in the format of ###-###-#### (separated by hyphens).  Other conventions should use the common local standard.  International numbers should be preceded by a plus symbol." ;
  rdfs:domain      reso:Teams ;
  rdfs:label       "TeamPreferredPhone" ;
  rdfs:range       xsd:string ;
  reso:CertificationLevel "Platinum" ;
  schema:sameAs    <http://ddwiki.reso.org/display/DDW/TeamPreferredPhone+Field> ;
  vs:term_status   "stable"
.
reso:TeamPreferredPhoneExt a rdf:Property ;
  rdfs:comment     "The extension of the given phone number (if applicable)." ;
  rdfs:domain      reso:Teams ;
  rdfs:label       "TeamPreferredPhoneExt" ;
  rdfs:range       xsd:string ;
  reso:CertificationLevel "Platinum" ;
  schema:sameAs    <http://ddwiki.reso.org/display/DDW/TeamPreferredPhoneExt+Field> ;
  vs:term_status   "stable"
.
reso:TeamStateOrProvince a rdf:Property ;
  rdfs:comment     "The state or province in which the Team is addressed." ;
  rdfs:domain      reso:Teams ;
  rdfs:label       "TeamStateOrProvince" ;
  rdfs:range       enum:StateOrProvince ;
  reso:CertificationLevel "Platinum" ;
  schema:sameAs    <http://ddwiki.reso.org/display/DDW/TeamStateOrProvince+Field> ;
  vs:term_status   "stable"
.
reso:TeamStatus a rdf:Property ;
  rdfs:comment     "Is the account active, inactive or under disciplinary action." ;
  rdfs:domain      reso:Teams ;
  rdfs:label       "TeamStatus" ;
  rdfs:range       enum:TeamStatus ;
  reso:CertificationLevel "Platinum" ;
  schema:sameAs    <http://ddwiki.reso.org/display/DDW/TeamStatus+Field> ;
  vs:term_status   "stable"
.
reso:TeamTollFreePhone a rdf:Property ;
  rdfs:comment     "North American 10 digit phone numbers should be in the format of ###-###-#### (separated by hyphens).  Other conventions should use the common local standard.  International numbers should be preceded by a plus symbol." ;
  rdfs:domain      reso:Teams ;
  rdfs:label       "TeamTollFreePhone" ;
  rdfs:range       xsd:string ;
  reso:CertificationLevel "Platinum" ;
  schema:sameAs    <http://ddwiki.reso.org/display/DDW/TeamTollFreePhone+Field> ;
  vs:term_status   "stable"
.
reso:TeamVoiceMail a rdf:Property ;
  rdfs:comment     "North American 10 digit phone numbers should be in the format of ###-###-#### (separated by hyphens).  Other conventions should use the common local standard.  International numbers should be preceded by a plus symbol." ;
  rdfs:domain      reso:Teams ;
  rdfs:label       "TeamVoiceMail" ;
  rdfs:range       xsd:string ;
  reso:CertificationLevel "Platinum" ;
  schema:sameAs    <http://ddwiki.reso.org/display/DDW/TeamVoiceMail+Field> ;
  vs:term_status   "stable"
.
reso:TeamVoiceMailExt a rdf:Property ;
  rdfs:comment     "The extension of the given phone number (if applicable)." ;
  rdfs:domain      reso:Teams ;
  rdfs:label       "TeamVoiceMailExt" ;
  rdfs:range       xsd:string ;
  reso:CertificationLevel "Platinum" ;
  schema:sameAs    <http://ddwiki.reso.org/display/DDW/TeamVoiceMailExt+Field> ;
  vs:term_status   "stable"
.
reso:MemberKey a rdf:Property ;
  rdfs:comment     "A unique identifier for this record from the immediate source. This is a string that can include URI or other forms.  Alternatively use the MemberKeyNumeric for a numeric only key field.  This is the local key of the system.  When records are received from other systems, a local key is commonly applied.  If conveying the original keys from the source or originating systems, see SourceSystemMemberKey and OriginatingSystemMemberKey.","A system unique identifier. Specifically, in aggregation systems, the MemberKey is the system unique identifier from the system that the record was retrieved. This may be identical to the related xxxId.  This is a foreign key relating to the Member resource's MemberKey.","A system unique identifier. Specifically, the foreign key relating to the Member resource's MemberKey." ;
  rdfs:domain      reso:Member,reso:SavedSearch,reso:TeamMembers ;
  rdfs:label       "MemberKey" ;
  rdfs:range       xsd:string ;
  reso:CertificationLevel "Core","Gold","Platinum" ;
  schema:sameAs    <http://ddwiki.reso.org/display/DDW/MemberKey+Field>,<http://ddwiki.reso.org/display/DDW/MemberKey+%28SavedSearch%29+Field>,<http://ddwiki.reso.org/display/DDW/MemberKey+%28TeamMembers%29+Field> ;
  vs:term_status   "stable"
.
reso:MemberKeyNumeric a rdf:Property ;
  rdfs:comment     "A unique identifier for this record from the immediate source. This is the numeric only key and used as an alternative to the MemberKey fields.  This is the local key of the system.  When records are received from other systems, a local key is commonly applied.  If conveying the original keys from the source or originating systems, see SourceSystemMemberKey and OriginatingSystemMemberKey.","A system unique identifier. Specifically, in aggregation systems, the MemberKey is the system unique identifier from the system that the record was retrieved. This may be identical to the related xxxId.  This is a foreign key relating to the Member resource's MemberKey.  This is the numeric only key and used as an alternative to the MemberKey field.","A system unique identifier. Specifically, the foreign key relating to the Member resource's MemberKey.  This is the numeric only key and used as an alternative to the MemberKey field." ;
  rdfs:domain      reso:Member,reso:SavedSearch,reso:TeamMembers ;
  rdfs:label       "MemberKeyNumeric" ;
  rdfs:range       xsd:decimal ;
  reso:CertificationLevel "Platinum" ;
  schema:sameAs    <http://ddwiki.reso.org/display/DDW/MemberKeyNumeric+Field>,<http://ddwiki.reso.org/display/DDW/MemberKeyNumeric+%28SavedSearch%29+Field>,<http://ddwiki.reso.org/display/DDW/MemberKeyNumeric+%28TeamMembers%29+Field> ;
  vs:term_status   "stable"
.
reso:MemberLoginId a rdf:Property ;
  rdfs:comment     "The ID used to logon to the MLS system." ;
  rdfs:domain      reso:Member,reso:TeamMembers ;
  rdfs:label       "MemberLoginId" ;
  rdfs:range       xsd:string ;
  reso:CertificationLevel "Bronze","Platinum" ;
  schema:sameAs    <http://ddwiki.reso.org/display/DDW/MemberLoginId+Field>,<http://ddwiki.reso.org/display/DDW/MemberLoginId+%28TeamMembers%29+Field> ;
  vs:term_status   "stable"
.
reso:MemberMlsId a rdf:Property ;
  rdfs:comment     "The local, well-known identifier for the member. This value may not be unique, specifically in the case of aggregation systems, this value should be the identifier from the original system." ;
  rdfs:domain      reso:Member,reso:SavedSearch,reso:TeamMembers ;
  rdfs:label       "MemberMlsId" ;
  rdfs:range       xsd:string ;
  reso:CertificationLevel "Core","Gold","Platinum" ;
  schema:sameAs    <http://ddwiki.reso.org/display/DDW/MemberMlsId+Field>,<http://ddwiki.reso.org/display/DDW/MemberMlsId+%28SavedSearch%29+Field>,<http://ddwiki.reso.org/display/DDW/MemberMlsId+%28TeamMembers%29+Field> ;
  vs:term_status   "stable"
.
reso:ModificationTimestamp a rdf:Property ;
  rdfs:comment     "The transactional timestamp automatically recorded by the MLS system representing the date/time the listing was last modified.","Date/time the roster (member or office) record was last modified.","Date/time the contact record was last modified.","The transactional timestamp automatically recorded by the MLS system representing the date/time the media record was last modified.","Timestamp of the last major change on the listing (see also MajorChangeType).","The transactional timestamp automatically recorded by the MLS system representing the date/time the Open House was last modified.","Date/time the roster (Team or office) record was last modified." ;
  rdfs:domain      reso:Property,reso:Member,reso:Office,reso:Contacts,reso:Media,reso:HistoryTransactional,reso:SavedSearch,reso:OpenHouse,reso:Teams,reso:TeamMembers ;
  rdfs:label       "ModificationTimestamp" ;
  rdfs:range       xsd:dateTime ;
  reso:CertificationLevel "Core","Silver","Gold","Platinum" ;
  reso:PropertyTypes "RESI","RLSE","RINC","LAND","MOBI","FARM","COMS","COML","BUSO" ;
  schema:sameAs    <http://ddwiki.reso.org/display/DDW/ModificationTimestamp+Field>,<http://ddwiki.reso.org/display/DDW/ModificationTimestamp+%28Member%29+Field>,<http://ddwiki.reso.org/display/DDW/ModificationTimestamp+%28Office%29+Field>,<http://ddwiki.reso.org/display/DDW/ModificationTimestamp+%28Contacts%29+Field>,<http://ddwiki.reso.org/display/DDW/ModificationTimestamp+%28Media%29+Field>,<http://ddwiki.reso.org/display/DDW/ModificationTimestamp+%28HistoryTransactional%29+Field>,<http://ddwiki.reso.org/display/DDW/ModificationTimestamp+%28SavedSearch%29+Field>,<http://ddwiki.reso.org/display/DDW/ModificationTimestamp+%28OpenHouse%29+Field>,<http://ddwiki.reso.org/display/DDW/ModificationTimestamp+%28Teams%29+Field>,<http://ddwiki.reso.org/display/DDW/ModificationTimestamp+%28TeamMembers%29+Field> ;
  vs:term_status   "stable"
.
reso:OriginalEntryTimestamp a rdf:Property ;
  rdfs:comment     "The transactional timestamp automatically recorded by the MLS system representing the date/time the listing was entered and made visible to members of the MLS.","Date/time the roster (member or office) record was originally input into the source system.","Date/time the contact record was originally input into the source system.","The transactional timestamp automatically recorded by the MLS system representing the date/time the Open House was entered and made visible to members of the MLS.","Date/time the roster (Team or office) record was originally input into the source system." ;
  rdfs:domain      reso:Property,reso:Member,reso:Office,reso:Contacts,reso:SavedSearch,reso:OpenHouse,reso:Teams,reso:TeamMembers ;
  rdfs:label       "OriginalEntryTimestamp" ;
  rdfs:range       xsd:dateTime ;
  reso:CertificationLevel "Core","Silver","Gold","Bronze","Platinum" ;
  reso:PropertyTypes "RESI","RLSE","RINC","LAND","MOBI","FARM","COMS","COML","BUSO" ;
  schema:sameAs    <http://ddwiki.reso.org/display/DDW/OriginalEntryTimestamp+Field>,<http://ddwiki.reso.org/display/DDW/OriginalEntryTimestamp+%28Member%29+Field>,<http://ddwiki.reso.org/display/DDW/OriginalEntryTimestamp+%28Office%29+Field>,<http://ddwiki.reso.org/display/DDW/OriginalEntryTimestamp+%28Contacts%29+Field>,<http://ddwiki.reso.org/display/DDW/OriginalEntryTimestamp+%28SavedSearch%29+Field>,<http://ddwiki.reso.org/display/DDW/OriginalEntryTimestamp+%28OpenHouse%29+Field>,<http://ddwiki.reso.org/display/DDW/OriginalEntryTimestamp+%28Teams%29+Field>,<http://ddwiki.reso.org/display/DDW/OriginalEntryTimestamp+%28TeamMembers%29+Field> ;
  vs:term_status   "stable"
.
reso:OriginatingSystemID a rdf:Property ;
  rdfs:comment     "The RESO OUID's OrganizationUniqueId of the Originating record provider.  The Originating system is the system with authoritative control over the record.  For example; the name of the MLS where the listing was input.  In cases where the Originating system was not where the record originated (the authoritative system), see the Originating System fields.","The RESO OUID's OrganizationUniqueId of the Originating record provider.  The Originating system is the system with authoritative control over the record.  For example; the name of the MLS where the member was input.  In cases where the Originating system was not where the record originated (the authoritative system), see the Originating System fields.","The RESO OUID's OrganizationUniqueId of the Originating record provider.  The Originating system is the system with authoritative control over the record.  For example; the name of the MLS where the office was input.  In cases where the Originating system was not where the record originated (the authoritative system), see the Originating System fields.","The RESO OUID's OrganizationUniqueId of the Originating record provider.  The Originating system is the system with authoritative control over the record.  For example; the name of the MLS where the Contact was input.  In cases where the Originating system was not where the record originated (the authoritative system), see the Originating System fields.","The RESO OUID's OrganizationUniqueId of the Originating record provider.  The Originating system is the system with authoritative control over the record.  For example; the name of the MLS where the Media was input.  In cases where the Originating system was not where the record originated (the authoritative system), see the Originating System fields.","The RESO OUID's OrganizationUniqueId of the Originating record provider.  The Originating system is the system with authoritative control over the record.  For example; the name of the MLS where the History was input.  In cases where the Originating system was not where the record originated (the authoritative system), see the Originating System fields.","The RESO OUID's OrganizationUniqueId of the Originating record provider.  The Originating system is the system with authoritative control over the record.  For example; the name of the MLS where the Saved Search was input.  In cases where the Originating system was not where the record originated (the authoritative system), see the Originating System fields.","The RESO OUID's OrganizationUniqueId of the Originating record provider.  The Originating system is the system with authoritative control over the record.  For example; the name of the MLS where the Open House was input.  In cases where the Originating system was not where the record originated (the authoritative system), see the Originating System fields.","The RESO OUID's OrganizationUniqueId of the Originating record provider.  The Originating system is the system with authoritative control over the record.  For example; the name of the MLS where the Team was input.  In cases where the Originating system was not where the record originated (the authoritative system), see the Originating System fields.","The RESO OUID's OrganizationUniqueId of the Originating record provider.  The Originating system is the system with authoritative control over the record.  For example; the name of the MLS where the Team Member was input.  In cases where the Originating system was not where the record originated (the authoritative system), see the Originating System fields." ;
  rdfs:domain      reso:Property,reso:Member,reso:Office,reso:Contacts,reso:Media,reso:HistoryTransactional,reso:SavedSearch,reso:OpenHouse,reso:Teams,reso:TeamMembers ;
  rdfs:label       "OriginatingSystemID" ;
  rdfs:range       xsd:string ;
  reso:CertificationLevel "Platinum" ;
  reso:PropertyTypes "RESI","RLSE","RINC","LAND","MOBI","FARM","COMS","COML","BUSO" ;
  schema:sameAs    <http://ddwiki.reso.org/display/DDW/OriginatingSystemID+Field>,<http://ddwiki.reso.org/display/DDW/OriginatingSystemID+%28Member%29+Field>,<http://ddwiki.reso.org/display/DDW/OriginatingSystemID+%28Office%29+Field>,<http://ddwiki.reso.org/display/DDW/OriginatingSystemID+%28Contacts%29+Field>,<http://ddwiki.reso.org/display/DDW/OriginatingSystemID+%28Media%29+Field>,<http://ddwiki.reso.org/display/DDW/OriginatingSystemID+%28HistoryTransactional%29+Field>,<http://ddwiki.reso.org/display/DDW/OriginatingSystemID+%28SavedSearch%29+Field>,<http://ddwiki.reso.org/display/DDW/OriginatingSystemID+%28OpenHouse%29+Field>,<http://ddwiki.reso.org/display/DDW/OriginatingSystemID+%28Teams%29+Field>,<http://ddwiki.reso.org/display/DDW/OriginatingSystemID+%28TeamMembers%29+Field> ;
  vs:term_status   "stable"
.
reso:OriginatingSystemKey a rdf:Property ;
  rdfs:comment     "The system key, a unique record identifier, from the Originating system.  The Originating system is the system with authoritative control over the record.  For example, the Multiple Listing Service where the listing was input.  There may be cases where the Source System (how you received the record) is not the Originating System.  See Source System Key for more information.","The system key, a unique record identifier, from the Originating system.  The Originating system is the system with authoritative control over the record.  For example, the Multiple Listing Service where the Saved Search was input.  There may be cases where the Source System (how you received the record) is not the Originating System.  See Source System Key for more information.","The system key, a unique record identifier, from the Originating system.  The Originating system is the system with authoritative control over the record.  For example, the Multiple Listing Service where the Open House was input.  There may be cases where the Source System (how you received the record) is not the Originating System.  See Source System Key for more information.","The system key, a unique record identifier, from the Originating system.  The Originating system is the system with authoritative control over the record.  For example, the Multiple Listing Service where the Team was input.  There may be cases where the Source System (how you received the record) is not the Originating System.  See Source System Key for more information.","The system key, a unique record identifier, from the Originating system.  The Originating system is the system with authoritative control over the record.  For example, the Multiple Listing Service where the Team Member was input.  There may be cases where the Source System (how you received the record) is not the Originating System.  See Source System Key for more information." ;
  rdfs:domain      reso:Property,reso:SavedSearch,reso:OpenHouse,reso:Teams,reso:TeamMembers ;
  rdfs:label       "OriginatingSystemKey" ;
  rdfs:range       xsd:string ;
  reso:CertificationLevel "Core","Gold","Platinum" ;
  reso:PropertyTypes "RESI","RLSE","RINC","LAND","MOBI","FARM","COMS","COML","BUSO" ;
  schema:sameAs    <http://ddwiki.reso.org/display/DDW/OriginatingSystemKey+Field>,<http://ddwiki.reso.org/display/DDW/OriginatingSystemKey+%28SavedSearch%29+Field>,<http://ddwiki.reso.org/display/DDW/OriginatingSystemKey+%28OpenHouse%29+Field>,<http://ddwiki.reso.org/display/DDW/OriginatingSystemKey+%28Teams%29+Field>,<http://ddwiki.reso.org/display/DDW/OriginatingSystemKey+%28TeamMembers%29+Field> ;
  vs:term_status   "stable"
.
reso:OriginatingSystemName a rdf:Property ;
  rdfs:comment     "The name of the Originating record provider.  Most commonly the name of the MLS. The place where the listing is originally input by the member.  The legal name of the company.","The name of the Originating record provider.  Most commonly the name of the MLS. The place where the member is originally input by the member.  The legal name of the company.","The name of the Originating record provider.  Most commonly the name of the MLS. The place where the office is originally input by the member.  The legal name of the company.","The name of the Originating record provider.  Most commonly the name of the MLS. The place where the Contact is originally input by the member.  The legal name of the company.","The name of the Originating record provider.  Most commonly the name of the MLS. The place where the Media is originally input by the member.  The legal name of the company.","The name of the Originating record provider.  Most commonly the name of the MLS. The place where the History is originally input.  The legal name of the company.","The name of the Originating record provider.  Most commonly the name of the MLS. The place where the Saved Search is originally input.  The legal name of the company.","The name of the Originating record provider.  Most commonly the name of the MLS. The place where the Open House is originally input.  The legal name of the company.","The name of the Originating record provider.  Most commonly the name of the MLS. The place where the Team is originally input.  The legal name of the company.","The name of the Originating record provider.  Most commonly the name of the MLS. The place where the Team Member is originally input.  The legal name of the company." ;
  rdfs:domain      reso:Property,reso:Member,reso:Office,reso:Contacts,reso:Media,reso:HistoryTransactional,reso:SavedSearch,reso:OpenHouse,reso:Teams,reso:TeamMembers ;
  rdfs:label       "OriginatingSystemName" ;
  rdfs:range       xsd:string ;
  reso:CertificationLevel "Core","Bronze","Silver","Gold","Platinum" ;
  reso:PropertyTypes "RESI","RLSE","RINC","LAND","MOBI","FARM","COMS","COML","BUSO" ;
  schema:sameAs    <http://ddwiki.reso.org/display/DDW/OriginatingSystemName+Field>,<http://ddwiki.reso.org/display/DDW/OriginatingSystemName+%28Member%29+Field>,<http://ddwiki.reso.org/display/DDW/OriginatingSystemName+%28Office%29+Field>,<http://ddwiki.reso.org/display/DDW/OriginatingSystemName+%28Contacts%29+Field>,<http://ddwiki.reso.org/display/DDW/OriginatingSystemName+%28Media%29+Field>,<http://ddwiki.reso.org/display/DDW/OriginatingSystemName+%28HistoryTransactional%29+Field>,<http://ddwiki.reso.org/display/DDW/OriginatingSystemName+%28SavedSearch%29+Field>,<http://ddwiki.reso.org/display/DDW/OriginatingSystemName+%28OpenHouse%29+Field>,<http://ddwiki.reso.org/display/DDW/OriginatingSystemName+%28Teams%29+Field>,<http://ddwiki.reso.org/display/DDW/OriginatingSystemName+%28TeamMembers%29+Field> ;
  vs:term_status   "stable"
.
reso:SourceSystemID a rdf:Property ;
  rdfs:comment     "The RESO OUID's OrganizationUniqueId of the Source record provider. The source system is the system from which the record was directly received. In cases where the source system was not where the record originated (the authoritative system), see the Originating System fields.","The RESO OUID's OrganizationUniqueId of the Source record provider.  The source system is the system from which the record was directly received.  In cases where the source system was not where the record originated (the authoritative system), see the Originating System fields." ;
  rdfs:domain      reso:Property,reso:Member,reso:Office,reso:Contacts,reso:Media,reso:HistoryTransactional,reso:SavedSearch,reso:OpenHouse,reso:Teams,reso:TeamMembers ;
  rdfs:label       "SourceSystemID" ;
  rdfs:range       xsd:string ;
  reso:CertificationLevel "Platinum" ;
  reso:PropertyTypes "RESI","RLSE","RINC","LAND","MOBI","FARM","COMS","COML","BUSO" ;
  schema:sameAs    <http://ddwiki.reso.org/display/DDW/SourceSystemID+Field>,<http://ddwiki.reso.org/display/DDW/SourceSystemID+%28Member%29+Field>,<http://ddwiki.reso.org/display/DDW/SourceSystemID+%28Office%29+Field>,<http://ddwiki.reso.org/display/DDW/SourceSystemID+%28Contacts%29+Field>,<http://ddwiki.reso.org/display/DDW/SourceSystemID+%28Media%29+Field>,<http://ddwiki.reso.org/display/DDW/SourceSystemID+%28HistoryTransactional%29+Field>,<http://ddwiki.reso.org/display/DDW/SourceSystemID+%28SavedSearch%29+Field>,<http://ddwiki.reso.org/display/DDW/SourceSystemID+%28OpenHouse%29+Field>,<http://ddwiki.reso.org/display/DDW/SourceSystemID+%28Teams%29+Field>,<http://ddwiki.reso.org/display/DDW/SourceSystemID+%28TeamMembers%29+Field> ;
  vs:term_status   "stable"
.
reso:SourceSystemKey a rdf:Property ;
  rdfs:comment     "The system key, a unique record identifier, from the Source System. The Source System is the system from which the record was directly received. In cases where the Source System was not where the record originated (the authoritative system), see the Originating System fields.","The system key, a unique record identifier, from the Source System.  The Source System is the system from which the record was directly received.  In cases where the Source System was not where the record originated (the authoritative system), see the Originating System fields." ;
  rdfs:domain      reso:Property,reso:SavedSearch,reso:OpenHouse,reso:Teams,reso:TeamMembers ;
  rdfs:label       "SourceSystemKey" ;
  rdfs:range       xsd:string ;
  reso:CertificationLevel "Core","Silver" ;
  reso:PropertyTypes "RESI","RLSE","RINC","LAND","MOBI","FARM","COMS","COML","BUSO" ;
  schema:sameAs    <http://ddwiki.reso.org/display/DDW/SourceSystemKey+Field>,<http://ddwiki.reso.org/display/DDW/SourceSystemKey+%28SavedSearch%29+Field>,<http://ddwiki.reso.org/display/DDW/SourceSystemKey+%28OpenHouse%29+Field>,<http://ddwiki.reso.org/display/DDW/SourceSystemKey+%28Teams%29+Field>,<http://ddwiki.reso.org/display/DDW/SourceSystemKey+%28TeamMembers%29+Field> ;
  vs:term_status   "stable"
.
reso:SourceSystemName a rdf:Property ;
  rdfs:comment     "The name of the immediate record provider. The system from which the record was directly received. The legal name of the company.","The name of the immediate record provider.  The system from which the record was directly received.  The legal name of the company.","The name of the History record provider.  The system from which the record was directly received.  The legal name of the company.","The name of the Saved Search record provider.  The system from which the record was directly received.  The legal name of the company.","The name of the Open House record provider.  The system from which the record was directly received.  The legal name of the company.","The name of the Team record provider.  The system from which the record was directly received.  The legal name of the company.","The name of the Team Member record provider.  The system from which the record was directly received.  The legal name of the company." ;
  rdfs:domain      reso:Property,reso:Member,reso:Office,reso:Contacts,reso:Media,reso:HistoryTransactional,reso:SavedSearch,reso:OpenHouse,reso:Teams,reso:TeamMembers ;
  rdfs:label       "SourceSystemName" ;
  rdfs:range       xsd:string ;
  reso:CertificationLevel "Core","Silver" ;
  reso:PropertyTypes "RESI","RLSE","RINC","LAND","MOBI","FARM","COMS","COML","BUSO" ;
  schema:sameAs    <http://ddwiki.reso.org/display/DDW/SourceSystemName+Field>,<http://ddwiki.reso.org/display/DDW/SourceSystemName+%28Member%29+Field>,<http://ddwiki.reso.org/display/DDW/SourceSystemName+%28Office%29+Field>,<http://ddwiki.reso.org/display/DDW/SourceSystemName+%28Contacts%29+Field>,<http://ddwiki.reso.org/display/DDW/SourceSystemName+%28Media%29+Field>,<http://ddwiki.reso.org/display/DDW/SourceSystemName+%28HistoryTransactional%29+Field>,<http://ddwiki.reso.org/display/DDW/SourceSystemName+%28SavedSearch%29+Field>,<http://ddwiki.reso.org/display/DDW/SourceSystemName+%28OpenHouse%29+Field>,<http://ddwiki.reso.org/display/DDW/SourceSystemName+%28Teams%29+Field>,<http://ddwiki.reso.org/display/DDW/SourceSystemName+%28TeamMembers%29+Field> ;
  vs:term_status   "stable"
.
reso:TeamImpersonationLevel a rdf:Property ;
  rdfs:comment     "The level of impersonation the member is allowed within the team.  i.e. Impersonate (to work as the team), On Behalf (to show the team name, but also show the member's info, None (don't allow this member to appear as part of team)." ;
  rdfs:domain      reso:TeamMembers ;
  rdfs:label       "TeamImpersonationLevel" ;
  rdfs:range       xsd:string ;
  reso:CertificationLevel "Platinum" ;
  schema:sameAs    <http://ddwiki.reso.org/display/DDW/TeamImpersonationLevel+Field> ;
  vs:term_status   "stable"
.
reso:TeamKey a rdf:Property ;
  rdfs:comment     "A system unique identifier. Specifically, in aggregation systems, the TeamKey is the system unique identifier from the system that the record was retrieved.","A system unique identifier. Specifically, a foreign key referencing the Teams resource's primary key." ;
  rdfs:domain      reso:Teams,reso:TeamMembers ;
  rdfs:label       "TeamKey" ;
  rdfs:range       xsd:string ;
  reso:CertificationLevel "Platinum" ;
  schema:sameAs    <http://ddwiki.reso.org/display/DDW/TeamKey+Field>,<http://ddwiki.reso.org/display/DDW/TeamKey+%28TeamMembers%29+Field> ;
  vs:term_status   "stable"
.
reso:TeamKeyNumeric a rdf:Property ;
  rdfs:comment     "A system unique identifier. Specifically, in aggregation systems, the TeamKey is the system unique identifier from the system that the record was retrieved.  This is the numeric only key and used as an alternative to the TeamKey field.","A system unique identifier. Specifically, a foreign key referencing the Teams resource's primary key.  This is the numeric only key and used as an alternative to the TeamKey field." ;
  rdfs:domain      reso:Teams,reso:TeamMembers ;
  rdfs:label       "TeamKeyNumeric" ;
  rdfs:range       xsd:decimal ;
  reso:CertificationLevel "Platinum" ;
  schema:sameAs    <http://ddwiki.reso.org/display/DDW/TeamKeyNumeric+Field>,<http://ddwiki.reso.org/display/DDW/TeamKeyNumeric+%28TeamMembers%29+Field> ;
  vs:term_status   "stable"
.
reso:TeamMemberKey a rdf:Property ;
  rdfs:comment     "A system unique identifier. Specifically, the local key to the TeamMembers resource." ;
  rdfs:domain      reso:TeamMembers ;
  rdfs:label       "TeamMemberKey" ;
  rdfs:range       xsd:string ;
  reso:CertificationLevel "Platinum" ;
  schema:sameAs    <http://ddwiki.reso.org/display/DDW/TeamMemberKey+Field> ;
  vs:term_status   "stable"
.
reso:TeamMemberKeyNumeric a rdf:Property ;
  rdfs:comment     "A system unique identifier. Specifically, the local key to the TeamMembers resource.  This is the numeric only key and used as an alternative to the TeamKey field." ;
  rdfs:domain      reso:TeamMembers ;
  rdfs:label       "TeamMemberKeyNumeric" ;
  rdfs:range       xsd:decimal ;
  reso:CertificationLevel "Platinum" ;
  schema:sameAs    <http://ddwiki.reso.org/display/DDW/TeamMemberKeyNumeric+Field> ;
  vs:term_status   "stable"
.
reso:TeamMemberNationalAssociationId a rdf:Property ;
  rdfs:comment     "The national association ID of the member.  i.e. in the U.S. is the NRDS number." ;
  rdfs:domain      reso:TeamMembers ;
  rdfs:label       "TeamMemberNationalAssociationId" ;
  rdfs:range       xsd:string ;
  reso:CertificationLevel "Platinum" ;
  schema:sameAs    <http://ddwiki.reso.org/display/DDW/TeamMemberNationalAssociationId+Field> ;
  vs:term_status   "stable"
.
reso:TeamMemberStateLicense a rdf:Property ;
  rdfs:comment     "The license of the member. Separate multiple licenses with a comma and space." ;
  rdfs:domain      reso:TeamMembers ;
  rdfs:label       "TeamMemberStateLicense" ;
  rdfs:range       xsd:string ;
  reso:CertificationLevel "Platinum" ;
  schema:sameAs    <http://ddwiki.reso.org/display/DDW/TeamMemberStateLicense+Field> ;
  vs:term_status   "stable"
.
reso:TeamMemberType a rdf:Property ;
  rdfs:comment     "The role of the member within the team.  i.e. team lead, principle, associate, assistant, etc." ;
  rdfs:domain      reso:TeamMembers ;
  rdfs:label       "TeamMemberType" ;
  rdfs:range       enum:MemberType ;
  reso:CertificationLevel "Platinum" ;
  schema:sameAs    <http://ddwiki.reso.org/display/DDW/TeamMemberType+Field> ;
  vs:term_status   "stable"
.
reso:ChangedByMemberID a rdf:Property ;
  rdfs:comment     "ID of the user, agent, member, etc., that uploaded the media this record refers to.","The local, well-know identifier of the member (user) who made the change." ;
  rdfs:domain      reso:Media,reso:HistoryTransactional,reso:OUID ;
  rdfs:label       "ChangedByMemberID" ;
  rdfs:range       xsd:string ;
  reso:CertificationLevel "Core","Silver","Platinum" ;
  schema:sameAs    <http://ddwiki.reso.org/display/DDW/ChangedByMemberID+Field>,<http://ddwiki.reso.org/display/DDW/ChangedByMemberID+%28HistoryTransactional%29+Field>,<http://ddwiki.reso.org/display/DDW/ChangedByMemberID+%28OUID%29+Field> ;
  vs:term_status   "stable"
.
reso:ChangedByMemberKey a rdf:Property ;
  rdfs:comment     "The primary key of the member who uploaded the media this record refers to.  This is a foreign key relating to the Member resource's MemberKey.","The unique identifier of the member (user) who made the change.  This is a foreign key relating to the Member resource's MemberKey." ;
  rdfs:domain      reso:Media,reso:HistoryTransactional,reso:OUID ;
  rdfs:label       "ChangedByMemberKey" ;
  rdfs:range       xsd:string ;
  reso:CertificationLevel "Core","Silver","Platinum" ;
  schema:sameAs    <http://ddwiki.reso.org/display/DDW/ChangedByMemberKey+Field>,<http://ddwiki.reso.org/display/DDW/ChangedByMemberKey+%28HistoryTransactional%29+Field>,<http://ddwiki.reso.org/display/DDW/ChangedByMemberKey+%28OUID%29+Field> ;
  vs:term_status   "stable"
.
reso:ChangedByMemberKeyNumeric a rdf:Property ;
  rdfs:comment     "The primary key of the member who uploaded the media this record refers to.  This is a foreign key relating to the Member resource's MemberKey.  This is the numeric only key and used as an alternative to the ChangedByMemberKey field.","The unique identifier of the member (user) who made the change.  This is a foreign key relating to the Member resource's MemberKey.  This is the numeric only key and used as an alternative to the ChangedByMemberKey field." ;
  rdfs:domain      reso:Media,reso:HistoryTransactional,reso:OUID ;
  rdfs:label       "ChangedByMemberKeyNumeric" ;
  rdfs:range       xsd:decimal ;
  reso:CertificationLevel "Platinum" ;
  schema:sameAs    <http://ddwiki.reso.org/display/DDW/ChangedByMemberKeyNumeric+Field>,<http://ddwiki.reso.org/display/DDW/ChangedByMemberKeyNumeric+%28HistoryTransactional%29+Field>,<http://ddwiki.reso.org/display/DDW/ChangedByMemberKeyNumeric+%28OUID%29+Field> ;
  vs:term_status   "stable"
.
reso:ModificationTimestamp a rdf:Property ;
  rdfs:comment     "The transactional timestamp automatically recorded by the MLS system representing the date/time the listing was last modified.","Date/time the roster (member or office) record was last modified.","Date/time the contact record was last modified.","The transactional timestamp automatically recorded by the MLS system representing the date/time the media record was last modified.","Timestamp of the last major change on the listing (see also MajorChangeType).","The transactional timestamp automatically recorded by the MLS system representing the date/time the Open House was last modified.","Date/time the roster (Team or office) record was last modified.","Date/time the Organization record was last modified." ;
  rdfs:domain      reso:Property,reso:Member,reso:Office,reso:Contacts,reso:Media,reso:HistoryTransactional,reso:SavedSearch,reso:OpenHouse,reso:Teams,reso:TeamMembers,reso:OUID ;
  rdfs:label       "ModificationTimestamp" ;
  rdfs:range       xsd:dateTime ;
  reso:CertificationLevel "Core","Silver","Gold","Platinum" ;
  reso:PropertyTypes "RESI","RLSE","RINC","LAND","MOBI","FARM","COMS","COML","BUSO" ;
  schema:sameAs    <http://ddwiki.reso.org/display/DDW/ModificationTimestamp+Field>,<http://ddwiki.reso.org/display/DDW/ModificationTimestamp+%28Member%29+Field>,<http://ddwiki.reso.org/display/DDW/ModificationTimestamp+%28Office%29+Field>,<http://ddwiki.reso.org/display/DDW/ModificationTimestamp+%28Contacts%29+Field>,<http://ddwiki.reso.org/display/DDW/ModificationTimestamp+%28Media%29+Field>,<http://ddwiki.reso.org/display/DDW/ModificationTimestamp+%28HistoryTransactional%29+Field>,<http://ddwiki.reso.org/display/DDW/ModificationTimestamp+%28SavedSearch%29+Field>,<http://ddwiki.reso.org/display/DDW/ModificationTimestamp+%28OpenHouse%29+Field>,<http://ddwiki.reso.org/display/DDW/ModificationTimestamp+%28Teams%29+Field>,<http://ddwiki.reso.org/display/DDW/ModificationTimestamp+%28TeamMembers%29+Field>,<http://ddwiki.reso.org/display/DDW/ModificationTimestamp+%28OUID%29+Field> ;
  vs:term_status   "stable"
.
reso:OrganizationAOR a rdf:Property ;
  rdfs:comment     "The Organization's Primary Board or Association of REALTORS if applicable." ;
  rdfs:domain      reso:OUID ;
  rdfs:label       "OrganizationAOR" ;
  rdfs:range       xsd:string ;
  reso:CertificationLevel "Platinum" ;
  schema:sameAs    <http://ddwiki.reso.org/display/DDW/OrganizationAOR+Field> ;
  vs:term_status   "stable"
.
reso:OrganizationAddress1 a rdf:Property ;
  rdfs:comment     "The street number, direction, name and suffix of the organization." ;
  rdfs:domain      reso:OUID ;
  rdfs:label       "OrganizationAddress1" ;
  rdfs:range       xsd:string ;
  reso:CertificationLevel "Platinum" ;
  schema:sameAs    <http://ddwiki.reso.org/display/DDW/OrganizationAddress1+Field> ;
  vs:term_status   "stable"
.
reso:OrganizationAddress2 a rdf:Property ;
  rdfs:comment     "The unit/suite number of the organization." ;
  rdfs:domain      reso:OUID ;
  rdfs:label       "OrganizationAddress2" ;
  rdfs:range       xsd:string ;
  reso:CertificationLevel "Platinum" ;
  schema:sameAs    <http://ddwiki.reso.org/display/DDW/OrganizationAddress2+Field> ;
  vs:term_status   "stable"
.
reso:OrganizationAorOuid a rdf:Property ;
  rdfs:comment     "The OUID for the Organization's Association of REALTORS if applicable." ;
  rdfs:domain      reso:OUID ;
  rdfs:label       "OrganizationAorOuid" ;
  rdfs:range       xsd:string ;
  reso:CertificationLevel "Platinum" ;
  schema:sameAs    <http://ddwiki.reso.org/display/DDW/OrganizationAorOuid+Field> ;
  vs:term_status   "stable"
.
reso:OrganizationAorOuidKey a rdf:Property ;
  rdfs:comment     "The OrganizationUniqueIdKey of the AOR from the system serving the OUID resource." ;
  rdfs:domain      reso:OUID ;
  rdfs:label       "OrganizationAorOuidKey" ;
  rdfs:range       xsd:string ;
  reso:CertificationLevel "Platinum" ;
  schema:sameAs    <http://ddwiki.reso.org/display/DDW/OrganizationAorOuidKey+Field> ;
  vs:term_status   "stable"
.
reso:OrganizationAorOuidKeyNumeric a rdf:Property ;
  rdfs:comment     "The OrganizationUniqueIdKey of the AOR from the system serving the OUID resource.  This is the numeric only key and used as an alternative to the OrganizationAorOuidKey field." ;
  rdfs:domain      reso:OUID ;
  rdfs:label       "OrganizationAorOuidKeyNumeric" ;
  rdfs:range       xsd:decimal ;
  reso:CertificationLevel "Platinum" ;
  schema:sameAs    <http://ddwiki.reso.org/display/DDW/OrganizationAorOuidKeyNumeric+Field> ;
  vs:term_status   "stable"
.
reso:OrganizationCarrierRoute a rdf:Property ;
  rdfs:domain      reso:OUID ;
  rdfs:label       "OrganizationCarrierRoute" ;
  rdfs:range       xsd:string ;
  reso:CertificationLevel "Platinum" ;
  schema:sameAs    <http://ddwiki.reso.org/display/DDW/OrganizationCarrierRoute+Field> ;
  vs:term_status   "stable"
.
reso:OrganizationCity a rdf:Property ;
  rdfs:comment     "The city of the organization." ;
  rdfs:domain      reso:OUID ;
  rdfs:label       "OrganizationCity" ;
  rdfs:range       xsd:string ;
  reso:CertificationLevel "Platinum" ;
  schema:sameAs    <http://ddwiki.reso.org/display/DDW/OrganizationCity+Field> ;
  vs:term_status   "stable"
.
reso:OrganizationComments a rdf:Property ;
  rdfs:comment     "Comments or notes about the Organization." ;
  rdfs:domain      reso:OUID ;
  rdfs:label       "OrganizationComments" ;
  rdfs:range       xsd:string ;
  reso:CertificationLevel "Platinum" ;
  schema:sameAs    <http://ddwiki.reso.org/display/DDW/OrganizationComments+Field> ;
  vs:term_status   "stable"
.
reso:OrganizationContactEmail a rdf:Property ;
  rdfs:comment     "The email address of the Organization Contact." ;
  rdfs:domain      reso:OUID ;
  rdfs:label       "OrganizationContactEmail" ;
  rdfs:range       xsd:string ;
  reso:CertificationLevel "Platinum" ;
  schema:sameAs    <http://ddwiki.reso.org/display/DDW/OrganizationContactEmail+Field> ;
  vs:term_status   "stable"
.
reso:OrganizationContactFax a rdf:Property ;
  rdfs:comment     "North American 10 digit phone numbers should be in the format of ###-###-#### (separated by hyphens).  Other conventions should use the common local standard.  International numbers should be preceded by a plus symbol." ;
  rdfs:domain      reso:OUID ;
  rdfs:label       "OrganizationContactFax" ;
  rdfs:range       xsd:string ;
  reso:CertificationLevel "Platinum" ;
  schema:sameAs    <http://ddwiki.reso.org/display/DDW/OrganizationContactFax+Field> ;
  vs:term_status   "stable"
.
reso:OrganizationContactFirstName a rdf:Property ;
  rdfs:comment     "The first name of the Organization Contact." ;
  rdfs:domain      reso:OUID ;
  rdfs:label       "OrganizationContactFirstName" ;
  rdfs:range       xsd:string ;
  reso:CertificationLevel "Platinum" ;
  schema:sameAs    <http://ddwiki.reso.org/display/DDW/OrganizationContactFirstName+Field> ;
  vs:term_status   "stable"
.
reso:OrganizationContactFullName a rdf:Property ;
  rdfs:comment     "The full name of the Organization Contact. (First Middle Last) or a alternate full name." ;
  rdfs:domain      reso:OUID ;
  rdfs:label       "OrganizationContactFullName" ;
  rdfs:range       xsd:string ;
  reso:CertificationLevel "Platinum" ;
  schema:sameAs    <http://ddwiki.reso.org/display/DDW/OrganizationContactFullName+Field> ;
  vs:term_status   "stable"
.
reso:OrganizationContactJobTitle a rdf:Property ;
  rdfs:comment     "The title or position of the Organization Contact." ;
  rdfs:domain      reso:OUID ;
  rdfs:label       "OrganizationContactJobTitle" ;
  rdfs:range       xsd:string ;
  reso:CertificationLevel "Platinum" ;
  schema:sameAs    <http://ddwiki.reso.org/display/DDW/OrganizationContactJobTitle+Field> ;
  vs:term_status   "stable"
.
reso:OrganizationContactLastName a rdf:Property ;
  rdfs:comment     "The last name of the Organization Contact." ;
  rdfs:domain      reso:OUID ;
  rdfs:label       "OrganizationContactLastName" ;
  rdfs:range       xsd:string ;
  reso:CertificationLevel "Platinum" ;
  schema:sameAs    <http://ddwiki.reso.org/display/DDW/OrganizationContactLastName+Field> ;
  vs:term_status   "stable"
.
reso:OrganizationContactMiddleName a rdf:Property ;
  rdfs:comment     "The middle name of the Organization Contact." ;
  rdfs:domain      reso:OUID ;
  rdfs:label       "OrganizationContactMiddleName" ;
  rdfs:range       xsd:string ;
  reso:CertificationLevel "Platinum" ;
  schema:sameAs    <http://ddwiki.reso.org/display/DDW/OrganizationContactMiddleName+Field> ;
  vs:term_status   "stable"
.
reso:OrganizationContactNamePrefix a rdf:Property ;
  rdfs:comment     "Prefix to the name of the Organization Contact. (e.g. Dr. Mr. Ms. etc.)" ;
  rdfs:domain      reso:OUID ;
  rdfs:label       "OrganizationContactNamePrefix" ;
  rdfs:range       xsd:string ;
  reso:CertificationLevel "Platinum" ;
  schema:sameAs    <http://ddwiki.reso.org/display/DDW/OrganizationContactNamePrefix+Field> ;
  vs:term_status   "stable"
.
reso:OrganizationContactNameSuffix a rdf:Property ;
  rdfs:comment     "Suffix to the surname (e.g. Esq.,  Jr.,  III etc.) of the Organization Contact." ;
  rdfs:domain      reso:OUID ;
  rdfs:label       "OrganizationContactNameSuffix" ;
  rdfs:range       xsd:string ;
  reso:CertificationLevel "Platinum" ;
  schema:sameAs    <http://ddwiki.reso.org/display/DDW/OrganizationContactNameSuffix+Field> ;
  vs:term_status   "stable"
.
reso:OrganizationContactPhone a rdf:Property ;
  rdfs:comment     "North American 10 digit phone numbers should be in the format of ###-###-#### (separated by hyphens).  Other conventions should use the common local standard.  International numbers should be preceded by a plus symbol." ;
  rdfs:domain      reso:OUID ;
  rdfs:label       "OrganizationContactPhone" ;
  rdfs:range       xsd:string ;
  reso:CertificationLevel "Platinum" ;
  schema:sameAs    <http://ddwiki.reso.org/display/DDW/OrganizationContactPhone+Field> ;
  vs:term_status   "stable"
.
reso:OrganizationContactPhoneExt a rdf:Property ;
  rdfs:comment     "The extension of the given phone number (if applicable)." ;
  rdfs:domain      reso:OUID ;
  rdfs:label       "OrganizationContactPhoneExt" ;
  rdfs:range       xsd:string ;
  reso:CertificationLevel "Platinum" ;
  schema:sameAs    <http://ddwiki.reso.org/display/DDW/OrganizationContactPhoneExt+Field> ;
  vs:term_status   "stable"
.
reso:OrganizationCountry a rdf:Property ;
  rdfs:comment     "The country abbreviation in a postal address." ;
  rdfs:domain      reso:OUID ;
  rdfs:label       "OrganizationCountry" ;
  rdfs:range       enum:Country ;
  reso:CertificationLevel "Platinum" ;
  schema:sameAs    <http://ddwiki.reso.org/display/DDW/OrganizationCountry+Field> ;
  vs:term_status   "stable"
.
reso:OrganizationCountyOrParish a rdf:Property ;
  rdfs:comment     "The county or parish in which the organization is addressed." ;
  rdfs:domain      reso:OUID ;
  rdfs:label       "OrganizationCountyOrParish" ;
  rdfs:range       xsd:string ;
  reso:CertificationLevel "Platinum" ;
  schema:sameAs    <http://ddwiki.reso.org/display/DDW/OrganizationCountyOrParish+Field> ;
  vs:term_status   "stable"
.
reso:OrganizationMemberCount a rdf:Property ;
  rdfs:comment     "The total number of active members in the Organization if applicable." ;
  rdfs:domain      reso:OUID ;
  rdfs:label       "OrganizationMemberCount" ;
  rdfs:range       xsd:decimal ;
  reso:CertificationLevel "Platinum" ;
  schema:sameAs    <http://ddwiki.reso.org/display/DDW/OrganizationMemberCount+Field> ;
  vs:term_status   "stable"
.
reso:OrganizationMlsCode a rdf:Property ;
  rdfs:comment     "If the organization is an MLS it is likely they already have an ID or code based on their name or an abbreviation.  This field supports the continued use/reference to that legacy code." ;
  rdfs:domain      reso:OUID ;
  rdfs:label       "OrganizationMlsCode" ;
  rdfs:range       xsd:string ;
  reso:CertificationLevel "Platinum" ;
  schema:sameAs    <http://ddwiki.reso.org/display/DDW/OrganizationMlsCode+Field> ;
  vs:term_status   "stable"
.
reso:OrganizationMlsVendorName a rdf:Property ;
  rdfs:comment     "If the organization uses an MLS system, this is the textual name of the vendor." ;
  rdfs:domain      reso:OUID ;
  rdfs:label       "OrganizationMlsVendorName" ;
  rdfs:range       xsd:string ;
  reso:CertificationLevel "Platinum" ;
  schema:sameAs    <http://ddwiki.reso.org/display/DDW/OrganizationMlsVendorName+Field> ;
  vs:term_status   "stable"
.
reso:OrganizationMlsVendorOuid a rdf:Property ;
  rdfs:comment     "If the organization uses an MLS system, this is that vendor's OUID." ;
  rdfs:domain      reso:OUID ;
  rdfs:label       "OrganizationMlsVendorOuid" ;
  rdfs:range       xsd:string ;
  reso:CertificationLevel "Platinum" ;
  schema:sameAs    <http://ddwiki.reso.org/display/DDW/OrganizationMlsVendorOuid+Field> ;
  vs:term_status   "stable"
.
reso:OrganizationName a rdf:Property ;
  rdfs:comment     "The textual name of the organization represented by a given OUID record." ;
  rdfs:domain      reso:OUID ;
  rdfs:label       "OrganizationName" ;
  rdfs:range       xsd:string ;
  reso:CertificationLevel "Platinum" ;
  schema:sameAs    <http://ddwiki.reso.org/display/DDW/OrganizationName+Field> ;
  vs:term_status   "stable"
.
reso:OrganizationNationalAssociationId a rdf:Property ;
  rdfs:comment     "The national association ID of the Organization if applicable.  i.e. in the U.S. is the NRDS number." ;
  rdfs:domain      reso:OUID ;
  rdfs:label       "OrganizationNationalAssociationId" ;
  rdfs:range       xsd:string ;
  reso:CertificationLevel "Platinum" ;
  schema:sameAs    <http://ddwiki.reso.org/display/DDW/OrganizationNationalAssociationId+Field> ;
  vs:term_status   "stable"
.
reso:OrganizationPostalCode a rdf:Property ;
  rdfs:comment     "The postal code of the organization." ;
  rdfs:domain      reso:OUID ;
  rdfs:label       "OrganizationPostalCode" ;
  rdfs:range       xsd:string ;
  reso:CertificationLevel "Platinum" ;
  schema:sameAs    <http://ddwiki.reso.org/display/DDW/OrganizationPostalCode+Field> ;
  vs:term_status   "stable"
.
reso:OrganizationPostalCodePlus4 a rdf:Property ;
  rdfs:comment     "The extension of the postal/zip code.  i.e. +4" ;
  rdfs:domain      reso:OUID ;
  rdfs:label       "OrganizationPostalCodePlus4" ;
  rdfs:range       xsd:string ;
  reso:CertificationLevel "Platinum" ;
  schema:sameAs    <http://ddwiki.reso.org/display/DDW/OrganizationPostalCodePlus4+Field> ;
  vs:term_status   "stable"
.
reso:OrganizationSocialMediaType a rdf:Property ;
  rdfs:comment     "A list of types of sites, blog, social media, the Organization URL or ID is referring to.  i.e. Website, Blog, Facebook, Twitter, LinkedIn, Skype, etc.,  This list is used to populate the Type with repeating Social Media URL or ID types." ;
  rdfs:domain      reso:OUID ;
  rdfs:label       "OrganizationSocialMediaType" ;
  rdfs:range       xsd:string ;
  reso:CertificationLevel "Platinum" ;
  schema:sameAs    <http://ddwiki.reso.org/display/DDW/OrganizationSocialMediaType+Field> ;
  vs:term_status   "stable"
.
reso:OrganizationSocialMedia a rdf:Property ;
  rdfs:domain      reso:OUID ;
  rdfs:label       "OrganizationSocialMedia" ;
  rdfs:range       xsd:string ;
  reso:CertificationLevel "Platinum" ;
  schema:sameAs    <http://ddwiki.reso.org/display/DDW/OrganizationSocialMedia%5BType%5DUrlOrId+Field> ;
  vs:term_status   "stable"
.
reso:OrganizationStateLicense a rdf:Property ;
  rdfs:comment     "The license of the Organization if applicable. Separate multiple licenses with a comma and space." ;
  rdfs:domain      reso:OUID ;
  rdfs:label       "OrganizationStateLicense" ;
  rdfs:range       xsd:string ;
  reso:CertificationLevel "Platinum" ;
  schema:sameAs    <http://ddwiki.reso.org/display/DDW/OrganizationStateLicense+Field> ;
  vs:term_status   "stable"
.
reso:OrganizationStateLicenseState a rdf:Property ;
  rdfs:comment     "The state in which the Organization is licensed if applicable." ;
  rdfs:domain      reso:OUID ;
  rdfs:label       "OrganizationStateLicenseState" ;
  rdfs:range       enum:StateOrProvince ;
  reso:CertificationLevel "Platinum" ;
  schema:sameAs    <http://ddwiki.reso.org/display/DDW/OrganizationStateLicenseState+Field> ;
  vs:term_status   "stable"
.
reso:OrganizationStateOrProvince a rdf:Property ;
  rdfs:comment     "The state or province in which the organization is addressed." ;
  rdfs:domain      reso:OUID ;
  rdfs:label       "OrganizationStateOrProvince" ;
  rdfs:range       enum:StateOrProvince ;
  reso:CertificationLevel "Platinum" ;
  schema:sameAs    <http://ddwiki.reso.org/display/DDW/OrganizationStateOrProvince+Field> ;
  vs:term_status   "stable"
.
reso:OrganizationStatus a rdf:Property ;
  rdfs:comment     "Is the Organization active or inactive.  1 or true is active, 0 or false is inactive.  This field is not nullable." ;
  rdfs:domain      reso:OUID ;
  rdfs:label       "OrganizationStatus" ;
  rdfs:range       xsd:boolean ;
  reso:CertificationLevel "Platinum" ;
  schema:sameAs    <http://ddwiki.reso.org/display/DDW/OrganizationStatus+Field> ;
  vs:term_status   "stable"
.
reso:OrganizationStatusChangeTimestamp a rdf:Property ;
  rdfs:comment     "The date/time of when the Organization Status was last changed." ;
  rdfs:domain      reso:OUID ;
  rdfs:label       "OrganizationStatusChangeTimestamp" ;
  rdfs:range       xsd:dateTime ;
  reso:CertificationLevel "Platinum" ;
  schema:sameAs    <http://ddwiki.reso.org/display/DDW/OrganizationStatusChangeTimestamp+Field> ;
  vs:term_status   "stable"
.
reso:OrganizationType a rdf:Property ;
  rdfs:comment     "The type of organization.  i.e. MLS, Vendor, Association, etc.  This is not a substitute or alternative for the Office resource, however it may be that a brokerage has a record in this table for a non-listing purpose." ;
  rdfs:domain      reso:OUID ;
  rdfs:label       "OrganizationType" ;
  rdfs:range       xsd:string ;
  reso:CertificationLevel "Platinum" ;
  schema:sameAs    <http://ddwiki.reso.org/display/DDW/OrganizationType+Field> ;
  vs:term_status   "stable"
.
reso:OrganizationUniqueId a rdf:Property ;
  rdfs:comment     "The OUID.  This is the unique ID assigned to organizations included in the OUID resource.  Assignment of OUIDs will be centralized and may not be created by systems hosting the OUID resource.  Contact info@RESO.org for information on obtaining an OUID." ;
  rdfs:domain      reso:OUID ;
  rdfs:label       "OrganizationUniqueId" ;
  rdfs:range       xsd:string ;
  reso:CertificationLevel "Platinum" ;
  schema:sameAs    <http://ddwiki.reso.org/display/DDW/OrganizationUniqueId+Field> ;
  vs:term_status   "stable"
.
reso:OrganizationUniqueIdKey a rdf:Property ;
  rdfs:comment     "The key field used by the system hosting a table of OUIDs.  This key is likely to be unique to each hosting system and is not meant to be a universal ID for an organization, but rather a key used by clients of the hosting system.  The actual OUID is the Organization Unique ID field." ;
  rdfs:domain      reso:OUID ;
  rdfs:label       "OrganizationUniqueIdKey" ;
  rdfs:range       xsd:string ;
  reso:CertificationLevel "Platinum" ;
  schema:sameAs    <http://ddwiki.reso.org/display/DDW/OrganizationUniqueIdKey+Field> ;
  vs:term_status   "stable"
.
reso:OrganizationUniqueIdKeyNumeric a rdf:Property ;
  rdfs:comment     "The key field used by the system hosting a table of OUIDs.  This key is likely to be unique to each hosting system and is not meant to be a universal ID for an organization, but rather a key used by clients of the hosting system.  The actual OUID is the Organization Unique ID field.  This is the numeric only key and used as an alternative to the OrganizationUniqueIdKey field." ;
  rdfs:domain      reso:OUID ;
  rdfs:label       "OrganizationUniqueIdKeyNumeric" ;
  rdfs:range       xsd:decimal ;
  reso:CertificationLevel "Platinum" ;
  schema:sameAs    <http://ddwiki.reso.org/display/DDW/OrganizationUniqueIdKeyNumeric+Field> ;
  vs:term_status   "stable"
.
reso:OriginalEntryTimestamp a rdf:Property ;
  rdfs:comment     "The transactional timestamp automatically recorded by the MLS system representing the date/time the listing was entered and made visible to members of the MLS.","Date/time the roster (member or office) record was originally input into the source system.","Date/time the contact record was originally input into the source system.","The transactional timestamp automatically recorded by the MLS system representing the date/time the Open House was entered and made visible to members of the MLS.","Date/time the roster (Team or office) record was originally input into the source system.","Date/time the Organization record was originally input into the source system." ;
  rdfs:domain      reso:Property,reso:Member,reso:Office,reso:Contacts,reso:SavedSearch,reso:OpenHouse,reso:Teams,reso:TeamMembers,reso:OUID ;
  rdfs:label       "OriginalEntryTimestamp" ;
  rdfs:range       xsd:dateTime ;
  reso:CertificationLevel "Core","Silver","Gold","Bronze","Platinum" ;
  reso:PropertyTypes "RESI","RLSE","RINC","LAND","MOBI","FARM","COMS","COML","BUSO" ;
  schema:sameAs    <http://ddwiki.reso.org/display/DDW/OriginalEntryTimestamp+Field>,<http://ddwiki.reso.org/display/DDW/OriginalEntryTimestamp+%28Member%29+Field>,<http://ddwiki.reso.org/display/DDW/OriginalEntryTimestamp+%28Office%29+Field>,<http://ddwiki.reso.org/display/DDW/OriginalEntryTimestamp+%28Contacts%29+Field>,<http://ddwiki.reso.org/display/DDW/OriginalEntryTimestamp+%28SavedSearch%29+Field>,<http://ddwiki.reso.org/display/DDW/OriginalEntryTimestamp+%28OpenHouse%29+Field>,<http://ddwiki.reso.org/display/DDW/OriginalEntryTimestamp+%28Teams%29+Field>,<http://ddwiki.reso.org/display/DDW/OriginalEntryTimestamp+%28TeamMembers%29+Field>,<http://ddwiki.reso.org/display/DDW/OriginalEntryTimestamp+%28OUID%29+Field> ;
  vs:term_status   "stable"
.
